## 문제
일차함수 $f(x) = ax + b$ 가 $f^{-1}(1) = 0$ 과 $f^{-1}(f^{-1}(b)) = 2b$ 를 만족할 때, $f(a^2 - b^2)$ 의 값은?

## 보기
① $-\frac{7}{3}$   ② $-\frac{5}{4}$   ③ $\frac{7}{2}$   ④ $\frac{11}{8}$   ⑤ $\frac{17}{10}$

## 풀이
주어진 조건에 의하여
$f(0) = 1$, $f(f(2b)) = b$

$f(x) = ax + b$ 이므로
$f(0) = b = 1$

$f(f(2b)) = f(f(2)) = f(2a + 1) = a(2a + 1) + 1 = 2a^2 + a + 1 = 1$
$2a^2 + a = 0$
$\therefore a = -\frac{1}{2}$ ($\because a \neq 0$)

따라서, 구하고자 하는 식의 값은
$f(a^2 - b^2) = f(-\frac{3}{4}) = -\frac{1}{2} \cdot (-\frac{3}{4}) + 1 = \frac{11}{8}$