## ë¬¸ì œ
ì‚¼ê°ë°©ì •ì‹ $6 \sin^{2} x + \sqrt{3} \sin x \cos x + 7 \cos^{2} x = 6$ ì˜ ëª¨ë“  ê·¼ì˜ í•©ì€? (ë‹¨, $-\pi \le x \le \pi$)



> [!example] ğŸ“¸ (ê·¸ë¦¼/ê·¸ë˜í”„)

## ë³´ê¸°
â‘  $-\frac{\pi}{3}$   â‘¡ $0$   â‘¢ $\frac{\pi}{3}$   â‘£ $\frac{2}{3} \pi$   â‘¤ $\pi$

## í’€ì´
[ì •ë‹µ] â‘£

$\sin^{2} x = \frac{1 - \cos 2x}{2}$, $\cos^{2} x = \frac{1 + \cos 2x}{2}$ ì´ë¯€ë¡œ ì£¼ì–´ì§„ ì‹ì€
$3(1 - \cos 2x) + \frac{\sqrt{3}}{2} \sin 2x + \frac{7}{2} (1 + \cos 2x) = 6$
$1 + \cos 2x + \sqrt{3} \sin 2x = 0$
$2 \sin (2x + \frac{\pi}{6}) = -1$
$\sin (2x + \frac{\pi}{6}) = -\frac{1}{2} \cdots$ ($1$)

$x$ ì˜ ë²”ìœ„ê°€ $-\pi \le x \le \pi$ ì´ë¯€ë¡œ
$-2 \pi + \frac{\pi}{6} \le 2x + \frac{\pi}{6} \le 2 \pi + \frac{\pi}{6}$

ê·¸ë¦¼ì—ì„œ ì‹ ($1$)ì˜ í•´ë¥¼ êµ¬í•˜ë©´
$2x + \frac{\pi}{6} = -\pi + \frac{\pi}{6}, -\frac{\pi}{6}, \pi + \frac{\pi}{6}, 2 \pi - \frac{\pi}{6}$
$x = -\frac{\pi}{2}, -\frac{\pi}{6}, \frac{\pi}{2}, \frac{5}{6} \pi$

ë”°ë¼ì„œ, ëª¨ë“  ê·¼ì˜ í•©ì€
$-\frac{\pi}{2} - \frac{\pi}{6} + \frac{\pi}{2} + \frac{5}{6} \pi = \frac{2}{3} \pi$