## 문제
두 함수 $f(\theta)$와 $g(\theta)$를 
$$ f(\theta) = \frac{\sin(\pi + \theta)}{1 + \cos(\frac{\pi}{2} + \theta)}, \quad g(\theta) = \frac{\cos(\pi + \theta)}{1 + \cos(\frac{3\pi}{2} - \theta)} $$
로 정의할 때, $f(\theta)f(-\theta)g(\theta)g(-\theta)$를 간단히 하면?

## 보기
① $-\cot^{2} \theta$   ② $-\tan^{2} \theta$   ③ $\sec^{2} \theta$   ④ $\tan^{2} \theta$   ⑤ $\cot^{2} \theta$

## 풀이
삼각함수의 성질을 이용하여 각을 $\theta$로 표현하면 
$f(\theta) = -\frac{\sin \theta}{1 - \sin \theta}$, $g(\theta) = -\frac{\cos \theta}{1 - \sin \theta}$ 

$\theta$ 대신 $-\theta$를 대입한 경우에 
$f(-\theta) = -\frac{\sin (-\theta)}{1 - \sin (-\theta)} = \frac{\sin \theta}{1 + \sin \theta}$ 
$g(-\theta) = -\frac{\cos (-\theta)}{1 - \sin (-\theta)} = -\frac{\cos \theta}{1 + \sin \theta}$ 

따라서, 
준 식 $= -\frac{\sin \theta}{1 - \sin \theta} \cdot \frac{\sin \theta}{1 + \sin \theta} \cdot -\frac{\cos \theta}{1 - \sin \theta} \cdot -\frac{\cos \theta}{1 + \sin \theta}$ 
$= -\frac{\sin^{2} \theta}{1 - \sin^{2} \theta} \cdot \frac{\cos^{2} \theta}{1 - \sin^{2} \theta}$ 
$= -\frac{\sin^{2} \theta}{\cos^{2} \theta} \cdot \frac{\cos^{2} \theta}{\cos^{2} \theta}$
$= -\left(\frac{\sin \theta}{\cos \theta}\right)^{2}$ 
$= -\tan^{2} \theta$ 

정답 ②