## 문제
$\sum_{k=1}^{100} (k-2)^{2} - \sum_{k=1}^{101} 4 + 4 \sum_{k=1}^{100} k - \sum_{k=2}^{101} (k-1)^{2}$ 의 값은?

## 보기
① $-400$   ② $-4$   ③ $0$   ④ $4$   ⑤ $400$

## 풀이
(준식)
$$= \sum_{k=1}^{100} (k-2)^{2} - \left( \sum_{k=1}^{100} 4 + 4 \right) + \sum_{k=1}^{100} 4k - \left( \sum_{k=1}^{100} (k-1)^{2} + 100^{2} \right)$$
$$= \sum_{k=1}^{100} \{ (k-2)^{2} - 4 + 4k - (k-1)^{2} \} - 4 - 100^{2}$$
$$= \sum_{k=1}^{100} (2k-1) - 4 - 100^{2}$$
$$= 100 \times 101 - 100 - 4 - 100^{2}$$
$$= 10100 - 100 - 4 - 10000 = -4$$

정답: ②