## ë¬¸ì œ

ê·¸ë¦¼ê³¼ ê°™ì´ ì‚¼ì°¨í•¨ìˆ˜ $y=f(x)$ ê°€ ê·¹ëŒ“ê°’ $f(1)=1$ ê³¼ ê·¹ì†Ÿê°’ $f(3)=-3$ ì„ ê°€ì§€ë©°, $f(0)=-3$ ì´ë‹¤. ì´ë•Œ, $\int_{0}^{3} |f'(x)| dx$ ì˜ ê°’ì€?

> [!example] ğŸ“¸ (ê·¸ë¦¼/ê·¸ë˜í”„)

## ë³´ê¸°

â‘  $6$   â‘¡ $7$   â‘¢ $8$   â‘£ $9$   â‘¤ $10$

## í’€ì´

[ì •ë‹µ] â‘¢ 

$f'(x)=a(x-1)(x-3)$ ì´ë¯€ë¡œ 
$f(x)=a ( \frac{1}{3} x^{3} -2x^{2} +3x ) +C$ ($C$ ëŠ” ì ë¶„ìƒìˆ˜) $\dots$ ã‰  

ë˜, $f(1)=1, f(0)=-3$ ì´ë¯€ë¡œ ã‰ ì— ëŒ€ì…í•˜ì—¬ í’€ë©´ 
$a=3, C=-3$ ì´ë¯€ë¡œ 
$f'(x)=3(x-1)(x-3)$ 

$\therefore \int_{0}^{3} | f'(x) | dx$ 
$=3\int_{0}^{1} (x-1)(x-3)dx-3\int_{1}^{3} (x-1)(x-3)dx$ 
$=8$