## 문제
이차방정식 $x^{2}-3x+1=0$ 의 두 근 $a$, $\beta$ 에 대하여 
$$(1-\frac{1}{a})(1-\frac{1}{\beta}) + (1-\frac{2}{a})(1-\frac{2}{\beta}) + \cdots + (1-\frac{10}{a})(1-\frac{10}{\beta})$$ 
의 값은?

## 보기
① $230$   ② $240$   ③ $250$   ④ $260$   ⑤ $270$

## 풀이
이차방정식 $x^{2}-3x+1=0$ 의 두 근이 $a$, $\beta$ 이므로 근과 계수의 관계에서 
$a+\beta=3$, $a\beta=1$ 

(주어진 식) 
$= \sum_{k=1}^{10} (1-\frac{k}{a}) (1-\frac{k}{\beta})$ 
$= \sum_{k=1}^{10} \frac{1}{a\beta}(a-k)(\beta-k)$ 
$= \sum_{k=1}^{10} \{k^{2}-(a+\beta)k+a\beta\}$ ($\because a\beta=1$) 
$= \sum_{k=1}^{10} (k^{2}-3k+1)$ 
$= \frac{10 \cdot 11 \cdot 21}{6}-3 \cdot \frac{10 \cdot 11}{2}+10$ 
$= 385-165+10$
$= 230$

정답: ①