## ë¬¸ì œ
ì•„ë˜ ê·¸ë¦¼ì€ $0 \le x \le 2\pi$ ì—ì„œ ì •ì˜ëœ í•¨ìˆ˜ $f(x) = \cos x + |\cos x|$ ì˜ ê·¸ë˜í”„ì´ë‹¤. ì´ë•Œ, $\int_{\frac{\pi}{6}}^{\pi} f(2x - \frac{\pi}{6}) dx$ ì˜ ê°’ì€?

> [!example] ğŸ“¸ (ê·¸ë¦¼/ê·¸ë˜í”„)

## ë³´ê¸°
â‘  $\frac{1}{2}$   â‘¡ $\frac{\sqrt{3}}{2}$   â‘¢ $1$   â‘£ $\sqrt{3}$   â‘¤ $\frac{3\sqrt{3}}{2}$

## í’€ì´
$\int_{\frac{\pi}{6}}^{\pi} f(2x - \frac{\pi}{6}) dx$
$= \int_{\frac{\pi}{6}}^{\pi} \{ \cos(2x - \frac{\pi}{6}) + |\cos(2x - \frac{\pi}{6})| \} dx$

$\cos(2x - \frac{\pi}{6}) < 0$ ì¸ ê²½ìš° $f(2x - \frac{\pi}{6}) = 0$ ì´ë¯€ë¡œ ì ë¶„ êµ¬ê°„ì„ ë‚˜ëˆ„ë©´ ë‹¤ìŒê³¼ ê°™ë‹¤.

$\int_{\frac{\pi}{6}}^{\pi} f(2x - \frac{\pi}{6}) dx$
$= \int_{\frac{\pi}{6}}^{\frac{\pi}{3}} 2\cos(2x - \frac{\pi}{6}) dx + \int_{\frac{5\pi}{6}}^{\pi} 2\cos(2x - \frac{\pi}{6}) dx$
$= [\sin(2x - \frac{\pi}{6})]_{\frac{\pi}{6}}^{\frac{\pi}{3}} + [\sin(2x - \frac{\pi}{6})]_{\frac{5\pi}{6}}^{\pi}$
$= (\sin\frac{\pi}{2} - \sin\frac{\pi}{6}) + (\sin\frac{11\pi}{6} - \sin\frac{3\pi}{2})$
$= (1 - \frac{1}{2}) + (-\frac{1}{2} - (-1))$
$= \frac{1}{2} + \frac{1}{2} = 1$

ì •ë‹µ: â‘¢