## 문제
다항식 $f(x)$를 $x+1$로 나누었을 때의 몫과 나머지가 각각 $x^{2}+2 x+3$, $4$일 때, 다항식 $x f(x)+2$를 $x+1$로 나누었을 때의 몫은?

## 보기
① $x^{3}+2 x^{2}+3 x+4$
② $x^{3}-2 x^{2}+2 x+3$
③ $x^{3}+x^{2}+x+4$
④ $x^{3}+3 x^{2}-2 x+4$
⑤ $x^{3}+4 x^{2}-3 x+2$

## 풀이
주어진 조건에 의해 
$$f(x)=(x+1) (x^{2}+2 x+3 )+4$$
이므로 
$$x f(x)+2 = x(x+1) (x^{2}+2 x+3 )+4 x+2$$ 
$$=x(x+1) (x^{2}+2 x+3 )+4(x+1)-2$$ 
$$=(x+1) (x(x^{2}+2 x+3)+4 )-2$$
$$=(x+1) (x^{3}+2 x^{2}+3 x+4 )-2$$ 
따라서 다항식 $x f(x)+2$를 $x+1$로 나누었을 때의 몫은 $x^{3}+2 x^{2}+3 x+4$이다.

정답: ①