## ë¬¸ì œ
ê·¸ë¦¼ê³¼ ê°™ì´ ì‚¼ì°¨í•¨ìˆ˜ $y=f(x)$ ê°€ ê·¹ëŒ“ê°’ $f(1)=1$ ê³¼ ê·¹ì†Ÿê°’ $f(3)=-3$ ì„ ê°€ì§€ë©°, $f(0)=-3$ ì´ë‹¤. ì´ë•Œ, $\int_{0}^{3} |f'(x)| dx$ ì˜ ê°’ì€?

> [!example] ğŸ“¸ (ê·¸ë¦¼/ê·¸ë˜í”„)

## ë³´ê¸°
â‘  $6$   â‘¡ $7$   â‘¢ $8$   â‘£ $9$   â‘¤ $10$

## í’€ì´
$f'(x)=a(x-1)(x-3)$ ì´ë¯€ë¡œ
$f(x)=a \left( \frac{1}{3} x^{3} -2x^{2} +3x \right) +C$ ($C$ ëŠ” ì ë¶„ìƒìˆ˜) $\cdots \cdots$ ã‰ 
ë˜, $f(1)=1, f(0)=-3$ ì´ë¯€ë¡œ ã‰ ì— ëŒ€ì…í•˜ì—¬ í’€ë©´
$a=3, C=-3$ ì´ë¯€ë¡œ
$f'(x)=3(x-1)(x-3)$
$\therefore \int_{0}^{3} |f'(x)| dx$
$= 3 \int_{0}^{1} (x-1)(x-3)dx - 3 \int_{1}^{3} (x-1)(x-3)dx$
$= [f(x)]_{0}^{1} - [f(x)]_{1}^{3}$
$= \{ f(1)-f(0) \} - \{ f(3)-f(1) \}$
$= \{ 1-(-3) \} - \{ -3-1 \}$
$= 4 - (-4) = 8$

[ì •ë‹µ] â‘¢