## 문제
이차정사각행렬 $A$, $B$가 
$$ (A-B)^{2} = \left( \begin{array}{cc} 5 & 3 \\ 3 & 2 \end{array} \right) , A^{2} + B^{2} = \left( \begin{array}{cc} 4 & 0 \\ 1 & 3 \end{array} \right) $$
를 만족할 때, 행렬 $(A+B)^{2}$의 모든 성분의 합은?

## 보기
① $1$   ② $3$   ③ $5$   ④ $7$   ⑤ $9$

## 풀이
$$ (A-B)^{2} = A^{2} - AB - BA + B^{2} = \left( \begin{array}{cc} 5 & 3 \\ 3 & 2 \end{array} \right) $$
이므로
$$ AB + BA = (A^{2} + B^{2}) - (A-B)^{2} $$
$$ = \left( \begin{array}{cc} 4 & 0 \\ 1 & 3 \end{array} \right) - \left( \begin{array}{cc} 5 & 3 \\ 3 & 2 \end{array} \right) = \left( \begin{array}{cc} -1 & -3 \\ -2 & 1 \end{array} \right) $$
이다.
$$ (A+B)^{2} = A^{2} + AB + BA + B^{2} = (A^{2} + B^{2}) + (AB + BA) $$
$$ = \left( \begin{array}{cc} 4 & 0 \\ 1 & 3 \end{array} \right) + \left( \begin{array}{cc} -1 & -3 \\ -2 & 1 \end{array} \right) = \left( \begin{array}{cc} 3 & -3 \\ -1 & 4 \end{array} \right) $$
따라서 $(A+B)^{2}$의 모든 성분의 합은 
$$ 3 + (-3) + (-1) + 4 = 3 $$
이다.

정답: ②