## ë¬¸ì œ
$0 \le x \le 2$ ì—ì„œ í•¨ìˆ˜ $y=f(x)$ ì˜ ê·¸ë˜í”„ê°€ ì˜¤ë¥¸ìª½ ê·¸ë¦¼ê³¼ ê°™ì„ ë•Œ, $f^{2002} (\frac{5}{4})$ ì˜ ê°’ì€?

> [!example] ğŸ“¸ (ê·¸ë¦¼/ê·¸ë˜í”„)

(ë‹¨, $f^{1}(x)=f(x)$, $f^{2}(x)=f(f(x))$, $f^{3}(x)=f (f^{2}(x) )$, $\cdots$, $f^{n+1}(x)=f (f^{n}(x) )$, $n$ ì€ ìì—°ìˆ˜)

## ë³´ê¸°
â‘  $0$   â‘¡ $1$   â‘¢ $\frac{3}{2}$   â‘£ $\frac{5}{4}$   â‘¤ $2$

## í’€ì´
í•¨ìˆ˜ $y=f(x)$ ì˜ ê·¸ë˜í”„ì—ì„œ
$f (\frac{5}{4} )=\frac{3}{2}$, $f (\frac{3}{2} )=1$, $f(1)=2$, $f(2)=0$, $f(0)=1$ ì´ë¯€ë¡œ

$f^{2} (\frac{5}{4} )=f (f (\frac{5}{4} ) )=f (\frac{3}{2} )=1$
$f^{3} (\frac{5}{4} )=f (f^{2} (\frac{5}{4} ) )=f(1)=2$
$f^{4} (\frac{5}{4} )=f (f^{3} (\frac{5}{4} ) )=f(2)=0$
$f^{5} (\frac{5}{4} )=f (f^{4} (\frac{5}{4} ) )=f(0)=1$
$f^{6} (\frac{5}{4} )=f (f^{5} (\frac{5}{4} ) )=f(1)=2$

ë”°ë¼ì„œ, $f^{n} (\frac{5}{4} )$ ì€ $\frac{3}{2}$, $1$, $2$, $0$, $1$, $2$, $0$, $\cdots$ ì™€ ê°™ì´ $n \ge 2$ ì¼ ë•Œ, $1$, $2$, $0$ ì˜ ê°’ì´ ë°˜ë³µë˜ë¯€ë¡œ 
$\therefore f^{2002} (\frac{5}{4} )=f^{3 \times 666+4} (\frac{5}{4} )=f^{4} (\frac{5}{4} )=0$

ì •ë‹µ: â‘ 