## 문제
이차정사각행렬 $A$, $B$가 
$$(A-B)^{2} = \left( \begin{array}{cc} 5 & 3 \\ 3 & 2 \end{array} \right), A^{2} + B^{2} = \left( \begin{array}{cc} 4 & 0 \\ 1 & 3 \end{array} \right)$$
를 만족할 때, 행렬 $(A+B)^{2}$의 모든 성분의 합은?

## 보기
① $1$   ② $3$   ③ $5$   ④ $7$   ⑤ $9$

## 풀이
$$(A-B)^{2} = A^{2} - AB - BA + B^{2} = \left( \begin{array}{cc} 5 & 3 \\ 3 & 2 \end{array} \right)$$ 

따라서 
$$AB + BA = (A^{2} + B^{2}) - (A-B)^{2}$$ 
$$= \left( \begin{array}{cc} 4 & 0 \\ 1 & 3 \end{array} \right) - \left( \begin{array}{cc} 5 & 3 \\ 3 & 2 \end{array} \right) = \left( \begin{array}{cc} -1 & -3 \\ -2 & 1 \end{array} \right)$$ 

$$(A+B)^{2} = A^{2} + AB + BA + B^{2} = (A^{2} + B^{2}) + (AB + BA)$$ 
$$= \left( \begin{array}{cc} 4 & 0 \\ 1 & 3 \end{array} \right) + \left( \begin{array}{cc} -1 & -3 \\ -2 & 1 \end{array} \right) = \left( \begin{array}{cc} 3 & -3 \\ -1 & 4 \end{array} \right)$$ 

따라서 행렬 $(A+B)^{2}$의 모든 성분의 합은 
$$3 - 3 - 1 + 4 = 3$$ 

정답은 ②입니다.