## 문제
행렬 $A = \left( \begin{array}{cc} 1 & 1 \\ 4 & 3 \end{array} \right)$ 에 대하여 $(A^{2})^{-1}$ 의 모든 성분의 합을 구하시오. (단, $X^{-1}$ 는 $X$ 의 역행렬이다.)

## 풀이
$$ A^{2} = \left( \begin{array}{cc} 1 & 1 \\ 4 & 3 \end{array} \right) \left( \begin{array}{cc} 1 & 1 \\ 4 & 3 \end{array} \right) $$
$$ = \left( \begin{array}{cc} 5 & 4 \\ 16 & 13 \end{array} \right) $$
$$ (A^{2})^{-1} = \left( \begin{array}{cc} 5 & 4 \\ 16 & 13 \end{array} \right)^{-1} $$
$$ = \frac{1}{5 \times 13 - 4 \times 16} \left( \begin{array}{cc} 13 & -4 \\ -16 & 5 \end{array} \right) $$
$$ = \left( \begin{array}{cc} 13 & -4 \\ -16 & 5 \end{array} \right) $$
따라서, $(A^{2})^{-1}$ 의 모든 성분의 합은 $13 + (-16) + (-4) + 5 = -2$ 이다.

정답: $-2$