## ë¬¸ì œ
ì§‘í•© $X=\{1, 2, 3, 4\}$ì— ëŒ€í•˜ì—¬ í•¨ìˆ˜ $f: X \to X$ë¥¼ ë‹¤ìŒê³¼ ê°™ì´ ì •ì˜í•˜ì˜€ë‹¤.

$$
\begin{array}{c|c|c|c|c}
\hline x & 1 & 2 & 3 & 4 \\
\hline f(x) & 2 & 3 & 4 & 1 \\
\hline
\end{array}
$$

í•¨ìˆ˜ $g: X \to X$ì— ëŒ€í•˜ì—¬ $g(1)=3$ì´ê³ , $f \circ g = g \circ f$ê°€ ì„±ë¦½í•  ë•Œ, $g(2)+g(3)$ì˜ ê°’ì„ êµ¬í•˜ì‹œì˜¤.



> [!example] ğŸ“¸ (ê·¸ë¦¼/ê·¸ë˜í”„)

## ë³´ê¸°
â‘  $1$   â‘¡ $2$   â‘¢ $3$   â‘£ $4$   â‘¤ $5$

## í’€ì´
$g(1)=3$ì´ë¯€ë¡œ 
$(f \circ g)(1)=f(g(1))=f(3)=4$ì—ì„œ 
$(g \circ f)(1)=g(f(1))=g(2)=4$ 

$g(2)=4$ì´ë¯€ë¡œ 
$(f \circ g)(2)=f(g(2))=f(4)=1$ì—ì„œ 
$(g \circ f)(2)=g(f(2))=g(3)=1$ 

$\therefore g(2)+g(3)=5$