## ๋ฌธ์
๋ชจ๋ ์ค์ $x$ ์ ๋ํ์ฌ $y=f(x)$ ๊ฐ $f(x-2)=f(x+2)$ ๋ฅผ ๋ง์กฑํ๋ ๊ทธ๋ํ์ ์ผ๋ถ๊ฐ ์ค๋ฅธ์ชฝ ๊ทธ๋ฆผ๊ณผ ๊ฐ๋ค. $-2 \leq x \leq 2$ ์ ๋ฒ์์์ $y=\frac{1}{2} \{ f(x-1)+f(x+3) \}$ ์ ๊ทธ๋ํ๋ก ์๋ง์ ๊ฒ์?

> [!example] ๐ธ (๊ทธ๋ฆผ/๊ทธ๋ํ)

## ๋ณด๊ธฐ
โ > [!example] ๐ธ (๊ทธ๋ฆผ/๊ทธ๋ํ)   โก > [!example] ๐ธ (๊ทธ๋ฆผ/๊ทธ๋ํ)   โข > [!example] ๐ธ (๊ทธ๋ฆผ/๊ทธ๋ํ)   โฃ > [!example] ๐ธ (๊ทธ๋ฆผ/๊ทธ๋ํ)   โค > [!example] ๐ธ (๊ทธ๋ฆผ/๊ทธ๋ํ)

## ํ์ด
$f(x-2)=f(x+2)$ ์์ $f(x)=f(x+4)$ ์ด๋ฏ๋ก $f(x)$ ๋ ์ฃผ๊ธฐ๊ฐ $4$ ์ธ ํจ์์ด๋ค. ๊ทธ๋ฌ๋ฏ๋ก 
$$ f(x+3)=f((x+4)-1)=f(x-1) $$
$$ y = \frac{1}{2} \{ f(x-1)+f(x+3) \} $$
$$ = \frac{1}{2} \{ f(x-1)+f(x-1) \} $$
$$ = f(x-1) $$
๋ฐ๋ผ์, ๊ตฌํ๊ณ์ ํ๋ ๊ทธ๋ํ๋ $y=f(x)$ ์ ๊ทธ๋ํ๋ฅผ $x$ ์ถ ๋ฐฉํฅ์ผ๋ก $1$ ๋งํผ ํํ์ด๋ํ ๊ฒ์ด๋ค.

์๋ต: โก