## 문제
두 행렬 $A = \left( \begin{array}{cc} 2 & 1 \\ 3 & 2 \end{array} \right)$ 와 $B = \left( \begin{array}{cc} 5 & -3 \\ 4 & 1 \end{array} \right)$ 에 대하여 행렬 $(A B^{-1} )^{-1}$ 의 모든 성분의 합을 구하시오.

## 보기

## 풀이
[정답] $11$

$(A B^{-1})^{-1} = (B^{-1})^{-1} A^{-1} = B A^{-1}$ 

$A^{-1} = \frac{1}{2 \cdot 2 - 1 \cdot 3} \left( \begin{array}{cc} 2 & -1 \\ -3 & 2 \end{array} \right) = \left( \begin{array}{cc} 2 & -1 \\ -3 & 2 \end{array} \right)$

$\therefore (A B^{-1} )^{-1} = B A^{-1}$
$= \left( \begin{array}{cc} 5 & -3 \\ 4 & 1 \end{array} \right) \left( \begin{array}{cc} 2 & -1 \\ -3 & 2 \end{array} \right)$
$= \left( \begin{array}{cc} 19 & -11 \\ 5 & -2 \end{array} \right)$

따라서, 구하는 모든 성분의 합은 
$19 + (-11) + 5 + (-2) = 11$