## 문제
$x = \sqrt{2}$ 일 때, $\frac{3}{x - \frac{x - 1}{x + 1}}$ 의 값은?

## 보기
① $\sqrt{2} + 1$   ② $2(\sqrt{2} + 1)$   ③ $3(\sqrt{2} + 1)$   ④ $4(\sqrt{2} + 1)$   ⑤ $5(\sqrt{2} + 1)$

## 풀이
주어진 식을 정리하면 다음과 같다.
$$ \frac{3}{x - \frac{x - 1}{x + 1}} = \frac{3(x + 1)}{x(x + 1) - (x - 1)} $$
$$ = \frac{3(x + 1)}{x^{2} + x - x + 1} = \frac{3(x + 1)}{x^{2} + 1} $$
식에 $x = \sqrt{2}$ 를 대입하면,
$$ \frac{3(\sqrt{2} + 1)}{(\sqrt{2})^{2} + 1} = \frac{3(\sqrt{2} + 1)}{2 + 1} = \frac{3(\sqrt{2} + 1)}{3} = \sqrt{2} + 1 $$

따라서 정답은 ①이다.