## 문제
행렬 $A$, $B$에 대하여,
$$ A+B = \left( \begin{array}{cc} -2 & 1 \\ -1 & 1 \end{array} \right), A-B = \left( \begin{array}{cc} 2 & -1 \\ 3 & 3 \end{array} \right) $$
일 때, $A^{2}-B^{2}$은?

## 보기
① $\left( \begin{array}{cc} -2 & 3 \\ -4 & 5 \end{array} \right)$   ② $\left( \begin{array}{cc} 2 & -3 \\ -4 & 5 \end{array} \right)$   ③ $\left( \begin{array}{cc} -1 & 5 \\ 1 & 4 \end{array} \right)$   ④ $\left( \begin{array}{cc} 1 & -5 \\ -1 & 4 \end{array} \right)$   ⑤ $\left( \begin{array}{cc} 2 & 5 \\ -1 & 4 \end{array} \right)$

## 풀이
$$ A+B = \left( \begin{array}{cc} -2 & 1 \\ -1 & 1 \end{array} \right) \cdots (1) $$
$$ A-B = \left( \begin{array}{cc} 2 & -1 \\ 3 & 3 \end{array} \right) \cdots (2) $$

$(1)+(2)$ 하면
$$ 2A = \left( \begin{array}{cc} 0 & 0 \\ 2 & 4 \end{array} \right), A = \left( \begin{array}{cc} 0 & 0 \\ 1 & 2 \end{array} \right) $$

$(1)-(2)$ 하면
$$ 2B = \left( \begin{array}{cc} -4 & 2 \\ -4 & -2 \end{array} \right), B = \left( \begin{array}{cc} -2 & 1 \\ -2 & -1 \end{array} \right) $$

$$ A^{2} = \left( \begin{array}{cc} 0 & 0 \\ 1 & 2 \end{array} \right) \left( \begin{array}{cc} 0 & 0 \\ 1 & 2 \end{array} \right) = \left( \begin{array}{cc} 0 & 0 \\ 2 & 4 \end{array} \right) $$
$$ B^{2} = \left( \begin{array}{cc} -2 & 1 \\ -2 & -1 \end{array} \right) \left( \begin{array}{cc} -2 & 1 \\ -2 & -1 \end{array} \right) = \left( \begin{array}{cc} 2 & -3 \\ 6 & -1 \end{array} \right) $$

따라서
$$ A^{2}-B^{2} = \left( \begin{array}{cc} 0 & 0 \\ 2 & 4 \end{array} \right) - \left( \begin{array}{cc} 2 & -3 \\ 6 & -1 \end{array} \right) = \left( \begin{array}{cc} -2 & 3 \\ -4 & 5 \end{array} \right) $$

정답은 ①이다.