## ๋ฌธ์
์ค์ $x$ ์ ๋ํ์ฌ ์์๋ ๋ ํจ์ $f(x) = x - [x]$ ์ $g(x) = [x] + 1$ ์ ๋ํ์ฌ ๋ค์ ์ค $y = (g \circ f)(x)$ ์ ๊ทธ๋ํ์ ๊ฐํ์?
(๋จ, $[x]$ ๋ $x$ ๋ฅผ ๋์ง ์๋ ์ต๋์์์ด๋ค.)

## ๋ณด๊ธฐ
โ > [!example] ๐ธ (๊ทธ๋ฆผ/๊ทธ๋ํ)
โก > [!example] ๐ธ (๊ทธ๋ฆผ/๊ทธ๋ํ)
โข > [!example] ๐ธ (๊ทธ๋ฆผ/๊ทธ๋ํ)
โฃ > [!example] ๐ธ (๊ทธ๋ฆผ/๊ทธ๋ํ)
โค > [!example] ๐ธ (๊ทธ๋ฆผ/๊ทธ๋ํ)

## ํ์ด
$f(x) = x - [x]$ ์์ 
$0 \leq f(x) < 1$ ์ด๋ฏ๋ก 
๋ชจ๋ ์ค์ $x$ ์ ๋ํ์ฌ $[f(x)] = 0$ ์ด๋ค.

$\therefore (g \circ f)(x) = g(f(x)) = [f(x)] + 1 = 0 + 1 = 1$

๋ฐ๋ผ์ ํจ์ $y = (g \circ f)(x)$ ์ ๊ทธ๋ํ๋ $y = 1$ ์ธ ์์ํจ์์ด๋ค.

์๋ต: โ