## 문제
이차방정식 $x^{2}+x+1=0$의 두 근을 $\alpha$, $\beta$라 할 때, $\frac{(\alpha^{2}+1)(\beta^{2}+1)}{\alpha+\beta}$의 값은?

## 보기
① $-2$   ② $-1$   ③ $1$   ④ $2$   ⑤ $3$

## 풀이
근과 계수의 관계에 의해 
$\alpha+\beta=-1$, $\alpha\beta=1$이다.

$x^{2}+x+1=0$의 두 근이 $\alpha$, $\beta$이므로 
$\alpha^{2}+\alpha+1=0$, $\beta^{2}+\beta+1=0$이다.

$\therefore \alpha^{2}+1=-\alpha$, $\beta^{2}+1=-\beta$

따라서 구하고자 하는 값은
$\frac{(\alpha^{2}+1)(\beta^{2}+1)}{\alpha+\beta} = \frac{(-\alpha)(-\beta)}{\alpha+\beta} = \frac{\alpha\beta}{\alpha+\beta} = \frac{1}{-1} = -1$

정답: ②