## ๋ฌธ์
์์์ ์ค์ $x$ ์ ๋ํ์ฌ ๋ถ๋ฑ์ $x^{2} + 2 a x + 2 b - b^{2} \geq 0$ ์ด ์ฑ๋ฆฝํ ๋, ๋ค์ ์ค ์ $P(a, b)$ ๊ฐ ์กด์ฌํ๋ ์์ญ์ผ๋ก ์๋ง์ ๊ฒ์?

## ๋ณด๊ธฐ
โ > [!example] ๐ธ (๊ทธ๋ฆผ/๊ทธ๋ํ)   โก > [!example] ๐ธ (๊ทธ๋ฆผ/๊ทธ๋ํ)   โข > [!example] ๐ธ (๊ทธ๋ฆผ/๊ทธ๋ํ)   โฃ > [!example] ๐ธ (๊ทธ๋ฆผ/๊ทธ๋ํ)   โค > [!example] ๐ธ (๊ทธ๋ฆผ/๊ทธ๋ํ)

## ํ์ด
์๋ต: โก

์์์ ์ค์ $x$ ์ ๋ํ์ฌ ๋ถ๋ฑ์ $x^{2} + 2 a x + 2 b - b^{2} \geq 0$ ์ด๋ฏ๋ก ํ๋ณ์์ $D$ ๋ผ ํ๋ฉด
$\frac{D}{4} = a^{2} - (2 b - b^{2}) \leq 0$
$a^{2} + b^{2} - 2 b \leq 0$
$\therefore a^{2} + (b - 1)^{2} \leq 1$
์ด๊ฒ์ ์ขํํ๋ฉด์ ๋ํ๋ด๋ฉด โก๋ฒ์ด๋ค.