## 문제
$f(x)=x^{3}-3 x^{2}+\int_{0}^{2} g(t) dt$, $g(x)=3 x^{2}+2+\int_{-1}^{1} f(t) dt$ 일 때, $f(x)+g(x)$ 는?

## 보기
① $x^{3}-8$   ② $x^{3}-12$   ③ $x^{3}-\frac{8}{3}$   ④ $x^{3}-\frac{16}{3}$   ⑤ $x^{3}-16$

## 풀이
$$ \begin{array}{l} a = \int_{0}^{2} g(t) dt, \quad b = \int_{-1}^{1} f(t) dt \text{ 라 하면} \\ f(x)=x^{3}-3 x^{2}+a, \quad g(x)=3 x^{2}+2+b \text{ 이다.} \\ a = \int_{0}^{2} (3 t^{2}+2+b ) dt = [ t^{3}+(2+b) t ]_{0}^{2} \\ a = (8-0)+(4+2 b)=2 b+12 \quad \cdots (1) \\ b = \int_{-1}^{1} (x^{3}-3 x^{2}+a ) dx = 2 \int_{0}^{1} (-3 x^{2}+a ) dx \\ b = 2 [ -x^{3}+a x ]_{0}^{1}=2 a-2 \quad \cdots (2) \\ \text{식 (1)과 (2)로부터 } a=-\frac{8}{3}, \quad b=-\frac{22}{3} \\ g(x) = 3x^{2} + 2 - \frac{22}{3} = 3x^{2} - \frac{16}{3} \\ \therefore f(x)+g(x)= \left(x^{3}-3 x^{2}-\frac{8}{3} \right)+ \left(3 x^{2}-\frac{16}{3} \right)=x^{3}-8 \end{array} $$

정답: ①