## 문제
$a_{1} = 1$, $a_{n+1} = a_{n} + f(n)$ ($n = 1, 2, 3, \dots$)으로 정의되는 수열 $\{ a_{n} \}$에서 $\sum_{k=1}^{n} f(k) = n^{2} - 1$일 때, $a_{2004}$의 값은?

## 보기
① $2003^{2}$   ② $2003^{2} - 1$   ③ $2003 \times 2004$   ④ $2004^{2}$   ⑤ $2004^{2} - 1$

## 풀이
$a_{n+1} = a_{n} + f(n)$에서
$a_{n+1} - a_{n} = f(n)$이므로
$a_{n} = 1 + \sum_{k=1}^{n-1} f(k)$ (∵ $a_{1} = 1$)
양변에 $f(n)$을 더하면
$a_{n} + f(n) = 1 + \sum_{k=1}^{n} f(k)$
문제에서 $a_{n+1} = a_{n} + f(n)$이고 $\sum_{k=1}^{n} f(k) = n^{2} - 1$이므로
$a_{n+1} = 1 + (n^{2} - 1) = n^{2}$ ($n = 1, 2, 3, \dots$)
$\therefore a_{2004} = a_{2003+1} = 2003^{2}$

[정답] ①