## 문제
자연수의 집합에서 정의된 함수 $f$ 가 다음 조건을 만족한다.

$f(1)=1$, $f(1)+f(2)+ \cdots +f(n)=n^{2} \cdot f(n)$

이때, $f(2003)$ 을 구하면?

## 보기
① $\frac{1}{2003}$   ② $\frac{3}{2005}$   ③ $\frac{1}{2003 \cdot 1003}$   ④ $\frac{1}{1002 \cdot 2003}$   ⑤ $\frac{1}{1002 \cdot 2005}$

## 풀이
$f(1)=a_{1}$, $f(2)=a_{2}$, $\cdots$, $f(n)=a_{n}$ 이라 하면,
$S_{n} = a_{1} + a_{2} + \cdots + a_{n} = n^{2} \cdot a_{n} \cdots$ ①
$S_{n+1} = (n+1)^{2} a_{n+1} \cdots$ ②

그러므로
$S_{n+1} - S_{n} = a_{n+1} = (n+1)^{2} a_{n+1} - n^{2} a_{n}$
$\frac{a_{n+1}}{a_{n}} = \frac{n^{2}}{(n+1)^{2}-1} = \frac{n^{2}}{n(n+2)} = \frac{n}{n+2} \cdots$ ③

식 ③은 $n=1$, $2$, $3$, $\cdots$ 인 경우 다음과 같다.
$n=1$ 일 때 : $\frac{a_{2}}{a_{1}} = \frac{1}{3}$
$n=2$ 일 때 : $\frac{a_{3}}{a_{2}} = \frac{2}{4}$
$n=3$ 일 때 : $\frac{a_{4}}{a_{3}} = \frac{3}{5}$
$\vdots$
$n=n-2$ 일 때 : $\frac{a_{n-1}}{a_{n-2}} = \frac{n-2}{n}$
$n=n-1$ 일 때 : $\frac{a_{n}}{a_{n-1}} = \frac{n-1}{n+1}$

따라서, 모든 변을 곱하면
$\frac{a_{n}}{a_{1}} = \frac{1 \cdot 2}{n(n+1)} = \frac{2}{n(n+1)}$,
$\therefore a_{n} = \frac{2}{n(n+1)}$

$\therefore f(2003) = a_{2003} = \frac{2}{2003 \cdot 2004} = \frac{1}{2003 \cdot 1002}$
정답은 ④이다.