## 문제
방정식 $x^{3}=1$의 한 허근을 $\omega$라 할 때, 〈보기〉 중 옳은 것을 모두 고르면?

$$ \begin{array}{|l|} \hline \text{〈보기〉} \\ \text{ㄱ. } (1+\omega)^{2}=\omega \\ \text{ㄴ. } (1+\omega)^{10}=-\omega^{2} \\ \text{ㄷ. 모든 자연수 } n \text{에 대하여 } (1+\omega)^{3n}=(-1)^{n} \\ \hline \end{array} $$

## 보기
① $ㄱ$   ② $ㄴ$   ③ $ㄱ, ㄴ$   ④ $ㄱ, ㄷ$   ⑤ $ㄱ, ㄴ, ㄷ$

## 풀이
$\omega$는 $x^{3}-1=(x-1)(x^{2}+x+1)=0$의 근이므로
$\omega^{3}=1$, $\omega^{2}+\omega+1=0$
따라서 $1+\omega=-\omega^{2}$

$(1+\omega)^{2}=(-\omega^{2})^{2}=\omega^{4}=\omega$
$(1+\omega)^{3}=(-\omega^{2})^{3}=-(\omega^{3})^{2}=-1^{2}=-1$
$(1+\omega)^{4}=(1+\omega)^{3}(1+\omega)=-(1+\omega)$
$(1+\omega)^{5}=(1+\omega)^{3}(1+\omega)^{2}=-(1+\omega)^{2}$
$(1+\omega)^{6}=(1+\omega)^{3}(1+\omega)^{3}=(-1)(-1)=1$
$\cdots \cdots$

$\therefore (1+\omega)^{10}=(1+\omega)^{6}(1+\omega)^{4}=(1+\omega)^{4}=-(1+\omega)=\omega^{2}$

또, $(1+\omega)^{3}=(1+\omega)^{9}=\cdots=-1$
$(1+\omega)^{6}=(1+\omega)^{12}=\cdots=1$이므로
$(1+\omega)^{3n}=(-1)^{n}$

따라서 옳은 것은 $ㄱ$, $ㄷ$

정답 $④$