## 문제
$a_{1}=1$ 이고 $\lim_{n \to \infty} n^{2} a_{n}=0$ 인 수열 $\{ a_{n} \}$ 에 대하여 $\sum_{n=1}^{\infty} a_{n}=A$, $\sum_{n=1}^{\infty} n a_{n}=B$ ($A$, $B$ 는 상수)라 할 때, $\sum_{n=1}^{\infty} (n+1)^{2} (a_{n+1}-a_{n} )$ 을 구하면?

## 보기
① $-A-2 B-1$   ② $-A-B-1$   ③ $-A-2 B+1$   ④ $-A+B-1$   ⑤ $A+2 B-1$

## 풀이
$\sum_{n=1}^{\infty} (n+1)^{2} (a_{n+1}-a_{n} )$
$= \lim_{n \to \infty} \sum_{k=1}^{n} (k+1)^{2} (a_{k+1}-a_{k} )$
$= \lim_{n \to \infty} \{ 2^{2} (a_{2}-a_{1} )+3^{2} (a_{3}-a_{2} )+ \cdots +(n+1)^{2} (a_{n+1}-a_{n} ) \}$
$= \lim_{n \to \infty} [ - \{ 4 a_{1}+5 a_{2}+7 a_{3}+ \cdots +(2 n+1) a_{n} \} + (n+1)^{2} a_{n+1} ]$
$= \lim_{n \to \infty} [ -a_{1} - \{ 3 a_{1}+5 a_{2}+7 a_{3}+ \cdots +(2 n+1) a_{n} \} ] + \lim_{n \to \infty} (n+1)^{2} a_{n+1}$
$= \lim_{n \to \infty} \{ -a_{1} - \sum_{k=1}^{n} (2 k+1) a_{k} \}$
(∵ $\lim_{n \to \infty} n^{2} a_{n} = \lim_{n \to \infty} (n+1)^{2} a_{n+1} = 0$)
$= -a_{1} - \sum_{n=1}^{\infty} (2 n+1) a_{n}$
$= -a_{1} - 2 \sum_{n=1}^{\infty} n a_{n} - \sum_{n=1}^{\infty} a_{n}$
$= -1 - 2 B - A$
$= -A - 2 B - 1$

정답: ①