## 문제
두 행렬 $A = \left( \begin{array}{rr} 1 & -1 \\ -1 & -1 \end{array} \right)$, $B = \left( \begin{array}{rr} 1 & 1 \\ -1 & 0 \end{array} \right)$ 에 대하여 $AB - A$ 는?

## 보기
① $\left( \begin{array}{rr} 1 & 2 \\ 1 & 0 \end{array} \right)$   ② $\left( \begin{array}{rr} 1 & 0 \\ 0 & 2 \end{array} \right)$   ③ $\left( \begin{array}{rr} 1 & 1 \\ 1 & 0 \end{array} \right)$   ④ $\left( \begin{array}{rr} 2 & 0 \\ 0 & 2 \end{array} \right)$   ⑤ $\left( \begin{array}{rr} 0 & 1 \\ 2 & 0 \end{array} \right)$

## 풀이
정답 ①

$$ AB - A = A ( B - E ) $$
$$ = \left( \begin{array}{rr} 1 & -1 \\ -1 & -1 \end{array} \right) \left( \begin{array}{rr} 0 & 1 \\ -1 & -1 \end{array} \right) $$
$$ = \left( \begin{array}{rr} 1 & 2 \\ 1 & 0 \end{array} \right) $$

두 행렬 $A = \left( \begin{array}{rr} 1 & -1 \\ -1 & -1 \end{array} \right)$, $B = \left( \begin{array}{rr} 1 & 1 \\ -1 & 0 \end{array} \right)$ 에 대하여 계산하면 위와 같다.