## ๋ฌธ์

์ค์ $a$ ($a > 1$)์ ๋ํ์ฌ $b = \sum_{n=1}^{\infty} \left( \frac{1}{a} \right)^{n}$์ [๊ทธ๋ฆผ $1$]๊ณผ ๊ฐ์ด ๋ํ๋ด๊ณ, ์ค์ $c$์ ๋ํ์ฌ $d = 16^{c}$์ [๊ทธ๋ฆผ $2$]์ ๊ฐ์ด ๋ํ๋ด๊ธฐ๋ก ํ๋ค.

> [!example] ๐ธ (๊ทธ๋ฆผ/๊ทธ๋ํ)
[๊ทธ๋ฆผ $1$]

> [!example] ๐ธ (๊ทธ๋ฆผ/๊ทธ๋ํ)
[๊ทธ๋ฆผ $2$]

์๋ ๊ทธ๋ฆผ์ ์ค์ $x$, $y$, $z$์ ๋ํ์ฌ $\frac{xz}{y}$์ ๊ฐ์ ๊ตฌํ์์ค.

> [!example] ๐ธ (๊ทธ๋ฆผ/๊ทธ๋ํ)

## ํ์ด

[๊ทธ๋ฆผ $1$]์ ๊ด๊ณ์์์ 
$$1 = \sum_{n=1}^{\infty} \left( \frac{1}{z} \right)^{n} = \frac{\frac{1}{z}}{1 - \frac{1}{z}} = \frac{1}{z - 1}$$
($\because z > 1$์ด๋ฏ๋ก $\left| \frac{1}{z} \right| < 1$)
์ฆ, $z - 1 = 1$์์ $z = 2$์ด๋ค.

> [!example] ๐ธ (๊ทธ๋ฆผ/๊ทธ๋ํ)

[๊ทธ๋ฆผ $2$]์ ๊ด๊ณ์์์
$$2 = 16^{y} \Rightarrow y = \frac{1}{4}$$

๋ํ, 
> [!example] ๐ธ (๊ทธ๋ฆผ/๊ทธ๋ํ)

[๊ทธ๋ฆผ $1$]์ ๊ด๊ณ์์์
$$\frac{1}{4} = \sum_{n=1}^{\infty} \left( \frac{1}{x} \right)^{n} = \frac{\frac{1}{x}}{1 - \frac{1}{x}} = \frac{1}{x - 1}$$
($\because x > 1$์ด๋ฏ๋ก $\left| \frac{1}{x} \right| < 1$)
์ฆ, $x - 1 = 4$์์ $x = 5$์ด๋ค.

๋ฐ๋ผ์ ๊ตฌํ๊ณ์ ํ๋ ๊ฐ์
$$\therefore \frac{xz}{y} = \frac{5 \cdot 2}{\frac{1}{4}} = 40$$