## 문제
두 행렬 $A = \left( \begin{array}{cc} -3 & 2 \\ -2 & 1 \end{array} \right)$, $E = \left( \begin{array}{cc} 1 & 0 \\ 0 & 1 \end{array} \right)$이 $A = (p A + q E)^{-1}$를 만족하도록 상수 $p$, $q$의 값을 정할 때, $p + q$의 값은?

## 보기
① $3$   ② $1$   ③ $0$   ④ $-1$   ⑤ $-3$

## 풀이
$A = (p A + q E)^{-1}$ 이면 
$$ A^{-1} = p A + q E $$ 
이다.
$$ A^{-1} = \left( \begin{array}{cc} 1 & -2 \\ 2 & -3 \end{array} \right) $$
$$ = p \left( \begin{array}{cc} -3 & 2 \\ -2 & 1 \end{array} \right) + q \left( \begin{array}{cc} 1 & 0 \\ 0 & 1 \end{array} \right) $$
$$ = \left( \begin{array}{cc} -3p + q & 2p \\ -2p & p + q \end{array} \right) $$
위의 행렬에서 성분을 비교하면
$2p = -2$ 이므로 $p = -1$ 이고,
$p + q = -3$ 임을 알 수 있다.

$\therefore p + q = -3$

정답: ⑤