## 문제
$f(x) = \sqrt{4x + 2\sqrt{4x^{2} - 1}}$ ($x \ge 1$)에 대하여
$\frac{1}{f(1)} + \frac{1}{f(2)} + \frac{1}{f(3)} + \cdots + \frac{1}{f(59)} + \frac{1}{f(60)}$의 값을 구하시오.

## 보기
① $1$   ② $2$   ③ $3$   ④ $4$   ⑤ $5$

## 풀이
$f(x) = \sqrt{4x + 2\sqrt{4x^{2} - 1}} = \sqrt{(2x+1) + (2x-1) + 2\sqrt{(2x+1)(2x-1)}} = \sqrt{2x+1} + \sqrt{2x-1}$ 이므로
$\frac{1}{f(x)} = \frac{1}{\sqrt{2x+1} + \sqrt{2x-1}} = \frac{\sqrt{2x+1} - \sqrt{2x-1}}{(2x+1) - (2x-1)} = \frac{1}{2}(\sqrt{2x+1} - \sqrt{2x-1})$ 이다.

따라서 구하는 식의 값은 다음과 같다.
$\frac{1}{2} \{ (\sqrt{3} - \sqrt{1}) + (\sqrt{5} - \sqrt{3}) + \cdots + (\sqrt{121} - \sqrt{119}) \}$
$= \frac{1}{2}(-1 + 11) = 5$

정답은 ⑤이다.