## ๋ฌธ์
$x$์ ๊ฐ์ ๊ด๊ณ์์ด ์ $\frac{a-3x}{x+b}$ ๊ฐ ํญ์ ์ผ์ํ ๊ฐ์ ๊ฐ์ง ๋, ์ค์ $a$์ $b$์ ๊ด๊ณ๋ฅผ ๋ํ๋ธ ๊ทธ๋ํ๋ก ๊ฐ์ฅ ์์ํ ๊ฒ์? (๋จ, $x \neq -b$)

## ๋ณด๊ธฐ
โ > [!example] ๐ธ (๊ทธ๋ฆผ/๊ทธ๋ํ)
โก > [!example] ๐ธ (๊ทธ๋ฆผ/๊ทธ๋ํ)
โข > [!example] ๐ธ (๊ทธ๋ฆผ/๊ทธ๋ํ)
โฃ > [!example] ๐ธ (๊ทธ๋ฆผ/๊ทธ๋ํ)
โค > [!example] ๐ธ (๊ทธ๋ฆผ/๊ทธ๋ํ)

## ํ์ด
$\frac{a-3x}{x+b} = p$๋ผ ๋์ผ๋ฉด,
$px + bp = -3x + a$ $\cdots\cdots$ ใ
ใ์ $x$์ ๋ํ ํญ๋ฑ์์ด๋ฏ๋ก $p = -3$, $bp = a$์ด๋ค.
๋ฐ๋ผ์ $b = -\frac{1}{3}a$์ ๊ทธ๋ํ๋ โ๋ฒ์ด๋ค.

์๋ต: โ