## ë¬¸ì œ
ë‘ í•¨ìˆ˜ $f(x)$, $g(x)$ì˜ ê·¸ë˜í”„ê°€ ì•„ë˜ ê·¸ë¦¼ê³¼ ê°™ì„ ë•Œ <ë³´ê¸°>ì—ì„œ ì˜³ì€ ê²ƒì„ ëª¨ë‘ ê³ ë¥¸ ê²ƒì€?

> [!example] ğŸ“¸ (ê·¸ë¦¼/ê·¸ë˜í”„)

ã„±. $\lim_{x \to -2} \{f(x)+5g(x)\} = -4$
ã„´. $\lim_{x \to 1} f(x)g(x) = -4$
ã„·. $\lim_{x \to 2} \frac{f(x)}{g(x)} = 0$

## ë³´ê¸°
â‘  ã„±   â‘¡ ã„´   â‘¢ ã„±, ã„´   â‘£ ã„±, ã„·   â‘¤ ã„±, ã„´, ã„·

## í’€ì´
ã„±. $\lim_{x \to -2} f(x) = 1$, $\lim_{x \to -2} g(x) = -1$ ì´ë¯€ë¡œ 
$\therefore \lim_{x \to -2} \{f(x)+5g(x)\} = -4$ (ì°¸) 

ã„´. $\lim_{x \to 1} f(x) = 2$, $\lim_{x \to 1-} g(x) = -2$, $\lim_{x \to 1+} g(x) = -1$ ì´ê³  
$\lim_{x \to 1-} f(x)g(x) = -4$, $\lim_{x \to 1+} f(x)g(x) = -2$ ì´ë¯€ë¡œ 
$\therefore \lim_{x \to 1} f(x)g(x) = -4$ (ê±°ì§“) 

ã„·. $\lim_{x \to 2} f(x) = 1$, $\lim_{x \to 2} g(x) = 0$ ì´ë¯€ë¡œ 
$\therefore \lim_{x \to 2} \frac{f(x)}{g(x)} = \infty$ (ê±°ì§“) 

ë”°ë¼ì„œ ì˜³ì€ ê²ƒì€ ã„±ì´ë‹¤.

ì •ë‹µ: â‘ 