## 문제
수열 $\{ a_{n} \}$ 에서 $a_{1} = 1$, $a_{n+1} = a_{n} + \frac{1}{4 n^{2} - 1}$ ($n \geq 1$) 일 때, $\lim_{n \to \infty} a_{n}$ 의 값은?

## 보기
① $\frac{1}{3}$   ② $\frac{1}{2}$   ③ $1$   ④ $\frac{5}{4}$   ⑤ $\frac{3}{2}$

## 풀이
수열 $\{ a_{n} \}$ 의 일반항을 구하면 다음과 같다.
$$ \begin{array}{l} a_{n} = a_{1} + \sum_{k=1}^{n-1} \frac{1}{4k^{2}-1} \\ = 1 + \sum_{k=1}^{n-1} \frac{1}{(2k-1)(2k+1)} \\ = 1 + \frac{1}{2} \sum_{k=1}^{n-1} \left( \frac{1}{2k-1} - \frac{1}{2k+1} \right) \\ = 1 + \frac{1}{2} \left\{ \left( 1 - \frac{1}{3} \right) + \left( \frac{1}{3} - \frac{1}{5} \right) + \cdots + \left( \frac{1}{2n-3} - \frac{1}{2n-1} \right) \right\} \\ = 1 + \frac{1}{2} \left( 1 - \frac{1}{2n-1} \right) \\ = 1 + \frac{n-1}{2n-1} \end{array} $$

따라서 극한값은 다음과 같다.
$$ \begin{array}{l} \therefore \lim_{n \to \infty} a_{n} = \lim_{n \to \infty} \left( 1 + \frac{n-1}{2n-1} \right) \\ = 1 + \frac{1}{2} = \frac{3}{2} \end{array} $$

정답: ⑤