## 문제
행렬 $A = \left( \begin{array}{cc} 3 & -1 \\ 5 & -3 \end{array} \right)$ 에 대하여 $(A^{8})^{-1} = \left( \begin{array}{cc} a & b \\ c & d \end{array} \right)$ 일 때, $a+d$ 의 값은?

## 보기
① $2^{-9}$   ② $2^{-8}$   ③ $2^{-7}$   ④ $2^{-6}$   ⑤ $2^{-5}$

## 풀이
$A^{2} = \left( \begin{array}{cc} 3 & -1 \\ 5 & -3 \end{array} \right) \left( \begin{array}{cc} 3 & -1 \\ 5 & -3 \end{array} \right) = \left( \begin{array}{cc} 4 & 0 \\ 0 & 4 \end{array} \right) = 4 E$

$A^{8} = (A^{2})^{4} = (4 E)^{4} = 4^{4} E = 2^{8} E$

$\therefore (A^{8})^{-1} = (2^{8} E)^{-1} = 2^{-8} E$

$(A^{8})^{-1} = \left( \begin{array}{cc} 2^{-8} & 0 \\ 0 & 2^{-8} \end{array} \right) = \left( \begin{array}{cc} a & b \\ c & d \end{array} \right)$ 이므로

$\therefore a+d = 2^{-8} + 2^{-8} = 2 \times 2^{-8} = 2^{-7}$

정답은 ③입니다.