## 문제
두 이차정사각행렬 $$ A = \left( \begin{array}{cc} 23 & -1 \\ -1 & 0 \end{array} \right) $$, $$ B = \left( \begin{array}{cc} 0 & -1 \\ -1 & -23 \end{array} \right) $$ 에 대하여 행렬 $$ A^{2} B + B^{-1} A B $$ 의 모든 성분의 합을 구하시오.

## 보기

## 풀이
$$ A = \left( \begin{array}{cc} 23 & -1 \\ -1 & 0 \end{array} \right) $$, $$ B = \left( \begin{array}{cc} 0 & -1 \\ -1 & -23 \end{array} \right) $$ 에서 

$$ AB = \left( \begin{array}{cc} 23 & -1 \\ -1 & 0 \end{array} \right) \left( \begin{array}{cc} 0 & -1 \\ -1 & -23 \end{array} \right) = \left( \begin{array}{cc} 1 & 0 \\ 0 & 1 \end{array} \right) = E $$ 

$$ B^{-1} = A = \left( \begin{array}{cc} 23 & -1 \\ -1 & 0 \end{array} \right) $$ 이므로 

$$ A^{2} B + B^{-1} AB = (A + B^{-1}) AB = A + B^{-1} = \left( \begin{array}{cc} 46 & -2 \\ -2 & 0 \end{array} \right) $$ 

$$ \therefore $$ 모든 성분의 합은 
$$ 46 + (-2) + (-2) + 0 = 42 $$

정답: $$ 42 $$