## ë¬¸ì œ
ìì—°ìˆ˜ $n$ì— ëŒ€í•˜ì—¬ ë‘ ì§€ìˆ˜ í•¨ìˆ˜ $y=5^{x}$, $y=3^{x}$ì˜ ê·¸ë˜í”„ì™€ ì§ì„  $x=n$ê³¼ì˜ êµì ì„ ê°ê° $P_{n}$, $Q_{n}$ì´ë¼ í•˜ì. ì´ë•Œ, $\lim_{n \to \infty} \frac{\overline{P_{n+1} Q_{n+1}}}{\overline{P_{n} Q_{n}}}$ì˜ ê°’ì€?



> [!example] ğŸ“¸ (ê·¸ë¦¼/ê·¸ë˜í”„)

## ë³´ê¸°
â‘  $1$   â‘¡ $2$   â‘¢ $3$   â‘£ $4$   â‘¤ $5$

## í’€ì´
ì  $P_{n}$ì˜ $y$ì¢Œí‘œëŠ” $5^{n}$, ì  $Q_{n}$ì˜ $y$ì¢Œí‘œëŠ” $3^{n}$ì´ë¯€ë¡œ $\overline{P_{n} Q_{n}} = 5^{n} - 3^{n}$ì´ë‹¤.
ë”°ë¼ì„œ êµ¬í•˜ê³ ì í•˜ëŠ” ê·¹í•œê°’ì€ ë‹¤ìŒê³¼ ê°™ë‹¤.
$$\lim_{n \to \infty} \frac{\overline{P_{n+1} Q_{n+1}}}{\overline{P_{n} Q_{n}}} = \lim_{n \to \infty} \frac{5^{n+1}-3^{n+1}}{5^{n}-3^{n}} = \lim_{n \to \infty} \frac{5 - 3 \cdot (\frac{3}{5})^{n}}{1 - (\frac{3}{5})^{n}} = 5$$

ì •ë‹µ: â‘¤