## 문제
일반항이 $S_n = \sum_{k=1}^{n} \left( \frac{1}{2} \right)^{k-1}$, $T_n = \sum_{k=1}^{n} \frac{1}{k(k+1)}$인 두 수열 $\{S_n\}$, $\{T_n\}$에 대하여 이차방정식 $x^2 - S_n x + T_n = 0$의 두 근을 $\alpha_n$, $\beta_n$이라 할 때, $\lim_{n \to \infty} (\alpha_n^2 + \beta_n^2)$의 값은?

## 보기
① $0$   ② $\frac{1}{2}$   ③ $1$   ④ $\frac{3}{2}$   ⑤ $2$

## 풀이
$S_n = \sum_{k=1}^{n} \left( \frac{1}{2} \right)^{k-1} = \frac{1 - \left( \frac{1}{2} \right)^n}{1 - \frac{1}{2}} = 2 - \left( \frac{1}{2} \right)^{n-1}$
$T_n = \sum_{k=1}^{n} \frac{1}{k(k+1)} = \sum_{k=1}^{n} \left( \frac{1}{k} - \frac{1}{k+1} \right)$
$= \left( 1 - \frac{1}{2} \right) + \left( \frac{1}{2} - \frac{1}{3} \right) + \cdots + \left( \frac{1}{n} - \frac{1}{n+1} \right)$
$= 1 - \frac{1}{n+1}$

이차방정식 $x^2 - S_n x + T_n = 0$의 두 근이 $\alpha_n, \beta_n$이므로 근과 계수와의 관계에서
$\alpha_n + \beta_n = S_n, \alpha_n \beta_n = T_n$

$\alpha_n^2 + \beta_n^2 = (\alpha_n + \beta_n)^2 - 2 \alpha_n \beta_n = S_n^2 - 2 T_n$
$= \left\{ 2 - \left( \frac{1}{2} \right)^{n-1} \right\}^2 - 2 \left( 1 - \frac{1}{n+1} \right)$
$= 4 - 4 \cdot \left( \frac{1}{2} \right)^{n-1} + \left( \frac{1}{4} \right)^{n-1} - 2 + \frac{2}{n+1}$
$= 2 - 4 \cdot \left( \frac{1}{2} \right)^{n-1} + \left( \frac{1}{4} \right)^{n-1} + \frac{2}{n+1}$

따라서 $\lim_{n \to \infty} (\alpha_n^2 + \beta_n^2) = 2$

정답: ⑤