## 문제
$23$. 수열 $\{ a_{n} \}$ 에 대하여 다항식 $a_{n} x^{2} + a_{n} x + 2$ 를 $x - n$ 으로 나눈 나머지가 $25$ 일 때, 무한급수 $\sum_{n=1}^{\infty} a_{n}$ 의 합을 구하시오.

## 보기

## 풀이
$a_{n} x^{2} + a_{n} x + 2$ 를 $x - n$ 으로 나눈 나머지가 $25$ 이므로 나머지 정리에 의해
$a_{n} n^{2} + a_{n} n + 2 = 25$
$n ( n + 1 ) a_{n} = 23$
$\therefore a_{n} = \frac{23}{n ( n + 1 )}$
$\therefore \sum_{n=1}^{\infty} a_{n} = \sum_{n=1}^{\infty} \frac{23}{n ( n + 1 )}$
$= 23 \lim_{n \to \infty} \sum_{k=1}^{n} \frac{1}{k ( k + 1 )}$
이때,
$\sum_{k=1}^{n} \frac{1}{k ( k + 1 )} = \sum_{k=1}^{n} \left( \frac{1}{k} - \frac{1}{k + 1} \right)$
$= \left( 1 - \frac{1}{2} \right) + \left( \frac{1}{2} - \frac{1}{3} \right) + \cdots + \left( \frac{1}{n} - \frac{1}{n + 1} \right)$
$= 1 - \frac{1}{n + 1}$
이므로
$23 \lim_{n \to \infty} \sum_{k=1}^{n} \frac{1}{k ( k + 1 )} = 23 \lim_{n \to \infty} \left( 1 - \frac{1}{n + 1} \right) = 23$
따라서 구하는 합은 $23$ 이다.

정답: $23$