## 문제
이차방정식 $x^{2}+3x+1=0$의 두 근을 $\alpha$, $\beta$라 하자. 두 행렬 $A = \left( \begin{array}{cc} \alpha & 1 \\ 0 & -\alpha \end{array} \right)$, $B = \left( \begin{array}{cc} \beta & -1 \\ 0 & -\beta \end{array} \right)$에 대하여 $B^{-1} A^{-1}$은?

## 보기
① $\left( \begin{array}{cc} 1 & 3 \\ 0 & 1 \end{array} \right)$ ② $\left( \begin{array}{cc} 1 & -3 \\ 0 & 1 \end{array} \right)$ ③ $\left( \begin{array}{cc} -1 & -3 \\ 0 & 1 \end{array} \right)$ ④ $\left( \begin{array}{cc} 1 & -3 \\ 0 & -1 \end{array} \right)$ ⑤ $\left( \begin{array}{cc} -1 & 3 \\ 0 & -1 \end{array} \right)$

## 풀이
이차방정식 $x^{2}+3x+1=0$의 두 근이 $\alpha$, $\beta$이므로 근과 계수의 관계에 의해
$$\alpha+\beta=-3, \alpha\beta=1$$
이다.
두 행렬 $A$, $B$의 곱 $AB$를 구하면
$$AB = \left( \begin{array}{cc} \alpha & 1 \\ 0 & -\alpha \end{array} \right) \left( \begin{array}{cc} \beta & -1 \\ 0 & -\beta \end{array} \right) = \left( \begin{array}{cc} \alpha\beta & -\alpha-\beta \\ 0 & \alpha\beta \end{array} \right)$$
여기에 $\alpha+\beta=-3$, $\alpha\beta=1$을 대입하면
$$AB = \left( \begin{array}{cc} 1 & -(-3) \\ 0 & 1 \end{array} \right) = \left( \begin{array}{cc} 1 & 3 \\ 0 & 1 \end{array} \right)$$
이다.
따라서 구하는 행렬 $B^{-1} A^{-1}$은
$$B^{-1} A^{-1} = (AB)^{-1} = \left( \begin{array}{cc} 1 & 3 \\ 0 & 1 \end{array} \right)^{-1} = \left( \begin{array}{cc} 1 & -3 \\ 0 & 1 \end{array} \right)$$
이다.

정답: ②