## 문제
이차정사각행렬 $A$ 에 대하여 다음이 성립한다. 
$$ A \left( \begin{array}{c} 1 \\ 0 \end{array} \right) = \left( \begin{array}{c} 2 \\ 3 \end{array} \right) , A \left( \begin{array}{c} 2 \\ 3 \end{array} \right) = \left( \begin{array}{c} 4 \\ 3 \end{array} \right) $$
이때, $A$ 의 모든 성분의 합은? 

## 보기
① $1$   ② $2$   ③ $3$   ④ $4$   ⑤ $5$

## 풀이
$A = \left( \begin{array}{cc} a & b \\ c & d \end{array} \right)$ 라 하면 
$\left( \begin{array}{cc} a & b \\ c & d \end{array} \right) \left( \begin{array}{c} 1 \\ 0 \end{array} \right) = \left( \begin{array}{c} 2 \\ 3 \end{array} \right)$ 에서 
$a = 2$, $c = 3$ $\cdots$ ㉠ 

$\left( \begin{array}{cc} a & b \\ c & d \end{array} \right) \left( \begin{array}{c} 2 \\ 3 \end{array} \right) = \left( \begin{array}{c} 4 \\ 3 \end{array} \right)$ $\iff$ $\left( \begin{array}{cc} 2 & b \\ 3 & d \end{array} \right) \left( \begin{array}{c} 2 \\ 3 \end{array} \right) = \left( \begin{array}{c} 4 \\ 3 \end{array} \right)$ 
($\because$ ㉠)에서 
$4 + 3b = 4$, $6 + 3d = 3$ 

$\therefore$ $b = 0$, $d = -1$ 
따라서, 행렬 $A$ 의 모든 성분의 합은 
$a + b + c + d = 2 + 0 + 3 + (-1) = 4$ 

[다른 풀이] 
주어진 조건에서 $A \left( \begin{array}{cc} 1 & 2 \\ 0 & 3 \end{array} \right) = \left( \begin{array}{cc} 2 & 4 \\ 3 & 3 \end{array} \right)$ 

$\therefore$ $A = \left( \begin{array}{cc} 2 & 4 \\ 3 & 3 \end{array} \right) \left( \begin{array}{cc} 1 & 2 \\ 0 & 3 \end{array} \right)^{-1}$ 
$= \frac{1}{3} \left( \begin{array}{cc} 2 & 4 \\ 3 & 3 \end{array} \right) \left( \begin{array}{cc} 3 & -2 \\ 0 & 1 \end{array} \right)$ 
$= \frac{1}{3} \left( \begin{array}{cc} 6 & 0 \\ 9 & -3 \end{array} \right)$ 
$= \left( \begin{array}{cc} 2 & 0 \\ 3 & -1 \end{array} \right)$ 
모든 성분의 합은 $2 + 0 + 3 + (-1) = 4$

[정답] ④