## 문제
두 수열 $\{a_n\}$, $\{b_n\}$에 대한 설명 중 옳은 것을 <보기>에서 모두 고르면?

$$ \begin{array}{|l|} \hline \text{ㄱ. } \sum_{n=1}^{\infty} a_n \text{ 과 } \sum_{n=1}^{\infty} (a_n + b_n) \text{ 이 수렴하면 } \sum_{n=1}^{\infty} b_n \text{ 도 수렴한다.} \\ \text{ㄴ. } \sum_{n=1}^{\infty} a_n \text{ 과 } \sum_{n=1}^{\infty} b_n \text{ 이 수렴하면 } \lim_{n \to \infty} a_n b_n = 0 \text{ 이다.} \\ \text{ㄷ. } \sum_{n=1}^{\infty} a_n b_n \text{ 이 수렴하고 } \lim_{n \to \infty} a_n \neq 0 \text{ 이면 } \lim_{n \to \infty} b_n = 0 \text{ 이다.} \\ \hline \end{array} $$

## 보기
① ㄱ   ② ㄱ, ㄴ   ③ ㄱ, ㄷ   ④ ㄴ, ㄷ   ⑤ ㄱ, ㄴ, ㄷ

## 풀이
[정답] ②

ㄱ. $\sum_{n=1}^{\infty} a_n = \alpha$, $\sum_{n=1}^{\infty} (a_n + b_n) = \beta$ 라 하면 
$$ \sum_{n=1}^{\infty} b_n = \sum_{n=1}^{\infty} \{(a_n + b_n) - a_n\} $$
$$ = \sum_{n=1}^{\infty} (a_n + b_n) - \sum_{n=1}^{\infty} a_n $$
$$ = \beta - \alpha \text{ (수렴)} $$
$\therefore$ 참

ㄴ. $\sum_{n=1}^{\infty} a_n$ 이 수렴하므로 $\lim_{n \to \infty} a_n = 0$, 
$\sum_{n=1}^{\infty} b_n$ 이 수렴하므로 $\lim_{n \to \infty} b_n = 0$
$$ \lim_{n \to \infty} a_n b_n = 0 $$
$\therefore$ 참

ㄷ. 반례: 수열 $\{a_n\}$ 이 $1, 0, 1, 0, 1, \dots$
$\{b_n\}$ 이 $0, 1, 0, 1, 0, \dots$ 이면
$\sum_{n=1}^{\infty} a_n b_n = 0$ (수렴)이지만
$\lim_{n \to \infty} a_n \neq 0$, $\lim_{n \to \infty} b_n \neq 0$ 이다.
$\therefore$ 거짓