## ë¬¸ì œ
ê·¸ë¦¼ê³¼ ê°™ì´ ìì—°ìˆ˜ $n$ì— ëŒ€í•˜ì—¬ ê°€ë¡œì˜ ê¸¸ì´ê°€ $n$, ì„¸ë¡œì˜ ê¸¸ì´ê°€ $48$ì¸ ì§ì‚¬ê°í˜• $OA B_{n} C_{n}$ì´ ìˆë‹¤. ëŒ€ê°ì„  $A C_{n}$ê³¼ ì„ ë¶„ $B_{1} C_{1}$ì˜ êµì ì„ $D_{n}$ì´ë¼ í•œë‹¤.

> [!example] ğŸ“¸ (ê·¸ë¦¼/ê·¸ë˜í”„)

ì´ ë•Œ, $\lim _{n \rightarrow \infty} \frac{\overline{A C_{n}} - \overline{O C_{n}}}{\overline{B_{1} D_{n}}}$ì˜ ê°’ì„ êµ¬í•˜ì‹œì˜¤.

## ë³´ê¸°

## í’€ì´
$\overline{A C_{n}} - \overline{O C_{n}} = \sqrt{n^{2} + 48^{2}} - n$ì´ê³ , $\overline{B_{1} D_{n}} = \frac{48}{n}$ì´ë¯€ë¡œ

$$ \begin{aligned} \lim _{n \rightarrow \infty} \frac{\overline{A C_{n}} - \overline{O C_{n}}}{\overline{B_{1} D_{n}}} &= \lim _{n \rightarrow \infty} \frac{\sqrt{n^{2} + 48^{2}} - n}{\frac{48}{n}} \\ &= \lim _{n \rightarrow \infty} \frac{(\sqrt{n^{2} + 48^{2}} - n)(\sqrt{n^{2} + 48^{2}} + n)}{\frac{48}{n}(\sqrt{n^{2} + 48^{2}} + n)} \\ &= \lim _{n \rightarrow \infty} \frac{48^{2}}{48 \left( \sqrt{1 + \frac{48^{2}}{n^{2}}} + 1 \right)} \\ &= \frac{48}{2} \\ &= 24 \end{aligned} $$

ì •ë‹µ: $24$