## 문제
수렴하는 무한수열 $\{ a_{n} \}$ 에 대하여
$$\lim_{n \to \infty} ( n^{2} - 1 ) a_{n} = 2006$$
일 때,
$$\lim_{n \to \infty} ( \frac{1}{2} n^{2} + 1 ) a_{n}$$
의 값은?

## 보기
① $0$   ② $\frac{1}{2}$   ③ $1003$   ④ $2006$   ⑤ $4012$

## 풀이
$( n^{2} - 1 ) a_{n} = b_{n}$ 이라 하면
$$a_{n} = \frac{1}{n^{2} - 1} b_{n}$$
이고 $\lim_{n \to \infty} b_{n} = 2006$ 이다.

$$\lim_{n \to \infty} ( \frac{1}{2} n^{2} + 1 ) a_{n} = \lim_{n \to \infty} ( \frac{1}{2} n^{2} + 1 ) \cdot \frac{b_{n}}{n^{2} - 1}$$
$$= \lim_{n \to \infty} \frac{\frac{1}{2} n^{2} + 1}{n^{2} - 1} \cdot b_{n}$$
$$= \lim_{n \to \infty} \frac{\frac{1}{2} n^{2} + 1}{n^{2} - 1} \cdot \lim_{n \to \infty} b_{n}$$
$$= \frac{1}{2} \times 2006 = 1003$$

따라서 정답은 ③이다.