## 문제
$\sin^{2} \theta + \sin^{2} \left( \frac{\pi}{3} + \theta \right) + \sin^{2} \left( \frac{\pi}{3} - \theta \right)$의 값은?

## 보기
① $0$   ② $\frac{1}{2}$   ③ $1$   ④ $\frac{3}{2}$   ⑤ $2$

## 풀이
$\sin \left( \frac{\pi}{3} \pm \theta \right) = \sin \frac{\pi}{3} \cos \theta \pm \cos \frac{\pi}{3} \sin \theta$
$= \frac{\sqrt{3}}{2} \cos \theta \pm \frac{1}{2} \sin \theta$ (복부호동순)이므로
준 식은
$= \sin^{2} \theta + \left( \frac{\sqrt{3}}{2} \cos \theta + \frac{1}{2} \sin \theta \right)^{2} + \left( \frac{\sqrt{3}}{2} \cos \theta - \frac{1}{2} \sin \theta \right)^{2}$
$= \sin^{2} \theta + 2 \cdot \left( \frac{\sqrt{3}}{2} \right)^{2} \cos^{2} \theta + 2 \cdot \left( \frac{1}{2} \right)^{2} \sin^{2} \theta$
$= \sin^{2} \theta + \frac{3}{2} \cos^{2} \theta + \frac{1}{2} \sin^{2} \theta$
$= \frac{3}{2} \sin^{2} \theta + \frac{3}{2} \cos^{2} \theta$
$= \frac{3}{2} (\sin^{2} \theta + \cos^{2} \theta) = \frac{3}{2}$

정답은 ④입니다.