## 문제
$a = 2 - \sqrt{3}$, $b = \sqrt{2}$일 때, $\sqrt{(a + b)^{2}} + \sqrt{(a - b)^{2}}$의 값은?

## 보기
① $\sqrt{2} - 1$   ② $2$   ③ $2 \sqrt{2}$   ④ $2 \sqrt{3}$   ⑤ $\sqrt{2} + \sqrt{3}$

## 풀이
[정답] ③ 

$a + b = 2 - \sqrt{3} + \sqrt{2} > 0$이므로 
$\sqrt{(a + b)^{2}} = |a + b| = |2 - \sqrt{3} + \sqrt{2}| = 2 - \sqrt{3} + \sqrt{2}$ 
또, $a - b = 2 - \sqrt{3} - \sqrt{2} = (1 - \sqrt{3}) + (1 - \sqrt{2}) < 0$이므로 
$\sqrt{(a - b)^{2}} = |a - b| = |2 - \sqrt{3} - \sqrt{2}| = -2 + \sqrt{3} + \sqrt{2}$ 
$\therefore \sqrt{(a + b)^{2}} + \sqrt{(a - b)^{2}} = (2 - \sqrt{3} + \sqrt{2}) + (-2 + \sqrt{3} + \sqrt{2}) = 2 \sqrt{2}$