## 문제
두 행렬 $$ A = \left( \begin{array}{cc} 2 & 1 \\ 3 & 2 \end{array} \right) $$, $$ B = \left( \begin{array}{cc} -1 & 1 \\ 2 & 1 \end{array} \right) $$에 대하여 $A^{-1} + AB$의 모든 성분의 합을 구하시오. (단, $A^{-1}$은 $A$의 역행렬)

## 보기

## 풀이
$$ A = \left( \begin{array}{cc} 2 & 1 \\ 3 & 2 \end{array} \right), B = \left( \begin{array}{cc} -1 & 1 \\ 2 & 1 \end{array} \right) $$
$$ A^{-1} = \left( \begin{array}{cc} 2 & -1 \\ -3 & 2 \end{array} \right), AB = \left( \begin{array}{cc} 0 & 3 \\ 1 & 5 \end{array} \right) $$
$$ A^{-1} + AB = \left( \begin{array}{cc} 2 & 2 \\ -2 & 7 \end{array} \right) $$
$\therefore 2 + 2 - 2 + 7 = 9$

정답: $9$