## 문제
행렬 $A= \begin{pmatrix} 2 & 1 \\ -1 & -2 \end{pmatrix}$ 에 대하여 $\sum _{k=1} ^{n} A ^{2k} = \begin{pmatrix} a _{n} & 0 \\ 0 & d _{n} \end{pmatrix}$ 일 때, $\lim _{n \to \infty} \frac{a_{n+1}}{2^{n}+a_{n}}$ 의 값은?

## 보기
① $0$   ② $1$   ③ $3$   ④ $6$   ⑤ $9$

## 풀이
$A= \begin{pmatrix} 2 & 1 \\ -1 & -2 \end{pmatrix}$ 에서 
$A^{2}= \begin{pmatrix} 2 & 1 \\ -1 & -2 \end{pmatrix} \begin{pmatrix} 2 & 1 \\ -1 & -2 \end{pmatrix} = \begin{pmatrix} 3 & 0 \\ 0 & 3 \end{pmatrix} = 3E$ 

따라서 $A^{4}=3^{2} E$, $A^{6}=3^{3} E$, $\dots$, $A^{2n}=3^{n} E$ 이므로
$\sum_{k=1}^{n} A^{2k}=3 E+3^{2} E+3^{3} E+ \dots +3^{n} E = \frac{3 (3^{n}-1 )}{3-1} E = \frac{3 (3^{n}-1 )}{2} E$ 

그러므로 $a_{n}=\frac{3 (3^{n}-1 )}{2}$, $a_{n+1}=\frac{3 (3^{n+1}-1 )}{2}$ 이다. 

이를 구하고자 하는 극한식에 대입하면 
$\lim _{n \to \infty} \frac{a_{n+1}}{2^{n}+a_{n}} = \lim _{n \to \infty} \frac{\frac{3 (3^{n+1}-1 )}{2}}{2^{n} + \frac{3 (3^{n}-1 )}{2}}$ 
$= \lim _{n \to \infty} \frac{3 \cdot 3^{n+1}-3}{2 \cdot 2^{n} + 3 \cdot 3^{n}-3}$ 
$= \lim _{n \to \infty} \frac{9 \cdot 3^{n}-3}{2^{n+1} + 3^{n+1}-3}$ 
$= \lim _{n \to \infty} \frac{9 - \frac{3}{3^n}}{2 \cdot (\frac{2}{3})^n + 3 - \frac{3}{3^n}} = \frac{9}{3} = 3$ 

정답은 ③이다.