## ๋ฌธ์
๋ ์ค์ $a$, $r$์ ๋ํ์ฌ ๋ฌดํ๋ฑ๋น๊ธ์ $\sum_{n=1}^{\infty} ar^{n-1}$์ด ์๋ดํ๋ฉด [๊ทธ๋ฆผ $1$], $\sum_{n=1}^{\infty} ar^{n-1}$์ด ๋ฐ์ฐํ๋ฉด [๊ทธ๋ฆผ $2$]์ ๊ฐ์ด ๋ํ๋ด๊ณ, $0$์ด ์๋ ์ค์ $k$์ ๋ํ์ฌ $|k| \le 1$์ธ ๊ฒฝ์ฐ [๊ทธ๋ฆผ $3$], $|k| > 1$์ธ ๊ฒฝ์ฐ์๋ [๊ทธ๋ฆผ $4$]์ ๊ฐ์ด ๋ํ๋ด๊ธฐ๋ก ํ๋ค.

> [!example] ๐ธ (๊ทธ๋ฆผ $1$)

> [!example] ๐ธ (๊ทธ๋ฆผ $2$)

> [!example] ๐ธ (๊ทธ๋ฆผ $3$)

> [!example] ๐ธ (๊ทธ๋ฆผ $4$)

์๋ ๊ทธ๋ฆผ์ $\alpha$, $\beta$, $\gamma$์ ๋ํ์ฌ $\alpha + \beta + \gamma$์ ๊ฐ์?

> [!example] ๐ธ (๊ทธ๋ฆผ/๊ทธ๋ํ)

## ๋ณด๊ธฐ
โ $\frac{23}{12}$   โก $\frac{25}{12}$   โข $\frac{9}{4}$   โฃ $\frac{29}{12}$   โค $\frac{31}{12}$

## ํ์ด
(โฐ) $\sum_{n=1}^{\infty} \left( -\frac{1}{2} \right) (-1)^{n-1}$์์ ๊ณต๋น๊ฐ $-1$์ด๋ฏ๋ก ๊ธ์๋ ๋ฐ์ฐํ๋ค.
[๊ทธ๋ฆผ $2$]์ ๊ท์น์ ์ํ์ฌ $\beta = \frac{1}{4}$์ด๋ค.

(โฑ) $\sum_{n=1}^{\infty} \alpha \left( \frac{1}{3} \right)^{n-1}$์ ๊ณต๋น๊ฐ $\frac{1}{3}$์ด๋ฏ๋ก $| \frac{1}{3} | < 1$์ด ๋์ด ์๋ดํ๋ค.
[๊ทธ๋ฆผ $1$]์ ๊ท์น์ ์ํ์ฌ ๊ทธ ํฉ์ $\frac{\alpha}{1 - \frac{1}{3}} = 3$์ด๋ค.
$\frac{\alpha}{\frac{2}{3}} = 3$
$\frac{3}{2}\alpha = 3$
$\therefore \alpha = 2$

(โฒ) $k=3$์ผ ๋ $|3| > 1$์ด๋ฏ๋ก [๊ทธ๋ฆผ $4$]์ ๊ท์น์ ์ํ์ฌ $\gamma = -\frac{1}{3}$์ด๋ค.

๋ฐ๋ผ์,
$\alpha + \beta + \gamma = 2 + \frac{1}{4} - \frac{1}{3}$
$= \frac{24 + 3 - 4}{12}$
$= \frac{23}{12}$

์๋ต: โ