## 문제
두 행렬 $A = \begin{pmatrix} 1 & 2 \\ -1 & -3 \end{pmatrix}$, $B = \begin{pmatrix} 2 & 1 \\ 3 & 4 \end{pmatrix}$ 에 대하여 $A X + A = B$ 를 만족하는 행렬 $X$ 의 모든 성분의 합은?

## 보기
① $10$   ② $11$   ③ $12$   ④ $13$   ⑤ $14$

## 풀이
$A X + A = B$ 에서 $A X = B - A$ 이다.
$A = \begin{pmatrix} 1 & 2 \\ -1 & -3 \end{pmatrix}$ 이므로 역행렬 $A^{-1}$ 을 구하면
$A^{-1} = \frac{1}{(1)(-3) - (2)(-1)} \begin{pmatrix} -3 & -2 \\ 1 & 1 \end{pmatrix} = \frac{1}{-1} \begin{pmatrix} -3 & -2 \\ 1 & 1 \end{pmatrix} = \begin{pmatrix} 3 & 2 \\ -1 & -1 \end{pmatrix}$ 이다.

$X = A^{-1} (B - A)$ 이고,
$B - A = \begin{pmatrix} 2 & 1 \\ 3 & 4 \end{pmatrix} - \begin{pmatrix} 1 & 2 \\ -1 & -3 \end{pmatrix} = \begin{pmatrix} 1 & -1 \\ 4 & 7 \end{pmatrix}$ 이므로

$$ X = \begin{pmatrix} 3 & 2 \\ -1 & -1 \end{pmatrix} \begin{pmatrix} 1 & -1 \\ 4 & 7 \end{pmatrix} = \begin{pmatrix} 3+8 & -3+14 \\ -1-4 & 1-7 \end{pmatrix} = \begin{pmatrix} 11 & 11 \\ -5 & -6 \end{pmatrix} $$

따라서 행렬 $X$ 의 모든 성분의 합은
$11 + 11 + (-5) + (-6) = 11$ 이다.

정답: ②