## 문제
행렬 $A = \left( \begin{array}{cc} a & b \\ c & d \end{array} \right)$ 에 대하여 행렬 $A'$ 을 $A' = \left( \begin{array}{cc} a & c \\ b & d \end{array} \right)$ 로 정의할 때, <보기>에서 옳은 것만을 있는 대로 고른 것은?

## 보기
ㄱ. $(A')' = A$
ㄴ. $(A + A')' = A + A'$
ㄷ. $ad - bc \neq 0$ 일 때, $(A^{-1})' = (A')^{-1}$

① $ㄱ$   ② $ㄴ$   ③ $ㄱ, ㄴ$   ④ $ㄴ, ㄷ$   ⑤ $ㄱ, ㄴ, ㄷ$

## 풀이
[정답] ⑤ 

ㄱ. 
$$( A' )' = \left( \begin{array}{cc} a & c \\ b & d \end{array} \right)' = \left( \begin{array}{cc} a & b \\ c & d \end{array} \right) = A$$
(참)

ㄴ. 
$$A + A' = \left( \begin{array}{cc} a & b \\ c & d \end{array} \right) + \left( \begin{array}{cc} a & c \\ b & d \end{array} \right) = \left( \begin{array}{cc} 2a & b + c \\ b + c & 2d \end{array} \right)$$ 
$$( A + A' )' = \left( \begin{array}{cc} 2a & b + c \\ b + c & 2d \end{array} \right) = A + A'$$
(참)

ㄷ. 
$$( A^{-1} )' = \left\{ \frac{1}{ad - bc} \left( \begin{array}{cc} d & -b \\ -c & a \end{array} \right) \right\}' = \frac{1}{ad - bc} \left( \begin{array}{cc} d & -c \\ -b & a \end{array} \right)$$ 
$$( A' )^{-1} = \left( \begin{array}{cc} a & c \\ b & d \end{array} \right)^{-1} = \frac{1}{ad - bc} \left( \begin{array}{cc} d & -c \\ -b & a \end{array} \right)$$ 
따라서 $$( A^{-1} )' = ( A' )^{-1}$$
(참)