## 문제
곡선 $y = \sqrt{x}$ 위의 점 $(t, \sqrt{t})$ 에서 점 $(1, 0)$ 까지의 거리를 $d_{1}$, 점 $(2, 0)$ 까지의 거리를 $d_{2}$ 라 할 때, $\lim_{t \to \infty} (d_{1} - d_{2})$ 의 값은?

## 보기
① $1$   ② $\frac{1}{2}$   ③ $\frac{1}{4}$   ④ $\frac{1}{8}$   ⑤ $0$

## 풀이
점 $(t, \sqrt{t})$ 에서 두 점 $(1, 0)$, $(2, 0)$ 까지의 거리 $d_{1}$, $d_{2}$ 는
$d_{1} = \sqrt{(t-1)^{2} + (\sqrt{t})^{2}} = \sqrt{t^{2} - t + 1}$
$d_{2} = \sqrt{(t-2)^{2} + (\sqrt{t})^{2}} = \sqrt{t^{2} - 3t + 4}$
$\therefore \lim_{t \to \infty} (d_{1} - d_{2})$
$= \lim_{t \to \infty} (\sqrt{t^{2} - t + 1} - \sqrt{t^{2} - 3t + 4})$
$= \lim_{t \to \infty} \frac{(t^{2} - t + 1) - (t^{2} - 3t + 4)}{\sqrt{t^{2} - t + 1} + \sqrt{t^{2} - 3t + 4}}$
$= \lim_{t \to \infty} \frac{2t - 3}{\sqrt{t^{2} - t + 1} + \sqrt{t^{2} - 3t + 4}}$
$= \lim_{t \to \infty} \frac{2 - \frac{3}{t}}{\sqrt{1 - \frac{1}{t} + \frac{1}{t^{2}}} + \sqrt{1 - \frac{3}{t} + \frac{4}{t^{2}}}}$
$= \frac{2}{1 + 1} = 1$

정답: ①