## ë¬¸ì œ

> [!example] ğŸ“¸ (ê·¸ë¦¼/ê·¸ë˜í”„)

$x_{0} = 1$, $x_{1} = \frac{3}{4}$, $x_{2} = \frac{5}{8}$, $\dots$, $x_{n} = \frac{2^{n} + 1}{2^{n+1}}$, $\dots$ ì— ëŒ€í•˜ì—¬ ì¢Œí‘œí‰ë©´ ìœ„ì— ì  $P_{0} (1, 1)$ ê³¼ $P_{n} (x_{n}, x_{n}^{2})$, $Q_{n} (x_{n-1}, x_{n}^{2})$ ($n = 1, 2, 3, \dots$) ì„ ê·¸ë¦¼ê³¼ ê°™ì´ ë‚˜íƒ€ë‚¸ë‹¤. ë¬´í•œê¸‰ìˆ˜ $\overline{P_{0} Q_{1}} + \overline{Q_{1} P_{1}} + \overline{P_{1} Q_{2}} + \overline{Q_{2} P_{2}} + \overline{P_{2} Q_{3}} + \dots$ ì˜ í•©ì„ $S$ ë¼ í•  ë•Œ $100S$ ì˜ ê°’ì„ êµ¬í•˜ì‹œì˜¤.

## ë³´ê¸°


## í’€ì´

$S = \sum_{n=0}^{\infty} \overline{P_{n} Q_{n+1}} + \sum_{n=1}^{\infty} \overline{Q_{n} P_{n}}$ ì´ê³ ,
$x_{n} = \frac{1}{2} + \frac{1}{2^{n+1}}$ ì´ë¯€ë¡œ
$\sum_{n=0}^{\infty} \overline{P_{n} Q_{n+1}} = \sum_{n=0}^{\infty} (x_{n}^{2} - x_{n+1}^{2})$
$= \sum_{n=0}^{\infty} \left( \frac{1}{2^{n+2}} + \frac{3}{4^{n+2}} \right)$
$= \frac{\frac{1}{4}}{1 - \frac{1}{2}} + \frac{\frac{3}{16}}{1 - \frac{1}{4}} = \frac{1}{2} + \frac{1}{4} = \frac{3}{4}$

$\sum_{n=1}^{\infty} \overline{Q_{n} P_{n}} = \sum_{n=1}^{\infty} (x_{n-1} - x_{n}) = \sum_{n=1}^{\infty} \frac{1}{2^{n+1}}$
$= \frac{\frac{1}{4}}{1 - \frac{1}{2}} = \frac{1}{2}$

ë”°ë¼ì„œ,
$S = \frac{3}{4} + \frac{1}{2} = \frac{5}{4}$ ì´ë¯€ë¡œ
$100S = 125$

**[ë‹¤ë¥¸ í’€ì´]**

$\lim_{n \to \infty} x_{n} = \lim_{n \to \infty} \frac{2^{n} + 1}{2^{n+1}} = \frac{1}{2}$ ì´ë¯€ë¡œ ì  $P_{n}$ ê³¼ ì  $Q_{n}$ ì€ ì  $(\frac{1}{2}, \frac{1}{4})$ ì— í•œì—†ì´ ê°€ê¹Œì›Œì§„ë‹¤.
$A_{n} (x_{n}, 0)$, $B_{n} (0, x_{n}^{2})$ ì´ë¼ í•˜ë©´

$\sum_{n=0}^{\infty} \overline{P_{n} Q_{n+1}} = (1 - \overline{Q_{1} A_{0}}) + (\overline{Q_{1} A_{0}} - \overline{Q_{2} A_{1}}) + \dots$
$= 1 - \lim_{n \to \infty} \overline{Q_{n} A_{n-1}} = 1 - \lim_{n \to \infty} x_{n}^{2}$
$= 1 - \frac{1}{4} = \frac{3}{4}$

$\sum_{n=1}^{\infty} \overline{Q_{n} P_{n}} = (1 - \overline{B_{1} P_{1}}) + (\overline{B_{1} P_{1}} - \overline{B_{2} P_{2}}) + \dots$
$= 1 - \lim_{n \to \infty} \overline{B_{n} P_{n}} = 1 - \lim_{n \to \infty} x_{n}$
$= 1 - \frac{1}{2} = \frac{1}{2}$

ë”°ë¼ì„œ,
$S = \frac{3}{4} + \frac{1}{2} = \frac{5}{4}$ ì´ë¯€ë¡œ
$100S = 125$