## 문제
$( \log_{2} 10 ) ( \log_{5} 10 ) - ( \log_{4} 25 + \log_{25} 4 )$를 간단히 하면?

## 보기
① $0$   ② $2$   ③ $4$   ④ $2 \log_{5} 2$   ⑤ $2 \log_{2} 5$

## 풀이
$( \log_{2} 10 ) ( \log_{5} 10 ) - ( \log_{4} 25 + \log_{25} 4 )$에서 
$\log_{2} 10 = \log_{2} (2 \times 5) = 1 + \log_{2} 5$이고, 
$\log_{5} 10 = \log_{5} (5 \times 2) = 1 + \log_{5} 2$이다.
또한 $\log_{4} 25 = \log_{2^{2}} 5^{2} = \log_{2} 5$이며, $\log_{25} 4 = \log_{5^{2}} 2^{2} = \log_{5} 2$이므로 식을 정리하면 다음과 같다.

$$ (1 + \log_{2} 5) (1 + \log_{5} 2) - ( \log_{2} 5 + \log_{5} 2 ) $$
$$ = 1 + \log_{2} 5 + \log_{5} 2 + \log_{2} 5 \log_{5} 2 - \log_{2} 5 - \log_{5} 2 $$
$$ = 1 + \log_{2} 5 \cdot \frac{1}{\log_{2} 5} $$
$$ = 1 + 1 = 2 $$

정답: ②