## 문제
행렬 $A = \left( \begin{array}{rr} -2 & -3 \\ 1 & 1 \end{array} \right)$ 에 대하여 
$$ A^{2005} \left( \begin{array}{c} x \\ y \end{array} \right) = \left( \begin{array}{c} 1 \\ 2 \end{array} \right) $$ 
일 때, $x - y$ 의 값을 구하시오.

## 보기

## 풀이
$$ A^{2} = \left( \begin{array}{rr} -2 & -3 \\ 1 & 1 \end{array} \right) \left( \begin{array}{rr} -2 & -3 \\ 1 & 1 \end{array} \right) = \left( \begin{array}{rr} 1 & 3 \\ -1 & -2 \end{array} \right) $$ 
$$ A^{3} = A^{2} A = \left( \begin{array}{rr} 1 & 3 \\ -1 & -2 \end{array} \right) \left( \begin{array}{rr} -2 & -3 \\ 1 & 1 \end{array} \right) = \left( \begin{array}{rr} 1 & 0 \\ 0 & 1 \end{array} \right) = E $$ 
$$ \therefore A^{2005} = (A^{3})^{668} \cdot A = A \quad (\because A^{3} = E) $$ 
$$ \therefore A^{2005} \left( \begin{array}{c} x \\ y \end{array} \right) = \left( \begin{array}{c} 1 \\ 2 \end{array} \right) \text{ 에서 } A \left( \begin{array}{c} x \\ y \end{array} \right) = \left( \begin{array}{c} 1 \\ 2 \end{array} \right) $$ 
그런데 $A^{-1} = \left( \begin{array}{rr} 1 & 3 \\ -1 & -2 \end{array} \right)$ 이므로 
$$ \left( \begin{array}{c} x \\ y \end{array} \right) = A^{-1} \left( \begin{array}{c} 1 \\ 2 \end{array} \right) = \left( \begin{array}{rr} 1 & 3 \\ -1 & -2 \end{array} \right) \left( \begin{array}{c} 1 \\ 2 \end{array} \right) = \left( \begin{array}{r} 7 \\ -5 \end{array} \right) $$ 
$\therefore x - y = 7 - (-5) = 12$

정답: $12$