## 문제
두 행렬 $X$, $Y$에 대하여 
$X+Y= \left( \begin{array}{rr} -1 & -1 \\ 1 & 0 \end{array} \right)$, $X-Y= \left( \begin{array}{rr} -1 & 1 \\ -1 & -2 \end{array} \right)$
일 때, $X^{2}+XY$는?

## 보기
① $\left( \begin{array}{rr} -1 & 1 \\ -1 & -2 \end{array} \right)$   ② $\left( \begin{array}{rr} 1 & -1 \\ 1 & 2 \end{array} \right)$   ③ $\left( \begin{array}{rr} -1 & 0 \\ 0 & -1 \end{array} \right)$   ④ $\left( \begin{array}{rr} -1 & -1 \\ 1 & 0 \end{array} \right)$   ⑤ $\left( \begin{array}{rr} 1 & 1 \\ -1 & 0 \end{array} \right)$

## 풀이
$$ X+Y= \left( \begin{array}{rr} -1 & -1 \\ 1 & 0 \end{array} \right) \cdots \cdots ㉠ $$
$$ X-Y= \left( \begin{array}{rr} -1 & 1 \\ -1 & -2 \end{array} \right) \cdots \cdots ㉡ $$
㉠ $+$ ㉡을 하면
$$ 2X = \left( \begin{array}{rr} -2 & 0 \\ 0 & -2 \end{array} \right) $$
$$ \therefore X = \left( \begin{array}{rr} -1 & 0 \\ 0 & -1 \end{array} \right) $$
$$ \therefore X^{2}+XY = X(X+Y) $$
$$ = \left( \begin{array}{rr} -1 & 0 \\ 0 & -1 \end{array} \right) \left( \begin{array}{rr} -1 & -1 \\ 1 & 0 \end{array} \right) = \left( \begin{array}{rr} 1 & 1 \\ -1 & 0 \end{array} \right) $$
따라서 정답은 ⑤이다.