## 문제
행렬 $A = \left( \begin{array}{cc} 1 & 1 \\ 0 & 1 \end{array} \right)$ 에 대하여 행렬 $A^{10} + (A^{-1})^{10}$ 의 모든 성분의 합을 구하시오.

## 보기

## 풀이
$$ A^{2} = \left( \begin{array}{cc} 1 & 1 \\ 0 & 1 \end{array} \right) \left( \begin{array}{cc} 1 & 1 \\ 0 & 1 \end{array} \right) = \left( \begin{array}{cc} 1 & 2 \\ 0 & 1 \end{array} \right) $$
$$ A^{3} = \left( \begin{array}{cc} 1 & 1 \\ 0 & 1 \end{array} \right) \left( \begin{array}{cc} 1 & 2 \\ 0 & 1 \end{array} \right) = \left( \begin{array}{cc} 1 & 3 \\ 0 & 1 \end{array} \right) $$
$$ \vdots $$
$$ A^{10} = \left( \begin{array}{cc} 1 & 10 \\ 0 & 1 \end{array} \right) $$
$$ (A^{-1})^{10} = (A^{10})^{-1} = \left( \begin{array}{cc} 1 & -10 \\ 0 & 1 \end{array} \right) $$
$$ \therefore A^{10} + (A^{-1})^{10} = \left( \begin{array}{cc} 2 & 0 \\ 0 & 2 \end{array} \right) $$
따라서 모든 성분의 합은 $4$이다.

정답: $4$