## 문제
두 수열 $\{ a_{n} \}$, $\{ b_{n} \}$ 이 각각 
$$ a_{n} = \frac{1}{2^{n-1}} \cos \frac{(n-1) \pi}{2} , b_{n} = \frac{1+(-1)^{n-1}}{2^{n}} $$ 
일 때, <보기>에서 옳은 것을 모두 고른 것은?

$$
\begin{array}{|l|}
\hline
ㄱ. \text{ 모든 자연수 } k \text{ 에 대하여 } a_{3k} < 0 \text{ 이다.} \\
ㄴ. \text{ 모든 자연수 } k \text{ 에 대하여 } a_{4k-1} + b_{4k-1} = 0 \text{ 이다.} \\
ㄷ. \sum_{n=1}^{\infty} a_{n} = \frac{3}{5} \sum_{n=1}^{\infty} b_{n} \\
\hline
\end{array}
$$

## 보기
① $ㄱ$   ② $ㄴ$   ③ $ㄷ$   ④ $ㄱ, ㄴ$   ⑤ $ㄴ, ㄷ$

## 풀이
[정답] ⑤ 

$n = 1, 2, 3, \dots$ 을 대입하여 나열해 보면 

$\{ a_{n} \} : 1, 0, -\frac{1}{2^{2}}, 0, \frac{1}{2^{4}}, 0, \dots$ 

$\{ b_{n} \} : 1, 0, \frac{1}{2^{2}}, 0, \frac{1}{2^{4}}, 0, \dots$ 

ㄱ. $a_{6} = 0$ 이므로 거짓. 

ㄴ. $a_{4k-1} + b_{4k-1} = -\frac{1}{2^{4k-2}} + \frac{1}{2^{4k-2}} = 0$ (참) 

ㄷ. $\sum_{n=1}^{\infty} a_{n} = \frac{1}{1 - \left( -\frac{1}{4} \right)} = \frac{4}{5}$ 

$\frac{3}{5} \sum_{n=1}^{\infty} b_{n} = \frac{3}{5} \cdot \frac{1}{1 - \frac{1}{4}} = \frac{3}{5} \cdot \frac{4}{3} = \frac{4}{5}$ (참) 

따라서 옳은 것은 $ㄴ, ㄷ$이다.