## 문제
수열 $\{ a_{n} \}$ 의 첫째항부터 제 $n$ 항까지의 합 $S_{n}$ 이 $S_{n}=n^{2}+1$ 일 때, $\sum_{k=1}^{7} \frac{1}{a_{k} a_{k+1}}$ 의 값은?

## 보기
① $\frac{4}{15}$   ② $\frac{3}{10}$   ③ $\frac{7}{15}$   ④ $\frac{1}{2}$   ⑤ $\frac{7}{10}$

## 풀이
$a_{1} = S_{1} = 2$
$n \ge 2$ 일 때,
$a_{n} = S_{n} - S_{n-1} = (n^{2} + 1) - \{ (n-1)^{2} + 1 \} = 2n-1$
이므로 수열 $\{ a_{n} \}$ 은 $2, 3, 5, 7, \dots$ 이다.
따라서,
$\sum_{k=1}^{7} \frac{1}{a_{k} a_{k+1}} = \frac{1}{a_{1} a_{2}} + \sum_{k=2}^{7} \frac{1}{a_{k} a_{k+1}}$
$= \frac{1}{2 \cdot 3} + \sum_{k=2}^{7} \frac{1}{(2k-1)(2k+1)}$
$= \frac{1}{6} + \frac{1}{2} \sum_{k=2}^{7} \left( \frac{1}{2k-1} - \frac{1}{2k+1} \right)$
$= \frac{1}{6} + \frac{1}{2} \left\{ \left( \frac{1}{3} - \frac{1}{5} \right) + \left( \frac{1}{5} - \frac{1}{7} \right) + \cdots + \left( \frac{1}{13} - \frac{1}{15} \right) \right\}$
$= \frac{1}{6} + \frac{1}{2} \left( \frac{1}{3} - \frac{1}{15} \right)$
$= \frac{1}{6} + \frac{1}{2} \cdot \frac{4}{15}$
$= \frac{1}{6} + \frac{2}{15} = \frac{5+4}{30} = \frac{9}{30} = \frac{3}{10}$

정답: ②