## 문제
두 다항식 $A$, $B$에 대하여 $A \triangle B$를 
$$A \triangle B= \frac{A}{A+B}$$ 
로 정의할 때, $( x \triangle x ^{2}  ) +  \{ ( x ^{2} -x  ) \triangle (x-1  ) \}$을 간단히 하면? 

## 보기
① $\frac{1}{2}$   ② $1$   ③ $\frac{3}{x+1}$   ④ $\frac{1}{x-1}$   ⑤ $\frac{x^{2}}{x+1}$

## 풀이
$$x \triangle x^{2} = \frac{x}{x+x^{2}} = \frac{x}{x(x+1)} = \frac{1}{x+1}$$ 

$$(x^{2} - x) \triangle (x-1) = \frac{x^{2}-x}{x^{2}-x+x-1} = \frac{x(x-1)}{(x+1)(x-1)} = \frac{x}{x+1}$$ 

$$\therefore (x \triangle x^{2}) + \{ (x^{2} - x) \triangle (x-1) \}$$ 

$$= \frac{1}{x+1} + \frac{x}{x+1}$$ 

$$= \frac{x+1}{x+1} = 1$$ 

정답: ②