## 문제
$\sqrt{\frac{1}{\sqrt{5}+\sqrt{2}}} \left( \sqrt{\frac{1}{\sqrt{5}+\sqrt{2}}} - 1 \right) + \left( \sqrt{\frac{1}{\sqrt{5}+\sqrt{2}}} - 1 \right) \left( \sqrt{\frac{1}{\sqrt{5}+\sqrt{2}}} + 1 \right) + \sqrt{\frac{1}{\sqrt{5}+\sqrt{2}}} \left( \sqrt{\frac{1}{\sqrt{5}+\sqrt{2}}} + 1 \right)$ 의 값은?

## 보기
① $\sqrt{5}+\sqrt{2}-1$   ② $\sqrt{5}-\sqrt{2}-1$   ③ $\sqrt{5}+\sqrt{2}+1$   ④ $\sqrt{5}-\sqrt{2}+1$   ⑤ $2$

## 풀이
$\sqrt{\frac{1}{\sqrt{5}+\sqrt{2}}}=t$ 로 치환하면 주어진 식은
$t(t-1)+(t-1)(t+1)+t(t+1) = (t^{2}-t) + (t^{2}-1) + (t^{2}+t) = 3t^{2}-1$ 이다.
이때 $t^{2} = \frac{1}{\sqrt{5}+\sqrt{2}} = \frac{\sqrt{5}-\sqrt{2}}{(\sqrt{5}+\sqrt{2})(\sqrt{5}-\sqrt{2})} = \frac{\sqrt{5}-\sqrt{2}}{3}$ 이므로
$3t^{2}-1 = 3 \left( \frac{\sqrt{5}-\sqrt{2}}{3} \right) - 1 = \sqrt{5}-\sqrt{2}-1$ 이다.
따라서 정답은 ②이다.