## 문제
$\left( \frac{2}{3} \right)^{x^{3} + 6} = \left( \frac{3}{2} \right)^{-2x^{2} - 5x}$ 를 만족하는 모든 $x$의 값들의 곱은?

## 보기
① $-6$   ② $-4$   ③ $-2$   ④ $2$   ⑤ $4$

## 풀이
$\left( \frac{2}{3} \right)^{x^{3} + 6} = \left\{ \left( \frac{2}{3} \right)^{-1} \right\}^{-2x^{2} - 5x}$ 이므로 
$\left( \frac{2}{3} \right)^{x^{3} + 6} = \left( \frac{2}{3} \right)^{2x^{2} + 5x}$ 
$\therefore$ $x^{3} + 6 = 2x^{2} + 5x$ 
$\Leftrightarrow$ $x^{3} - 2x^{2} - 5x + 6 = 0$ 
$\Leftrightarrow$ $(x - 1)(x + 2)(x - 3) = 0$ 
$\therefore$ $x = -2$, $1$, $3$ 이다. 
따라서, 모든 $x$의 값들의 곱은 $-6$ 이다.

정답: ①