## 문제
자연수 $n$과 실수 $x$에 대하여 함수 $F_n(x)$가 
$$F_n(x) = \int \frac{x^{3n} - 1}{x^2 + x + 1} dx$$
$$F_n(1) = \frac{1}{3n - 1} - \frac{1}{3n - 2} + \frac{1}{3n - 4} - \frac{1}{3n - 5} + \dots + \frac{1}{2} - 1$$
와 같이 정의될 때, $F_n(0)$의 값은?

## 보기
① $\frac{n(n - 1)}{2}$   ② $\frac{n(n - 1)(n - 2)}{6}$   ③ $\frac{(n - 1)(n - 2)}{n + 1}$   ④ $0$   ⑤ $1$

## 풀이
$F_n(x) = \int \frac{x^{3n} - 1}{x^2 + x + 1} dx$ 에서 피적분함수를 정리하면 다음과 같다.
$$ \begin{array}{l} \frac{x^{3n} - 1}{x^2 + x + 1} = \frac{(x - 1)(x^{3n} - 1)}{(x - 1)(x^2 + x + 1)} \\ = \frac{(x - 1)(x^3 - 1)(x^{3(n - 1)} + x^{3(n - 2)} + \dots + x^3 + 1)}{x^3 - 1} \\ = (x - 1)(x^{3(n - 1)} + x^{3(n - 2)} + \dots + x^3 + 1) \\ = (x^{3n - 2} - x^{3n - 3}) + (x^{3n - 5} - x^{3n - 6}) + \dots + (x^4 - x^3) + (x - 1) \end{array} $$
이를 부정적분하면
$$F_n(x) = \frac{1}{3n - 1} x^{3n - 1} - \frac{1}{3n - 2} x^{3n - 2} + \frac{1}{3n - 4} x^{3n - 4} - \frac{1}{3n - 5} x^{3n - 5} + \dots + \frac{1}{2} x^2 - x + C$$
주어진 조건 $F_n(1) = \frac{1}{3n - 1} - \frac{1}{3n - 2} + \frac{1}{3n - 4} - \frac{1}{3n - 5} + \dots + \frac{1}{2} - 1$ 로부터 적분상수 $C = 0$ 이다.
따라서 $F_n(x)$ 에 $x = 0$ 을 대입하면
$$F_n(0) = 0$$
이다.

정답: ④