## 문제

$A + B = \left( \begin{array}{cc} 3 & 1 \\ 5 & 2 \end{array} \right)$, $A X = \left( \begin{array}{cc} 2 & 1 \\ 3 & 2 \end{array} \right)$, $B X = \left( \begin{array}{cc} -2 & -1 \\ 5 & 2 \end{array} \right)$를 만족시키는 이차정사각행렬 $X$는?

## 보기

① $\left( \begin{array}{cc} 8 & 4 \\ -24 & -12 \end{array} \right)$ ② $\left( \begin{array}{cc} 8 & -4 \\ 24 & -12 \end{array} \right)$ ③ $\left( \begin{array}{cc} -8 & -4 \\ 24 & 12 \end{array} \right)$ ④ $\left( \begin{array}{cc} 24 & 12 \\ -8 & -4 \end{array} \right)$ ⑤ $\left( \begin{array}{cc} 24 & -12 \\ 8 & -4 \end{array} \right)$

## 풀이

[정답] ③

$A X + B X = (A + B) X = \left( \begin{array}{cc} 2 & 1 \\ 3 & 2 \end{array} \right) + \left( \begin{array}{cc} -2 & -1 \\ 5 & 2 \end{array} \right) = \left( \begin{array}{cc} 0 & 0 \\ 8 & 4 \end{array} \right)$이므로

$\left( \begin{array}{cc} 3 & 1 \\ 5 & 2 \end{array} \right) X = \left( \begin{array}{cc} 0 & 0 \\ 8 & 4 \end{array} \right)$이 된다.

$\left( \begin{array}{cc} 3 & 1 \\ 5 & 2 \end{array} \right)^{-1} = \frac{1}{3 \cdot 2 - 1 \cdot 5} \left( \begin{array}{cc} 2 & -1 \\ -5 & 3 \end{array} \right) = \left( \begin{array}{cc} 2 & -1 \\ -5 & 3 \end{array} \right)$이므로

$\therefore X = \left( \begin{array}{cc} 2 & -1 \\ -5 & 3 \end{array} \right) \left( \begin{array}{cc} 0 & 0 \\ 8 & 4 \end{array} \right) = \left( \begin{array}{cc} -8 & -4 \\ 24 & 12 \end{array} \right)$