## ë¬¸ì œ
ê·¸ë¦¼ê³¼ ê°™ì´ ìì—°ìˆ˜ $n$ì— ëŒ€í•˜ì—¬ ê°€ë¡œì˜ ê¸¸ì´ê°€ $n$, ì„¸ë¡œì˜ ê¸¸ì´ê°€ $48$ì¸ ì§ì‚¬ê°í˜• $OAB_{n}C_{n}$ì´ ìˆë‹¤. ëŒ€ê°ì„  $AC_{n}$ê³¼ ì„ ë¶„ $B_{1}C_{1}$ì˜ êµì ì„ $D_{n}$ì´ë¼ í•œë‹¤. ì´ë•Œ, $\lim_{n \to \infty} \frac{\overline{AC_{n}} - \overline{OC_{n}}}{\overline{B_{1}D_{n}}}$ì˜ ê°’ì„ êµ¬í•˜ì‹œì˜¤.

> [!example] ğŸ“¸ (ê·¸ë¦¼/ê·¸ë˜í”„)

## ë³´ê¸°

## í’€ì´
$\overline{AC_{n}} - \overline{OC_{n}} = \sqrt{n^{2} + 48^{2}} - n$, $\overline{B_{1}D_{n}} = \frac{48}{n}$ì´ë¯€ë¡œ 
$$ \lim_{n \to \infty} \frac{\overline{AC_{n}} - \overline{OC_{n}}}{\overline{B_{1}D_{n}}} $$
$$ = \lim_{n \to \infty} \frac{\sqrt{n^{2} + 48^{2}} - n}{\frac{48}{n}} $$
$$ = \lim_{n \to \infty} \frac{(\sqrt{n^{2} + 48^{2}} - n)(\sqrt{n^{2} + 48^{2}} + n)}{\frac{48}{n} (\sqrt{n^{2} + 48^{2}} + n)} $$
$$ = \lim_{n \to \infty} \frac{48^{2}}{48\left(\sqrt{1+ \frac{48^{2}}{n^{2}}} + 1\right)} = \frac{48}{2} = 24 $$

ì •ë‹µ: $24$