## 문제
두 수열 $\{ a_{n} \}$, $\{ b_{n} \}$의 일반항이 $a_{n} = 2^{n} - 10$, $b_{n} = 2n - 6$일 때, $\sum_{i=1}^{6} \left( \sum_{j=1}^{6} a_{i} b_{j} \right)$의 값을 구하시오.

## 보기

## 풀이
$\sum_{i=1}^{6} \left( \sum_{j=1}^{6} a_{i} b_{j} \right) = \sum_{i=1}^{6} \left( a_{i} \sum_{j=1}^{6} b_{j} \right)$
$= \sum_{i=1}^{6} \left( a_{i} \left( 2 \cdot \frac{6 \cdot 7}{2} - 36 \right) \right)$
$= 6 \sum_{i=1}^{6} a_{i}$
$= 6 \left( \frac{2(2^{6} - 1)}{2 - 1} - 60 \right)$
$= 6 ( 126 - 60 )$
$= 6 \times 66 = 396$

따라서 정답은 $396$이다.