## 문제
행렬 $A= \left( \begin{array}{cc} 2 & 5 \\ 1 & 3 \end{array} \right)$, $E= \left( \begin{array}{cc} 1 & 0 \\ 0 & 1 \end{array} \right)$ 에 대하여 $(A+E) A^{-1}$ 의 모든 성분의 합은?

## 보기
① $1$   ② $2$   ③ $3$   ④ $4$   ⑤ $5$

## 풀이
$A= \left( \begin{array}{cc} 2 & 5 \\ 1 & 3 \end{array} \right)$ 에서 
$A^{-1}= \left( \begin{array}{cc} 3 & -5 \\ -1 & 2 \end{array} \right)$ 이므로 

$$(A+E) A^{-1}=E+A^{-1}$$ 

$$= \left( \begin{array}{cc} 1 & 0 \\ 0 & 1 \end{array} \right) + \left( \begin{array}{cc} 3 & -5 \\ -1 & 2 \end{array} \right) = \left( \begin{array}{cc} 4 & -5 \\ -1 & 3 \end{array} \right)$$ 
따라서, 모든 성분의 합은 $4 + (-5) + (-1) + 3 = 1$ 이다.

[정답] ①