## 문제
$x = \frac{\sqrt{3} + 1}{\sqrt{3} - 1}$ 일 때, $\frac{x^{3} - 5x^{2} + 6x - 3}{x^{2} - 4x + 2}$ 의 값은?

## 보기
① $1$   ② $\sqrt{3}$   ③ $-1 + \sqrt{3}$   ④ $1 + \sqrt{3}$   ⑤ $2 + \sqrt{3}$

## 풀이
$x = \frac{\sqrt{3} + 1}{\sqrt{3} - 1} = \frac{(\sqrt{3} + 1)^{2}}{(\sqrt{3} - 1)(\sqrt{3} + 1)} = 2 + \sqrt{3}$ 이므로
$x - 2 = \sqrt{3}$ $\cdots \cdots$ ㉠
위 식의 양변을 제곱하여 정리하면
$x^{2} - 4x + 1 = 0$
$\therefore x^{2} - 4x = -1$ $\cdots \cdots$ ㉡

따라서
$\frac{x^{3} - 5x^{2} + 6x - 3}{x^{2} - 4x + 2}$
$= \frac{x(x^{2} - 4x) - (x^{2} - 4x) + 2x - 3}{(x^{2} - 4x) + 2}$
$= \frac{-x - (-1) + 2x - 3}{-1 + 2}$ ($\because$ ㉡)
$= x - 2 = \sqrt{3}$ ($\because$ ㉠)

[정답] ②