## 문제
자연수 $n$에 대하여 이차방정식 $x^2 + (\sqrt{n} + 1)x - \frac{\sqrt{n}}{2} - \frac{3}{4} = 0$의 두 근을 $\alpha_{n}$, $\beta_{n}$이라 할 때, $\lim_{n \to \infty} \left( \frac{1}{\alpha_{n}} + \frac{1}{\beta_{n}} \right)$의 값을 구하시오.

## 보기

## 풀이
이차방정식의 근과 계수의 관계에서 
$\alpha_{n} + \beta_{n} = -\sqrt{n} - 1$, 
$\alpha_{n} \beta_{n} = -\frac{\sqrt{n}}{2} - \frac{3}{4}$ 이므로 

$\lim_{n \to \infty} \left( \frac{1}{\alpha_{n}} + \frac{1}{\beta_{n}} \right)$
$= \lim_{n \to \infty} \frac{\alpha_{n} + \beta_{n}}{\alpha_{n} \beta_{n}}$
$= \lim_{n \to \infty} \frac{-\sqrt{n} - 1}{-\frac{\sqrt{n}}{2} - \frac{3}{4}}$
$= \lim_{n \to \infty} \frac{1 + \frac{1}{\sqrt{n}}}{\frac{1}{2} + \frac{3}{4\sqrt{n}}}$
$= \frac{1 + 0}{\frac{1}{2} + 0} = 2$

정답: $2$