## 문제
$\sqrt{-3} \sqrt{-2} \sqrt{2} \sqrt{3} + \frac{\sqrt{6}}{\sqrt{-2}}$ 을 간단히 하면? (단, $i = \sqrt{-1}$)

## 보기
① $6 + \sqrt{3}i$   ② $6 - \sqrt{3}i$   ③ $0$   ④ $-6 + \sqrt{3}i$   ⑤ $-6 - \sqrt{3}i$

## 풀이
$\sqrt{-3} \sqrt{-2} = -\sqrt{(-3) \times (-2)} = -\sqrt{6}$ 이고,
$\frac{\sqrt{6}}{\sqrt{-2}} = -\sqrt{\frac{6}{-2}} = -\sqrt{-3} = -\sqrt{3}i$ 이므로

$\sqrt{-3} \sqrt{-2} \sqrt{2} \sqrt{3} + \frac{\sqrt{6}}{\sqrt{-2}}$
$= (-\sqrt{6}) \times \sqrt{2} \times \sqrt{3} - \sqrt{3}i$
$= -\sqrt{6} \times \sqrt{6} - \sqrt{3}i$
$= -6 - \sqrt{3}i$

따라서 정답은 ⑤이다.