## 문제
$x + \frac{1}{x} = -1$ 일 때, 양의 정수 $n$ 에 대하여 $P(n)$ 을 
$P(n) = (x^{2} + x)^{n} + (x^{2} + 1)^{n} + (x + 1)^{n}$ 이라 하자. 
$P(1) + P(2) + P(3) + \dots + P(2007)$ 의 값은?

## 보기
① $3$   ② $1$   ③ $0$   ④ $-1$   ⑤ $-3$

## 풀이
주어진 식을 정리하면 다음을 얻는다. 

$x^{2} + x + 1 = 0$, 
$(x - 1)(x^{2} + x + 1) = 0$, 
$x^{3} - 1 = 0$ $\therefore x^{3} = 1$ 

그러므로 $P(n)$ 의 값은 다음과 같다. 

$P(n) = (-1)^{n} + (-x)^{n} + (-x^{2})^{n}$ 
$P(1) = -1 - x - x^{2} = 0$ 
$P(2) = 1 + x^{2} + x^{4} = 1 + x^{2} + x = 0$ 
$P(3) = -1 - x^{3} - x^{6} = -1 - 1 - 1 = -3$ 
$P(4) = 1 + x^{4} + x^{8} = 1 + x + x^{2} = 0$ 
$P(5) = -1 - x^{5} - x^{10} = -1 - x^{2} - x = 0$ 
$P(6) = 1 + x^{6} + x^{12} = 1 + 1 + 1 = 3$ 

$\dots$ 이므로 자연수 $k$ 에 대하여 
$n = 6k - 3$ 이면 $P(n) = -3$ 
$n = 6k$ 이면 $P(n) = 3$ 
$n \neq 6k - 3$ 이고 $n \neq 6k$ 이면 $P(n) = 0$ 

그런데, $2007 = 6 \times 334 + 3$ 이므로 
$P(2007) = P(3) = -3$ 

$\therefore P(1) + P(2) + P(3) + \dots + P(2007)$ 
$= 0 + 0 + (-3) + 0 + 0 + 3 + 0 + \dots + 0 + (-3)$ 
$= -3$ 

정답: ⑤