## 문제
행렬 $A = \begin{pmatrix} 2 & 0 \\ 0 & 3 \end{pmatrix}$ 에 대하여 $A^{n} = \begin{pmatrix} a_{n} & 0 \\ 0 & b_{n} \end{pmatrix}$ 이라 할 때, $\lim_{n \to \infty} \frac{3a_{n} - 2b_{n}}{2a_{n} + 3b_{n}}$ 의 값은?

## 보기
① $-\frac{3}{2}$   ② $-\frac{2}{3}$   ③ $0$   ④ $\frac{2}{3}$   ⑤ $\frac{3}{2}$

## 풀이
$$A^{2} = \begin{pmatrix} 2 & 0 \\ 0 & 3 \end{pmatrix} \begin{pmatrix} 2 & 0 \\ 0 & 3 \end{pmatrix} = \begin{pmatrix} 2^{2} & 0 \\ 0 & 3^{2} \end{pmatrix}$$
$$A^{3} = A^{2} A = \begin{pmatrix} 2^{2} & 0 \\ 0 & 3^{2} \end{pmatrix} \begin{pmatrix} 2 & 0 \\ 0 & 3 \end{pmatrix} = \begin{pmatrix} 2^{3} & 0 \\ 0 & 3^{3} \end{pmatrix}$$
$\dots$,
$$A^{n} = \begin{pmatrix} 2^{n} & 0 \\ 0 & 3^{n} \end{pmatrix}$$
이므로 $a_{n} = 2^{n}$, $b_{n} = 3^{n}$ 이다.
$$\therefore \lim_{n \to \infty} \frac{3a_{n} - 2b_{n}}{2a_{n} + 3b_{n}} = \lim_{n \to \infty} \frac{3 \cdot 2^{n} - 2 \cdot 3^{n}}{2 \cdot 2^{n} + 3 \cdot 3^{n}}$$
$$= \lim_{n \to \infty} \frac{3 \cdot \left( \frac{2}{3} \right)^{n} - 2}{2 \cdot \left( \frac{2}{3} \right)^{n} + 3} = -\frac{2}{3}$$
정답 ②