## 문제
두 행렬 $A = \left( \begin{array}{cc} 2 & 5 \\ 1 & 3 \end{array} \right)$, $B = \left( \begin{array}{cc} 3 & 2 \\ 2 & 1 \end{array} \right)$ 에 대하여 $A^{-1} B$ 의 모든 성분의 합은?

## 보기
① $1$   ② $2$   ③ $3$   ④ $4$   ⑤ $5$

## 풀이
$A = \left( \begin{array}{cc} 2 & 5 \\ 1 & 3 \end{array} \right)$ 에서 $D = 2 \times 3 - 5 \times 1 = 1$ 이므로
$$ A^{-1} = \left( \begin{array}{cc} 3 & -5 \\ -1 & 2 \end{array} \right) $$
이다.
$$ A^{-1} B = \left( \begin{array}{cc} 3 & -5 \\ -1 & 2 \end{array} \right) \left( \begin{array}{cc} 3 & 2 \\ 2 & 1 \end{array} \right) = \left( \begin{array}{cc} 3 \times 3 + (-5) \times 2 & 3 \times 2 + (-5) \times 1 \\ -1 \times 3 + 2 \times 2 & -1 \times 2 + 2 \times 1 \end{array} \right) = \left( \begin{array}{cc} -1 & 1 \\ 1 & 0 \end{array} \right) $$
따라서 $A^{-1} B$ 의 모든 성분의 합은
$$ -1 + 1 + 1 + 0 = 1 $$
이다.

정답: ①