## ë¬¸ì œ
ì–‘ìˆ˜ $a$ì— ëŒ€í•˜ì—¬ ì‚¼ì°¨í•¨ìˆ˜ $f(x)=-x(x+a)(x-a)$ì˜ ê·¹ëŒ€ì ì˜ $x$ì¢Œí‘œë¥¼ $b$ë¼ í•˜ìž.
$\int_{-b}^{a} f(x) dx=A$, $\int_{b}^{a+b} f(x-b) dx=B$ì¼ ë•Œ, $\int_{-b}^{a} |f(x)| dx$ì˜ ê°’ì€?

## ë³´ê¸°
â‘  $-A+2B$   â‘¡ $-2A+B$   â‘¢ $-A+B$   â‘£ $A+B$   â‘¤ $A+2B$

## í’€ì´
$y=f(x)$ì˜ ê·¸ëž˜í”„ì™€ $y=f(x-b)$ì˜ ê·¸ëž˜í”„ëŠ” ë‹¤ìŒê³¼ ê°™ë‹¤.

> [!example] ðŸ“¸ (ê·¸ë¦¼/ê·¸ëž˜í”„)

> [!example] ðŸ“¸ (ê·¸ë¦¼/ê·¸ëž˜í”„)

$\int_{-b}^{a} f(x) dx=A$

$\int_{b}^{a+b} f(x-b) dx = \int_{0}^{a} f(x) dx=B$

$\therefore \int_{-b}^{0} f(x) dx = \int_{-b}^{a} f(x) dx - \int_{0}^{a} f(x) dx$
$=A-B$

$\therefore \int_{-b}^{a} |f(x)| dx = \int_{-b}^{0} \{-f(x)\} dx + \int_{0}^{a} f(x) dx$
$=-(A-B)+B$
$=-A+2B$

[ì •ë‹µ] â‘ 