## 문제
$a_{1} = 1$, $2a_{n+1} + a_{n} = 2$ ($n = 1, 2, 3, \dots$)를 만족시키는 수열 $\{ a_{n} \}$ 에 대하여 <보기>에서 옳은 것만을 있는 대로 고른 것은?

ㄱ. 수열 $\{ a_{n} - \frac{2}{3} \}$ 는 공비가 $-\frac{1}{2}$ 인 등비수열이다.  
ㄴ. $\lim_{n \to \infty} a_{n}$ 은 수렴한다.  
ㄷ. $\sum_{n=1}^{\infty} a_{n}$ 은 수렴한다.

## 보기
① ㄱ   ② ㄴ   ③ ㄱ, ㄴ   ④ ㄴ, ㄷ   ⑤ ㄱ, ㄴ, ㄷ

## 풀이
ㄱ. $2 a_{n+1} + a_{n} = 2$ 는 $2 ( a_{n+1} - \frac{2}{3} ) = - ( a_{n} - \frac{2}{3} )$ 이므로 수열 $\{ a_{n} - \frac{2}{3} \}$ 는 첫째항이 $a_{1} - \frac{2}{3} = 1 - \frac{2}{3} = \frac{1}{3}$, 공비는 $-\frac{1}{2}$ 인 등비수열이다. (참)

ㄴ. $a_{n} - \frac{2}{3} = \frac{1}{3} \left( -\frac{1}{2} \right)^{n-1}$ 이므로 $a_{n} = \frac{1}{3} \left( -\frac{1}{2} \right)^{n-1} + \frac{2}{3}$ 이다.
$\therefore \lim_{n \to \infty} a_{n} = \lim_{n \to \infty} \left\{ \frac{1}{3} \left( -\frac{1}{2} \right)^{n-1} + \frac{2}{3} \right\} = \frac{2}{3}$ (참)

ㄷ. $\lim_{n \to \infty} a_{n} = \frac{2}{3} \neq 0$ 이므로 급수 $\sum_{n=1}^{\infty} a_{n}$ 은 발산한다. (거짓)

정답 ③