## ë¬¸ì œ
ì—°ë¦½ë¶€ë“±ì‹ 
$$ \begin{cases} x(x-4)(x-5) \ge 0 \\ \frac{x-3}{x^{2}-3x+2} \le 0 \end{cases} $$ 
ì„ ë§Œì¡±ì‹œí‚¤ëŠ” ì •ìˆ˜ $x$ì˜ ê°œìˆ˜ëŠ”?



> [!example] ğŸ“¸ (ê·¸ë¦¼/ê·¸ë˜í”„)

## ë³´ê¸°
â‘  $1$   â‘¡ $2$   â‘¢ $3$   â‘£ $4$   â‘¤ $5$

## í’€ì´
$x(x-4)(x-5) \ge 0$ ì—ì„œ 
$0 \le x \le 4$ ë˜ëŠ” $x \ge 5$ $\cdots$ ã‰  

$\frac{x-3}{x^{2}-3x+2} = \frac{x-3}{(x-1)(x-2)} \le 0$ ì—ì„œ 
$(x-1)(x-2)(x-3) \le 0$ (ë‹¨, $x \neq 1, x \neq 2$) 
$\therefore x < 1$ ë˜ëŠ” $2 < x \le 3$ $\cdots$ ã‰¡ 

ã‰ , ã‰¡ì˜ ê³µí†µë²”ìœ„ëŠ” 
$0 \le x < 1$ ë˜ëŠ” $2 < x \le 3$ 
ì¦‰, ë§Œì¡±í•˜ëŠ” ì •ìˆ˜ $x$ëŠ” $0, 3$ì´ë‹¤.
ë”°ë¼ì„œ ì •ìˆ˜ $x$ì˜ ê°œìˆ˜ëŠ” $2$ì´ë‹¤.

ì •ë‹µ: â‘¡