## ë¬¸ì œ
ê·¸ë¦¼ê³¼ ê°™ì´ ì¢Œí‘œí‰ë©´ì—ì„œ ì› $x^{2}+y^{2}=2$ ì™€ í¬ë¬¼ì„  $y=x^{2}$ ìœ¼ë¡œ ë‘˜ëŸ¬ì‹¸ì¸ ì–´ë‘ìš´ ë¶€ë¶„ì„ $x$ ì¶• ë‘˜ë ˆë¡œ íšŒì „í•˜ì—¬ ìƒê¸°ëŠ” íšŒì „ì²´ì˜ ë¶€í”¼ëŠ”?

> [!example] ğŸ“¸ (ê·¸ë¦¼/ê·¸ë˜í”„)

## ë³´ê¸°
â‘  $\frac{41}{15}\pi$   â‘¡ $\frac{44}{15}\pi$   â‘¢ $\frac{47}{15}\pi$   â‘£ $\frac{43}{13}\pi$   â‘¤ $\frac{45}{13}\pi$

## í’€ì´
$$ \begin{array}{l} \text{(íšŒì „ì²´ì˜ ë¶€í”¼)} \\ = \pi \int_{-1}^{1} (2-x^{2}) dx - \pi \int_{-1}^{1} (x^{2})^{2} dx \\ = 2\pi \int_{0}^{1} (2-x^{2}) dx - 2\pi \int_{0}^{1} (x^{2})^{2} dx \\ = 2\pi \left[ 2x - \frac{1}{3}x^{3} \right]_{0}^{1} - 2\pi \left[ \frac{1}{5}x^{5} \right]_{0}^{1} \\ = 2\pi \left( 2 - \frac{1}{3} \right) - 2\pi \left( \frac{1}{5} \right) \\ = \frac{10}{3}\pi - \frac{2}{5}\pi \\ = \frac{44}{15}\pi \end{array} $$

[ì •ë‹µ] â‘¡