## 문제
두 함수 $f(x)=x+x^{3}+x^{5}$, $g(x)=x^{2}+x^{4}+x^{6}$ 에 대하여 $\lim_{h \to 0} \frac{f(1+2h)-g(1-h)}{3h}$ 의 값은?

## 보기
① $6$   ② $7$   ③ $8$   ④ $9$   ⑤ $10$

## 풀이
$f(x)=x+x^{3}+x^{5}$ 에서 $f'(x)=1+3x^{2}+5x^{4}$ 이므로
$f'(1)=1+3+5=9$
$g(x)=x^{2}+x^{4}+x^{6}$ 에서 $g'(x)=2x+4x^{3}+6x^{5}$ 이므로
$g'(1)=2+4+6=12$

이때 $f(1)=3$, $g(1)=3$ 이므로 $f(1)=g(1)$ 이다.
$\lim_{h \to 0} \frac{f(1+2h)-g(1-h)}{3h}$
$= \lim_{h \to 0} \frac{f(1+2h)-f(1)+g(1)-g(1-h)}{3h}$
$= \lim_{h \to 0} \frac{f(1+2h)-f(1)}{3h} + \lim_{h \to 0} \frac{g(1)-g(1-h)}{3h}$
$= \frac{2}{3} f'(1) + \frac{1}{3} g'(1)$
$= \frac{2}{3} \times 9 + \frac{1}{3} \times 12$
$= 6 + 4 = 10$

정답: ⑤