## 문제
수열 $\{ a_{n} \}$은 첫째항 $1$, 공비 $\frac{1}{3}$인 등비수열이고, 수열 $\{ b_{n} \}$은 첫째항 $1$, 공비 $\frac{1}{2}$인 등비수열이다. 다음 중 수렴하지 않는 무한급수는?

## 보기
① $\sum_{n=1}^{\infty} 2a_{n}$   ② $\sum_{n=1}^{\infty} (a_{n} - b_{n})$   ③ $\sum_{n=1}^{\infty} (-1)^{n} b_{n}$   ④ $\sum_{n=1}^{\infty} a_{n} b_{n}$   ⑤ $\sum_{n=1}^{\infty} \frac{b_{n}}{a_{n}}$

## 풀이
수열 $\{ a_{n} \}$은 첫째항이 $1$, 공비가 $\frac{1}{3}$인 등비수열이므로
$a_{n} = \left( \frac{1}{3} \right)^{n-1}$
수열 $\{ b_{n} \}$은 첫째항이 $1$, 공비가 $\frac{1}{2}$인 등비수열이므로
$b_{n} = \left( \frac{1}{2} \right)^{n-1}$

① $\sum_{n=1}^{\infty} 2a_{n} = 2 \sum_{n=1}^{\infty} \left( \frac{1}{3} \right)^{n-1} = 2 \times \frac{1}{1 - \frac{1}{3}} = 2 \times \frac{3}{2} = 3$ (수렴)

② $\sum_{n=1}^{\infty} (a_{n} - b_{n}) = \sum_{n=1}^{\infty} \left( \frac{1}{3} \right)^{n-1} - \sum_{n=1}^{\infty} \left( \frac{1}{2} \right)^{n-1} = \frac{1}{1 - \frac{1}{3}} - \frac{1}{1 - \frac{1}{2}} = \frac{3}{2} - 2 = -\frac{1}{2}$ (수렴)

③ $\sum_{n=1}^{\infty} (-1)^{n} b_{n} = \sum_{n=1}^{\infty} (-1)^{n} \left( \frac{1}{2} \right)^{n-1} = - \sum_{n=1}^{\infty} \left( -\frac{1}{2} \right)^{n-1} = - \frac{1}{1 - \left( -\frac{1}{2} \right)} = -\frac{2}{3}$ (수렴)

④ $\sum_{n=1}^{\infty} a_{n} b_{n} = \sum_{n=1}^{\infty} \left( \frac{1}{3} \right)^{n-1} \left( \frac{1}{2} \right)^{n-1} = \sum_{n=1}^{\infty} \left( \frac{1}{6} \right)^{n-1} = \frac{1}{1 - \frac{1}{6}} = \frac{6}{5}$ (수렴)

⑤ $\sum_{n=1}^{\infty} \frac{b_{n}}{a_{n}} = \sum_{n=1}^{\infty} \frac{(\frac{1}{2})^{n-1}}{(\frac{1}{3})^{n-1}} = \sum_{n=1}^{\infty} \left( \frac{3}{2} \right)^{n-1}$
이 급수는 공비가 $\frac{3}{2}$이고 $\left| \frac{3}{2} \right| \ge 1$이므로 발산한다.

따라서 수렴하지 않는 무한급수는 ⑤이다.

정답: ⑤