## 문제
자연수 $n$에 대하여 $f(n) = 2^{n} - \log_{2} n$이라 할 때, <보기>에서 옳은 것만을 있는 대로 고른 것은?

$$
\begin{array}{|l|}
\hline
\text{<보 기>} \\
ㄱ. \ f(2) = 3 \\
ㄴ. \ f(8) = -f(\log_{2} 8) \\
ㄷ. \ f(2^{n}) + n = \{f(2^{n-1}) + n - 1\}^{2} \\
\hline
\end{array}
$$

## 보기
① $ㄱ$   ② $ㄴ$   ③ $ㄱ, ㄴ$   ④ $ㄱ, ㄷ$   ⑤ $ㄱ, ㄴ, ㄷ$

## 풀이
$f(n) = 2^{n} - \log_{2} n$에서
ㄱ. $f(2) = 2^{2} - \log_{2} 2 = 4 - 1 = 3$ (참)
ㄴ. $f(8) = 2^{8} - \log_{2} 8 = 2^{8} - 3$
$-f(\log_{2} 8) = -f(3) = -(2^{3} - \log_{2} 3) = -2^{3} + \log_{2} 3$
$\therefore f(8) \neq -f(\log_{2} 8)$ (거짓)
ㄷ. $f(2^{n}) + n = 2^{2^{n}} - \log_{2} 2^{n} + n = 2^{2^{n}} - n + n = 2^{2^{n}}$
$\{f(2^{n-1}) + n - 1\}^{2} = \{2^{2^{n-1}} - \log_{2} 2^{n-1} + n - 1\}^{2}$
$= \{2^{2^{n-1}} - (n - 1) + n - 1\}^{2}$
$= (2^{2^{n-1}})^{2} = 2^{2^{n-1} \times 2} = 2^{2^{n}}$
$\therefore f(2^{n}) + n = \{f(2^{n-1}) + n - 1\}^{2}$ (참)

따라서 옳은 것은 $ㄱ, ㄷ$이다.

[정답] ④