## 문제
$\frac{1}{2-\sqrt{3}}-\frac{1}{2+\sqrt{3}}$ 의 값은?

## 보기
① $-2\sqrt{3}$   ② $-\sqrt{3}$   ③ $\sqrt{3}$   ④ $2\sqrt{3}$   ⑤ $4$

## 풀이
분모를 유리화하여 계산하면 다음과 같다.
$$ \frac{1}{2-\sqrt{3}}-\frac{1}{2+\sqrt{3}} $$
$$ = \frac{2+\sqrt{3}}{(2-\sqrt{3})(2+\sqrt{3})} - \frac{2-\sqrt{3}}{(2+\sqrt{3})(2-\sqrt{3})} $$
$$ = \frac{2+\sqrt{3}}{4-3} - \frac{2-\sqrt{3}}{4-3} $$
$$ = (2+\sqrt{3}) - (2-\sqrt{3}) $$
$$ = 2+\sqrt{3}-2+\sqrt{3} $$
$$ = 2\sqrt{3} $$

따라서 정답은 ④이다.

$2006$년 교육청 고$1$공통 $3$월 $3$ [$3.00$점]