## 문제
$a_{1} = 1$, $2a_{n+1} + a_{n} = 2$ ($n = 1, 2, 3, \dots$)를 만족시키는 수열 $\{a_{n}\}$에 대하여 <보기>에서 옳은 것만을 있는 대로 고른 것은?

---
**<보기>**
ㄱ. 수열 $\{ a_{n} - \frac{2}{3} \}$는 공비가 $-\frac{1}{2}$인 등비수열이다.
ㄴ. $\lim_{n \to \infty} a_{n}$은 수렴한다.
ㄷ. $\sum_{n=1}^{\infty} a_{n}$은 수렴한다.
---

## 보기
① ㄱ   ② ㄴ   ③ ㄱ, ㄴ   ④ ㄴ, ㄷ   ⑤ ㄱ, ㄴ, ㄷ

## 풀이
ㄱ. $2 a_{n+1} + a_{n} = 2$는 $2 ( a_{n+1} - \frac{2}{3} ) = - ( a_{n} - \frac{2}{3} )$이므로 수열 $\{ a_{n} - \frac{2}{3} \}$는 첫째항이 $a_{1} - \frac{2}{3} = 1 - \frac{2}{3} = \frac{1}{3}$, 공비가 $-\frac{1}{2}$인 등비수열이다. (참)

ㄴ. $a_{n} - \frac{2}{3} = \frac{1}{3} ( - \frac{1}{2} )^{n-1}$ 이므로 $a_{n} = \frac{1}{3} ( - \frac{1}{2} )^{n-1} + \frac{2}{3}$
$\therefore \lim_{n \to \infty} a_{n} = \lim_{n \to \infty} \{ \frac{1}{3} ( - \frac{1}{2} )^{n-1} + \frac{2}{3} \} = \frac{2}{3}$ (참)

ㄷ. $\lim_{n \to \infty} a_{n} = \frac{2}{3} \neq 0$이므로 급수 $\sum_{n=1}^{\infty} a_{n}$은 발산한다. (거짓)

따라서 옳은 것은 ㄱ, ㄴ이다.

정답: ③