## ë¬¸ì œ
ë‘ ì§‘í•©
$A = \{ x \mid (x - 1)(x - \sqrt[3]{4}) > 0 \}$,
$B = \{ x \mid (x - \sqrt[4]{8})(x - \sqrt[6]{6}) < 0 \}$
ì— ëŒ€í•˜ì—¬ $A \cup B$ëŠ”?

## ë³´ê¸°
â‘  $\{ x \mid x < 1 \text{ ë˜ëŠ” } x > \sqrt[3]{4} \}$   â‘¡ $\{ x \mid x < 1 \text{ ë˜ëŠ” } x > \sqrt[4]{8} \}$   â‘¢ $\{ x \mid x < 1 \text{ ë˜ëŠ” } x > \sqrt[6]{6} \}$   â‘£ $\{ x \mid 1 < x < \sqrt[4]{8} \}$   â‘¤ $\{ x \mid x \text{ ëŠ” ì‹¤ìˆ˜} \}$

## í’€ì´
$\sqrt[3]{4} = 4^{\frac{1}{3}}$, $\sqrt[4]{8} = 8^{\frac{1}{4}}$, $\sqrt[6]{6} = 6^{\frac{1}{6}}$ì´ë¯€ë¡œ
$(\sqrt[3]{4})^{12} = (4^{\frac{1}{3}})^{12} = 4^{4} = 256$
$(\sqrt[4]{8})^{12} = (8^{\frac{1}{4}})^{12} = 8^{3} = 512$
$(\sqrt[6]{6})^{12} = (6^{\frac{1}{6}})^{12} = 6^{2} = 36$
$\therefore 1 < \sqrt[6]{6} < \sqrt[3]{4} < \sqrt[4]{8}$

$(x - 1)(x - \sqrt[3]{4}) > 0$ ì—ì„œ ì§‘í•© $A$ì˜ í•´ëŠ” $x < 1$ ë˜ëŠ” $x > \sqrt[3]{4}$
$(x - \sqrt[4]{8})(x - \sqrt[6]{6}) < 0$ ì—ì„œ ì§‘í•© $B$ì˜ í•´ëŠ” $\sqrt[6]{6} < x < \sqrt[4]{8}$

ì´ë•Œ, ê°ê°ì˜ í•´ì§‘í•©ì„ ìˆ˜ì§ì„  ìœ„ì— ë‚˜íƒ€ë‚´ë©´ ë‹¤ìŒê³¼ ê°™ë‹¤.

> [!example] ğŸ“¸ (ê·¸ë¦¼/ê·¸ë˜í”„)

$\therefore A \cup B = \{ x \mid x < 1 \text{ ë˜ëŠ” } x > \sqrt[6]{6} \}$

ì •ë‹µ: â‘¢