## 문제
$\left\{ \frac{(\sqrt{10}+3)^{\frac{1}{2}}+(\sqrt{10}-3)^{\frac{1}{2}}}{(\sqrt{10}+1)^{\frac{1}{2}}} \right\}^{2}$ 의 값은?

## 보기
① $\sqrt{3}$   ② $2$   ③ $\sqrt{5}$   ④ $3$   ⑤ $\sqrt{10}$

## 풀이
(주어진 식) 
$$ = \frac{\left\{ (\sqrt{10}+3)^{\frac{1}{2}}+(\sqrt{10}-3)^{\frac{1}{2}} \right\}^{2}}{\left\{ (\sqrt{10}+1)^{\frac{1}{2}} \right\}^{2}} $$ 
$$ = \frac{(\sqrt{10}+3)+(\sqrt{10}-3)+2 \left\{ (\sqrt{10}+3)(\sqrt{10}-3) \right\}^{\frac{1}{2}}}{\sqrt{10}+1} $$ 
$$ = \frac{2\sqrt{10}+2 \cdot 1^{\frac{1}{2}}}{\sqrt{10}+1} $$ 
$$ = \frac{2(\sqrt{10}+1)}{\sqrt{10}+1} $$ 
$$ = 2 $$ 

정답: ②