## 문제
행렬 $$ A = \left( \begin{array}{cc} -1 & 3 \\ -1 & -1 \end{array} \right) $$ 에 대하여 $$ A^{6} \left( \begin{array}{c} 1 \\ 1 \end{array} \right) = \left( \begin{array}{c} a \\ b \end{array} \right) $$ 일 때, $$ a + b $$ 의 값을 구하시오.

## 풀이
$$ A \left( \begin{array}{c} 1 \\ 1 \end{array} \right) = \left( \begin{array}{cc} -1 & 3 \\ -1 & -1 \end{array} \right) \left( \begin{array}{c} 1 \\ 1 \end{array} \right) = \left( \begin{array}{c} 2 \\ -2 \end{array} \right) $$ 

$$ A^{2} \left( \begin{array}{c} 1 \\ 1 \end{array} \right) = \left( \begin{array}{cc} -1 & 3 \\ -1 & -1 \end{array} \right) \left( \begin{array}{c} 2 \\ -2 \end{array} \right) = \left( \begin{array}{c} -8 \\ 0 \end{array} \right) $$ 

$$ A^{3} \left( \begin{array}{c} 1 \\ 1 \end{array} \right) = \left( \begin{array}{cc} -1 & 3 \\ -1 & -1 \end{array} \right) \left( \begin{array}{c} -8 \\ 0 \end{array} \right) = \left( \begin{array}{c} 8 \\ 8 \end{array} \right) = 8 \left( \begin{array}{c} 1 \\ 1 \end{array} \right) $$ 

$$ A^{6} \left( \begin{array}{c} 1 \\ 1 \end{array} \right) = 8 A^{3} \left( \begin{array}{c} 1 \\ 1 \end{array} \right) = 64 \left( \begin{array}{c} 1 \\ 1 \end{array} \right) $$ 

따라서 $$ a = 64 $$, $$ b = 64 $$ 이므로
$$ a + b = 128 $$