## 문제
행렬 $A = \left( \begin{array}{cc} 1 & 0 \\ 1 & 2 \end{array} \right)$의 역행렬을 $B$라 할 때, $B^{n}$의 $(2, 1)$ 성분을 $a_{n}$이라 하자. $\sum_{k=1}^{10} a_{k}$의 값은?

## 보기
① $-11 - \frac{1}{2^{10}}$   ② $-10 - \frac{1}{2^{10}}$   ③ $-9 - \frac{1}{2^{10}}$   ④ $-10 - \frac{1}{2^{11}}$   ⑤ $-9 - \frac{1}{2^{11}}$

## 풀이
[정답] ③

$B = A^{-1} = \frac{1}{2} \left( \begin{array}{cc} 2 & 0 \\ -1 & 1 \end{array} \right)$

$B^{2} = \frac{1}{2} \left( \begin{array}{cc} 2 & 0 \\ -1 & 1 \end{array} \right) \cdot \frac{1}{2} \left( \begin{array}{cc} 2 & 0 \\ -1 & 1 \end{array} \right) = \frac{1}{2^{2}} \left( \begin{array}{cc} 2^{2} & 0 \\ -3 & 1 \end{array} \right)$

$B^{3} = \frac{1}{2^{2}} \left( \begin{array}{cc} 2^{2} & 0 \\ -3 & 1 \end{array} \right) \cdot \frac{1}{2} \left( \begin{array}{cc} 2 & 0 \\ -1 & 1 \end{array} \right) = \frac{1}{2^{3}} \left( \begin{array}{cc} 2^{3} & 0 \\ -7 & 1 \end{array} \right)$

$\vdots$

$B^{n} = \frac{1}{2^{n}} \left( \begin{array}{cc} 2^{n} & 0 \\ -2^{n} + 1 & 1 \end{array} \right)$

$a_{n} = \frac{-2^{n} + 1}{2^{n}}$

$\therefore \sum_{k=1}^{10} a_{k} = - \sum_{k=1}^{10} 1 + \sum_{k=1}^{10} \frac{1}{2^{k}} = -10 + \frac{\frac{1}{2} \left( 1 - \frac{1}{2^{10}} \right)}{1 - \frac{1}{2}}$

$= -10 + 1 - \frac{1}{2^{10}} = -9 - \frac{1}{2^{10}}$