## 문제
$\log_{10} 1.23 = \alpha$ 일 때, $\sum_{k=1}^{9}(-1)^{k-1} \log_{10} (123 \times 10^{k-1})$ 의 값은?

## 보기
① $2 + \alpha$   ② $3 - \alpha$   ③ $4 + \alpha$   ④ $5 - \alpha$   ⑤ $6 + \alpha$

## 풀이
$\log_{10} 1.23 = \alpha$ 이므로
$$ \sum_{k=1}^{9}(-1)^{k-1} \log_{10} (123 \times 10^{k-1}) $$
$$ = \sum_{k=1}^{9}(-1)^{k-1} \log_{10} (1.23 \times 10^{2} \times 10^{k-1}) $$
$$ = \sum_{k=1}^{9}(-1)^{k-1} \log_{10} (1.23 \times 10^{k+1}) $$
$$ = \sum_{k=1}^{9}(-1)^{k-1} (\log_{10} 1.23 + \log_{10} 10^{k+1}) $$
$$ = \sum_{k=1}^{9}(-1)^{k-1} (\alpha + k + 1) $$
이 식을 전개하면 다음과 같다.
$$ (\alpha + 2) - (\alpha + 3) + (\alpha + 4) - (\alpha + 5) + (\alpha + 6) - (\alpha + 7) + (\alpha + 8) - (\alpha + 9) + (\alpha + 10) $$
$$ = \{(\alpha + 2) - (\alpha + 3)\} + \{(\alpha + 4) - (\alpha + 5)\} + \{(\alpha + 6) - (\alpha + 7)\} + \{(\alpha + 8) - (\alpha + 9)\} + (\alpha + 10) $$
$$ = (-1) + (-1) + (-1) + (-1) + \alpha + 10 $$
$$ = 6 + \alpha $$

정답은 ⑤이다.