## 문제
두 행렬 $A = \begin{pmatrix} -1 & 0 \\ 0 & 1 \end{pmatrix}$, $B = \begin{pmatrix} 2 & 1 \\ 3 & 3 \end{pmatrix}$ 에 대하여 행렬 $(A+B)^{-1}$ 의 모든 성분의 합은?

## 보기
① $1$   ② $2$   ③ $3$   ④ $4$   ⑤ $5$

## 풀이
$A+B = \begin{pmatrix} -1 & 0 \\ 0 & 1 \end{pmatrix} + \begin{pmatrix} 2 & 1 \\ 3 & 3 \end{pmatrix} = \begin{pmatrix} 1 & 1 \\ 3 & 4 \end{pmatrix}$

$(A+B)^{-1} = \frac{1}{1 \times 4 - 1 \times 3} \begin{pmatrix} 4 & -1 \\ -3 & 1 \end{pmatrix}$
$= \frac{1}{1} \begin{pmatrix} 4 & -1 \\ -3 & 1 \end{pmatrix}$
$= \begin{pmatrix} 4 & -1 \\ -3 & 1 \end{pmatrix}$

따라서 모든 성분의 합은 
$4 + (-1) + (-3) + 1 = 1$

정답: ①