## 문제
두 등비수열 $\{ a_{n} \}$, $\{ b_{n} \}$ 에 대하여 <보기>에서 항상 옳은 것만을 있는 대로 고른 것은?

$$ \begin{array}{|l|} \hline \text{ㄱ. 두 등비급수 } \sum_{n=1}^{\infty} a_{n}, \sum_{n=1}^{\infty} b_{n} \text{ 이 수렴하면 } \sum_{n=1}^{\infty} a_{n} b_{n} \text{ 은 수렴한다.} \\ \text{ㄴ. 두 등비급수 } \sum_{n=1}^{\infty} a_{n}, \sum_{n=1}^{\infty} b_{n} \text{ 이 발산하면 } \lim_{n \to \infty} (a_{n} + b_{n}) \neq 0 \text{ 이다.} \\ \text{ㄷ. 두 등비급수 } \sum_{n=1}^{\infty} a_{n}^{3}, \sum_{n=1}^{\infty} b_{n}^{3} \text{ 이 수렴하면 } \sum_{n=1}^{\infty} (a_{n} + b_{n}) \text{ 은 수렴한다.} \\ \hline \end{array} $$

## 보기
① $ㄱ$   ② $ㄴ$   ③ $ㄷ$   ④ $ㄱ, ㄷ$   ⑤ $ㄱ, ㄴ, ㄷ$

## 풀이
[정답] ④

등비수열 $\{ a_{n} \}$, $\{ b_{n} \}$ 의 공비를 각각 $r_{1}$, $r_{2}$ 라 하자.

ㄱ. 두 등비급수 $\sum_{n=1}^{\infty} a_{n}$, $\sum_{n=1}^{\infty} b_{n}$ 이 수렴하면 $\sum_{n=1}^{\infty} a_{n} b_{n}$ 은 수렴한다. (참)
$\sum_{n=1}^{\infty} a_{n}$, $\sum_{n=1}^{\infty} b_{n}$ 이 각각 수렴하므로 $| r_{1} | < 1$, $| r_{2} | < 1$ 이다.
이때 수열 $\{ a_{n} b_{n} \}$ 의 공비가 $r_{1} r_{2}$ 이므로 $| r_{1} r_{2} | < 1$ 이다.
따라서 $\sum_{n=1}^{\infty} a_{n} b_{n}$ 은 수렴한다.

ㄴ. 두 등비급수 $\sum_{n=1}^{\infty} a_{n}$, $\sum_{n=1}^{\infty} b_{n}$ 이 발산하면 $\lim_{n \to \infty} (a_{n} + b_{n}) \neq 0$ 이다. (거짓)
(반례) 수열 $\{ a_{n} \}$ 이 $-1, 1, -1, 1, -1, 1, \dots$ 이고, 수열 $\{ b_{n} \}$ 이 $1, -1, 1, -1, 1, -1, \dots$ 이면
$\lim_{n \to \infty} a_{n} \neq 0$, $\lim_{n \to \infty} b_{n} \neq 0$ 이므로 $\sum_{n=1}^{\infty} a_{n}$, $\sum_{n=1}^{\infty} b_{n}$ 은 발산하지만 $\lim_{n \to \infty} (a_{n} + b_{n}) = 0$ 이다.

ㄷ. 두 등비급수 $\sum_{n=1}^{\infty} a_{n}^{3}$, $\sum_{n=1}^{\infty} b_{n}^{3}$ 이 수렴하면 $\sum_{n=1}^{\infty} (a_{n} + b_{n})$ 은 수렴한다. (참)
$-1 < (r_{1})^{3} < 1$, $-1 < (r_{2})^{3} < 1$ 이므로
$\therefore -1 < r_{1} < 1$, $-1 < r_{2} < 1$ 이다.
따라서 $\sum_{n=1}^{\infty} a_{n}$, $\sum_{n=1}^{\infty} b_{n}$ 이 수렴하고
$\sum_{n=1}^{\infty} (a_{n} + b_{n}) = \sum_{n=1}^{\infty} a_{n} + \sum_{n=1}^{\infty} b_{n}$ 이므로 $\sum_{n=1}^{\infty} (a_{n} + b_{n})$ 은 수렴한다.