## 문제
두 이차 정사각행렬 $A$, $B$가 
$$ A-B = \left( \begin{array}{cc} 0 & -3 \\ 12 & 2 \end{array} \right), 2A+B = \left( \begin{array}{cc} 6 & 3 \\ 9 & 7 \end{array} \right) $$
을 만족시킬 때, 행렬 $A$의 $(2, 1)$ 성분과 행렬 $B$의 $(2, 2)$ 성분의 합을 구하시오.

## 보기

## 풀이
$$ A-B = \left( \begin{array}{cc} 0 & -3 \\ 12 & 2 \end{array} \right) \cdots\cdots ㉠ $$
$$ 2A+B = \left( \begin{array}{cc} 6 & 3 \\ 9 & 7 \end{array} \right) \cdots\cdots ㉡ $$
㉠$+$㉡에서 
$$ A = \left( \begin{array}{cc} 2 & 0 \\ 7 & 3 \end{array} \right), B = \left( \begin{array}{cc} 2 & 3 \\ -5 & 1 \end{array} \right) $$
따라서 $A$의 $(2, 1)$ 성분은 $7$이고 $B$의 $(2, 2)$ 성분은 $1$이므로 합은 $8$이다.

[정답] $8$