## 문제
유리수 $a$, $b$에 대하여 $a + \frac{b}{2 - \sqrt{2}} = \sqrt{6 - 4\sqrt{2}}$가 성립할 때, $2a - b$의 값을 구하시오.

## 풀이
$a + \frac{b}{2 - \sqrt{2}} = \sqrt{6 - 4\sqrt{2}}$
$\sqrt{6 - 4\sqrt{2}} = \sqrt{6 - 2\sqrt{8}} = \sqrt{4} - \sqrt{2} = 2 - \sqrt{2}$이므로
$a + \frac{b(2 + \sqrt{2})}{(2 - \sqrt{2})(2 + \sqrt{2})} = 2 - \sqrt{2}$
$a + \frac{b(2 + \sqrt{2})}{2} = 2 - \sqrt{2}$
양변에 $2$를 곱하여 정리하면
$(2a + 2b) + b\sqrt{2} = 4 - 2\sqrt{2}$
$a$, $b$가 유리수이므로
$2a + 2b = 4$, $b = -2$
$b = -2$를 대입하면 $2a - 4 = 4$에서 $a = 4$이다.
따라서 $2a - b = 2 \times 4 - (-2) = 10$

정답: $10$