## 문제
두 행렬 $A = \left( \begin{array}{cc} 2 & 5 \\ 1 & 3 \end{array} \right)$, $B = \left( \begin{array}{cc} 3 & 2 \\ 2 & 1 \end{array} \right)$에 대하여 $A^{-1} B$의 모든 성분의 합은?

## 보기
① $1$   ② $2$   ③ $3$   ④ $4$   ⑤ $5$

## 풀이
$A = \left( \begin{array}{cc} 2 & 5 \\ 1 & 3 \end{array} \right)$이므로 역행렬 $A^{-1}$을 구하면 다음과 같다.
$$ A^{-1} = \frac{1}{2 \cdot 3 - 5 \cdot 1} \left( \begin{array}{cc} 3 & -5 \\ -1 & 2 \end{array} \right) = \left( \begin{array}{cc} 3 & -5 \\ -1 & 2 \end{array} \right) $$

따라서 $A^{-1} B$를 계산하면
$$ A^{-1} B = \left( \begin{array}{cc} 3 & -5 \\ -1 & 2 \end{array} \right) \left( \begin{array}{cc} 3 & 2 \\ 2 & 1 \end{array} \right) = \left( \begin{array}{cc} -1 & 1 \\ 1 & 0 \end{array} \right) $$
이 행렬의 모든 성분의 합은
$$ -1 + 1 + 1 + 0 = 1 $$
이다.

[정답] ①