## 문제
두 행렬 $A = \left( \begin{array}{cc} 2 & 1 \\ 1 & 1 \end{array} \right)$, $B = \left( \begin{array}{cc} 0 & 1 \\ 1 & 0 \end{array} \right)$ 에 대하여 행렬 $(AB)^{-1}$ 는?
(단, $X^{-1}$ 는 $X$ 의 역행렬)

## 보기
① $\left( \begin{array}{cc} 1 & 2 \\ 1 & 1 \end{array} \right)$ ② $\left( \begin{array}{cc} -1 & 2 \\ 1 & -1 \end{array} \right)$ ③ $\left( \begin{array}{cc} 1 & -2 \\ -1 & 1 \end{array} \right)$ ④ $\left( \begin{array}{cc} 1 & -2 \\ 1 & -1 \end{array} \right)$ ⑤ $\left( \begin{array}{cc} 1 & -2 \\ 1 & 1 \end{array} \right)$

## 풀이
두 행렬 $A = \left( \begin{array}{cc} 2 & 1 \\ 1 & 1 \end{array} \right)$, $B = \left( \begin{array}{cc} 0 & 1 \\ 1 & 0 \end{array} \right)$ 의 곱 $AB$를 구하면 다음과 같다.
$$ AB = \left( \begin{array}{cc} 2 & 1 \\ 1 & 1 \end{array} \right) \left( \begin{array}{cc} 0 & 1 \\ 1 & 0 \end{array} \right) = \left( \begin{array}{cc} 1 & 2 \\ 1 & 1 \end{array} \right) $$
행렬 $AB$의 역행렬 $(AB)^{-1}$는 다음과 같이 계산된다.
$$ (AB)^{-1} = \frac{1}{1 \times 1 - 2 \times 1} \left( \begin{array}{cc} 1 & -2 \\ -1 & 1 \end{array} \right) = - \left( \begin{array}{cc} 1 & -2 \\ -1 & 1 \end{array} \right) = \left( \begin{array}{cc} -1 & 2 \\ 1 & -1 \end{array} \right) $$

정답 ②