## 문제
두 행렬 $A = \left( \begin{array}{cc} -1 & 0 \\ 0 & 1 \end{array} \right)$, $B = \left( \begin{array}{cc} 2 & 1 \\ 3 & 3 \end{array} \right)$에 대하여 행렬 $(A+B)^{-1}$의 모든 성분의 합은?

## 보기
① $1$   ② $2$   ③ $3$   ④ $4$   ⑤ $5$

## 풀이
$$ A+B = \left( \begin{array}{cc} -1 & 0 \\ 0 & 1 \end{array} \right) + \left( \begin{array}{cc} 2 & 1 \\ 3 & 3 \end{array} \right) = \left( \begin{array}{cc} 1 & 1 \\ 3 & 4 \end{array} \right) $$

$$ (A+B)^{-1} = \frac{1}{1 \times 4 - 1 \times 3} \left( \begin{array}{cc} 4 & -1 \\ -3 & 1 \end{array} \right) = \left( \begin{array}{cc} 4 & -1 \\ -3 & 1 \end{array} \right) $$

따라서 모든 성분의 합은
$$ 4 + (-1) + (-3) + 1 = 1 $$
정답: ①