## 문제
이차정사각행렬 $A$에 대하여 
$$ A + A^{-1} = \left( \begin{array}{cc} -1 & 2 \\ 6 & 1 \end{array} \right) $$ 
일 때, $A^{2} + (A^{2})^{-1}$의 모든 성분의 합을 구하시오.

## 보기

## 풀이
$A A^{-1} = A^{-1} A = E$, $(A^{2})^{-1} = (A^{-1})^{2}$이고 
$$ (A + A^{-1})^{2} = \left( \begin{array}{cc} -1 & 2 \\ 6 & 1 \end{array} \right) \left( \begin{array}{cc} -1 & 2 \\ 6 & 1 \end{array} \right) = \left( \begin{array}{cc} 13 & 0 \\ 0 & 13 \end{array} \right) = 13 E $$ 
이므로 
$A^{2} + (A^{2})^{-1} = (A + A^{-1})^{2} - 2 A A^{-1} = 13 E - 2 E = 11 E$ 
따라서 구하는 모든 성분의 합은 $22$이다.