## ë¬¸ì œ
ë‘ ê³¡ì„  $y = \frac{1}{x}$, $y = \frac{1}{x+1}$ê³¼ ì§ì„  $x = n$ ($n$ì€ ìžì—°ìˆ˜)ì´ ë§Œë‚˜ëŠ” ì ì„ ê°ê° $A_n$, $B_n$ì´ë¼ í•˜ê³ , ì‚¬ê°í˜• $A_n B_n B_{n+1} A_{n+1}$ì˜ ë„“ì´ë¥¼ $S_n$ì´ë¼ í•˜ìž. ì´ë•Œ, $100 \sum_{n=1}^{\infty} S_n$ì˜ ê°’ì„ êµ¬í•˜ì‹œì˜¤.

## ë³´ê¸°

## í’€ì´
[ì •ë‹µ] $75$

$$
\begin{array}{l}
S_n \\
= 
\end{array}
$$

> [!example] ðŸ“¸ (ê·¸ë¦¼/ê·¸ëž˜í”„)

$$
\begin{array}{l}
- 
\end{array}
$$

> [!example] ðŸ“¸ (ê·¸ë¦¼/ê·¸ëž˜í”„)

$$
\begin{array}{l}
= \frac{1}{2} \cdot 1 \cdot \left( \frac{1}{n} + \frac{1}{n+1} \right) - \frac{1}{2} \cdot 1 \cdot \left( \frac{1}{n+1} + \frac{1}{n+2} \right) \\
= \frac{1}{2} \left( \frac{1}{n} - \frac{1}{n+2} \right)
\end{array}
$$

$$
\begin{array}{l}
\therefore \sum_{n=1}^{\infty} S_n = \lim_{n \to \infty} \sum_{k=1}^{n} S_k \\
= \lim_{n \to \infty} \left\{ \frac{1}{2} \left( 1 + \frac{1}{2} - \frac{1}{n+1} - \frac{1}{n+2} \right) \right\} \\
= \frac{3}{4}
\end{array}
$$

$$
\begin{array}{l}
\therefore 100 \sum_{n=1}^{\infty} S_n = 100 \cdot \frac{3}{4} = 75
\end{array}
$$