## 문제
다음 식을 간단히 한 것은?
$$(2^{x+y} + 2^{x-y})^{2} - (2^{x+y} - 2^{x-y})^{2}$$

## 보기
① $2^{2x}$   ② $2^{2x+2}$   ③ $2^{2x+2y}$   ④ $2^{-2y}$   ⑤ $2^{-2y+2}$

## 풀이
$$(2^{x+y} + 2^{x-y})^{2} - (2^{x+y} - 2^{x-y})^{2}$$
$$= \{2^{2(x+y)} + 2 \cdot 2^{x+y} \cdot 2^{x-y} + 2^{2(x-y)}\} - \{2^{2(x+y)} - 2 \cdot 2^{x+y} \cdot 2^{x-y} + 2^{2(x-y)}\}$$
$$= 2 \cdot 2^{x+y} \cdot 2^{x-y} + 2 \cdot 2^{x+y} \cdot 2^{x-y}$$
$$= 2 \cdot 2^{2x} + 2 \cdot 2^{2x}$$
$$= 4 \cdot 2^{2x}$$
$$= 2^{2} \cdot 2^{2x}$$
$$= 2^{2x+2}$$

정답은 ②이다.