## 문제
이차방정식 $9x^{2} - 6x - 1 = 0$ 의 두 근을 $\alpha$, $\beta$ 라 할 때, $\frac{1}{\beta - \alpha} \sum_{n=1}^{\infty} (\beta^{n} - \alpha^{n}) = \frac{q}{p}$ 이다. 이때, $p+q$ 의 값을 구하시오. (단, $p$ 와 $q$ 는 서로소인 자연수이다.)

## 보기

## 풀이
$9x^{2} - 6x - 1 = 0$ 의 두 근은 $x = \frac{1 \pm \sqrt{2}}{3}$ 이고, $|\alpha| < 1$, $|\beta| < 1$ 이므로 $\sum_{n=1}^{\infty} \alpha^{n}$, $\sum_{n=1}^{\infty} \beta^{n}$ 은 수렴한다.
근과 계수와의 관계에서 $\alpha + \beta = \frac{2}{3}$, $\alpha\beta = -\frac{1}{9}$ 이므로
$\frac{1}{\beta - \alpha} \sum_{n=1}^{\infty} (\beta^{n} - \alpha^{n}) = \frac{1}{\beta - \alpha} \left( \frac{\beta}{1 - \beta} - \frac{\alpha}{1 - \alpha} \right)$
$= \frac{1}{\beta - \alpha} \left( \frac{\beta(1 - \alpha) - \alpha(1 - \beta)}{(1 - \beta)(1 - \alpha)} \right)$
$= \frac{1}{\beta - \alpha} \cdot \frac{\beta - \alpha}{1 - (\alpha + \beta) + \alpha\beta}$
$= \frac{1}{1 - (\alpha + \beta) + \alpha\beta}$
$= \frac{1}{1 - \frac{2}{3} - \frac{1}{9}} = \frac{1}{\frac{2}{9}} = \frac{9}{2}$
따라서 $p = 2$, $q = 9$ 이므로 $p + q = 2 + 9 = 11$ 이다.