## 문제
$0$이 아닌 세 실수 $x$, $y$, $z$가 
$$\sqrt{x} \sqrt{y} = \sqrt{xy}$$
$$\frac{\sqrt{z}}{\sqrt{y}} = -\sqrt{\frac{z}{y}}$$
를 만족할 때, $|x-y| + |y-z| - \sqrt{(x-y+z)^2}$을 간단히 하면?

## 보기
① $2x$   ② $-y$   ③ $2x-y$   ④ $y-2z$   ⑤ $x-2z$

## 풀이
$\sqrt{x} \sqrt{y} = \sqrt{xy}$, $\frac{\sqrt{z}}{\sqrt{y}} = -\sqrt{\frac{z}{y}}$를 만족시키므로 
$x > 0$, $y < 0$, $z > 0$이다.

따라서 
$x - y > 0$, 
$y - z < 0$, 
$x - y + z > 0$이므로 

$|x - y| + |y - z| - \sqrt{(x - y + z)^2}$
$= (x - y) - (y - z) - (x - y + z)$
$= x - y - y + z - x + y - z$
$= -y$

정답: ②