## ë¬¸ì œ
ì‹¤ìˆ˜ ì „ì²´ì˜ ì§‘í•©ì—ì„œ ì •ì˜ëœ ë‘ í•¨ìˆ˜ $f(x)=5x+20$, $g(x)=\begin{cases} 2x & (x < 25) \\ x+25 & (x \geq 25) \end{cases}$ ì— ëŒ€í•˜ì—¬ $f(g^{-1}(40)) + f^{-1}(g(40))$ ì˜ ê°’ì„ êµ¬í•˜ì‹œì˜¤. (ë‹¨, $f^{-1}$, $g^{-1}$ ëŠ” ê°ê° $f$, $g$ ì˜ ì—­í•¨ìˆ˜ì´ë‹¤.)



> [!example] ğŸ“¸ (ê·¸ë¦¼/ê·¸ë˜í”„)

## ë³´ê¸°

## í’€ì´
$f(x)=5x+20$ ì—ì„œ $f(x)$ ì˜ ì—­í•¨ìˆ˜ëŠ” 
$f^{-1}(x)=\frac{1}{5}x-4$ 
$g(x)=\begin{cases} 2x & (x < 25) \\ x+25 & (x \geq 25) \end{cases}$ ì—ì„œ $g(x)$ ì˜ ì—­í•¨ìˆ˜ëŠ” 
$g^{-1}(x)=\begin{cases} \frac{1}{2}x & (x < 50) \\ x-25 & (x \geq 50) \end{cases}$ 
$\therefore f(g^{-1}(40)) + f^{-1}(g(40))$
$= f\left(\frac{1}{2} \cdot 40\right) + f^{-1}(40+25)$
$= f(20) + f^{-1}(65) = 120 + 9 = 129$

ì •ë‹µ: $129$