## 문제
$|\sqrt{2} - \sqrt[3]{3}| + |\sqrt[3]{3} - \sqrt[5]{5}| + |\sqrt[5]{5} - \sqrt{2}|$를 간단히 하면?

## 보기
① $0$   ② $2\sqrt[3]{3}$   ③ $2(\sqrt[5]{5} - \sqrt{2})$   ④ $2(\sqrt[3]{3} - \sqrt{2})$   ⑤ $2(\sqrt[3]{3} - \sqrt[5]{5})$

## 풀이
$[$정답$]$ ⑤

$\sqrt{2} = 2^{\frac{1}{2}}$,
$\sqrt[3]{3} = 3^{\frac{1}{3}}$,
$\sqrt[5]{5} = 5^{\frac{1}{5}}$

$2^{\frac{1}{2}}$, $3^{\frac{1}{3}}$에서
$(2^{\frac{1}{2}})^{6} = 2^{3} = 8$,
$(3^{\frac{1}{3}})^{6} = 3^{2} = 9$
$\therefore \sqrt{2} < \sqrt[3]{3} \cdots$ ㉠

$2^{\frac{1}{2}}$, $5^{\frac{1}{5}}$에서
$(2^{\frac{1}{2}})^{10} = 2^{5} = 32$,
$(5^{\frac{1}{5}})^{10} = 5^{2} = 25$
$\therefore \sqrt[5]{5} < \sqrt{2} \cdots$ ㉡

㉠, ㉡에서
$\sqrt[5]{5} < \sqrt{2} < \sqrt[3]{3}$

$\therefore |\sqrt{2} - \sqrt[3]{3}| + |\sqrt[3]{3} - \sqrt[5]{5}| + |\sqrt[5]{5} - \sqrt{2}|$
$= -(\sqrt{2} - \sqrt[3]{3}) + (\sqrt[3]{3} - \sqrt[5]{5}) - (\sqrt[5]{5} - \sqrt{2})$
$= -\sqrt{2} + \sqrt[3]{3} + \sqrt[3]{3} - \sqrt[5]{5} - \sqrt[5]{5} + \sqrt{2}$
$= 2(\sqrt[3]{3} - \sqrt[5]{5})$