## ë¬¸ì œ
$\int_{0}^{2} | x^{2} (x - 1) | dx$ ì˜ ê°’ì€?

## ë³´ê¸°
â‘  $\frac{3}{2}$   â‘¡ $2$   â‘¢ $\frac{5}{2}$   â‘£ $3$   â‘¤ $\frac{7}{2}$

## í’€ì´
ì˜¤ë¥¸ìª½ ê·¸ë¦¼ì—ì„œ $\int_{0}^{2} | x^{2} (x - 1) | dx$ ëŠ” $y = x^{2} (x - 1)$ ì˜ ì–´ë‘ìš´ ë¶€ë¶„ì˜ ë„“ì´ì´ë‹¤.

> [!example] ğŸ“¸ (ê·¸ë¦¼/ê·¸ë˜í”„)

$\therefore$ (ì£¼ì–´ì§„ ì‹)
$= \int_{0}^{1} \{ -x^{2} (x - 1) \} dx + \int_{1}^{2} \{ x^{2} (x - 1) \} dx$
$= - \int_{0}^{1} (x^{3} - x^{2}) dx + \int_{1}^{2} (x^{3} - x^{2}) dx$
$= - [ \frac{1}{4} x^{4} - \frac{1}{3} x^{3} ]_{0}^{1} + [ \frac{1}{4} x^{4} - \frac{1}{3} x^{3} ]_{1}^{2}$
$= - ( \frac{1}{4} - \frac{1}{3} ) + \frac{1}{4} (2^{4} - 1^{4}) - \frac{1}{3} (2^{3} - 1^{3}) = \frac{3}{2}$

ì •ë‹µ: â‘ 