## 문제
첫째항이 $1$, 공비가 $\frac{1}{2}$인 등비수열 $\{ a_{n} \}$에 대하여 $S_{n}$, $T_{n}$을 다음과 같이 정의하자. 
$$ S_{n} = \sum_{k=1}^{n} a_{k}, \quad T_{n} = \sum_{k=n}^{\infty} a_{k} $$
다음 <보기>에서 옳은 것을 모두 고른 것은?

<보기>
ㄱ. $a_{n} + S_{n} = 2$ (단, $n=1, 2, 3, \dots$)
ㄴ. $T_{n} = a_{n-1}$ (단, $n=2, 3, 4, \dots$)
ㄷ. $\lim_{n \to \infty} ( S_{n} + T_{n} ) = \sum_{k=1}^{\infty} a_{k}$

## 보기
① ㄱ   ② ㄴ   ③ ㄱ, ㄴ   ④ ㄴ, ㄷ   ⑤ ㄱ, ㄴ, ㄷ

## 풀이
[정답] ⑤ 

$a_{n} = 1 \cdot \left( \frac{1}{2} \right)^{n-1} = \left( \frac{1}{2} \right)^{n-1}$ 

$\therefore S_{n} = \frac{1 \cdot \left( 1 - \left( \frac{1}{2} \right)^{n} \right)}{1 - \frac{1}{2}} = 2 - \left( \frac{1}{2} \right)^{n-1}$

$T_{n} = \frac{\left( \frac{1}{2} \right)^{n-1}}{1 - \frac{1}{2}} = \left( \frac{1}{2} \right)^{n-2} = a_{n-1}$

ㄱ) $a_{n} + S_{n} = 2$ 

ㄴ) $T_{n} = a_{n-1}$ 

ㄷ) $\lim_{n \to \infty} ( S_{n} + T_{n} ) = \lim_{n \to \infty} ( 2 - a_{n} + a_{n-1} ) = 2$ 

($\because \lim_{n \to \infty} a_{n} = \lim_{n \to \infty} a_{n-1} = 0$) 

$\sum_{k=1}^{\infty} a_{k} = \frac{1}{1 - \frac{1}{2}} = 2$ 

$\therefore \lim_{n \to \infty} ( S_{n} + T_{n} ) = \sum_{k=1}^{\infty} a_{k} = 2$ 

그러므로 ㄱ, ㄴ, ㄷ 모두 옳다.