## 문제
$a=1+\sqrt{2}-\sqrt{3}$, $b=1-\sqrt{2}+\sqrt{3}$ 일 때, $\sqrt{a^{3}+b^{3}+1}$ 을 간단히 하면 $p+2\sqrt{q}$ 이다. 이때 $p+q$ 의 값을 구하시오. (단, $p$, $q$ 는 유리수이다.)

## 보기

## 풀이
$s=1$, $t=\sqrt{2}-\sqrt{3}$ 이라 하면
$a=s+t$, $b=s-t$ 이다.
$a^{3}+b^{3} = (s+t)^{3}+(s-t)^{3} = 2s^{3}+6st^{2}$
$= 2+6(\sqrt{2}-\sqrt{3})^{2}$
$= 2+6(2-2\sqrt{6}+3)$
$= 2+6(5-2\sqrt{6})$
$= 32-12\sqrt{6}$

$\therefore a^{3}+b^{3}+1 = 33-12\sqrt{6} = 33-2\sqrt{216}$

$\sqrt{a^{3}+b^{3}+1} = \sqrt{33-2\sqrt{216}}$
$= \sqrt{(24+9)-2\sqrt{24 \times 9}}$
$= \sqrt{24}-\sqrt{9}$
$= 2\sqrt{6}-3$
$= -3+2\sqrt{6}$

따라서 $p+2\sqrt{q} = -3+2\sqrt{6}$ 이므로
$p = -3$, $q = 6$ 이다.
$\therefore p+q = -3+6 = 3$

[정답] $3$