## 문제
두 행렬 $$ A = \left( \begin{array}{cc} 1 & -2 \\ x & -1 \end{array} \right) $$, $$ B = \left( \begin{array}{cc} 1 & 2 \\ -3 & y \end{array} \right) $$ 에 대하여 $$ (A+B)^{2}=A^{2}+B^{2} $$ 이 성립하도록 실수 $$ x $$, $$ y $$ 를 정할 때, $$ x^{2}+y^{2} $$ 의 값을 구하시오.

## 보기

## 풀이
$$ (A+B)^{2}=A^{2}+B^{2} $$ 이 성립하려면 $$ AB+BA=O $$ 이어야 하므로 $$ AB=-BA $$ 이다.

$$ \left( \begin{array}{cc} 1 & -2 \\ x & -1 \end{array} \right) \left( \begin{array}{cc} 1 & 2 \\ -3 & y \end{array} \right) = - \left( \begin{array}{cc} 1 & 2 \\ -3 & y \end{array} \right) \left( \begin{array}{cc} 1 & -2 \\ x & -1 \end{array} \right) $$

$$ \left( \begin{array}{cc} 7 & 2-2y \\ x+3 & 2x-y \end{array} \right) = - \left( \begin{array}{cc} 1+2x & -4 \\ -3+xy & 6-y \end{array} \right) $$

$$ \left( \begin{array}{cc} 7 & 2-2y \\ x+3 & 2x-y \end{array} \right) = \left( \begin{array}{cc} -1-2x & 4 \\ 3-xy & -6+y \end{array} \right) $$

두 행렬이 서로 같을 조건에 의해
$$ 7 = -1-2x $$ 에서 $$ x = -4 $$
$$ 2-2y = 4 $$ 에서 $$ y = -1 $$

$$ \therefore x^{2}+y^{2} = (-4)^{2}+(-1)^{2} = 17 $$