## 문제
$(x^2 - x)(x^2 + 3x + 2) - 3$을 인수분해하면 $(x^2 + ax + b)(x^2 + cx + d)$이다. 이때, $a+b+c+d$의 값은? (단, $a$, $b$, $c$, $d$는 상수이다.)

## 보기
① $-2$   ② $-1$   ③ $0$   ④ $1$   ⑤ $2$

## 풀이
$(x^2 - x)(x^2 + 3x + 2) - 3$
$= x(x - 1)(x + 1)(x + 2) - 3$
$= \{x(x + 1)\}\{(x - 1)(x + 2)\} - 3$
$= (x^2 + x)(x^2 + x - 2) - 3$
에서 $x^2 + x = A$로 놓으면
$(x^2 + x)(x^2 + x - 2) - 3$
$= A(A - 2) - 3$
$= A^2 - 2A - 3$
$= (A + 1)(A - 3)$
$= (x^2 + x + 1)(x^2 + x - 3)$
이 식을 $(x^2 + ax + b)(x^2 + cx + d)$와 비교하면 상수 $a$, $b$, $c$, $d$의 합은 다음과 같다.
$a = 1, b = 1, c = 1, d = -3$ (또는 순서가 바뀜)
따라서 $a + b + c + d = 1 + 1 + 1 + (-3) = 0$

정답: ③