## 문제

함수 $f_n(x) = \left( nx - \sum_{k=1}^{n} a_k \right)^2$ ($a_1, a_2, a_3, \dots, a_n$은 상수)가 $\int_{0}^{1} f_n'(x) dx = -n^3$을 만족할 때, <보기>에서 옳은 것만을 있는 대로 고른 것은?

$$ \begin{array}{|l|} \hline \text{<보 기>} \\ \text{ㄱ. } \sum_{k=1}^{n} a_k = \frac{n(n+1)}{2} \\ \text{ㄴ. } f_2(2) = 3 \\ \text{ㄷ. } \int_{0}^{n+1} f_n(x) dx = 2 \int_{0}^{\frac{n+1}{2}} f_n(x) dx \\ \hline \end{array} $$

## 보기

① $ㄱ$   ② $ㄴ$   ③ $ㄷ$   ④ $ㄱ, ㄷ$   ⑤ $ㄱ, ㄴ, ㄷ$

## 풀이

[정답] ④

$f_n(x) = \left( nx - \sum_{k=1}^{n} a_k \right)^2 = (nx - S_n)^2$

ㄱ. $\sum_{k=1}^{n} a_k = S_n$이라 하면
$\int_{0}^{1} f_n'(x) dx = [f_n(x)]_0^1 = f_n(1) - f_n(0) = -n^3$에서
$(n - S_n)^2 - (-S_n)^2 = -n^3$
$n^2 - 2nS_n + S_n^2 - S_n^2 = -n^3$
$n^2 - 2nS_n = -n^3$
$n - 2S_n = -n^2$
$2S_n = n^2 + n = n(n+1)$
$S_n = \frac{n(n+1)}{2}$ (참)

ㄴ. $n=2$일 때, $S_2 = \frac{2(3)}{2} = 3$이므로
$f_2(x) = (2x - 3)^2$
$f_2(2) = (4 - 3)^2 = 1 \neq 3$ (거짓)

ㄷ. $f_n(x) = \left( nx - \frac{n(n+1)}{2} \right)^2 = n^2 \left( x - \frac{n+1}{2} \right)^2$는 
$x = \frac{n+1}{2}$에 대하여 대칭인 이차함수이므로
$\int_{0}^{n+1} f_n(x) dx = 2 \int_{0}^{\frac{n+1}{2}} f_n(x) dx$ (참)

따라서 옳은 것은 ㄱ, ㄷ이다.