## 문제
방정식 $3 ( 1 - \log_{ 2 } x )^{ 2 } - 2 ( 1 - \log_{ 2 } x ) - 4 = 0$의 두 근을 각각 $\alpha$, $\beta$라 할 때, $\alpha^{ 3 } \beta^{ 3 }$의 값을 구하시오.

## 풀이
$\log_{ 2 } x = t$라 두면 주어진 방정식의 두 근은 $\log_{ 2 } \alpha$, $\log_{ 2 } \beta$가 된다. 
$3 ( 1 - t )^{ 2 } - 2 ( 1 - t ) - 4 = 0$
$3 t^{ 2 } - 4 t - 3 = 0$
이 방정식의 두 근의 합은 
$\log_{ 2 } \alpha + \log_{ 2 } \beta = \log_{ 2 } \alpha \beta = - \frac{ -4 }{ 3 } = \frac{ 4 }{ 3 }$
따라서 $\alpha \beta = 2^{ \frac{ 4 }{ 3 } }$
$\therefore \alpha^{ 3 } \beta^{ 3 } = ( \alpha \beta )^{ 3 } = ( 2^{ \frac{ 4 }{ 3 } } )^{ 3 } = 2^{ 4 } = 16$

정답: $16$