## 문제
이차정사각행렬 $A$ 가 
$$ A^{2}+A = \left( \begin{array}{cc} 11 & -6 \\ 6 & 5 \end{array} \right) $$ 
$$ A^{2}-A = \left( \begin{array}{cc} 5 & -4 \\ 4 & 1 \end{array} \right) $$ 
을 만족시킬 때, 행렬 $A$ 의 모든 성분의 합은? 

## 보기
① $1$   ② $2$   ③ $3$   ④ $4$   ⑤ $5$

## 풀이
주어진 두 식을 빼면 다음과 같다.
$$ (A^{2}+A) - (A^{2}-A) $$ 
$$ = \left( \begin{array}{cc} 11 & -6 \\ 6 & 5 \end{array} \right) - \left( \begin{array}{cc} 5 & -4 \\ 4 & 1 \end{array} \right) $$ 
$$ 2A = \left( \begin{array}{cc} 6 & -2 \\ 2 & 4 \end{array} \right) $$ 
$$ A = \left( \begin{array}{cc} 3 & -1 \\ 1 & 2 \end{array} \right) $$ 
따라서 행렬 $A$ 의 모든 성분의 합은 
$$ 3 + (-1) + 1 + 2 = 5 $$ 
정답은 ⑤이다.