## 문제
수열 $\{a_{n}\}$에 대하여 $S_{n} = \sum_{k=1}^{n} a_{k}$라 하자. $\lim_{n \to \infty} \frac{S_{n}}{n^{2}} = \frac{1}{2}$일 때, $\lim_{n \to \infty} \frac{\sum_{k=1}^{n} (2+a_{k})}{\sum_{k=1}^{n} (2k+a_{k})}$의 값은?

## 보기
① $2$   ② $1$   ③ $\frac{1}{2}$   ④ $\frac{1}{3}$   ⑤ $\frac{1}{4}$

## 풀이
$\sum_{k=1}^{n} (2+a_{k}) = 2n+S_{n}$, 
$\sum_{k=1}^{n} (2k+a_{k}) = n(n+1)+ \sum_{k=1}^{n} a_{k} = n^{2} +n+S_{n}$이므로 
$\lim_{n \to \infty} \frac{\sum_{k=1}^{n} (2+a_{k})}{\sum_{k=1}^{n} (2k+a_{k})}$
$= \lim_{n \to \infty} \frac{2n +S_{n}}{n^{2} +n+S_{n}}$ 
$= \lim_{n \to \infty} \frac{\frac{2}{n} + \frac{S_{n}}{n^{2}}}{1+ \frac{1}{n} + \frac{S_{n}}{n^{2}}}$ 
$= \frac{0+ \frac{1}{2}}{1+ 0+ \frac{1}{2}} = \frac{1}{3}$
따라서 정답은 ④이다.