## 문제
두 행렬 $A = \left( \begin{array}{cc} 1 & 3 \\ 1 & 2 \end{array} \right)$, $B = \left( \begin{array}{cc} -2 & 3 \\ 1 & -1 \end{array} \right)$에 대하여 행렬 $AB(A+B)$는?

## 보기
① $\left( \begin{array}{cc} -1 & 6 \\ 2 & 1 \end{array} \right)$   ② $\left( \begin{array}{cc} -1 & 6 \\ 1 & 2 \end{array} \right)$   ③ $\left( \begin{array}{cc} -1 & 2 \\ 2 & 6 \end{array} \right)$   ④ $\left( \begin{array}{cc} 1 & 6 \\ -2 & 1 \end{array} \right)$   ⑤ $\left( \begin{array}{cc} 1 & 6 \\ 2 & 2 \end{array} \right)$

## 풀이
$$ AB = \left( \begin{array}{cc} 1 & 3 \\ 1 & 2 \end{array} \right) \left( \begin{array}{cc} -2 & 3 \\ 1 & -1 \end{array} \right) = \left( \begin{array}{cc} 1 & 0 \\ 0 & 1 \end{array} \right) = E $$
이므로
$$ AB(A+B) = E(A+B) = A+B = \left( \begin{array}{cc} -1 & 6 \\ 2 & 1 \end{array} \right) $$
따라서 정답은 ①이다.