## ë¬¸ì œ
ì§‘í•© $X = \{ 1, 2, 3 \}$ì— ëŒ€í•˜ì—¬ í•¨ìˆ˜ $f : X \to X$ë¥¼ ë‹¤ìŒê³¼ ê°™ì´ ì •ì˜í•œë‹¤.

> [!example] ğŸ“¸ (ê·¸ë¦¼/ê·¸ë˜í”„)

$f^{1}(x) = f(x)$, $f^{n+1}(x) = f(f^{n}(x))$ ($n = 1, 2, 3, \dots$)ë¼ í•  ë•Œ, $f^{100}(1) - f^{200}(3)$ì˜ ê°’ì€?

## ë³´ê¸°
â‘  $-2$   â‘¡ $2$   â‘¢ $-1$   â‘£ $1$   â‘¤ $0$

## í’€ì´
ì •ë‹µ: â‘¤

ê·¸ë¦¼ê³¼ ê°™ì´ ëŒ€ì‘ê´€ê³„ë¥¼ ì´ìš©í•˜ì—¬ í•©ì„±í•¨ìˆ˜ì˜ ê°’ì„ êµ¬í•˜ë©´ 

$$f^{3}(1) = f(f(f(1))) = f(f(2)) = f(3) = 1$$ 

ê°™ì€ ë°©ë²•ìœ¼ë¡œ 
$$f^{3}(2) = 2$$, 
$$f^{3}(3) = 3$$ì´ë‹¤. 

$$\therefore f^{3}(x) = x$$ 

$$f^{100}(x) = (f^{3 \cdot 33} \circ f)(x) = f(x)$$, 
$$f^{200}(x) = (f^{3 \cdot 66} \circ f^{2})(x) = f^{2}(x)$$ 

$$\therefore f^{100}(1) = f(1) = 2$$ 

$$f^{200}(3) = f^{2}(3) = f(f(3)) = f(1) = 2$$ 

$$\therefore f^{100}(1) - f^{200}(3) = 2 - 2 = 0$$