## ë¬¸ì œ
$a_{1}=1$ ì´ê³  ëª¨ë“  ìì—°ìˆ˜ $n$ ì— ëŒ€í•˜ì—¬ $a_{n}<a_{n+1}$ ì¸ ìˆ˜ì—´ $\{ a_{n} \}$ ì´ ìˆë‹¤. ê³¡ì„  $y=x^{2}$ ê³¼ $x$ ì¶• ë° ë‘ ì§ì„  $x=a_{n}$, $x=a_{n+1}$ ë¡œ ë‘˜ëŸ¬ì‹¸ì¸ ë„í˜•ì˜ ë„“ì´ê°€ $14 \left( \frac{1}{3} \right)^{n-1}$ ì¼ ë•Œ, $\lim_{n \to \infty} a_{n}$ ì˜ ê°’ì€?

> [!example] ğŸ“¸ (ê·¸ë¦¼/ê·¸ë˜í”„)

## ë³´ê¸°
â‘  $\sqrt[3]{5}$   â‘¡ $\sqrt[3]{4}$   â‘¢ $\sqrt[3]{3}$   â‘£ $4$   â‘¤ $5$

## í’€ì´
[ì •ë‹µ] â‘£

$$ \int_{a_{n}}^{a_{n+1}} x^{2} dx = \frac{1}{3} (a_{n+1}^{3} - a_{n}^{3}) = 14 \left( \frac{1}{3} \right)^{n-1} $$

$$ \therefore a_{n+1}^{3} - a_{n}^{3} = 42 \left( \frac{1}{3} \right)^{n-1} $$

$$ a_{n}^{3} = 1 + \sum_{k=1}^{n-1} 42 \left( \frac{1}{3} \right)^{k-1} = 1 + 63 \left\{ 1 - \left( \frac{1}{3} \right)^{n-1} \right\} $$

$$ \therefore \lim_{n \to \infty} a_{n} = \alpha \text{ ë¼ í•˜ë©´} $$

$$ \lim_{n \to \infty} a_{n}^{3} = \alpha^{3} = 1 + 63 = 64 $$

$$ \therefore \lim_{n \to \infty} a_{n} = \alpha = 4 $$