## 문제
일반항이 $a_{n} = \sqrt{9 n^{2}-2 n} - [ \sqrt{9 n^{2}-2 n} ]$인 수열 $\{ a_{n} \}$에 대하여 $\lim_{n \to \infty} a_{n}$의 값은? (단, $[x]$는 $x$보다 크지 않은 최대의 정수이다.)

## 보기
① $\frac{1}{9}$   ② $\frac{1}{7}$   ③ $\frac{2}{9}$   ④ $\frac{1}{3}$   ⑤ $\frac{2}{3}$

## 풀이
[정답] ⑤

수열 $\{ a_{n} \}$은 $\sqrt{9 n^{2}-2 n}$의 소수부분이다.
$\sqrt{(3 n-1)^{2}} < \sqrt{9 n^{2}-2 n} < \sqrt{(3 n)^{2}}$ 이므로 $\sqrt{9 n^{2}-2 n}$의 정수부분은 $3 n-1$이다.
즉, $a_{n} = \sqrt{9 n^{2}-2 n} - (3 n-1)$로 나타낼 수 있다.
따라서
$\lim_{n \to \infty} a_{n} = \lim_{n \to \infty} \{ \sqrt{9 n^{2}-2 n} - (3 n-1) \}$
$= \lim_{n \to \infty} \frac{(\sqrt{9 n^{2}-2 n} - (3 n-1))(\sqrt{9 n^{2}-2 n} + (3 n-1))}{\sqrt{9 n^{2}-2 n} + (3 n-1)}$
$= \lim_{n \to \infty} \frac{(9 n^{2}-2 n) - (3 n-1)^{2}}{\sqrt{9 n^{2}-2 n} + (3 n-1)}$
$= \lim_{n \to \infty} \frac{(9 n^{2}-2 n) - (9 n^{2}-6 n+1)}{\sqrt{9 n^{2}-2 n} + (3 n-1)}$
$= \lim_{n \to \infty} \frac{4 n-1}{\sqrt{9 n^{2}-2 n} + (3 n-1)}$
분모, 분자를 $n$으로 나누면
$= \lim_{n \to \infty} \frac{4 - \frac{1}{n}}{\sqrt{9 - \frac{2}{n}} + (3 - \frac{1}{n})}$
$= \frac{4}{\sqrt{9} + 3} = \frac{4}{3+3} = \frac{4}{6} = \frac{2}{3}$