## 문제
두 다항함수 $f(x)$, $g(x)$가 다음 조건을 만족시킬 때, $g'(0)$의 값을 구하시오.

(가) $f(0)=1$, $f'(0)=-6$, $g(0)=4$
(나) $\lim_{x \to 0} \frac{f(x)g(x)-4}{x} = 0$

## 풀이
(나)에서 $f(0)g(0)=4$이므로 
$\lim_{x \to 0} \frac{f(x)g(x)-4}{x} = \lim_{x \to 0} \frac{f(x)g(x)-f(0)g(0)}{x}$이다. 
여기서 $f(x)g(x)=k(x)$라 하면 
(주어진 식) $= \lim_{x \to 0} \frac{k(x)-k(0)}{x} = k'(0)$
$k'(x) = f'(x)g(x) + f(x)g'(x)$에서 
$k'(0) = f'(0)g(0) + f(0)g'(0)$
$= -6 \times 4 + 1 \times g'(0)$
$= -24 + g'(0)$
따라서 $-24 + g'(0) = 0$
$\therefore g'(0) = 24$

정답: $24$