## 문제
두 행렬 $$ A = \left( \begin{array}{cc} 2 & -2 \\ -5 & 12 \end{array} \right) $$, $$ B = \left( \begin{array}{cc} a & b \\ c & d \end{array} \right) $$ 에 대하여
$$ (A-E) B=E $$
가 성립할 때, 상수 $a$, $d$의 합 $a+d$의 값을 구하시오. (단, $E$는 단위행렬이다.)

## 보기

## 풀이
$$ (A-E) B=E $$ 에서
$$ B=(A-E)^{-1} $$
이때,
$$ A-E = \left( \begin{array}{cc} 2-1 & -2 \\ -5 & 12-1 \end{array} \right) = \left( \begin{array}{cc} 1 & -2 \\ -5 & 11 \end{array} \right) $$
이므로
$$ B = \left( \begin{array}{cc} 1 & -2 \\ -5 & 11 \end{array} \right)^{-1} = \frac{1}{1 \times 11 - (-2) \times (-5)} \left( \begin{array}{cc} 11 & 2 \\ 5 & 1 \end{array} \right) = \left( \begin{array}{cc} 11 & 2 \\ 5 & 1 \end{array} \right) $$
이다. 따라서
$$ a=11, d=1 $$
이므로
$$ a+d=12 $$
[정답] $12$