## 문제
다음 중 항상 옳은 것을 모두 고르면?
ㄱ. $\sum_{k=1}^{n}(2 k-1)=n^{2}$
ㄴ. $\sum_{k=1}^{n} \frac{1}{k}=\frac{2}{n(n+1)}$
ㄷ. $\sum_{k=1}^{n} \left( \sum_{l=1}^{k} l \right)=\frac{n(n+1)(n+2)}{6}$

## 보기
① $ㄱ$   ② $ㄴ$   ③ $ㄱ, ㄷ$   ④ $ㄴ, ㄷ$   ⑤ $ㄱ, ㄴ, ㄷ$

## 풀이
ㄱ. $\sum_{k=1}^{n}(2 k-1)=2 \cdot \frac{n(n+1)}{2} - n = n^{2}+n-n=n^{2}$ (참) 
ㄴ. $\sum_{k=1}^{n} \frac{1}{k}$은 조화급수의 부분합으로 $\frac{2}{n(n+1)}$와 같지 않다. (거짓) 
ㄷ. $\sum_{k=1}^{n} \left( \sum_{l=1}^{k} l \right)= \sum_{k=1}^{n} \frac{k(k+1)}{2}=\frac{n(n+1)(n+2)}{6}$ (참) 

따라서 옳은 것은 $ㄱ, ㄷ$이다.

정답: ③