## 문제
두 행렬 $A = \left( \begin{array}{rr} 2 & -1 \\ 1 & 3 \end{array} \right)$, $B = \left( \begin{array}{rr} 1 & -1 \\ 0 & 2 \end{array} \right)$에 대하여 $2 A + X = 2 ( X + B ) - A$를 만족시키는 행렬 $X$의 모든 성분의 합을 구하시오.

## 보기

## 풀이
주어진 식을 정리하면
$2 A + X = 2 X + 2 B - A$
$X = 3 A - 2 B$
$$ X = 3 \left( \begin{array}{rr} 2 & -1 \\ 1 & 3 \end{array} \right) - 2 \left( \begin{array}{rr} 1 & -1 \\ 0 & 2 \end{array} \right) = \left( \begin{array}{rr} 4 & -1 \\ 3 & 5 \end{array} \right) $$
이므로 행렬 $X$의 모든 성분의 합은
$4 + ( -1 ) + 3 + 5 = 11$
이다.

정답: $11$