## 문제
두 행렬 $A = \left( \begin{array}{cc} 0 & a \\ 3 & 3 \end{array} \right)$, $B = \left( \begin{array}{cc} 3 & -5 \\ -1 & 2 \end{array} \right)$ 가 $A B^{-1} = B^{-1} A$ 를 만족시킬 때, $a$ 의 값을 구하시오.

## 보기

## 풀이
$A B^{-1} = B^{-1} A$ 에서 
$B A B^{-1} = A$, 
$B A = A B$ 이다.
$$ \left( \begin{array}{cc} 0 & a \\ 3 & 3 \end{array} \right) \left( \begin{array}{cc} 3 & -5 \\ -1 & 2 \end{array} \right) = \left( \begin{array}{cc} 3 & -5 \\ -1 & 2 \end{array} \right) \left( \begin{array}{cc} 0 & a \\ 3 & 3 \end{array} \right) $$
$$ \left( \begin{array}{cc} -a & 2a \\ 6 & -9 \end{array} \right) = \left( \begin{array}{cc} -15 & 3a - 15 \\ 6 & -a + 6 \end{array} \right) $$
따라서 $-a = -15$ 이므로 $a = 15$ 이다.

[정답] $15$