## 문제
두 행렬 $A$, $B$ 가 $A=B^{-1} \left( \begin{array}{cc} 2 & 1 \\ 5 & 3 \end{array} \right)$, $B= \left( \begin{array}{cc} -1 & 2 \\ -3 & 2 \end{array} \right)$ 일 때, 행렬 $B A B$ 의 모든 성분의 합은? (단, $X^{-1}$ 는 $X$ 의 역행렬)

## 보기
① $2$   ② $3$   ③ $4$   ④ $5$   ⑤ $6$

## 풀이
$A=B^{-1} \left( \begin{array}{cc} 2 & 1 \\ 5 & 3 \end{array} \right)$ 의 양변의 왼쪽에 $B$ 를 곱하면
$B A= \left( \begin{array}{cc} 2 & 1 \\ 5 & 3 \end{array} \right)$ 이다.
따라서 
$$ B A B = \left( \begin{array}{cc} 2 & 1 \\ 5 & 3 \end{array} \right) \left( \begin{array}{cc} -1 & 2 \\ -3 & 2 \end{array} \right) = \left( \begin{array}{cc} -5 & 6 \\ -14 & 16 \end{array} \right) $$
이 행렬의 모든 성분의 합은
$(-5) + 6 + (-14) + 16 = 3$
이다.

정답: ②