## 문제
기울기가 $-1$인 직선 $l$이 곡선 $y = \log_{2} x$와 만나는 점을 $A(a, b)$, 직선 $l$이 곡선 $y = \log_{4}(x + 2)$와 만나는 점을 $B(c, d)$라고 하자. $\overline{AB} = \sqrt{2}$일 때, $a + c$의 값은? (단, $1 < a < c$)

## 보기
① $9$   ② $10$   ③ $11$   ④ $12$   ⑤ $13$

## 풀이
직선 $l$을 $y = -x + m$이라 두면 
$A(a, -a + m)$, $B(c, -c + m)$
그러므로 조건에 의해 
$\overline{AB} = \sqrt{(a - c)^{2} + (-a + m - (-c + m))^{2}} = \sqrt{(a - c)^{2} + (c - a)^{2}} = \sqrt{2(a - c)^{2}}$
$\sqrt{2(a - c)^{2}} = \sqrt{2} \therefore a - c = -1$ ($\because 1 < a < c$)

또, 점 $A(a, b)$는 곡선 $y = \log_{2} x$ 위의 점이고, 점 $B(c, d)$는 곡선 $y = \log_{4}(x + 2)$ 위의 점이므로 
$b = \log_{2} a$, $d = \log_{4}(c + 2)$이다. 

$\overline{AB}$의 기울기가 $-1$이므로 
$\frac{b - d}{a - c} = \frac{\log_{2} a - \log_{4}(c + 2)}{a - c} = -1$
$\log_{2} a - \frac{1}{2} \log_{2}(c + 2) = 1$ ($\because a - c = -1$)
$2 \log_{2} a - \log_{2}(c + 2) = 2$
$\log_{2} \frac{a^{2}}{c + 2} = 2$
$a^{2} = 4(c + 2)$

$c = a + 1$이므로 대입하면
$a^{2} = 4(a + 1 + 2) = 4a + 12$
$a^{2} - 4a - 12 = (a - 6)(a + 2) = 0$
$\therefore a = 6$ ($\because a > 1$)

따라서 $c = 6 + 1 = 7$이므로
$a + c = 6 + 7 = 13$이다.

정답: ⑤