## 문제
$\frac{a+a^{5}}{a^{-1}+a^{-5}}=3$ 일 때, $\frac{a^{2}+a^{4}+a^{6}}{a^{-2}+a^{-4}+a^{-6}}$ 의 값은? (단, $a>0$ 이다.)

## 보기
① $1$   ② $\sqrt[3]{3}$   ③ $\sqrt[3]{3^{2}}$   ④ $3$   ⑤ $\sqrt[3]{3^{4}}$

## 풀이
$\frac{a+a^{5}}{a^{-1}+a^{-5}}=3$ 의 좌변의 분자, 분모에 $a^{5}$ 을 곱하면 
$\frac{a^{6}+a^{10}}{a^{4}+1}=\frac{a^{6} (1+a^{4} )}{a^{4}+1}=a^{6}=3$ 이다. 

$\therefore \frac{a^{2}+a^{4}+a^{6}}{a^{-2}+a^{-4}+a^{-6}}$ 의 분자, 분모에 $a^{6}$ 을 곱하면
$\frac{a^{8}+a^{10}+a^{12}}{a^{4}+a^{2}+1} = \frac{a^{8} (1+a^{2}+a^{4} )}{a^{4}+a^{2}+1}=a^{8}$ 이다.

$a^{6}=3$ 이므로 $a^{8}= (a^{6} )^{\frac{4}{3}}= 3^{\frac{4}{3}} = \sqrt[3]{3^{4}}$ 이다.

정답: ⑤