## 문제
두 수열 $\{ a_{n} \}$, $\{ b_{n} \}$ 이 모든 자연수 $n$ 에 대하여 
$a_{1} = 1$, $a_{2} = 3$, $a_{n+1} = \frac{a_{n} + a_{n+2}}{2}$, 
$\sum_{k=1}^{n} a_{k} b_{k} = ( 4 n^{2} - 1 ) 2^{n} + 1$
을 만족시킬 때, $b_{6}$ 의 값을 구하시오.

## 보기

## 풀이
$a_{1} = 1$, $a_{2} = 3$ 이고 $a_{n+1} = \frac{a_{n} + a_{n+2}}{2}$ 이므로 수열 $\{ a_{n} \}$ 은 초항이 $1$ 이고 공차가 $a_{2} - a_{1} = 2$ 인 등차수열이다. 
$\therefore a_{n} = 2 n - 1$

$S_{n} = \sum_{k=1}^{n} a_{k} b_{k}$ 라 두면 
$a_{6} b_{6} = S_{6} - S_{5}$
$= ( 143 \cdot 2^{6} + 1 ) - ( 99 \cdot 2^{5} + 1 )$
$= 2^{5} \cdot ( 143 \cdot 2 - 99 )$
$= 2^{5} \cdot ( 286 - 99 ) = 2^{5} \cdot 187$

$a_{6} = 2 \cdot 6 - 1 = 11$ 이므로 
$b_{6} = \frac{2^{5} \cdot 187}{11} = \frac{32 \cdot 187}{11} = 32 \cdot 17 = 544$

정답: $544$