## 문제
다음을 만족시키는 수열 $\{ a_{n} \}$ 에 대하여 $a_{20}$ 의 값은?

$$ a_{1} = 0 , \quad n^{2} a_{n+1} = ( n + 1 )^{2} a_{n} + 2 n + 1 \quad ( n = 1 , 2 , 3 , \cdots ) $$

## 보기
① $399$   ② $400$   ③ $401$   ④ $402$   ⑤ $403$

## 풀이
$n^{2} a_{n+1} = ( n + 1 )^{2} a_{n} + 2 n + 1$ 의 양변을 $n^{2} ( n + 1 )^{2}$ 으로 나누면
$$ \frac{1}{( n + 1 )^{2}} a_{n+1} = \frac{1}{n^{2}} a_{n} + \frac{2 n + 1}{n^{2} ( n + 1 )^{2}} $$
이제, $b_{n} = \frac{a_{n}}{n^{2}}$ 이라 두면
$$ b_{n+1} = b_{n} + \frac{2 n + 1}{n^{2} ( n + 1 )^{2}} $$
그러므로
$$ \begin{aligned} b_{n} &= b_{1} + \sum_{k=1}^{n-1} \frac{2k+1}{k^{2} ( k + 1 )^{2}} \\ &= \sum_{k=1}^{n-1} \left\{ \frac{1}{k^{2}} - \frac{1}{( k + 1 )^{2}} \right\} \quad \left( \because b_{1} = \frac{a_{1}}{1^{2}} = 0 \right) \\ &= 1 - \frac{1}{n^{2}} = \frac{n^{2} - 1}{n^{2}} \end{aligned} $$
$\therefore a_{n} = n^{2} b_{n} = n^{2} - 1$
따라서 $a_{20} = 20^{2} - 1 = 399$

정답: ①