## 문제
연립방정식 $$ \left\{ \begin{array}{l} \log_{2} x + \log_{3} y = 2 \\ (\log_{3} x)(\log_{4} y) = -\frac{3}{2} \end{array} \right. $$ 의 해가 $x = a$, $y = b$ 일 때, $3ab$ 의 값은? (단, $a > 1$)

## 보기
① $6$   ② $8$   ③ $10$   ④ $12$   ⑤ $14$

## 풀이
$(\log_{3} x)(\log_{4} y) = \frac{\log_{2} x}{\log_{2} 3} \cdot \frac{\log_{3} y}{\log_{3} 4}$ 이고, $\log_{3} 4 = 2\log_{3} 2 = \frac{2}{\log_{2} 3}$ 이므로
$(\log_{3} x)(\log_{4} y) = \frac{\log_{2} x}{\log_{2} 3} \cdot \frac{\log_{3} y \cdot \log_{2} 3}{2} = \frac{\log_{2} x \log_{3} y}{2}$ 이다.

문제의 조건에서 $(\log_{3} x)(\log_{4} y) = -\frac{3}{2}$ 이므로
$\frac{\log_{2} x \log_{3} y}{2} = -\frac{3}{2}$
$\log_{2} x \log_{3} y = -3$

$\log_{2} x + \log_{3} y = 2$ 이므로 $\log_{2} x$ 와 $\log_{3} y$ 를 두 근으로 하는 $t$ 에 관한 이차방정식은
$t^{2} - 2t - 3 = 0$
$(t - 3)(t + 1) = 0$
이를 풀면 $t = -1$ 또는 $t = 3$

$a > 1$ 이므로 $\log_{2} a > 0$ 이다.
따라서 $\log_{2} x = 3, \log_{3} y = -1$ 이고
$x = a = 2^{3} = 8, y = b = 3^{-1} = \frac{1}{3}$ 이다.
$\therefore 3ab = 3 \cdot 8 \cdot \frac{1}{3} = 8$

정답: ②