## 문제
다음을 만족시키는 행렬 $A$ 에 대하여 $(A^{-1})^{3}$ 의 모든 성분의 합은?

$$ \left( \begin{array}{cc} 1 & 0 \\ 2 & 1 \end{array} \right) A = \left( \begin{array}{cc} 2 & 0 \\ 0 & 2 \end{array} \right) $$

## 보기
① $1$   ② $2$   ③ $3$   ④ $4$   ⑤ $5$

## 풀이
$B = \left( \begin{array}{cc} 1 & 0 \\ 2 & 1 \end{array} \right)$ 라 두면 
$$ \left( \begin{array}{cc} 1 & 0 \\ 2 & 1 \end{array} \right) A = \left( \begin{array}{cc} 2 & 0 \\ 0 & 2 \end{array} \right) $$ 
이므로 $B A = 2 E$ 이다.

$\therefore A^{-1} = \frac{1}{2} B$

$(A^{-1})^{3} = \left( \frac{1}{2} B \right)^{3} = \frac{1}{8} B^{3}$

$B^{3} = \left( \begin{array}{cc} 1 & 0 \\ 2 & 1 \end{array} \right) \left( \begin{array}{cc} 1 & 0 \\ 2 & 1 \end{array} \right) \left( \begin{array}{cc} 1 & 0 \\ 2 & 1 \end{array} \right) = \left( \begin{array}{cc} 1 & 0 \\ 4 & 1 \end{array} \right) \left( \begin{array}{cc} 1 & 0 \\ 2 & 1 \end{array} \right) = \left( \begin{array}{cc} 1 & 0 \\ 6 & 1 \end{array} \right)$

따라서 $(A^{-1})^{3}$ 의 모든 성분의 합은 
$\frac{1}{8} (1 + 0 + 6 + 1) = 1$ 이다.

정답: ①