## 문제
다음은 $\sum_{r=0}^{29} (-1)^{r} {}_{59}C_{2r}$의 값을 구하는 과정이다.

$(1+x)^{59} = {}_{59}C_{0} + {}_{59}C_{1}x + {}_{59}C_{2}x^{2} + \cdots + {}_{59}C_{59}x^{59}$을 이용하면
$(1+i)^{59} = \sum_{r=0}^{29} (-1)^{r} {}_{59}C_{2r} + (\text{가})i$이다.
한편, $(1+i)^{59} = \{(1+i)^{2}\}^{29} \times (1+i) = (\text{나}) + 2^{29}i$이므로 $\sum_{r=0}^{29} (-1)^{r} {}_{59}C_{2r}$의 값은 $(\text{나})$이다.
(가), (나)에 알맞은 것을 바르게 짝지은 것은? (단, $i = \sqrt{-1}$이다.)

## 보기
① (가) $\sum_{r=0}^{29} (-1)^{r} {}_{59}C_{2r+1}$, (나) $2^{29}$   ② (가) $\sum_{r=0}^{29} (-1)^{r} {}_{59}C_{2r+1}$, (나) $-2^{29}$   ③ (가) $\sum_{r=0}^{29} (-1)^{r+1} {}_{59}C_{2r+1}$, (나) $2^{29}$   ④ (가) $\sum_{r=0}^{29} (-1)^{r+1} {}_{59}C_{2r+1}$, (나) $-2^{29}$   ⑤ (가) $\sum_{r=0}^{28} (-1)^{r+1} {}_{59}C_{2r+3}$, (나) $2^{29}$

## 풀이
$(1+x)^{59} = {}_{59}C_{0} + {}_{59}C_{1}x + {}_{59}C_{2}x^{2} + \cdots + {}_{59}C_{59}x^{59}$ 이고, 양변에 $x$ 대신 $i$를 대입하면,
$(1+i)^{59} = ({}_{59}C_{0} - {}_{59}C_{2} + {}_{59}C_{4} - \cdots - {}_{59}C_{58}) + ({}_{59}C_{1} - {}_{59}C_{3} + {}_{59}C_{5} - \cdots - {}_{59}C_{59})i$
$= \sum_{r=0}^{29} (-1)^{r} {}_{59}C_{2r} + \sum_{r=0}^{29} (-1)^{r} {}_{59}C_{2r+1}i$
따라서 (가)는 $\sum_{r=0}^{29} (-1)^{r} {}_{59}C_{2r+1}$이다.

한편, $(1+i)^{59} = \{(1+i)^{2}\}^{29} \times (1+i) = (2i)^{29}(1+i) = 2^{29}i^{29}(1+i)$
$i^{29} = (i^{4})^{7} \times i = 1^{7} \times i = i$이므로
$2^{29}i(1+i) = 2^{29}i + 2^{29}i^{2} = -2^{29} + 2^{29}i$
따라서 (나)는 $-2^{29}$이다.

이를 정리하면 다음과 같다.
$$ \begin{array}{|c|c|c|} \hline \text{구분} & \text{(가)} & \text{(나)} \\ \hline \text{내용} & \sum_{r=0}^{29} (-1)^{r} {}_{59}C_{2r+1} & -2^{29} \\ \hline \end{array} $$
정답은 ②이다.