## 문제
두 수열 $\{ a_{n} \}$, $\{ b_{n} \}$이 모든 자연수 $n$에 대하여
$a_{1} = 1$, $a_{2} = 3$, $a_{n+1} = \frac{a_{n} + a_{n+2}}{2}$
$\sum_{k=1}^{n} a_{k} b_{k} = (4 n^{2} - 1) 2^{n} + 1$
을 만족시킬 때, $b_{6}$의 값을 구하시오.

## 보기

## 풀이
$a_{1} = 1$, $a_{2} = 3$이고 $a_{n+1} = \frac{a_{n} + a_{n+2}}{2}$이므로 수열 $\{ a_{n} \}$은 공차가 $a_{2} - a_{1} = 2$인 등차수열이다.
$\therefore a_{n} = 2 n - 1$
$S_{n} = \sum_{k=1}^{n} a_{k} b_{k}$라 두면
$a_{6} b_{6} = S_{6} - S_{5}$
$= (4 \cdot 6^{2} - 1) \cdot 2^{6} + 1 - \{ (4 \cdot 5^{2} - 1) \cdot 2^{5} + 1 \}$
$= 143 \cdot 2^{6} - 99 \cdot 2^{5}$
$= 2^{5} \cdot (286 - 99) = 2^{5} \cdot 187$
이때 $a_{6} = 2 \cdot 6 - 1 = 11$이므로
$11 \cdot b_{6} = 32 \cdot 187$
$b_{6} = \frac{32 \cdot 187}{11} = 32 \cdot 17 = 544$

정답: $544$