## 문제
$\lim _{x \to -3} \frac{\sqrt{x^{2} -x-3 } +ax}{x+3} = b$ 가 성립하도록 상수 $a$, $b$ 의 값을 정할 때, $a+b$ 의 값은?

## 보기
① $-\frac{5}{6}$   ② $-\frac{1}{2}$   ③ $0$   ④ $\frac{1}{2}$   ⑤ $\frac{5}{6}$

## 풀이
$x \to -3$ 일 때 (분모) $\to 0$ 이므로 (분자) $\to 0$ 이어야 한다.

$\lim_{x \to -3} (\sqrt{x^{2} - x - 3} + ax)$
$= \sqrt{(-3)^{2} - (-3) - 3} - 3a$
$= 3 - 3a = 0$

따라서 $a = 1$

$\lim_{x \to -3} \frac{\sqrt{x^{2} - x - 3} + x}{x+3}$
$= \lim_{x \to -3} \frac{(\sqrt{x^{2} - x - 3} + x)(\sqrt{x^{2} - x - 3} - x)}{(x+3)(\sqrt{x^{2} - x - 3} - x)}$
$= \lim_{x \to -3} \frac{-(x+3)}{(x+3)(\sqrt{x^{2} - x - 3} - x)}$
$= \lim_{x \to -3} \frac{-1}{\sqrt{x^{2} - x - 3} - x}$
$= -\frac{1}{\sqrt{(-3)^{2} - (-3) - 3} - (-3)} = -\frac{1}{6}$

즉, $b = -\frac{1}{6}$ 이므로
$a + b = \frac{5}{6}$

정답: ⑤