## 문제
두 행렬 $A = \left( \begin{array}{cc} 2 & 3 \\ 1 & -2 \end{array} \right)$, $B = \left( \begin{array}{cc} 3 & 2 \\ 1 & -2 \end{array} \right)$ 에 대하여 $A^{-1} X = B$ 를 만족시키는 행렬 $X$ 의 모든 성분의 합은?

## 보기
① $11$   ② $12$   ③ $13$   ④ $14$   ⑤ $15$

## 풀이
$A^{-1} X = B$ 의 양변의 왼쪽에 행렬 $A$ 를 곱하면 

$$ A A^{-1} X = AB $$ 

$$ \therefore X = AB = \left( \begin{array}{cc} 2 & 3 \\ 1 & -2 \end{array} \right) \left( \begin{array}{cc} 3 & 2 \\ 1 & -2 \end{array} \right) = \left( \begin{array}{cc} 9 & -2 \\ 1 & 6 \end{array} \right) $$ 

따라서 행렬 $X$ 의 모든 성분의 합은 $9 + (-2) + 1 + 6 = 14$ 이다. 

정답은 ④ 이다.