## 문제
자연수 $n$에 대하여 $x$에 대한 이차방정식 $(4n^{2}-1)x^{2}-4nx+1=0$의 두 근이 $\alpha_{n}$, $\beta_{n}$ ($\alpha_{n} > \beta_{n}$)일 때, 급수 $\sum_{n=1}^{\infty} (\alpha_{n} - \beta_{n})$의 값은?

## 보기
① $1$   ② $2$   ③ $3$   ④ $4$   ⑤ $5$

## 풀이
이차방정식 $(4n^{2}-1)x^{2}-4nx+1=0$에서 좌변을 인수분해하면
$\{(2n-1)x-1\}\{(2n+1)x-1\} = 0$
$\therefore x = \frac{1}{2n-1}$ 또는 $x = \frac{1}{2n+1}$

$\alpha_{n} > \beta_{n}$이므로
$\alpha_{n} = \frac{1}{2n-1}$, $\beta_{n} = \frac{1}{2n+1}$

$\therefore \sum_{n=1}^{\infty} (\alpha_{n} - \beta_{n}) = \lim_{n \to \infty} \sum_{k=1}^{n} (\alpha_{k} - \beta_{k})$
$= \lim_{n \to \infty} \sum_{k=1}^{n} \left( \frac{1}{2k-1} - \frac{1}{2k+1} \right)$
$= \lim_{n \to \infty} \left( 1 - \frac{1}{2n+1} \right)$
$= 1$

정답: ①