## 문제
정적분 $\int_{2}^{6} \frac{x^{2}(x^{2} + 2x + 4)}{x + 2} dx + \int_{6}^{2} \frac{4(y^{2} + 2y + 4)}{y + 2} dy$ 의 값을 구하시오.

## 보기

## 풀이
$\int_{a}^{b} f(x) dx = -\int_{b}^{a} f(x) dx$ 이고 $\int_{a}^{b} f(t) dt = \int_{a}^{b} f(x) dx$ 이므로
$\int_{6}^{2} \frac{4(y^{2} + 2y + 4)}{y + 2} dy = \int_{6}^{2} \frac{4(x^{2} + 2x + 4)}{x + 2} dx = -\int_{2}^{6} \frac{4(x^{2} + 2x + 4)}{x + 2} dx$ 이다.

따라서
$\int_{2}^{6} \frac{x^{2} (x^{2} + 2x + 4)}{x + 2} dx + \int_{6}^{2} \frac{4(y^{2} + 2y + 4)}{y + 2} dy$
$= \int_{2}^{6} \left( \frac{x^{2} (x^{2} + 2x + 4)}{x + 2} - \frac{4 (x^{2} + 2x + 4)}{x + 2} \right) dx$
$= \int_{2}^{6} \frac{(x^{2} + 2x + 4)(x^{2} - 4)}{x + 2} dx$
$= \int_{2}^{6} \frac{(x^{2} + 2x + 4)(x - 2)(x + 2)}{x + 2} dx$
$= \int_{2}^{6} (x^{2} + 2x + 4)(x - 2) dx$
$= \int_{2}^{6} (x^{3} - 8) dx$
$= \left[ \frac{1}{4} x^{4} - 8x \right]_{2}^{6}$
$= \frac{1}{4} (1296 - 16) - 8(6 - 2)$
$= 320 - 32$
$= 288$

[정답] $288$