## 문제
실수 $x$ 가 $\frac{\sqrt{x+1}}{\sqrt{x-1}} = -\sqrt{\frac{x+1}{x-1}}$ 을 만족할 때, $\sqrt{(x-1)^{2} + 4x} - \sqrt{(x+1)^{2} - 4x}$ 를 간단히 하면?

## 보기
① $2$   ② $2x$   ③ $-2x$   ④ $2x+2$   ⑤ $-2x+2$

## 풀이
$\frac{\sqrt{x+1}}{\sqrt{x-1}} = -\sqrt{\frac{x+1}{x-1}}$ 이므로
$x+1 \geq 0$ , $x-1 < 0$
$\therefore -1 \leq x < 1$

따라서 
$\sqrt{(x-1)^{2} + 4x} - \sqrt{(x+1)^{2} - 4x}$
$= \sqrt{(x+1)^{2}} - \sqrt{(x-1)^{2}}$
$= |x+1| - |x-1|$
$-1 \leq x < 1$ 일 때, $x+1 \geq 0$ 이고 $x-1 < 0$ 이므로
$= (x+1) - (-(x-1))$
$= x+1 + x-1$
$= 2x$

정답: ②