## 문제
부등식 $1 < m^{n-5} < n^{m-8}$을 만족시키는 자연수 $m$, $n$에 대하여
$A = m^{\frac{1}{m-8}} \times n^{\frac{1}{n-5}}$, $B = m^{-\frac{1}{m-8}} \times n^{\frac{1}{n-5}}$, $C = m^{\frac{1}{m-8}} \times n^{-\frac{1}{n-5}}$
이라고 할 때, $A$, $B$, $C$의 대소 관계로 옳은 것은?

## 보기
① $A > B > C$   ② $A > C > B$   ③ $B > A > C$   ④ $B > C > A$   ⑤ $C > A > B$

## 풀이
$m$, $n$이 자연수이므로 
$1 < m^{n-5}$에서 $n-5 > 0$ $\cdots$ ㉠
$1 < n^{m-8}$에서 $m-8 > 0$ $\cdots$ ㉡
또, $m^{n-5} < n^{m-8}$에서 $\frac{n^{m-8}}{m^{n-5}} > 1$ $\cdots$ ㉢

$\frac{A}{B} = \frac{m^{\frac{1}{m-8}} \cdot n^{\frac{1}{n-5}}}{m^{-\frac{1}{m-8}} \cdot n^{\frac{1}{n-5}}} = m^{\frac{2}{m-8}} > 1$ ($\because$ ㉡)
$\therefore A > B$

$\frac{A}{C} = \frac{m^{\frac{1}{m-8}} \cdot n^{\frac{1}{n-5}}}{m^{\frac{1}{m-8}} \cdot n^{-\frac{1}{n-5}}} = n^{\frac{2}{n-5}} > 1$ ($\because$ ㉠)
$\therefore A > C$

$\frac{B}{C} = \frac{m^{-\frac{1}{m-8}} \cdot n^{\frac{1}{n-5}}}{m^{\frac{1}{m-8}} \cdot n^{-\frac{1}{n-5}}}$
$= m^{-\frac{2}{m-8}} \cdot n^{\frac{2}{n-5}}$
$= (m^{-(n-5)} \cdot n^{m-8})^{\frac{2}{(m-8)(n-5)}}$
$= (\frac{n^{m-8}}{m^{n-5}})^{\frac{2}{(m-8)(n-5)}}$
$> 1$ ($\because$ ㉢)
$\therefore B > C$

따라서 $A > B > C$ 이다.

정답: ①