## 문제
두 무한수열 $\{ a_{n} \}$, $\{ b_{n} \}$에 대하여 
$$\lim_{n \to \infty} (2n-1)a_{n} = 3$$
$$\lim_{n \to \infty} (n^{2} + 3n + 2)b_{n} = 2$$
일 때, $\lim_{n \to \infty} (2n+1)^{3} a_{n}b_{n}$의 값을 구하시오.

## 풀이
$(2n-1)a_{n} = c_{n}$이라 하면 $a_{n} = \frac{c_{n}}{2n-1}$, 
$(n^{2} + 3n + 2)b_{n} = d_{n}$라 하면 $b_{n} = \frac{d_{n}}{n^{2} + 3n + 2}$, 
$\lim_{n \to \infty} c_{n} = 3$, $\lim_{n \to \infty} d_{n} = 2$이므로 
$$\lim_{n \to \infty} (2n+1)^{3} a_{n}b_{n}$$ 
$$= \lim_{n \to \infty} \frac{(2n+1)^{3}}{(2n-1)(n^{2} + 3n + 2)} \lim_{n \to \infty} c_{n} \lim_{n \to \infty} d_{n}$$ 
$$= 4 \times 3 \times 2 = 24$$

정답: $24$