## 문제
행렬 $A = \left( \begin{array}{cc} 3 & 1 \\ 2 & 1 \end{array} \right)$, $B = \left( \begin{array}{cc} 2 & 5 \\ 1 & 3 \end{array} \right)$ 에 대하여 $(A - B^{-1}) A^{-1}$ 의 모든 성분의 합은? (단, $A^{-1}$ 는 $A$ 의 역행렬이다.)

## 보기
① $4$   ② $5$   ③ $6$   ④ $7$   ⑤ $8$

## 풀이
$(A - B^{-1}) A^{-1} = A A^{-1} - B^{-1} A^{-1} = E - (AB)^{-1}$

$AB = \left( \begin{array}{cc} 3 & 1 \\ 2 & 1 \end{array} \right) \left( \begin{array}{cc} 2 & 5 \\ 1 & 3 \end{array} \right) = \left( \begin{array}{cc} 7 & 18 \\ 5 & 13 \end{array} \right)$ 이므로,
$(AB)^{-1} = \frac{1}{7 \times 13 - 18 \times 5} \left( \begin{array}{cc} 13 & -18 \\ -5 & 7 \end{array} \right) = \frac{1}{91 - 90} \left( \begin{array}{cc} 13 & -18 \\ -5 & 7 \end{array} \right) = \left( \begin{array}{cc} 13 & -18 \\ -5 & 7 \end{array} \right)$ 이다.

따라서 
$(A - B^{-1}) A^{-1} = E - (AB)^{-1}$
$= \left( \begin{array}{cc} 1 & 0 \\ 0 & 1 \end{array} \right) - \left( \begin{array}{cc} 13 & -18 \\ -5 & 7 \end{array} \right) = \left( \begin{array}{cc} -12 & 18 \\ 5 & -6 \end{array} \right)$

모든 성분의 합은
$(-12) + 18 + 5 + (-6) = 5$

정답: ②