## 문제
$x = \frac{1}{1 - \frac{1}{1 + \frac{1}{3\sqrt{7}-1}}}$ 일 때, $x^{2}$ 의 값을 구하시오.

## 보기


## 풀이
$x = \frac{1}{1 - \frac{1}{1 + \frac{1}{3\sqrt{7}-1}}} = \frac{1}{1 - \frac{1}{\frac{(3\sqrt{7}-1)+1}{3\sqrt{7}-1}}}$
$= \frac{1}{1 - \frac{3\sqrt{7}-1}{3\sqrt{7}}} = \frac{1}{\frac{3\sqrt{7}-(3\sqrt{7}-1)}{3\sqrt{7}}} = 3\sqrt{7}$
$\therefore x^{2} = (3\sqrt{7})^{2} = 63$

[다른 풀이]
$3\sqrt{7}-1 = t$ 로 치환하면
$x = \frac{1}{1 - \frac{1}{1 + \frac{1}{t}}} = \frac{1}{1 - \frac{1}{\frac{t+1}{t}}}$
$= \frac{1}{1 - \frac{t}{t+1}} = \frac{1}{\frac{t+1-t}{t+1}} = t+1$
$\therefore x = t+1 = 3\sqrt{7}$
따라서 $x^{2} = (3\sqrt{7})^{2} = 63$ 이다.

정답: $63$