## 문제
양의 실수 전체의 집합에서 연속인 함수 $f(x)$가 모든 자연수 $n$에 대하여 
$$\int_{n}^{n+1} f(x)dx = \frac{1}{n^{2} + 2n}$$ 
를 만족시킬 때, $\lim_{n \to \infty} n \left( \int_{1}^{n} f(x)dx - \frac{3}{4} \right)$의 값은?

## 보기
① $-1$   ② $-\frac{1}{2}$   ③ $0$   ④ $\frac{1}{2}$   ⑤ $1$

## 풀이
$\int_{n}^{n+1} f(x)dx = \frac{1}{n^{2} + 2n}$ 이므로 
$$\int_{1}^{n} f(x)dx = \int_{1}^{2} f(x)dx + \int_{2}^{3} f(x)dx + \cdots + \int_{n-1}^{n} f(x)dx$$ 
$$= \frac{1}{1 \cdot 3} + \frac{1}{2 \cdot 4} + \cdots + \frac{1}{(n-1) \cdot (n+1)}$$ 
$$= \frac{1}{2} \left\{ \left( 1 - \frac{1}{3} \right) + \left( \frac{1}{2} - \frac{1}{4} \right) + \cdots + \left( \frac{1}{n-1} - \frac{1}{n+1} \right) \right\}$$ 
$$= \frac{1}{2} \left( 1 + \frac{1}{2} - \frac{1}{n} - \frac{1}{n+1} \right)$$ 
따라서 
$$\lim_{n \to \infty} n \left( \int_{1}^{n} f(x)dx - \frac{3}{4} \right) = \lim_{n \to \infty} n \left\{ \frac{1}{2} \left( \frac{3}{2} - \frac{1}{n} - \frac{1}{n+1} \right) - \frac{3}{4} \right\}$$ 
$$= \lim_{n \to \infty} -\frac{n}{2} \left( \frac{1}{n} + \frac{1}{n+1} \right) = -1$$ 

정답: ①