## 문제
수열 $\{ a_{n} \}$에 대하여
$$ a_{n} = \frac{1}{\sqrt{n+1} + \sqrt{n}} \quad (n = 1, 2, 3, \dots) $$
일 때, <보기>에서 옳은 것만을 있는 대로 고른 것은?

## 보기
$$ \begin{array}{|l|} \hline \text{ㄱ. } \lim_{n \to \infty} a_{n} = 0 \\ \text{ㄴ. } \sum_{n=1}^{99} a_{n} = 9 \\ \text{ㄷ. } \sum_{n=1}^{\infty} a_{n} \text{은 수렴한다.} \\ \hline \end{array} $$

① $ㄱ$   ② $ㄱ, ㄴ$   ③ $ㄱ, ㄷ$   ④ $ㄴ, ㄷ$   ⑤ $ㄱ, ㄴ, ㄷ$

## 풀이
ㄱ. 
$$ \lim_{n \to \infty} a_{n} = \lim_{n \to \infty} \frac{1}{\sqrt{n+1} + \sqrt{n}} = 0 $$
따라서 참이다.

ㄴ. 
$$ \sum_{n=1}^{99} a_{n} = \sum_{n=1}^{99} (\sqrt{n+1} - \sqrt{n}) $$
$$ = (\sqrt{2} - 1) + (\sqrt{3} - \sqrt{2}) + \dots + (\sqrt{100} - \sqrt{99}) $$
$$ = \sqrt{100} - 1 = 10 - 1 = 9 $$
따라서 참이다.

ㄷ. 
$$ \sum_{n=1}^{\infty} a_{n} = \lim_{n \to \infty} \sum_{k=1}^{n} \frac{1}{\sqrt{k+1} + \sqrt{k}} $$
$$ = \lim_{n \to \infty} \sum_{k=1}^{n} (\sqrt{k+1} - \sqrt{k}) $$
$$ = \lim_{n \to \infty} (\sqrt{n+1} - 1) = \infty $$
따라서 합은 발산하므로 거짓이다.

옳은 것은 $ㄱ$, $ㄴ$이다.

정답: ②