## 문제
행렬 $A= \left( \begin{array}{cc} 1 & 0 \\ 2 & 1 \end{array} \right)$, $B= \left( \begin{array}{cc} 3 & 2 \\ 1 & 1 \end{array} \right)$에 대하여 $AB+AX=E$를 만족하는 행렬 $X$의 모든 성분의 합은?

## 보기
① $-7$   ② $-3$   ③ $0$   ④ $3$   ⑤ $7$

## 풀이
$AB+AX=A(B+X)=E$
$B+X=A^{-1}$
따라서 $X=A^{-1}-B$이다.

$A= \left( \begin{array}{cc} 1 & 0 \\ 2 & 1 \end{array} \right)$이므로 역행렬 $A^{-1}$을 구하면
$A^{-1}= \frac{1}{1 \cdot 1 - 0 \cdot 2} \left( \begin{array}{cc} 1 & 0 \\ -2 & 1 \end{array} \right) = \left( \begin{array}{cc} 1 & 0 \\ -2 & 1 \end{array} \right)$

$X = \left( \begin{array}{cc} 1 & 0 \\ -2 & 1 \end{array} \right) - \left( \begin{array}{cc} 3 & 2 \\ 1 & 1 \end{array} \right) = \left( \begin{array}{cc} 1-3 & 0-2 \\ -2-1 & 1-1 \end{array} \right) = \left( \begin{array}{cc} -2 & -2 \\ -3 & 0 \end{array} \right)$

그러므로 행렬 $X$의 모든 성분의 합은
$(-2) + (-2) + (-3) + 0 = -7$

정답: ①