## 문제
$\sum_{k=1}^{10} \frac{k^{3}}{k^{2}-k+1} + \sum_{k=2}^{10} \frac{1}{k^{2}-k+1}$ 의 값은?

## 보기
① $62$   ② $64$   ③ $66$   ④ $68$   ⑤ $70$

## 풀이
$$ \sum_{k=1}^{10} \frac{k^{3}}{k^{2}-k+1} + \sum_{k=2}^{10} \frac{1}{k^{2}-k+1} $$
두 번째 항의 시그마 범위를 $k=1$부터 시작하도록 조정하면 $k=1$일 때의 값인 $1$을 빼주어야 하므로 다음과 같이 정리할 수 있다.
$$ = \sum_{k=1}^{10} \frac{k^{3}}{k^{2}-k+1} + \left( \sum_{k=1}^{10} \frac{1}{k^{2}-k+1} - 1 \right) $$
$$ = \sum_{k=1}^{10} \frac{k^{3}+1}{k^{2}-k+1} - 1 $$
분자를 인수분해하면 $k^{3}+1 = (k+1)(k^{2}-k+1)$ 이므로
$$ = \sum_{k=1}^{10} \frac{(k+1)(k^{2}-k+1)}{k^{2}-k+1} - 1 $$
$$ = \sum_{k=1}^{10} (k+1) - 1 $$
$$ = (2+3+4+5+6+7+8+9+10+11) - 1 $$
$$ = 65 - 1 = 64 $$
정답은 ② 이다.