## 문제
서로 다른 네 양수 $a$, $b$, $c$, $d$에 대하여 $a d-b c=0$일 때, 보기에서 옳은 것만을 있는 대로 고른 것은? (단, $n$은 자연수)

$$
\begin{array}{|l|}
\hline
\text{ㄱ. } \frac{a}{c}=\frac{b}{d} \\
\text{ㄴ. } \frac{a^{2}+b^{2}}{c^{2}+d^{2}}=\frac{(a+b)^{2}}{(c+d)^{2}} \\
\text{ㄷ. } \frac{a^{n}+b^{n}}{c^{n}+d^{n}}=\frac{(a+b)^{n}}{(c+d)^{n}} \\
\hline
\end{array}
$$

## 보기
① ㄱ   ② ㄴ   ③ ㄱ, ㄴ   ④ ㄴ, ㄷ   ⑤ ㄱ, ㄴ, ㄷ

## 풀이
[정답] ⑤ 

ㄱ. $a d-b c=0 \leftrightarrow a d=b c \leftrightarrow \frac{a}{c}=\frac{b}{d}$ (참)

ㄴ. $\frac{a}{c}=\frac{b}{d}$ 에서 $a=c k, b=d k$ ($k$는 비례상수)
$\frac{a^{2}+b^{2}}{c^{2}+d^{2}}=\frac{(c k)^{2}+(d k)^{2}}{c^{2}+d^{2}}=\frac{k^{2} (c^{2}+d^{2} )}{c^{2}+d^{2}}=k^{2}$
$\frac{(a+b)^{2}}{(c+d)^{2}}=\frac{(c k+d k)^{2}}{(c+d)^{2}}=\frac{k^{2}(c+d)^{2}}{(c+d)^{2}}=k^{2}$ (참)

ㄷ. $\frac{a^{n}+b^{n}}{c^{n}+d^{n}}=\frac{(c k)^{n}+(d k)^{n}}{c^{n}+d^{n}}=\frac{k^{n} (c^{n}+d^{n} )}{c^{n}+d^{n}}=k^{n}$
$\frac{(a+b)^{n}}{(c+d)^{n}}=\frac{(c k+d k)^{n}}{(c+d)^{n}}=\frac{k^{n}(c+d)^{n}}{(c+d)^{n}}=k^{n}$ (참)