## 문제
이차정사각행렬 $A$와 행렬 $B = \left( \begin{array}{cc} 1 & 0 \\ 1 & 1 \end{array} \right)$에 대하여 $(B A)^{2} = \left( \begin{array}{cc} 1 & 1 \\ 1 & 2 \end{array} \right)$일 때, 행렬 $(A B)^{2}$은?

## 보기
① $\left( \begin{array}{cc} 1 & 1 \\ 1 & 2 \end{array} \right)$   ② $\left( \begin{array}{cc} 2 & 1 \\ 1 & 2 \end{array} \right)$   ③ $\left( \begin{array}{cc} 2 & 1 \\ 1 & 1 \end{array} \right)$   ④ $\left( \begin{array}{cc} 1 & 2 \\ 2 & 1 \end{array} \right)$   ⑤ $\left( \begin{array}{cc} 1 & 1 \\ 2 & 1 \end{array} \right)$

## 풀이
$(B A)^{2} = B A B A = \left( \begin{array}{cc} 1 & 1 \\ 1 & 2 \end{array} \right)$이다. 

$(A B)^{2} = A B A B$ 이므로 다음과 같이 변형할 수 있다.
$$ (A B)^{2} = B^{-1} (B A B A) B = B^{-1} (B A)^{2} B $$

$B = \left( \begin{array}{cc} 1 & 0 \\ 1 & 1 \end{array} \right)$ 의 역행렬 $B^{-1}$을 구하면 다음과 같다.
$$ B^{-1} = \frac{1}{1 \cdot 1 - 0 \cdot 1} \left( \begin{array}{cc} 1 & 0 \\ -1 & 1 \end{array} \right) = \left( \begin{array}{cc} 1 & 0 \\ -1 & 1 \end{array} \right) $$

따라서 구하고자 하는 행렬 $(A B)^{2}$은 다음과 같다.
$$ (A B)^{2} = \left( \begin{array}{cc} 1 & 0 \\ -1 & 1 \end{array} \right) \left( \begin{array}{cc} 1 & 1 \\ 1 & 2 \end{array} \right) \left( \begin{array}{cc} 1 & 0 \\ 1 & 1 \end{array} \right) $$
$$ (A B)^{2} = \left( \begin{array}{cc} 1 & 1 \\ 0 & 1 \end{array} \right) \left( \begin{array}{cc} 1 & 0 \\ 1 & 1 \end{array} \right) = \left( \begin{array}{cc} 2 & 1 \\ 1 & 1 \end{array} \right) $$

정답은 ③이다.