## 문제
두 행렬 $A = \left( \begin{array}{cc} 2 & -1 \\ 0 & 1 \end{array} \right)$, $B = \left( \begin{array}{cc} 4 & 0 \\ 2 & 3 \end{array} \right)$ 에 대하여 $X - B = 3(X - 2A) + B$ 를 만족하는 행렬 $X$ 는?

## 보기
① $\left( \begin{array}{cc} 2 & -3 \\ -2 & 0 \end{array} \right)$  ② $\left( \begin{array}{cc} -2 & -3 \\ 2 & 0 \end{array} \right)$  ③ $\left( \begin{array}{cc} -2 & 3 \\ 2 & 0 \end{array} \right)$  ④ $\left( \begin{array}{cc} 10 & -3 \\ -2 & 4 \end{array} \right)$  ⑤ $\left( \begin{array}{cc} 10 & -1 \\ 2 & 4 \end{array} \right)$

## 풀이
주어진 식 $X - B = 3(X - 2A) + B$ 를 $X$ 에 관하여 정리하면 다음과 같다.
$$ \begin{array}{l} X - B = 3X - 6A + B \\ 2X = 6A - 2B \\ X = 3A - B \end{array} $$

행렬 $A$ 와 $B$ 를 대입하면
$$ \begin{array}{l} X = 3 \left( \begin{array}{cc} 2 & -1 \\ 0 & 1 \end{array} \right) - \left( \begin{array}{cc} 4 & 0 \\ 2 & 3 \end{array} \right) \\ X = \left( \begin{array}{cc} 6 & -3 \\ 0 & 3 \end{array} \right) - \left( \begin{array}{cc} 4 & 0 \\ 2 & 3 \end{array} \right) \\ X = \left( \begin{array}{cc} 2 & -3 \\ -2 & 0 \end{array} \right) \end{array} $$

따라서 정답은 ①이다.