## ë¬¸ì œ
ì •ìœ¡ê°í˜• $ABCDEF$ì—ì„œ $\overline{EF}$ì˜ ì¤‘ì ì„ $M$, $\overline{EM}$ì˜ ì¤‘ì ì„ $N$, $\angle MCN = \theta$ë¼ í•  ë•Œ, $\tan \theta$ì˜ ê°’ì€?

> [!example] ğŸ“¸ (ê·¸ë¦¼/ê·¸ë˜í”„)

## ë³´ê¸°
â‘  $\frac{2 \sqrt{3}}{25}$   â‘¡ $\frac{2 \sqrt{3}}{23}$   â‘¢ $\frac{4 \sqrt{3}}{23}$   â‘£ $\frac{6 \sqrt{3}}{25}$   â‘¤ $\frac{6 \sqrt{3}}{23}$

## í’€ì´
ì •ìœ¡ê°í˜•ì˜ í•œ ë³€ì˜ ê¸¸ì´ë¥¼ $4a$ë¼ í•˜ë©´ 
$\overline{CE} = 4 \sqrt{3} a$, $\overline{EM} = 2a$, $\overline{EN} = a$ì´ë‹¤.

$\angle MCE = \alpha$, $\angle NCE = \beta$ë¼ í•˜ë©´ 
$\tan \alpha = \frac{2a}{4 \sqrt{3} a} = \frac{1}{2 \sqrt{3}}$, $\tan \beta = \frac{a}{4 \sqrt{3} a} = \frac{1}{4 \sqrt{3}}$ì´ë‹¤.

$\tan \theta = \tan(\alpha - \beta)$
$= \frac{\tan \alpha - \tan \beta}{1 + \tan \alpha \tan \beta}$
$= \frac{\frac{1}{2 \sqrt{3}} - \frac{1}{4 \sqrt{3}}}{1 + \frac{1}{2 \sqrt{3}} \cdot \frac{1}{4 \sqrt{3}}}$
$= \frac{\frac{1}{4 \sqrt{3}}}{\frac{25}{24}} = \frac{1}{4 \sqrt{3}} \cdot \frac{24}{25} = \frac{6}{25 \sqrt{3}}$
$= \frac{2 \sqrt{3}}{25}$

ì •ë‹µ: â‘ 