## 문제
다항함수 $f(x)$ 가
$\lim _{x \to 0+} \frac{x^{3} f\left(\frac{1}{x}\right)-1}{x^{3}+x}=5, \lim _{x \to 1} \frac{f(x)}{x^{2}+x-2}=\frac{1}{3}$
을 만족시킬 때, $f(2)$ 의 값을 구하시오.

## 풀이
$\lim _{x \to 0+} \frac{x^{3} f\left(\frac{1}{x}\right)-1}{x^{3}+x}$ 에서 $\frac{1}{x}=t$ 라 하면 $x \to 0+$ 일 때 $t \to \infty$ 이므로
$\lim _{x \to 0+} \frac{x^{3} f\left(\frac{1}{x}\right)-1}{x^{3}+x} = \lim _{t \to \infty} \frac{\frac{1}{t^{3}} f(t)-1}{\frac{1}{t^{3}}+\frac{1}{t}} = \lim _{t \to \infty} \frac{f(t)-t^{3}}{t^{2}+1}=5$
따라서 $f(t)=t^{3}+5 t^{2}+a t+b$ 라 하면 
$\lim _{x \to 1} \frac{f(x)}{x^{2}+x-2}=\frac{1}{3}$ 에서 $x \to 1$ 일 때 (분모) $\to 0$ 이므로 (분자) $\to 0$ 이어야 한다. 즉,
$\lim _{x \to 1} f(x)=1+5+a+b=0$
$\therefore a+b=-6 \cdots$ ㉠
$\lim _{x \to 1} \frac{f(x)}{x^{2}+x-2} = \lim _{x \to 1} \frac{x^{3}+5 x^{2}+a x+b}{(x+2)(x-1)}$
$= \lim _{x \to 1} \frac{(x-1)\left(x^{2}+6 x+a+6\right)}{(x+2)(x-1)} = \lim _{x \to 1} \frac{x^{2}+6 x+a+6}{x+2}$
$= \frac{a+13}{3}=\frac{1}{3}$
$\therefore a=-12$
따라서 ㉠에서 $b=6$ 이므로
$f(x)=x^{3}+5 x^{2}-12 x+6$
$\therefore f(2)=10$