## 문제
수열 $\{ a_n \}$ 에 대하여 <보기>에서 옳은 것만을 있는 대로 고른 것은?

$$ \begin{array}{|l|} \hline \text{ㄱ. } \lim_{n \to \infty} a_n = \frac{1}{2} \text{ 이면 } \sum_{n=1}^{\infty} a_n \text{ 은 발산한다.} \\ \text{ㄴ. } a_n = \sum_{k=1}^n \frac{1}{\sqrt{k+1} + \sqrt{k}} \text{ 이면 수열 } \{ a_n \} \text{ 은 수렴한다.} \\ \text{ㄷ. } | 1 + (a_1 + a_2 + \cdots + a_n) | < \frac{1}{n} \text{ 이면 } \sum_{n=1}^{\infty} a_n \text{ 은 수렴한다.} \\ \hline \end{array} $$

## 보기
① ㄱ   ② ㄴ   ③ ㄱ, ㄴ   ④ ㄱ, ㄷ   ⑤ ㄱ, ㄴ, ㄷ

## 풀이
[정답] ④

ㄱ. $\lim_{n \to \infty} a_n = \frac{1}{2} \neq 0$ 이므로 $\sum_{n=1}^{\infty} a_n$ 은 발산한다. (참)

ㄴ. $a_n = \sum_{k=1}^n \frac{1}{\sqrt{k+1} + \sqrt{k}}$
$= \sum_{k=1}^n \frac{\sqrt{k+1} - \sqrt{k}}{(\sqrt{k+1} + \sqrt{k})(\sqrt{k+1} - \sqrt{k})}$
$= \sum_{k=1}^n (\sqrt{k+1} - \sqrt{k})$
$= (\sqrt{2} - \sqrt{1}) + (\sqrt{3} - \sqrt{2}) + \cdots + (\sqrt{n+1} - \sqrt{n})$
$= \sqrt{n+1} - 1$
따라서 $\lim_{n \to \infty} a_n = \lim_{n \to \infty} (\sqrt{n+1} - 1) = \infty$ (거짓)

ㄷ. $a_1 + a_2 + \cdots + a_n = \sum_{k=1}^n a_k$ 이므로 주어진 식은
$|1 + \sum_{k=1}^n a_k| < \frac{1}{n}$
$- \frac{1}{n} < 1 + \sum_{k=1}^n a_k < \frac{1}{n}$
$-1 - \frac{1}{n} < \sum_{k=1}^n a_k < -1 + \frac{1}{n}$
각 변에 극한을 취하면
$\lim_{n \to \infty} (-1 - \frac{1}{n}) \le \lim_{n \to \infty} \sum_{k=1}^n a_k \le \lim_{n \to \infty} (-1 + \frac{1}{n})$
$-1 \le \lim_{n \to \infty} \sum_{k=1}^n a_k \le -1$
즉, $\lim_{n \to \infty} \sum_{k=1}^n a_k = -1$ 이므로 수렴한다. (참)