## 문제
$\lim _{x \to 2} \frac{\sqrt{6-x} - 2}{\sqrt{3-x} - 1}$ 의 값은?

## 보기
① $\frac{1}{3}$   ② $\frac{1}{2}$   ③ $\frac{2}{3}$   ④ $\frac{3}{2}$   ⑤ $2$

## 풀이
정답: ②

$\frac{0}{0}$ 꼴이므로 분모와 분자에 $(\sqrt{3-x}+1)(\sqrt{6-x}+2)$ 를 곱하면

$$ \lim _{x \to 2} \frac{\sqrt{6-x} - 2}{\sqrt{3-x} - 1} $$
$$ = \lim _{x \to 2} \frac{(\sqrt{6-x} - 2) \times (\sqrt{3-x} + 1)(\sqrt{6-x} + 2)}{(\sqrt{3-x} - 1) \times (\sqrt{3-x} + 1)(\sqrt{6-x} + 2)} $$
$$ = \lim_{x \to 2} \frac{(2-x)(\sqrt{3-x}+1)}{(2-x)(\sqrt{6-x}+2)} $$
$$ = \lim_{x \to 2} \frac{\sqrt{3-x}+1}{\sqrt{6-x}+2} = \frac{1}{2} $$