## ë¬¸ì œ
$n$ì´ $3$ ì´ìƒì˜ ìì—°ìˆ˜ì¼ ë•Œ, ë„¤ ì  $(n, 0)$, $\left( \frac{3n}{2}, 0 \right)$, $\left( \frac{3n}{2}, \frac{n}{2} \right)$, $(n, \frac{n}{2})$ì„ ê¼­ì§“ì ìœ¼ë¡œ í•˜ëŠ” ì •ì‚¬ê°í˜•ì„ $A_{n}$ì´ë¼ í•˜ì. ë‘ ì •ì‚¬ê°í˜• $A_{n}$, $A_{n+1}$ì´ ê²¹ì¹˜ëŠ” ë¶€ë¶„(ì–´ë‘ìš´ ë¶€ë¶„)ì˜ ë„“ì´ë¥¼ $a_{n}$ì´ë¼ í•  ë•Œ, $\sum_{n=3}^{10} \frac{1}{a_{n}}$ì˜ ê°’ì€?

> [!example] ğŸ“¸ (ê·¸ë¦¼/ê·¸ë˜í”„)

## ë³´ê¸°
â‘  $\frac{113}{45}$   â‘¡ $\frac{116}{45}$   â‘¢ $\frac{118}{45}$   â‘£ $\frac{121}{45}$   â‘¤ $\frac{124}{45}$

## í’€ì´
[ì •ë‹µ] â‘¡

ë‘ ì •ì‚¬ê°í˜• $A_{n}, A_{n+1}$ì´ ê²¹ì¹˜ëŠ” ë¶€ë¶„(ì–´ë‘ìš´ ë¶€ë¶„)ì˜ ë„“ì´ê°€ $a_{n}$ì´ë¯€ë¡œ
$a_{n} = \left\{ \frac{3n}{2} - (n+1) \right\} \times \frac{n}{2}$
$= \frac{n-2}{2} \times \frac{n}{2}$
$= \frac{(n-2)n}{4}$ ($n \ge 3$)

$\sum_{n=3}^{10} \frac{1}{a_{n}} = 4 \sum_{n=3}^{10} \frac{1}{(n-2)n}$
$= 2 \sum_{n=3}^{10} \left( \frac{1}{n-2} - \frac{1}{n} \right)$
$= 2 \left\{ \left( \frac{1}{1} - \frac{1}{3} \right) + \left( \frac{1}{2} - \frac{1}{4} \right) + \left( \frac{1}{3} - \frac{1}{5} \right) + \cdots + \left( \frac{1}{7} - \frac{1}{9} \right) + \left( \frac{1}{8} - \frac{1}{10} \right) \right\}$
$= 2 \left( 1 + \frac{1}{2} - \frac{1}{9} - \frac{1}{10} \right)$
$= \frac{116}{45}$