## ë¬¸ì œ

ì§‘í•© $A = \{ 1, 2, 3, 4 \}$ì— ëŒ€í•˜ì—¬ ì§‘í•© $A$ì—ì„œ $A$ë¡œì˜ ë‘ í•¨ìˆ˜ $y = f(x)$, $y = g(x)$ì˜ ê·¸ë˜í”„ê°€ ê°ê° ê·¸ë¦¼ê³¼ ê°™ì„ ë•Œ, $(g \circ f)(1) + (f \circ g)^{-1}(3)$ì˜ ê°’ì€?

> [!example] ğŸ“¸ (ê·¸ë¦¼/ê·¸ë˜í”„)

> [!example] ğŸ“¸ (ê·¸ë¦¼/ê·¸ë˜í”„)

## ë³´ê¸°

â‘  $4$   â‘¡ $5$   â‘¢ $6$   â‘£ $7$   â‘¤ $8$

## í’€ì´

ë‘ í•¨ìˆ˜ $y = f(x)$, $y = g(x)$ì˜ ê·¸ë˜í”„ë¡œë¶€í„° 
$f(1) = 1$, $g(1) = 2$, $g^{-1}(4) = 4$, $f^{-1}(3) = 4$ì´ë‹¤. 

ê·¸ëŸ¬ë¯€ë¡œ 
$(g \circ f)(1) = g(f(1)) = g(1) = 2$ì´ê³  

$(f \circ g)^{-1}(3) = (g^{-1} \circ f^{-1})(3) = g^{-1}(f^{-1}(3)) = g^{-1}(4) = 4$ì´ë‹¤. 

ë”°ë¼ì„œ 
$(g \circ f)(1) + (f \circ g)^{-1}(3) = 2 + 4 = 6$

ì •ë‹µ: â‘¢