## 문제
이차정사각행렬 $A$ 에 대하여 $A^{4}=E$ 이고 $A^{2}+A+E$ 의 역행렬이 $A^{2}-A+E$ 일 때, $(A^{-1})^{3}+A^{-1}$ 을 간단히 나타낸 것은? (단, $E$ 는 단위행렬이고 $O$ 는 영행렬이다.)

## 보기
① $O$   ② $E$   ③ $A$   ④ $-A$   ⑤ $A+E$

## 풀이
$A^{2}+A+E$ 의 역행렬이 $A^{2}-A+E$ 이므로 
$$(A^{2}+A+E)(A^{2}-A+E)=E$$ 
$$A^{4}-A^{3}+A^{2}+A^{3}-A^{2}+A+A^{2}-A+E=E$$ 
$$A^{4}+A^{2}+E=E$$ 
$$A^{2}=-E$$ 
($\because A^{4}=(-E)^{2}=E$) 

$A(-A)=E$ 이므로
$\therefore A^{-1}=-A$ $\cdots$ ㉠ 

또한 $A^{4}=A^{3}A=E$ 에서 $(A^{3})^{-1}=A$ 이므로 
$$(A^{-1})^{3}=(A^{3})^{-1}=A$$ 
$\cdots$ ㉡ 

㉠, ㉡에 의해 
$$(A^{-1})^{3}+A^{-1}=A+(-A)=O$$

정답: ①