## ë¬¸ì œ
ê·¸ë¦¼ê³¼ ê°™ì´ í•¨ìˆ˜ $y=\sin 2x$ ($0 \le x \le \pi$)ì˜ ê·¸ë˜í”„ê°€ ì§ì„  $y = \frac{3}{5}$ê³¼ ë‘ ì  $A$, $B$ì—ì„œ ë§Œë‚˜ê³ , ì§ì„  $y = -\frac{3}{5}$ê³¼ ë‘ ì  $C$, $D$ì—ì„œ ë§Œë‚œë‹¤. ë„¤ ì  $A$, $B$, $C$, $D$ì˜ $x$ì¢Œí‘œë¥¼ ê°ê° $\alpha$, $\beta$, $\gamma$, $\delta$ë¼ í•  ë•Œ, $\alpha + 2\beta + 2\gamma + \delta$ì˜ ê°’ì€?

> [!example] ğŸ“¸ (ê·¸ë¦¼/ê·¸ë˜í”„)

## ë³´ê¸°
â‘  $\frac{9}{4}\pi$   â‘¡ $\frac{5}{2}\pi$   â‘¢ $3\pi$   â‘£ $\frac{7}{2}\pi$   â‘¤ $4\pi$

## í’€ì´
ë‘ ì  $A$, $B$ëŠ” ì§ì„  $x = \frac{\pi}{4}$ì— ëŒ€í•˜ì—¬ ëŒ€ì¹­ì´ë¯€ë¡œ 
$\frac{\alpha+\beta}{2} = \frac{\pi}{4}$ 
$\therefore \alpha + \beta = \frac{\pi}{2}$ â€¦â€¦ ã‰ 

ë‘ ì  $C$, $D$ëŠ” ì§ì„  $x = \frac{3}{4}\pi$ì— ëŒ€í•˜ì—¬ ëŒ€ì¹­ì´ë¯€ë¡œ 
$\frac{\gamma+\delta}{2} = \frac{3}{4}\pi$
$\therefore \gamma + \delta = \frac{3}{2}\pi$ â€¦â€¦ ã‰¡ 

ë‘ ì  $B$, $C$ëŠ” ì  $(\frac{\pi}{2}, 0)$ì— ëŒ€í•˜ì—¬ ëŒ€ì¹­ì´ë¯€ë¡œ 
$\frac{\beta+\gamma}{2} = \frac{\pi}{2}$ 
$\therefore \beta + \gamma = \pi$ â€¦â€¦ ã‰¢

ã‰ , ã‰¡, ã‰¢ì—ì„œ 
$\alpha + 2\beta + 2\gamma + \delta = (\alpha + \beta) + (\beta + \gamma) + (\gamma + \delta)$ 
$= \frac{\pi}{2} + \pi + \frac{3}{2}\pi$ 
$= 3\pi$ 

**[ë‹¤ë¥¸ í’€ì´]** 
ë‘ ì  $A$, $D$ëŠ” ì  $(\frac{\pi}{2}, 0)$ì— ëŒ€í•˜ì—¬ ëŒ€ì¹­ì´ë¯€ë¡œ 
$\frac{\alpha+\delta}{2} = \frac{\pi}{2}$ 
$\therefore \alpha + \delta = \pi$ â€¦â€¦ ã‰£

ë‘ ì  $B$, $C$ëŠ” ì  $(\frac{\pi}{2}, 0)$ì— ëŒ€í•˜ì—¬ ëŒ€ì¹­ì´ë¯€ë¡œ 
$\frac{\beta+\gamma}{2} = \frac{\pi}{2}$ 
$\therefore \beta + \gamma = \pi$ â€¦â€¦ ã‰¤ 

ã‰£, ã‰¤ì—ì„œ 
$\alpha + 2\beta + 2\gamma + \delta = (\alpha + \delta) + 2(\beta + \gamma)$ 
$= \pi + 2\pi$ 
$= 3\pi$

ì •ë‹µ: â‘¢