## ë¬¸ì œ
í•¨ìˆ˜ $f(x)=\sqrt{[x]+1-(x-[x])^{2}}$ ($x \ge 0$)ê³¼ ì§ì„  $x=n-1$, $x=n$ ë° $x$ì¶•ìœ¼ë¡œ ë‘˜ëŸ¬ì‹¸ì¸ ë„í˜•ì„ $x$ì¶• ë‘˜ë ˆë¡œ íšŒì „ì‹œí‚¨ ë„í˜•ì˜ ë¶€í”¼ë¥¼ $V_{n}$ì´ë¼ í•  ë•Œ, $\lim_{n \to \infty} \frac{\sum_{k=1}^{n} V_{k}}{n^{2}}$ì˜ ê°’ì€? (ë‹¨, $[x]$ëŠ” $x$ë³´ë‹¤ í¬ì§€ ì•Šì€ ìµœëŒ€ì˜ ì •ìˆ˜)

## ë³´ê¸°
â‘  $\frac{\pi}{2}$   â‘¡ $\pi$   â‘¢ $\frac{3\pi}{2}$   â‘£ $2\pi$   â‘¤ $\frac{5\pi}{2}$

## í’€ì´
[ì •ë‹µ] â‘ 

ê·¸ë˜í”„ëŠ” $(x-[x])^{2}+y^{2}=[x]+1$ ì´ë¯€ë¡œ

$0 \le x < 1$ ì´ë©´ $x^{2}+y^{2}=1$
$1 \le x < 2$ ì´ë©´ $(x-1)^{2}+y^{2}=2$
$2 \le x < 3$ ì´ë©´ $(x-2)^{2}+y^{2}=3$
$\vdots$
$n-1 \le x < n$ ì´ë©´ $(x-n+1)^{2}+y^{2}=n$

> [!example] ğŸ“¸ (ê·¸ë¦¼/ê·¸ë˜í”„)

$V_{n} = \pi \int_{n-1}^{n} \{f(x)\}^{2} dx$
$= \pi \int_{n-1}^{n} (n-(x-n+1)^{2}) dx = (n-\frac{1}{3}) \pi$

$\sum_{k=1}^{n} V_{k} = \sum_{k=1}^{n} (k-\frac{1}{3}) \pi = (\frac{1}{2} n^{2}+\frac{1}{6} n) \pi$

$\therefore \lim_{n \to \infty} \frac{\sum_{k=1}^{n} V_{k}}{n^{2}} = \frac{\pi}{2}$