## 문제
수열 $\{ a_{n} \}$ 에 대하여 급수 $\sum_{n=1}^{\infty} \left( \frac{a_{n}}{4^{n}} - 3 \right)$ 이 수렴할 때, $\lim_{n \to \infty} \frac{a_{n} - 4 \cdot 2^{n}}{a_{n} - 2 \cdot 4^{n}}$ 의 값은?

## 보기
① $0$   ② $1$   ③ $2$   ④ $3$   ⑤ $4$

## 풀이
급수 $\sum_{n=1}^{\infty} \left( \frac{a_{n}}{4^{n}} - 3 \right)$ 이 수렴하므로
$\lim_{n \to \infty} \left( \frac{a_{n}}{4^{n}} - 3 \right) = 0$
($\because \sum_{n=1}^{\infty} b_{n}$ 이 수렴하면 $\lim_{n \to \infty} b_{n} = 0$ 이다.)
따라서 $\lim_{n \to \infty} \frac{a_{n}}{4^{n}} = 3$ $\cdots \cdots$ ㉠

$\lim_{n \to \infty} \frac{a_{n} - 4 \cdot 2^{n}}{a_{n} - 2 \cdot 4^{n}}$
$= \lim_{n \to \infty} \frac{\frac{a_{n} - 4 \cdot 2^{n}}{4^{n}}}{\frac{a_{n} - 2 \cdot 4^{n}}{4^{n}}}$
$= \lim_{n \to \infty} \frac{\frac{a_{n}}{4^{n}} - 4 \cdot \frac{2^{n}}{4^{n}}}{\frac{a_{n}}{4^{n}} - \frac{2 \cdot 4^{n}}{4^{n}}}$
$= \lim_{n \to \infty} \frac{\frac{a_{n}}{4^{n}} - 4 \cdot \frac{1}{2^{n}}}{\frac{a_{n}}{4^{n}} - 2}$
$= \frac{3 - 0}{3 - 2}$ ($\because$ ㉠, $\lim_{n \to \infty} \frac{1}{2^{n}} = 0$)
$= 3$

정답: ④