## 문제
함수 $f(x)$를 
$$f(x) = \lim_{n \to \infty} \frac{x^{2n-1} + x^{2n}}{x^{2n} + 2}$$
으로 정의할 때, $f(-2) + f\left(\frac{1}{2}\right)$의 값은?

## 보기
① $-2$   ② $-\frac{1}{2}$   ③ $0$   ④ $\frac{1}{2}$   ⑤ $2$

## 풀이
$1.$ $x = -2$일 때,
$$f(-2) = \lim_{n \to \infty} \frac{(-2)^{2n-1} + (-2)^{2n}}{(-2)^{2n} + 2}$$
분모, 분자를 $(-2)^{2n}$으로 나누면
$$f(-2) = \lim_{n \to \infty} \frac{\frac{1}{-2} + 1}{1 + \frac{2}{(-2)^{2n}}} = \frac{-\frac{1}{2} + 1}{1 + 0} = \frac{1}{2}$$

$2.$ $x = \frac{1}{2}$일 때,
$$f\left(\frac{1}{2}\right) = \lim_{n \to \infty} \frac{\left(\frac{1}{2}\right)^{2n-1} + \left(\frac{1}{2}\right)^{2n}}{\left(\frac{1}{2}\right)^{2n} + 2} = \frac{0 + 0}{0 + 2} = 0$$

따라서, 
$$f(-2) + f\left(\frac{1}{2}\right) = \frac{1}{2} + 0 = \frac{1}{2}$$
정답은 ④이다.