## 문제
두 행렬 $A$, $B$에 대하여
$$ A-2 B = \begin{pmatrix} -7 & -2 \\ 6 & 0 \end{pmatrix} $$, $$ B = \begin{pmatrix} 2 & -1 \\ -3 & 1 \end{pmatrix} $$
일 때, 행렬 $A$의 모든 성분의 합은?

## 보기
① $-1$   ② $-2$   ③ $-3$   ④ $-4$   ⑤ $-5$

## 풀이
$$ B = \begin{pmatrix} 2 & -1 \\ -3 & 1 \end{pmatrix} $$에서 
$$ 2B = \begin{pmatrix} 4 & -2 \\ -6 & 2 \end{pmatrix} $$
이고 
$$ A - 2B + 2B = A $$이므로 
$$ A = \begin{pmatrix} -7 & -2 \\ 6 & 0 \end{pmatrix} + \begin{pmatrix} 4 & -2 \\ -6 & 2 \end{pmatrix} $$
$$ = \begin{pmatrix} -3 & -4 \\ 0 & 2 \end{pmatrix} $$
따라서 행렬 $A$의 모든 성분의 합은 
$$ -3 + (-4) + 0 + 2 = -5 $$
이다.

정답: ⑤