## 문제
이차정사각행렬 $X$에 대하여
$$ X \left( \begin{array}{c} 1 \\ 2 \end{array} \right) = \left( \begin{array}{c} 3 \\ 4 \end{array} \right) , X^{-1} \left( \begin{array}{c} 5 \\ 6 \end{array} \right) = \left( \begin{array}{c} 3 \\ 4 \end{array} \right) $$
일 때, $X^{2} \left( \begin{array}{c} 1 \\ 2 \end{array} \right)$의 모든 성분의 합은?

## 보기
① $8$   ② $9$   ③ $10$   ④ $11$   ⑤ $12$

## 풀이
$X^{-1} \left( \begin{array}{c} 5 \\ 6 \end{array} \right) = \left( \begin{array}{c} 3 \\ 4 \end{array} \right)$ 이므로 
$$ X \left( \begin{array}{c} 3 \\ 4 \end{array} \right) = \left( \begin{array}{c} 5 \\ 6 \end{array} \right) $$ 

$X \left( \begin{array}{c} 1 \\ 2 \end{array} \right) = \left( \begin{array}{c} 3 \\ 4 \end{array} \right)$ 이므로 
$$ X^{2} \left( \begin{array}{c} 1 \\ 2 \end{array} \right) = X \left( X \left( \begin{array}{c} 1 \\ 2 \end{array} \right) \right) = X \left( \begin{array}{c} 3 \\ 4 \end{array} \right) = \left( \begin{array}{c} 5 \\ 6 \end{array} \right) $$ 

따라서 $X^2 \left( \begin{array}{c} 1 \\ 2 \end{array} \right)$의 모든 성분의 합은 
$$ 5 + 6 = 11 $$
정답은 ④입니다.