## 문제
두 행렬 $A$, $B$ 에 대하여 
$$ A-2B = \left( \begin{array}{cc} -7 & -2 \\ 6 & 0 \end{array} \right), B = \left( \begin{array}{cc} 2 & -1 \\ -3 & 1 \end{array} \right) $$ 
일 때, 행렬 $A$ 의 모든 성분의 합은?

## 보기
① $-1$   ② $-2$   ③ $-3$   ④ $-4$   ⑤ $-5$

## 풀이
$$ B = \left( \begin{array}{cc} 2 & -1 \\ -3 & 1 \end{array} \right) $$ 에서 
$$ 2B = \left( \begin{array}{cc} 4 & -2 \\ -6 & 2 \end{array} \right) $$ 
이고 $A - 2B + 2B = A$ 이므로 
$$ A = \left( \begin{array}{cc} -7 & -2 \\ 6 & 0 \end{array} \right) + \left( \begin{array}{cc} 4 & -2 \\ -6 & 2 \end{array} \right) $$ 
$$ = \left( \begin{array}{cc} -3 & -4 \\ 0 & 2 \end{array} \right) $$ 
따라서 행렬 $A$ 의 모든 성분의 합은 $-3 + (-4) + 0 + 2 = -5$ 이다.

[정답] ⑤