## 문제
이차정사각행렬 $A$가
$$ A^{2}= \left( \begin{array}{cc} 1 & 0 \\ 0 & 2 \end{array} \right) $$
를 만족시킬 때, 행렬 $16 (A^{-1})^{8}$의 모든 성분의 합을 구하시오. (단, $A^{-1}$는 $A$의 역행렬이다.)

## 보기


## 풀이
$A^{2}= \left( \begin{array}{cc} 1 & 0 \\ 0 & 2 \end{array} \right)$ 이므로
$$ A^{4}= (A^{2})^{2} = \left( \begin{array}{cc} 1^{2} & 0 \\ 0 & 2^{2} \end{array} \right) = \left( \begin{array}{cc} 1 & 0 \\ 0 & 4 \end{array} \right) $$
$$ A^{8}= (A^{4})^{2} = \left( \begin{array}{cc} 1^{2} & 0 \\ 0 & 4^{2} \end{array} \right) = \left( \begin{array}{cc} 1 & 0 \\ 0 & 16 \end{array} \right) $$
이다. $(A^{-1})^{8} = (A^{8})^{-1}$ 이므로
$$ (A^{-1})^{8} = \left( \begin{array}{cc} 1 & 0 \\ 0 & 16 \end{array} \right)^{-1} = \frac{1}{1 \times 16 - 0} \left( \begin{array}{cc} 16 & 0 \\ 0 & 1 \end{array} \right) = \frac{1}{16} \left( \begin{array}{cc} 16 & 0 \\ 0 & 1 \end{array} \right) $$
따라서 행렬 $16 (A^{-1})^{8}$ 은
$$ 16 (A^{-1})^{8} = 16 \cdot \frac{1}{16} \left( \begin{array}{cc} 16 & 0 \\ 0 & 1 \end{array} \right) = \left( \begin{array}{cc} 16 & 0 \\ 0 & 1 \end{array} \right) $$
이며, 모든 성분의 합은 $16 + 0 + 0 + 1 = 17$ 이다.

정답: $17$