## ë¬¸ì œ

ê·¸ë¦¼ê³¼ ê°™ì´ ê³¡ì„  $y=x^{2}$ ìœ„ì˜ ì  ($-1$, $1$), ($0$, $0$), ($1$, $1$)ì„ ê¼­ì§“ì ìœ¼ë¡œ í•˜ëŠ” ì‚¼ê°í˜•ì„ $A_{1}$ì´ë¼ í•˜ìž. 

$y=x^{2}$ ìœ„ì˜ ì  ($-2$, $4$), ($-1$, $1$), ($0$, $0$), ($1$, $1$), ($2$, $4$)ë¥¼ ê¼­ì§“ì ìœ¼ë¡œ í•˜ëŠ” ì˜¤ê°í˜•ì„ $A_{2}$ë¼ í•˜ìž. 

$y=x^{2}$ ìœ„ì˜ ì  ($-3$, $9$), ($-2$, $4$), ($-1$, $1$), ($0$, $0$), ($1$, $1$), ($2$, $4$), ($3$, $9$)ë¥¼ ê¼­ì§“ì ìœ¼ë¡œ í•˜ëŠ” ì¹ ê°í˜•ì„ $A_{3}$ì´ë¼ í•˜ìž. ì´ì™€ ê°™ì€ ë°©ë²•ìœ¼ë¡œ $n$ ë²ˆì§¸ ì–»ì€ ë‹¤ê°í˜• $A_{n}$ì€ $y=x^{2}$ ìœ„ì˜ ì  ($-n$, $n^{2}$), ($-n+1$, ($n-1$)$^{2}$), $\cdots$, ($-1$, $1$), ($0$, $0$), ($1$, $1$), $\cdots$, ($n-1$, ($n-1$)$^{2}$), ($n$, $n^{2}$)ì„ ê¼­ì§“ì ìœ¼ë¡œ í•˜ëŠ” ë‹¤ê°í˜•ì´ë‹¤. ë‹¤ê°í˜• $A_{n}$ì˜ ë„“ì´ë¥¼ $a_{n}$ì´ë¼ í•  ë•Œ, $\lim_{n \to \infty} \frac{a_{n}}{n^{3}}$ì˜ ê°’ì€? 

> [!example] ðŸ“¸ (ê·¸ë¦¼/ê·¸ëž˜í”„)

> [!example] ðŸ“¸ (ê·¸ë¦¼/ê·¸ëž˜í”„)

## ë³´ê¸°

â‘  $2$   â‘¡ $\frac{3}{2}$   â‘¢ $\frac{4}{3}$   â‘£ $\frac{5}{4}$   â‘¤ $\frac{6}{5}$

## í’€ì´

[ì •ë‹µ] â‘¢ 

$$a_{n+1} - a_{n} = (2n+1)^{2}$$

> [!example] ðŸ“¸ (ê·¸ë¦¼/ê·¸ëž˜í”„)

$$a_{n} = 1 + \sum_{k=1}^{n-1} (2k+1)^{2}$$ 

$$= \frac{4n^{3} - n}{3}$$ 

$\therefore$ 

$$\lim_{n \to \infty} \frac{a_{n}}{n^{3}} = \frac{4}{3}$$