## 문제
수열 $\{ a_{n} \}$ 의 첫째항부터 제 $n$ 항까지의 합 $S_{n}$ 이 $S_{n} = n^{2} + 2n$ 일 때, 무한급수 $\sum_{n=1}^{\infty} \frac{2}{a_{n} a_{n+1}}$ 의 값은?

## 보기
① $\frac{1}{3}$   ② $\frac{1}{4}$   ③ $\frac{1}{5}$   ④ $\frac{1}{6}$   ⑤ $\frac{1}{7}$

## 풀이
$S_{n} = n^{2} + 2n$ 에서
$n = 1$ 일 때, $a_{1} = S_{1} = 1^{2} + 2 \times 1 = 3$
$n \ge 2$ 일 때,
$a_{n} = S_{n} - S_{n-1}$
$= (n^{2} + 2n) - \{ (n-1)^{2} + 2(n-1) \}$
$= n^{2} + 2n - (n^{2} - 2n + 1 + 2n - 2)$
$= 2n + 1$
이때 $a_{1} = 3$ 이므로 $a_{n} = 2n + 1$ ($n \ge 1$) 이 성립한다.

구하는 무한급수의 값은
$\sum_{n=1}^{\infty} \frac{2}{a_{n} a_{n+1}} = \lim_{n \to \infty} \sum_{k=1}^{n} \frac{2}{(2k+1)(2k+3)}$
$= \lim_{n \to \infty} \sum_{k=1}^{n} \left( \frac{1}{2k+1} - \frac{1}{2k+3} \right)$
$= \lim_{n \to \infty} \left\{ \left( \frac{1}{3} - \frac{1}{5} \right) + \left( \frac{1}{5} - \frac{1}{7} \right) + \dots + \left( \frac{1}{2n+1} - \frac{1}{2n+3} \right) \right\}$
$= \lim_{n \to \infty} \left( \frac{1}{3} - \frac{1}{2n+3} \right)$
$= \frac{1}{3}$

정답: ①