## 문제
두 수열 $\{ a_{n} \}$, $\{ b_{n} \}$ 에 대하여 무한급수 $\sum_{n=1}^{\infty} \left( a_{n} - \frac{3n}{n+1} \right)$ 과 $\sum_{n=1}^{\infty} ( a_{n} + b_{n} )$ 이 모두 수렴할 때, $\lim_{n \to \infty} \frac{3 - b_{n}}{a_{n}}$ 의 값은? (단, $a_{n} \neq 0$)

## 보기
① $1$   ② $2$   ③ $3$   ④ $4$   ⑤ $5$

## 풀이
$\sum_{n=1}^{\infty} \left( a_{n} - \frac{3n}{n+1} \right)$ 가 수렴하므로 급수의 성질에 의해
$$\lim_{n \to \infty} \left( a_{n} - \frac{3n}{n+1} \right) = 0$$
$$\lim_{n \to \infty} a_{n} = \lim_{n \to \infty} \frac{3n}{n+1} = 3$$
또한 $\sum_{n=1}^{\infty} ( a_{n} + b_{n} )$ 이 수렴하므로
$$\lim_{n \to \infty} ( a_{n} + b_{n} ) = 0$$
$$\lim_{n \to \infty} b_{n} = -\lim_{n \to \infty} a_{n} = -3$$
구하고자 하는 극한값은
$$\lim_{n \to \infty} \frac{3 - b_{n}}{a_{n}} = \frac{3 - \lim_{n \to \infty} b_{n}}{\lim_{n \to \infty} a_{n}} = \frac{3 - (-3)}{3} = \frac{6}{3} = 2$$
따라서 정답은 ② 이다.