## 문제
두 행렬 $A = \left( \begin{array}{cc} 1 & 0 \\ 3 & -2 \end{array} \right)$, $B = \left( \begin{array}{cc} 2 & -1 \\ 4 & 3 \end{array} \right)$에 대하여 $A + X = 3 B + 2 X$를 만족시키는 행렬 $X$는?

## 보기
① $\left( \begin{array}{cc} 5 & -3 \\ 9 & 11 \end{array} \right)$   ② $\left( \begin{array}{cc} -5 & 3 \\ -9 & -11 \end{array} \right)$   ③ $\left( \begin{array}{cc} 5 & 3 \\ -9 & -11 \end{array} \right)$   ④ $\left( \begin{array}{cc} -5 & 3 \\ -9 & 11 \end{array} \right)$   ⑤ $\left( \begin{array}{cc} -5 & -3 \\ 9 & -11 \end{array} \right)$

## 풀이
$A + X = 3 B + 2 X$를 정리하면 다음과 같다.
$$ X = A - 3 B $$
여기에 두 행렬 $A = \left( \begin{array}{cc} 1 & 0 \\ 3 & -2 \end{array} \right)$, $B = \left( \begin{array}{cc} 2 & -1 \\ 4 & 3 \end{array} \right)$를 대입하면
$$ X = \left( \begin{array}{cc} 1 & 0 \\ 3 & -2 \end{array} \right) - 3 \left( \begin{array}{cc} 2 & -1 \\ 4 & 3 \end{array} \right) $$
$$ X = \left( \begin{array}{cc} 1 & 0 \\ 3 & -2 \end{array} \right) - \left( \begin{array}{cc} 6 & -3 \\ 12 & 9 \end{array} \right) $$
$$ X = \left( \begin{array}{cc} 1 - 6 & 0 - (-3) \\ 3 - 12 & -2 - 9 \end{array} \right) $$
$$ X = \left( \begin{array}{cc} -5 & 3 \\ -9 & -11 \end{array} \right) $$
따라서 구하는 행렬 $X$는 ②이다.

정답: ②