## 문제
수열 $\{ a_{n} \}$ 이 $7 a_{1} + 7^{2} a_{2} + \cdots + 7^{n} a_{n} = 3^{n} - 1$ 을 만족시킬 때, $\sum_{n=1}^{\infty} \frac{a_{n}}{3^{n-1}}$ 의 값은?

## 보기
① $\frac{1}{3}$   ② $\frac{4}{9}$   ③ $\frac{5}{9}$   ④ $\frac{2}{3}$   ⑤ $\frac{7}{9}$

## 풀이
$7 a_{1} + 7^{2} a_{2} + \cdots + 7^{n-1} a_{n-1} + 7^{n} a_{n} = 3^{n} - 1$ $\cdots$ ㉠
$7 a_{1} + 7^{2} a_{2} + \cdots + 7^{n-1} a_{n-1} = 3^{n-1} - 1$ $\cdots$ ㉡

㉠ $-$ ㉡에서
$7^{n} a_{n} = 3^{n} - 3^{n-1} = 2 \cdot 3^{n-1}$
$\therefore a_{n} = \frac{2 \cdot 3^{n-1}}{7^{n}}$ ($n \ge 2$)

$n = 1$ 일 때, $7 a_{1} = 3^{1} - 1$ 에서 $a_{1} = \frac{2}{7}$ 이므로
$a_{n} = \frac{2 \cdot 3^{n-1}}{7^{n}}$ ($n \ge 1$)

$\therefore \sum_{n=1}^{\infty} \frac{a_{n}}{3^{n-1}} = \sum_{n=1}^{\infty} \left( \frac{1}{3^{n-1}} \cdot \frac{2 \cdot 3^{n-1}}{7^{n}} \right)$
$= \sum_{n=1}^{\infty} \frac{2}{7^{n}}$
$= \frac{\frac{2}{7}}{1 - \frac{1}{7}}$
$= \frac{1}{3}$

정답 ①