## 문제
두 행렬 $A$, $B$에 대하여 $A - B = \left( \begin{array}{cc} 3 & 1 \\ 5 & 2 \end{array} \right)$일 때, $AX = \left( \begin{array}{cc} 3 & 1 \\ 1 & 0 \end{array} \right)$, $BX = \left( \begin{array}{cc} 2 & 1 \\ 1 & -1 \end{array} \right)$을 만족시키는 행렬 $X$는?

## 보기
① $\left( \begin{array}{cc} 2 & -1 \\ -5 & 3 \end{array} \right)$ ② $\left( \begin{array}{cc} 1 & 3 \\ -1 & 2 \end{array} \right)$ ③ $\left( \begin{array}{cc} -2 & 1 \\ 5 & -3 \end{array} \right)$ ④ $\left( \begin{array}{cc} 5 & 1 \\ 1 & -2 \end{array} \right)$ ⑤ $\left( \begin{array}{cc} 3 & -1 \\ 0 & 1 \end{array} \right)$

## 풀이
$AX - BX = (A - B)X$이므로 
$$ \left( \begin{array}{cc} 3 & 1 \\ 5 & 2 \end{array} \right) X = \left( \begin{array}{cc} 3 & 1 \\ 1 & 0 \end{array} \right) - \left( \begin{array}{cc} 2 & 1 \\ 1 & -1 \end{array} \right) = \left( \begin{array}{cc} 1 & 0 \\ 0 & 1 \end{array} \right) = E $$ 
따라서 행렬 $X$는 행렬 $\left( \begin{array}{cc} 3 & 1 \\ 5 & 2 \end{array} \right)$의 역행렬이다.
$$ X = \left( \begin{array}{cc} 3 & 1 \\ 5 & 2 \end{array} \right)^{-1} = \frac{1}{3 \cdot 2 - 1 \cdot 5} \left( \begin{array}{cc} 2 & -1 \\ -5 & 3 \end{array} \right) = \left( \begin{array}{cc} 2 & -1 \\ -5 & 3 \end{array} \right) $$
정답은 ①이다.