## ë¬¸ì œ
ê·¸ë¦¼ê³¼ ê°™ì´ ì§ì„  $y=3$ì´ $x=0$, $y=a^{x}$, $y=b^{x}$ (ë‹¨, $1<b<a$)ì˜ ê·¸ë˜í”„ì™€ ë§Œë‚˜ëŠ” ì ì„ ê°ê° $A$, $B$, $C$ë¼ í•˜ê³ , ì  $B$ì—ì„œ $x$ì¶•ì— ë‚´ë¦° ìˆ˜ì„ ì˜ ë°œì„ $H$, $\overline{BH}$ê°€ $y=b^{x}$ì˜ ê·¸ë˜í”„ì™€ ë§Œë‚˜ëŠ” ì ì„ $D$ë¼ í•˜ì. $\overline{AB} = \overline{BC}$ì¼ ë•Œ, $\frac{\overline{BD}}{\overline{DH}}$ì˜ ê°’ì€?

> [!example] ğŸ“¸ (ê·¸ë¦¼/ê·¸ë˜í”„)

## ë³´ê¸°
â‘  $\sqrt{2}-1$   â‘¡ $\frac{\sqrt{3}}{3}$   â‘¢ $\frac{\sqrt{2}}{2}$   â‘£ $\sqrt{3}-1$   â‘¤ $\frac{\sqrt{3}}{2}$

## í’€ì´
ì  $H$ì˜ $x$ì¢Œí‘œë¥¼ $t$ë¼ í•˜ë©´ $\overline{AB} = \overline{BC}$ì´ë¯€ë¡œ $a^{t} = b^{2t} = 3$ì´ë‹¤. 
ë”°ë¼ì„œ $b^{t} = \sqrt{a^{t}} = \sqrt{3}$ì´ë‹¤. 
ê·¸ëŸ¬ë¯€ë¡œ $\frac{\overline{BD}}{\overline{DH}} = \frac{a^{t} - b^{t}}{b^{t}} = \frac{3 - \sqrt{3}}{\sqrt{3}} = \sqrt{3} - 1$ì´ë‹¤. 

ì •ë‹µ â‘£