## 문제
두 행렬 $A= \left( \begin{array}{cc} 1 & -2 \\ 0 & 1 \end{array} \right) $, $B= \left( \begin{array}{cc} 3 & 0 \\ 0 & 4 \end{array} \right) $ 에 대하여 
$$ A^{-1} B^{n} A= \left( \begin{array}{cc} a_{n} & b_{n} \\ c_{n} & d_{n} \end{array} \right) (n=1, 2, 3, \cdots) $$
이라 하자. $\lim _{n \to \infty} \frac{b_{n}+c_{n}}{a_{n}+d_{n}}$ 의 값은? 

## 보기
① $-2$   ② $-1$   ③ $0$   ④ $1$   ⑤ $2$

## 풀이
[정답] ⑤ 

$$ B^{2}= \left( \begin{array}{cc} 3 & 0 \\ 0 & 4 \end{array} \right) \left( \begin{array}{cc} 3 & 0 \\ 0 & 4 \end{array} \right) = \left( \begin{array}{cc} 3^{2} & 0 \\ 0 & 4^{2} \end{array} \right) $$ 

$$ B^{3}= \left( \begin{array}{cc} 3^{2} & 0 \\ 0 & 4^{2} \end{array} \right) \left( \begin{array}{cc} 3 & 0 \\ 0 & 4 \end{array} \right) = \left( \begin{array}{cc} 3^{3} & 0 \\ 0 & 4^{3} \end{array} \right) $$ 

$\cdots$ 이므로 
$B^{n}= \left( \begin{array}{cc} 3^{n} & 0 \\ 0 & 4^{n} \end{array} \right) $ 임을 알 수 있다. 

따라서 $A^{-1} B^{n} A= \left( \begin{array}{cc} 1 & 2 \\ 0 & 1 \end{array} \right) \left( \begin{array}{cc} 3^{n} & 0 \\ 0 & 4^{n} \end{array} \right) \left( \begin{array}{cc} 1 & -2 \\ 0 & 1 \end{array} \right) $ 

$$ = \left( \begin{array}{cc} 3^{n} & -2 \cdot 3^{n}+2 \cdot 4^{n} \\ 0 & 4^{n} \end{array} \right) $$ 

그러므로 $a_{n} = 3^{n}$, $b_{n} = -2 \cdot 3^{n}+2 \cdot 4^{n}$, $c_{n} = 0$, $d_{n} = 4^{n}$ 이다.

$$ \lim _{n \to \infty} \frac{b_{n}+c_{n}}{a_{n}+d_{n}} = \lim _{n \to \infty} \frac{-2 \cdot 3^{n}+2 \cdot 4^{n}}{3^{n}+4^{n}} $$ 

$$ = \lim _{n \to \infty} \frac{-2 \cdot (\frac{3}{4})^{n}+2}{(\frac{3}{4})^{n}+1} = 2 $$