## 문제
함수 $f(x) = x^{10} - x^{9} + x^{8} - x^{7} + \cdots + x^{2} - x + 2$ 일 때, $(f \circ f)(0)$ 의 값은?

## 보기
① $684$   ② $696$   ③ $708$   ④ $720$   ⑤ $732$

## 풀이
$f(0) = 2$ 이므로 
$$(f \circ f)(0) = f(f(0)) = f(2)$$
$$f(2) = 2^{10} - 2^{9} + 2^{8} - 2^{7} + \cdots + 2^{2} - 2 + 2$$
이때, $2^{10} - 2^{9} + 2^{8} - 2^{7} + \cdots + 2^{2} - 2$ 는 첫째항이 $-2$, 공비가 $-2$ 인 등비수열의 제 $10$ 항까지의 합이므로
$$f(2) = \frac{-2 \{ 1 - (-2)^{10} \} }{1 - (-2)} + 2$$
$$= \frac{-2 \times (1 - 1024)}{3} + 2$$
$$= \frac{-2 \times (-1023)}{3} + 2$$
$$= \frac{2046}{3} + 2$$
$$= 682 + 2 = 684$$

정답: ①