## 문제
행렬 $A = \left( \begin{array}{cc} 1 & 2 \\ -2 & 3 \end{array} \right)$에 대하여 행렬 $B$가 $A+B=2E$를 만족시킬 때, 행렬 $A-B$의 모든 성분의 합은? (단, $E$는 단위행렬이다.)

## 보기
① $1$   ② $2$   ③ $3$   ④ $4$   ⑤ $5$

## 풀이
$A+B=2E$에서 $B=2E-A$이므로
$A-B = A-(2E-A) = 2A-2E$

$$ 2A-2E = 2 \left( \begin{array}{cc} 1 & 2 \\ -2 & 3 \end{array} \right) - 2 \left( \begin{array}{cc} 1 & 0 \\ 0 & 1 \end{array} \right) $$
$$ = 2 \left( \begin{array}{cc} 0 & 2 \\ -2 & 2 \end{array} \right) $$
$$ = \left( \begin{array}{cc} 0 & 4 \\ -4 & 4 \end{array} \right) $$

따라서 모든 성분의 합은 $0+4+(-4)+4=4$이다.
정답: ④