## 문제
수열 $\{ a_{n} \}$ 이 모든 자연수 $n$ 에 대하여 
$$ 1 \cdot 2 a_{1} + 3 \cdot 4 a_{2} + 5 \cdot 6 a_{3} + \cdots + ( 2 n - 1 ) \cdot 2 n a_{n} \geq n $$ 
을 만족시킬 때, 다음은 부등식 
$$ a_{1} + a_{2} + a_{3} + \cdots + a_{n} \geq (가) $$ 
이 성립함을 증명한 것이다.

---
$a_{1} + a_{2} + a_{3} + \cdots + a_{n}$
$= ( 1 - \frac{1}{2} ) ( 1 \cdot 2 a_{1} ) + ( \frac{1}{3} - \frac{1}{4} ) ( 3 \cdot 4 a_{2} ) + ( \frac{1}{5} - \frac{1}{6} ) ( 5 \cdot 6 a_{3} ) + \cdots + ( \frac{1}{2 n - 1} - \frac{1}{2 n} ) \{ ( 2 n - 1 ) \cdot 2 n a_{n} \}$
$= ( 1 - \frac{1}{2} - \frac{1}{3} + \frac{1}{4} ) ( 1 \cdot 2 a_{1} ) + ( \frac{1}{3} - \frac{1}{4} - \frac{1}{5} + \frac{1}{6} ) ( 1 \cdot 2 a_{1} + 3 \cdot 4 a_{2} ) + ( \frac{1}{5} - \frac{1}{6} - \frac{1}{7} + \frac{1}{8} ) ( 1 \cdot 2 a_{1} + 3 \cdot 4 a_{2} + 5 \cdot 6 a_{3} ) + \cdots + ( \frac{1}{2 n - 1} - \frac{1}{2 n} ) \{ 1 \cdot 2 a_{1} + 3 \cdot 4 a_{2} + \cdots + ( 2 n - 1 ) \cdot 2 n a_{n} \}$
$\geq ( 1 - \frac{1}{2} - \frac{1}{3} + \frac{1}{4} ) + 2 ( \frac{1}{3} - \frac{1}{4} - \frac{1}{5} + \frac{1}{6} ) + 3 ( \frac{1}{5} - \frac{1}{6} - \frac{1}{7} + \frac{1}{8} ) + \cdots + (나)$
$= 1 - \frac{1}{2} + \frac{1}{3} - \frac{1}{4} + \frac{1}{5} - \frac{1}{6} + \cdots + \frac{1}{2 n - 1} - \frac{1}{2 n}$
$= 1 + \frac{1}{2} + \frac{1}{3} + \frac{1}{4} + \cdots + \frac{1}{2 n - 1} + \frac{1}{2 n} - (다)$
$= (가)$
---

위의 과정에서 $(가)$, $(나)$, $(다)$에 알맞은 것은?

## 보기
① $(가) \sum_{k=1}^{n} \frac{1}{n+k}$   ② $(가) \sum_{k=1}^{n} \frac{1}{n+k}$   ③ $(가) \sum_{k=1}^{2n} \frac{1}{n+k}$   ④ $(가) \sum_{k=1}^{2n} \frac{1}{n+k}$   ⑤ $(가) \sum_{k=1}^{2n} \frac{1}{n+k}$
$(나) (\frac{1}{2n-1} - \frac{1}{2n})$   $(나) n (\frac{1}{2n-1} - \frac{1}{2n})$   $(나) n (\frac{1}{2n-1} - \frac{1}{2n})$   $(나) n (\frac{1}{2n-1} - \frac{1}{2n})$   $(나) (\frac{1}{2n-1} - \frac{1}{2n})$
$(다) 2 (\frac{1}{2} + \frac{1}{4} + \cdots + \frac{1}{2n})$   $(다) 2 (\frac{1}{2} + \frac{1}{4} + \cdots + \frac{1}{2n})$   $(다) 2 (\frac{1}{2} + \frac{1}{4} + \cdots + \frac{1}{2n})$   $(다) (\frac{1}{2} + \frac{1}{4} + \cdots + \frac{1}{2n})$   $(다) (\frac{1}{2} + \frac{1}{4} + \cdots + \frac{1}{2n})$

## 풀이
$a_{1} + a_{2} + a_{3} + \cdots + a_{n}$
$= ( 1 - \frac{1}{2} ) ( 1 \cdot 2 a_{1} ) + ( \frac{1}{3} - \frac{1}{4} ) ( 3 \cdot 4 a_{2} ) + ( \frac{1}{5} - \frac{1}{6} ) ( 5 \cdot 6 a_{3} ) + \cdots + ( \frac{1}{2 n - 1} - \frac{1}{2 n} ) \{ ( 2 n - 1 ) \cdot 2 n a_{n} \}$
$= ( 1 - \frac{1}{2} - \frac{1}{3} + \frac{1}{4} ) ( 1 \cdot 2 a_{1} ) + ( \frac{1}{3} - \frac{1}{4} - \frac{1}{5} + \frac{1}{6} ) ( 1 \cdot 2 a_{1} + 3 \cdot 4 a_{2} ) + ( \frac{1}{5} - \frac{1}{6} - \frac{1}{7} + \frac{1}{8} ) ( 1 \cdot 2 a_{1} + 3 \cdot 4 a_{2} + 5 \cdot 6 a_{3} ) + \cdots + ( \frac{1}{2 n - 1} - \frac{1}{2 n} ) \{ 1 \cdot 2 a_{1} + 3 \cdot 4 a_{2} + \cdots + ( 2 n - 1 ) \cdot 2 n a_{n} \}$
$1 \cdot 2 a_{1} + 3 \cdot 4 a_{2} + \cdots + ( 2 n - 1 ) \cdot 2 n a_{n} \geq n$ 이므로
$\geq ( 1 - \frac{1}{2} - \frac{1}{3} + \frac{1}{4} ) + 2 ( \frac{1}{3} - \frac{1}{4} - \frac{1}{5} + \frac{1}{6} ) + 3 ( \frac{1}{5} - \frac{1}{6} - \frac{1}{7} + \frac{1}{8} ) + \cdots + n ( \frac{1}{2 n - 1} - \frac{1}{2 n} )$
따라서 $(나) = n ( \frac{1}{2 n - 1} - \frac{1}{2 n} )$ 이다.
이를 계산하면
$= 1 - \frac{1}{2} + \frac{1}{3} - \frac{1}{4} + \frac{1}{5} - \frac{1}{6} + \cdots + \frac{1}{2 n - 1} - \frac{1}{2 n}$
$= ( 1 + \frac{1}{2} + \frac{1}{3} + \frac{1}{4} + \cdots + \frac{1}{2 n } ) - 2 ( \frac{1}{2} + \frac{1}{4} + \frac{1}{6} + \cdots + \frac{1}{2 n} )$
따라서 $(다) = 2 ( \frac{1}{2} + \frac{1}{4} + \frac{1}{6} + \cdots + \frac{1}{2 n} )$ 이다.
$= \sum_{k=1}^{2 n} \frac{1}{k} - \sum_{k=1}^{n} \frac{1}{k} = \sum_{k=n+1}^{2 n} \frac{1}{k} = \sum_{k=1}^{n} \frac{1}{n+k}$
따라서 $(가) = \sum_{k=1}^{n} \frac{1}{n+k}$ 이다.

정답은 ② 이다.