## 문제
$x = \frac{b - c}{1 + bc}$, $y = \frac{c - a}{1 + ca}$, $z = \frac{a - b}{1 + ab}$ 일 때, $x + y + z = (가)$ 임을 증명하는 과정이다.

$x = \frac{b - c}{1 + bc}$ 에서 $(1 + bc)x = b - c$ 이고, 정리하면
$(bx + 1)c = b - x$ $\cdots$ ㉠
같은 방법으로 $y = \frac{c - a}{1 + ca}$ 에서
$(ay - 1)c = -a - y$ $\cdots$ ㉡
㉠과 ㉡에서
$(a + y)(bx + 1)c = (나)(ay - 1)c$ $\cdots$ ㉢
(ⅰ) ㉢에서 $c \neq 0$ 이면
$(a + y)(bx + 1) = (나)(ay - 1)$ 이고 정리하면
$(ab + 1)(x + y) = (다)(xy - 1)$
$ab + 1 \neq 0$ 이므로 $x + y = \frac{(다)}{ab + 1}(xy - 1)$
$x + y + z = (가)$
(ⅱ) ㉢에서 $c = 0$ 이면
$x = b$, $y = -a$, $z = \frac{a - b}{1 + ab}$ 이므로
$x + y + z = (가)$
따라서 $x = \frac{b - c}{1 + bc}$, $y = \frac{c - a}{1 + ca}$, $z = \frac{a - b}{1 + ab}$ 일 때, $x + y + z = (가)$ 이다.

위의 증명에서 $(가)$, $(나)$, $(다)$에 알맞은 것은?

## 보기
$$ \begin{array}{c|c|c|c} \hline & (가) & (나) & (다) \\ \hline ① & xyz & x - b & a - b \\ \hline ② & xyz & b - x & a - b \\ \hline ③ & xyz & x - b & a + b \\ \hline ④ & xy + yz + zx & x - b & a - b \\ \hline ⑤ & xy + yz + zx & b - x & a + b \\ \hline \end{array} $$

① $(가): xyz, (나): x - b, (다): a - b$   ② $(가): xyz, (나): b - x, (다): a - b$   ③ $(가): xyz, (나): x - b, (다): a + b$   ④ $(가): xy + yz + zx, (나): x - b, (다): a - b$   ⑤ $(가): xy + yz + zx, (나): b - x, (다): a + b$

## 풀이
[정답] ①

$x = \frac{b - c}{1 + bc}$ 에서 $(1 + bc)x = b - c$ 이고, 정리하면
$(bx + 1)c = b - x$ $\cdots$ ㉠
같은 방법으로 $y = \frac{c - a}{1 + ca}$ 에서
$(ay - 1)c = -a - y$ $\cdots$ ㉡
㉠과 ㉡에서
$(a + y)(bx + 1)c = (x - b)(ay - 1)c$ $\cdots$ ㉢
(ⅰ) ㉢에서 $c \neq 0$ 이면
$(a + y)(bx + 1) = (x - b)(ay - 1)$ 이고 정리하면
$(ab + 1)(x + y) = (a - b)(xy - 1)$
$ab + 1 \neq 0$ 이므로
$x + y = \frac{a - b}{ab + 1}(xy - 1)$
$x + y + z = xyz$
(ⅱ) ㉢에서 $c = 0$ 이면
$x = b$, $y = -a$, $z = \frac{a - b}{1 + ab}$ 이므로
$x + y + z = xyz$

따라서 $x = \frac{b - c}{1 + bc}$, $y = \frac{c - a}{1 + ca}$, $z = \frac{a - b}{1 + ab}$ 일 때, $x + y + z = xyz$ 이다.
그러므로 $(가): xyz$, $(나): x - b$, $(다): a - b$ 이다.