## 문제
수열 $\{ a_{n} \}$ 에 대하여 
$$ \sum_{n=1}^{\infty} \left( a_{n} - \frac{1^{3} + 2^{3} + 3^{3} + \cdots + n^{3}}{n^{4}} \right) $$
이 수렴할 때, $\lim_{n \to \infty} a_{n}$ 의 값은?

## 보기
① $\frac{1}{4}$   ② $\frac{1}{2}$   ③ $\frac{3}{4}$   ④ $1$   ⑤ $\frac{5}{4}$

## 풀이
$\sum_{n=1}^{\infty} \left( a_{n} - \frac{1^{3} + 2^{3} + 3^{3} + \cdots + n^{3}}{n^{4}} \right)$ 이 수렴하므로 
$\lim_{n \to \infty} \left( a_{n} - \frac{1^{3} + 2^{3} + 3^{3} + \cdots + n^{3}}{n^{4}} \right) = 0$ 이다. 
따라서 
$$ \begin{aligned} \lim_{n \to \infty} a_{n} &= \lim_{n \to \infty} \frac{1^{3} + 2^{3} + 3^{3} + \cdots + n^{3}}{n^{4}} \\ &= \lim_{n \to \infty} \frac{\left\{ \frac{n(n+1)}{2} \right\}^{2}}{n^{4}} \\ &= \lim_{n \to \infty} \frac{n^{2}(n+1)^{2}}{4n^{4}} \\ &= \frac{1}{4} \end{aligned} $$

정답: ①