## 문제
$\omega^{2}+\omega+1=0$ 일 때, 임의의 두 복소수 $\alpha$ 와 $\beta$ 에 대하여 $x=\alpha-\beta$, $y=\alpha\omega-\beta\omega^{2}$, $z=\alpha\omega^{2}-\beta\omega$ 라 하자. $x^{3}+y^{3}+z^{3}$ 을 $\alpha$ 와 $\beta$ 에 관한 식으로 나타낸 것은?

## 보기
① $\alpha^{3}-2\alpha^{2}\beta+2\alpha\beta^{2}-\beta^{3}$   ② $\alpha^{3}-\beta^{3}$   ③ $3(\alpha^{3}-2\alpha^{2}\beta+2\alpha\beta^{2}-\beta^{3})$   ④ $3(\alpha^{3}-\beta^{3})$   ⑤ $3(\alpha-\beta)^{3}$

## 풀이
$\omega^{2}+\omega+1=0$ 이고 $\omega \neq 1$ 이므로
$(\omega-1)(\omega^{2}+\omega+1)=\omega^{3}-1=0$ 에서 $\omega^{3}=1$ 이다.

$x+y+z=\alpha(1+\omega+\omega^{2})-\beta(1+\omega+\omega^{2})=0$ 이므로 
$x^{3}+y^{3}+z^{3}=3xyz$ 가 성립한다.

($\because x^{3}+y^{3}+z^{3}-3xyz=(x+y+z)(x^{2}+y^{2}+z^{2}-xy-yz-zx)$)

$3xyz=3(\alpha-\beta)(\alpha\omega-\beta\omega^{2})(\alpha\omega^{2}-\beta\omega)$
$=3(\alpha-\beta)(\alpha^{2}\omega^{3}-\alpha\beta\omega^{2}-\alpha\beta\omega^{4}+\beta^{2}\omega^{3})$
$=3(\alpha-\beta)(\alpha^{2}+\alpha\beta+\beta^{2})$ ($\because \omega^{2}+\omega=-1, \omega^{3}=1$)
$=3(\alpha^{3}-\beta^{3})$

정답: ④