## 문제
닫힌구간 $[ 0 , 2 \pi ]$ 에서 삼각방정식 
$$ ( \sqrt{3} \sin x + \cos x )^{2} - 2 \sin ( x + \frac{\pi}{6} ) = 0 $$ 
의 모든 해의 합은? 

## 보기
① $4 \pi$   ② $\frac{13}{3} \pi$   ③ $\frac{14}{3} \pi$   ④ $5 \pi$   ⑤ $\frac{16}{3} \pi$

## 풀이
삼각함수의 합성에 의해 $\sqrt{3} \sin x + \cos x = 2 ( \frac{\sqrt{3}}{2} \sin x + \frac{1}{2} \cos x ) = 2 \sin ( x + \frac{\pi}{6} )$ 이다.
주어진 방정식에 대입하면
$$ 4 \sin^{2} ( x + \frac{\pi}{6} ) - 2 \sin ( x + \frac{\pi}{6} ) = 0 $$ 
$$ 2 \sin ( x + \frac{\pi}{6} ) \{ 2 \sin ( x + \frac{\pi}{6} ) - 1 \} = 0 $$
따라서 $\sin ( x + \frac{\pi}{6} ) = 0$ 또는 $\sin ( x + \frac{\pi}{6} ) = \frac{1}{2}$ 이다.
$0 \le x \le 2 \pi$ 에서 $\frac{\pi}{6} \le x + \frac{\pi}{6} \le \frac{13}{6} \pi$ 이므로
$1)$ $\sin ( x + \frac{\pi}{6} ) = 0$ 에서
$x + \frac{\pi}{6} = \pi , 2 \pi$
$x = \frac{5}{6} \pi , \frac{11}{6} \pi$

$2)$ $\sin ( x + \frac{\pi}{6} ) = \frac{1}{2}$ 에서
$x + \frac{\pi}{6} = \frac{\pi}{6} , \frac{5}{6} \pi , \frac{13}{6} \pi$
$x = 0 , \frac{2}{3} \pi , 2 \pi$

따라서 모든 해 $x$ 는 $0 , \frac{2}{3} \pi , \frac{5}{6} \pi , \frac{11}{6} \pi , 2 \pi$ 이다.
모든 해의 합은
$$ 0 + \frac{4}{6} \pi + \frac{5}{6} \pi + \frac{11}{6} \pi + \frac{12}{6} \pi = \frac{32}{6} \pi = \frac{16}{3} \pi $$

정답: ⑤