## 문제
모든 항이 양수인 수열 $\{ a_{n} \}$ 에 대하여 $\sum_{n=1}^{\infty} ( 3^{n} a_{n} - 2 )$ 가 수렴할 때, $\lim_{n \to \infty} \frac{6 a_{n} + 5 \cdot 4^{-n}}{a_{n} + 3^{-n}}$ 의 값을 구하시오.

## 보기

## 풀이
$\sum_{n=1}^{\infty} ( 3^{n} a_{n} - 2 )$ 가 수렴하므로
$\lim_{n \to \infty} ( 3^{n} a_{n} - 2 ) = 0$
$\therefore \lim_{n \to \infty} 3^{n} a_{n} = 2$

따라서 구하고자 하는 극한값은 다음과 같다.
$\lim_{n \to \infty} \frac{6 a_{n} + 5 \cdot 4^{-n}}{a_{n} + 3^{-n}}$
$= \lim_{n \to \infty} \frac{6 \cdot 3^{n} a_{n} + 5 \cdot 3^{n} \cdot 4^{-n}}{3^{n} a_{n} + 3^{n} \cdot 3^{-n}}$
$= \lim_{n \to \infty} \frac{6 \cdot 3^{n} a_{n} + 5 \left( \frac{3}{4} \right)^{n}}{3^{n} a_{n} + 1}$
$= \frac{6 \cdot 2 + 5 \cdot 0}{2 + 1} = \frac{12}{3} = 4$

정답: $4$