## 문제
행렬 $A = \left( \begin{array}{cc} -2 & 3 \\ -1 & 2 \end{array} \right)$, $B = \left( \begin{array}{cc} -1 & 0 \\ 1 & 2 \end{array} \right)$에 대하여 행렬 $A^{-1}(2 A+B)$의 모든 성분의 합을 구하시오.

## 보기

## 풀이
$A^{-1}(2 A+B)$
$= 2 E+A^{-1} B$
$$ = \left( \begin{array}{cc} 2 & 0 \\ 0 & 2 \end{array} \right) + \left( \begin{array}{cc} -2 & 3 \\ -1 & 2 \end{array} \right) \left( \begin{array}{cc} -1 & 0 \\ 1 & 2 \end{array} \right) $$
$$ = \left( \begin{array}{cc} 7 & 6 \\ 3 & 6 \end{array} \right) $$
$\therefore$ 모든 성분의 합은 
$7+6+3+6=22$

정답: $22$