## 문제
두 행렬 $A$, $B$에 대하여 
$$ \begin{array}{c} A - B = \left( \begin{array}{cc} 3 & 1 \\ 5 & 2 \end{array} \right) \end{array} $$
일 때, 
$$ \begin{array}{c} AX = \left( \begin{array}{cc} 3 & 1 \\ 1 & 0 \end{array} \right), BX = \left( \begin{array}{cc} 2 & 1 \\ 1 & -1 \end{array} \right) \end{array} $$
을 만족시키는 행렬 $X$는?

## 보기
① $\left( \begin{array}{cc} 2 & -1 \\ -5 & 3 \end{array} \right)$   ② $\left( \begin{array}{cc} 1 & 3 \\ -1 & 2 \end{array} \right)$   ③ $\left( \begin{array}{cc} -2 & 1 \\ 5 & -3 \end{array} \right)$   ④ $\left( \begin{array}{cc} 5 & 1 \\ 1 & -2 \end{array} \right)$   ⑤ $\left( \begin{array}{cc} 3 & -1 \\ 0 & 1 \end{array} \right)$

## 풀이
$$ \begin{array}{c} AX - BX = (A - B)X \end{array} $$
이므로
$$ \begin{array}{c} \left( \begin{array}{cc} 3 & 1 \\ 5 & 2 \end{array} \right) X = \left( \begin{array}{cc} 3 & 1 \\ 1 & 0 \end{array} \right) - \left( \begin{array}{cc} 2 & 1 \\ 1 & -1 \end{array} \right) = \left( \begin{array}{cc} 1 & 0 \\ 0 & 1 \end{array} \right) = E \end{array} $$
따라서 
$$ \begin{array}{c} X = \left( \begin{array}{cc} 3 & 1 \\ 5 & 2 \end{array} \right)^{-1} = \frac{1}{3 \times 2 - 1 \times 5} \left( \begin{array}{cc} 2 & -1 \\ -5 & 3 \end{array} \right) = \left( \begin{array}{cc} 2 & -1 \\ -5 & 3 \end{array} \right) \end{array} $$
정답: ①