## 문제
이차정사각행렬 $A$, $B$가 $A+B=-E$, $AB=E$를 만족시킬 때, $(A+B)+ (A^{2}+B^{2} )+ \cdots+ (A^{2011}+B^{2011})$을 간단히 한 것은? (단, $E$는 단위행렬이다.)

## 보기
① $-2 E$   ② $-E$   ③ $E$   ④ $2 E$   ⑤ $3 E$

## 풀이
[정답] ②

$A+B=-E$, $AB=E$이므로,
$A(-E-A)=E$
$\therefore A^{2}+A+E=O$
같은 방법으로 $B^{2}+B+E=O$

한편,
$A^{3}=A^{2} A=(-A-E) A=-A^{2}-A=E$
같은 방법으로 $B^{3}=E$

$(A+B)+ (A^{2}+B^{2} )+ \cdots+ (A^{2011}+B^{2011})$
$= (A+A^{2}+A^{3}+ \cdots+A^{2011} )+ (B+B^{2}+B^{3}+ \cdots+B^{2011} )$
이때 $A+A^2+A^3 = A+A^2+E = O$이고, $2011 = 3 \times 670 + 1$이므로 각 급수의 합은 첫 번째 항인 $A$와 $B$만 남게 된다.
$= A+B = -E$