## 문제
수렴하는 무한수열만을 <보기>에서 있는 대로 고른 것은?

ㄱ. $\{ ( - \frac{1}{2} ) ^{n} \}$
ㄴ. $\{ \frac{5^{n+1} - 3^{n}}{5^{n} + 4^{n}} \}$
ㄷ. $\{ \frac{\sqrt{n^{2} + n} - n}{n} \}$

## 보기
① $ㄱ$   ② $ㄷ$   ③ $ㄱ, ㄴ$   ④ $ㄴ, ㄷ$   ⑤ $ㄱ, ㄴ, ㄷ$

## 풀이
[정답] ⑤

ㄱ. $\lim_{n \to \infty} ( - \frac{1}{2} ) ^{n} = 0$ (참)
ㄴ. $\lim_{n \to \infty} \frac{5^{n+1} - 3^{n}}{5^{n} + 4^{n}} = \lim_{n \to \infty} \frac{5 - ( \frac{3}{5} ) ^{n}}{1 + ( \frac{4}{5} ) ^{n}} = \frac{5 - 0}{1 + 0} = 5$ (참)
ㄷ. $\lim_{n \to \infty} \frac{\sqrt{n^{2} + n} - n}{n} = \lim_{n \to \infty} \frac{(\sqrt{n^{2} + n} - n)(\sqrt{n^{2} + n} + n)}{n(\sqrt{n^{2} + n} + n)} = \lim_{n \to \infty} \frac{n}{n(\sqrt{n^{2} + n} + n)} = \lim_{n \to \infty} \frac{1}{\sqrt{n^{2} + n} + n} = 0$ (참)