## 문제
$x = \sqrt{\log_{2} 3}$, $y = \sqrt{\log_{2} 6}$ 일 때, $(x^{2}+2xy+y^{2})(x^{2}-2xy+y^{2})$ 의 값은?

## 보기
① $1$   ② $\log_{2} 3$   ③ $2$   ④ $\log_{2} 6$   ⑤ $3$

## 풀이
$(x^{2}+2xy+y^{2})(x^{2}-2xy+y^{2}) = (x+y)^{2}(x-y)^{2}$
$= \{ (x+y)(x-y) \}^{2}$
$= (x^{2}-y^{2})^{2}$

$x = \sqrt{\log_{2} 3}$, $y = \sqrt{\log_{2} 6}$ 이므로 $x^{2} = \log_{2} 3$, $y^{2} = \log_{2} 6$ 이다.
이를 식에 대입하면
$( \log_{2} 3 - \log_{2} 6 )^{2} = ( \log_{2} \frac{3}{6} )^{2}$
$= ( \log_{2} \frac{1}{2} )^{2}$
$= ( -1 )^{2} = 1$

정답은 ① 이다.