## 문제
첫째항이 $1$인 무한등비수열 $\{a_{n}\}$에 대하여 $\sum_{n=1}^{\infty} a_{n} = 3$일 때, $\sum_{n=1}^{\infty} (a_{3n-2} - a_{3n-1})$의 값은?

## 보기
① $\frac{7}{19}$   ② $\frac{8}{19}$   ③ $\frac{9}{19}$   ④ $\frac{10}{19}$   ⑤ $\frac{11}{19}$

## 풀이
등비수열 $\{a_{n}\}$의 공비를 $r$라 하면 
$\sum_{n=1}^{\infty} a_{n} = \frac{1}{1-r} = 3$이므로 $r = \frac{2}{3}$이다. 
수열 $\{a_{3n-2}\}$는 첫째항이 $1$이고 공비가 $(\frac{2}{3})^3 = \frac{8}{27}$인 등비수열이고, 수열 $\{a_{3n-1}\}$은 첫째항이 $a_{2} = 1 \times \frac{2}{3} = \frac{2}{3}$이고 공비가 $(\frac{2}{3})^3 = \frac{8}{27}$인 등비수열이다. 따라서 
$\sum_{n=1}^{\infty} (a_{3n-2} - a_{3n-1}) = \frac{1}{1 - \frac{8}{27}} - \frac{\frac{2}{3}}{1 - \frac{8}{27}} = \frac{1 - \frac{2}{3}}{\frac{19}{27}} = \frac{\frac{1}{3}}{\frac{19}{27}} = \frac{9}{19}$

정답: ③