## 문제
수열 $\{ a_{n} \}$ 에 대하여 무한급수 $\sum_{n=1}^{\infty} \left( \frac{a_{n}}{n^{2} + n} - 1 \right)$ 이 수렴할 때, $\lim_{n \to \infty} \frac{a_{n} + 2n^{2}}{2a_{n} - n^{2}}$ 의 값은?

## 보기
① $-2$   ② $-1$   ③ $1$   ④ $2$   ⑤ $3$

## 풀이
$\sum_{n=1}^{\infty} \left( \frac{a_{n}}{n^{2} + n} - 1 \right)$ 이 수렴하므로 
$$\lim_{n \to \infty} \left( \frac{a_{n}}{n^{2} + n} - 1 \right) = 0$$, 
$$\lim_{n \to \infty} \frac{a_{n}}{n^{2} + n} = 1$$ 

$\frac{a_{n}}{n^{2} + n} = b_{n}$ 이라 하면 
$$\lim_{n \to \infty} \frac{a_{n} + 2n^{2}}{2a_{n} - n^{2}} = \lim_{n \to \infty} \frac{(n^{2} + n)b_{n} + 2n^{2}}{2(n^{2} + n)b_{n} - n^{2}}$$ 
$$= \lim_{n \to \infty} \frac{\left( 1 + \frac{1}{n} \right) b_{n} + 2}{2 \left( 1 + \frac{1}{n} \right) b_{n} - 1} = 3$$ 

정답은 ⑤이다.