## 문제
이차함수 $f(x)$는 $f(0)=-1$이고, 
$$\int_{-1}^{1} f(x)dx = \int_{0}^{1} f(x)dx = \int_{-1}^{0} f(x)dx$$
를 만족시킨다. $f(2)$의 값은?

## 보기
① $11$   ② $10$   ③ $9$   ④ $8$   ⑤ $7$

## 풀이
$f(0)=-1$이므로 
$f(x)=ax^{2} +bx-1$
한편, 
$\int_{-1}^{1} f(x)dx = \int_{0}^{1} f(x)dx$에서 
$\int_{-1}^{0} f(x)dx + \int_{0}^{1} f(x)dx = \int_{0}^{1} f(x)dx$ 
$\therefore \int_{-1}^{0} f(x)dx = 0$ 
그러므로 
$\int_{-1}^{0} f(x)dx$ 
$= \int_{-1}^{0} (ax^{2} +bx-1)dx$ 
$= \left[ \frac{a}{3}x^{3} + \frac{b}{2}x^{2} -x \right]_{-1}^{0}$ 
$= \frac{a}{3} - \frac{b}{2} -1=0$ $\cdots\cdots$ ㉠ 

마찬가지로, 
$\int_{-1}^{1} f(x)dx = \int_{-1}^{0} f(x)dx$에서 
$\int_{-1}^{0} f(x)dx + \int_{0}^{1} f(x)dx = \int_{-1}^{0} f(x)dx$ 
$\therefore \int_{0}^{1} f(x)dx = 0$ 
$\int_{0}^{1} f(x)dx$ 
$= \int_{0}^{1} (ax^{2} +bx-1)dx$ 
$= \left[ \frac{a}{3}x^{3} + \frac{b}{2}x^{2} -x \right]_{0}^{1}$ 
$= \frac{a}{3} + \frac{b}{2} -1=0$ $\cdots\cdots$ ㉡ 

㉠과 ㉡에서 
$a=3, b=0$ 
따라서 $f(x)=3x^{2}-1$이므로 
$f(2)=3 \cdot 2^{2} - 1 = 11$

정답: ①