## ë¬¸ì œ
ê·¸ë¦¼ê³¼ ê°™ì´ `$x$`ì¶• ìœ„ì˜ ì  `$A_{1}(1, 0)$`, `$A_{2}(1 + \frac{1}{2}, 0)$`, `$\cdots$`, `$A_{n}(1 + \frac{1}{2} + \cdots + \frac{1}{2^{n-1}}, 0)$`ì—ì„œ `$y$`ì¶•ì— í‰í–‰í•œ ì§ì„ ì„ ê·¸ì–´ ê³¡ì„  `$y = \frac{3}{x}$`ê³¼ ë§Œë‚˜ëŠ” ì ì„ ê°ê° `$B_{1}$`, `$B_{2}$`, `$\cdots$`, `$B_{n}$`ì´ë¼ í•˜ì. `$\triangle A_{0} A_{1} B_{1}$`ì˜ ë„“ì´ë¥¼ `$S_{1}$`, `$\triangle A_{1} A_{2} B_{2}$`ì˜ ë„“ì´ë¥¼ `$S_{2}$`, `$\triangle A_{2} A_{3} B_{3}$`ì˜ ë„“ì´ë¥¼ `$S_{3}$`, `$\cdots$`, `$\triangle A_{n-1} A_{n} B_{n}$`ì˜ ë„“ì´ë¥¼ `$S_{n}$`ì´ë¼ í•  ë•Œ, `$S_{10}$`ì˜ ê°’ì€? (ë‹¨, `$A_{0}$`ì€ ì›ì ì´ë‹¤.)



> [!example] ğŸ“¸ (ê·¸ë¦¼/ê·¸ë˜í”„)

## ë³´ê¸°
â‘  $\frac{1}{678}$   â‘¡ $\frac{1}{679}$   â‘¢ $\frac{1}{680}$   â‘£ $\frac{1}{681}$   â‘¤ $\frac{1}{682}$

## í’€ì´
[ì •ë‹µ] â‘¤

[í•´ì„¤]
ì  `$A_{n}$`ì˜ `$x$`ì¢Œí‘œëŠ” `$x_{n} = \sum_{k=1}^{n} \frac{1}{2^{k-1}}$`ì´ë¯€ë¡œ
`$S_{n} = \frac{1}{2} \overline{A_{n-1} A_{n}} \times \overline{A_{n} B_{n}}$`
`$= \frac{1}{2} \times \frac{1}{2^{n-1}} \times \frac{3}{\sum_{k=1}^{n} \frac{1}{2^{k-1}}}$`
`$= \frac{1}{2} \times \frac{1}{2^{n-1}} \times \frac{3}{\frac{1(1-(1/2)^{n})}{1-1/2}}$`
`$= \frac{1}{2} \times \frac{1}{2^{n-1}} \times \frac{3}{2(1-\frac{1}{2^{n}})}$`
`$= \frac{1}{2} \times \frac{1}{2^{n-1}} \times \frac{3}{\frac{2^{n}-1}{2^{n-1}}}$`
`$= \frac{3}{2(2^{n}-1)}$`

ë”°ë¼ì„œ `$n=10$`ì¼ ë•Œ,
`$\therefore S_{10} = \frac{3}{2(2^{10}-1)} = \frac{3}{2(1023)} = \frac{3}{2046} = \frac{1}{682}$`