## ë¬¸ì œ
ë¬´ë¦¬í•¨ìˆ˜ $f(x) = \sqrt{x+1}$ê³¼ ìì—°ìˆ˜ $n$ì— ëŒ€í•˜ì—¬ ê·¸ë¦¼ê³¼ ê°™ì´ $y=f(x)$ì˜ ê·¸ë˜í”„ ìœ„ì˜ í•œ ì  $P_{n}(n, f(n))$ì—ì„œ $x$ì¶•ì— ë‚´ë¦° ìˆ˜ì„ ì˜ ë°œì„ $Q_{n}$, $y$ì¶•ì— ë‚´ë¦° ìˆ˜ì„ ì˜ ë°œì„ $R_{n}$ì´ë¼ í•˜ì. ì  $A(-1, 0)$ì— ëŒ€í•˜ì—¬ ì‚¬ê°í˜• $AQ_{n}P_{n}R_{n}$ì˜ ë„“ì´ë¥¼ $S_{n}$, ì‚¼ê°í˜• $AQ_{n}P_{n}$ì˜ ë„“ì´ë¥¼ $T_{n}$ì´ë¼ í•  ë•Œ, $\lim_{n \to \infty} \frac{S_{n} + T_{n}}{S_{n} - T_{n}}$ì˜ ê°’ì€?

> [!example] ğŸ“¸ (ê·¸ë¦¼/ê·¸ë˜í”„)

## ë³´ê¸°
â‘  $1$   â‘¡ $2$   â‘¢ $3$   â‘£ $4$   â‘¤ $5$

## í’€ì´
$\triangle AQ_{n}P_{n} = \frac{1}{2} \overline{AQ_{n}} \times \overline{P_{n}Q_{n}} = \frac{1}{2} (n+1) \sqrt{n+1}$
$\triangle AP_{n}R_{n} = \frac{1}{2} \overline{P_{n}R_{n}} \times \overline{P_{n}Q_{n}} = \frac{1}{2} n \sqrt{n+1}$ ì´ë¯€ë¡œ

$S_{n} = \triangle AQ_{n}P_{n} + \triangle AP_{n}R_{n} = \frac{1}{2} (2n+1) \sqrt{n+1}$
$T_{n} = \frac{1}{2} (n+1) \sqrt{n+1}$

$\therefore \lim_{n \to \infty} \frac{S_{n} + T_{n}}{S_{n} - T_{n}} = \lim_{n \to \infty} \frac{\frac{1}{2} (3n+2) \sqrt{n+1}}{\frac{1}{2} n \sqrt{n+1}} = \lim_{n \to \infty} \left( 3 + \frac{2}{n} \right) = 3$

ì •ë‹µ: â‘¢