## ë¬¸ì œ
ìì—°ìˆ˜ $n$ì— ëŒ€í•˜ì—¬ ì§ì„  $x=n$ì´ ë‘ ê³¡ì„  $y=2^{x}$, $y=3^{x}$ê³¼ ë§Œë‚˜ëŠ” ì ì„ ê°ê° $P_{n}$, $Q_{n}$ì´ë¼ í•˜ì. ì‚¼ê°í˜• $P_{n} Q_{n} P_{n-1}$ì˜ ë„“ì´ë¥¼ $S_{n}$ì´ë¼ í•˜ê³ , $T_{n}= \sum_{k=1}^{n} S_{k}$ë¼ í•  ë•Œ, $\lim_{n \to \infty} \frac{T_{n}}{3^{n}}$ì˜ ê°’ì€? (ë‹¨, ì  $P_{0}$ì˜ ì¢Œí‘œëŠ” $(0,1)$ì´ë‹¤.)



> [!example] ğŸ“¸ (ê·¸ë¦¼/ê·¸ë˜í”„)

## ë³´ê¸°
â‘  $\frac{5}{8}$   â‘¡ $\frac{11}{16}$   â‘¢ $\frac{3}{4}$   â‘£ $\frac{13}{16}$   â‘¤ $\frac{7}{8}$

## í’€ì´
$$ \begin{array}{l} 
\text{ì ì˜ ì¢Œí‘œëŠ” } P_n(n, 2^n), Q_n(n, 3^n), P_{n-1}(n-1, 2^{n-1}) \text{ì´ë‹¤.} \\
\text{ì‚¼ê°í˜• } P_n Q_n P_{n-1} \text{ì˜ ë°‘ë³€ì„ ì„ ë¶„ } P_n Q_n \text{ì´ë¼ í•˜ë©´ ë†’ì´ëŠ” } n - (n-1) = 1 \text{ì´ë¯€ë¡œ} \\
S_n = \frac{1}{2} (3^n - 2^n) \times 1 = \frac{1}{2} (3^n - 2^n) \\
T_n = \sum_{k=1}^{n} S_k = \sum_{k=1}^{n} \frac{1}{2} (3^k - 2^k) \\
T_n = \frac{1}{2} \left( \sum_{k=1}^{n} 3^k - \sum_{k=1}^{n} 2^k \right) \\
T_n = \frac{1}{2} \left( \frac{3(3^n - 1)}{3-1} - \frac{2(2^n - 1)}{2-1} \right) \\
T_n = \frac{3(3^n - 1)}{4} - (2^n - 1) = \frac{3^{n+1}}{4} - 2^n + \frac{1}{4} \\
\lim_{n \to \infty} \frac{T_n}{3^n} = \lim_{n \to \infty} \frac{\frac{3^{n+1}}{4} - 2^n + \frac{1}{4}}{3^n} \\
= \lim_{n \to \infty} \left( \frac{3}{4} - \left( \frac{2}{3} \right)^n + \frac{1}{4 \cdot 3^n} \right) = \frac{3}{4}
\end{array} $$
ì •ë‹µ: â‘¢