## 문제
두 행렬 $A$, $B$에 대하여 
$$ A = \left( \begin{array}{cc} 1 & 2 \\ 0 & 1 \end{array} \right) , A-B = \left( \begin{array}{cc} 1 & 0 \\ 1 & -1 \end{array} \right) $$
일 때, 행렬 $A^{2}-AB$의 모든 성분의 합은?

## 보기
① $1$   ② $2$   ③ $3$   ④ $4$   ⑤ $5$

## 풀이
$A^{2}-AB = A(A-B)$ 이므로 주어진 행렬을 대입하면 다음과 같다.
$$ A^{2}-AB = \left( \begin{array}{cc} 1 & 2 \\ 0 & 1 \end{array} \right) \left( \begin{array}{cc} 1 & 0 \\ 1 & -1 \end{array} \right) = \left( \begin{array}{cc} 3 & -2 \\ 1 & -1 \end{array} \right) $$
따라서 모든 성분의 합은
$$ 3-2+1-1=1 $$
이다.

정답: ①