## 문제
수열 $\{ a_{n} \}$의 첫째항부터 제 $n$항까지의 합 $S_{n}$이 
$$ S_{n} = {}_{n+2}C_{3} \quad (n = 1, 2, 3, \dots) $$
일 때, $\sum_{n=1}^{10} (a_{n+1} - a_{n})$의 값을 구하시오.

## 보기

## 풀이
$S_{n} = {}_{n+2}C_{3} = \frac{(n + 2)(n + 1)n}{6}$이다.

$n = 1$ 일 때, 
$a_{1} = S_{1} = 1$ 이고 

$n \ge 2$ 일 때, 
$a_{n} = S_{n} - S_{n-1}$ 
$= \frac{(n + 2)(n + 1)n}{6} - \frac{(n + 1)n(n - 1)}{6}$ 
$= \frac{n(n + 1)}{2}$ 
이므로 $n \ge 1$ 일 때, $a_{n} = \frac{n(n + 1)}{2}$ 이다. 

$\therefore \sum_{k=1}^{10} ( a_{k+1} - a_{k} )$ 
$= ( a_{2} - a_{1} ) + ( a_{3} - a_{2} ) + \dots + ( a_{11} - a_{10} )$ 
$= a_{11} - a_{1}$ 
$= 66 - 1 = 65$ 

[다른 풀이] 
$\sum_{k=1}^{10} ( a_{k+1} - a_{k} )$ 
$= \sum_{k=1}^{10} a_{k+1} - \sum_{k=1}^{10} a_{k}$ 
$= \sum_{k=1}^{11} a_{k} - \sum_{k=1}^{10} a_{k} - a_{1}$ 
$= S_{11} - S_{10} - S_{1}$ 
$= {}_{13}C_{3} - {}_{12}C_{3} - {}_{3}C_{3}$ 
$= {}_{12}C_{2} - {}_{3}C_{3} = 65$

정답: $65$