## 문제
수열 $\{ a_{n} \}$ 을 $a _{n+1} = n(-1) ^{n} - 3a _{n}$ ($n = 1, 2, 3, \cdots$)으로 정의한다. $a_{1} = a_{2012} + 2$ 일 때, $\sum_{n=1}^{2011} a_{n}$ 의 값은?

## 보기
① $501$   ② $351$   ③ $251$   ④ $-251$   ⑤ $-501$

## 풀이
$a_{n+1} + 3a_{n} = n(-1)^{n}$ 에서 

$\sum_{n=1}^{2011} ( a_{n+1} + 3a_{n} ) = \sum_{n=1}^{2011} a_{n+1} + 3 \sum_{n=1}^{2011} a_{n}$
$= \sum_{n=2}^{2012} a_{n} + 3 \sum_{n=1}^{2011} a_{n}$
$= ( \sum_{n=1}^{2011} a_{n} - a_{1} + a_{2012} ) + 3 \sum_{n=1}^{2011} a_{n}$
$= 4 \sum_{n=1}^{2011} a_{n} + (a_{2012} - a_{1})$
$= 4 \sum_{n=1}^{2011} a_{n} - 2$ ($\because a_{1} = a_{2012} + 2$)

이고 

$\sum_{n=1}^{2011} n(-1)^{n} = -1 + 2 - 3 + 4 - \cdots - 2011$
$= -1 + (2 - 3) + (4 - 5) + \cdots + (2010 - 2011)$
$= (-1) \times 1006$
$= -1006$

$4 \sum_{n=1}^{2011} a_{n} - 2 = -1006$ 에서
$4 \sum_{n=1}^{2011} a_{n} = -1004$
$\sum_{n=1}^{2011} a_{n} = \frac{-1004}{4} = -251$

정답은 ④이다.