## 문제
두 다항식 $A = x^{2} + x y + y^{2}$, $B = - x^{2} + 2 x y$ 에 대하여 $( 3 A + B ) - ( A + 2 B )$ 를 간단히 하면?

## 보기
① $x^{2} + x y$   ② $3 x^{2} + 2 y^{2}$   ③ $x^{2} - 2 x y$   ④ $x^{2} + 2 x y + 2 y^{2}$   ⑤ $- x^{2} + 3 x y + y^{2}$

## 풀이
주어진 식을 정리하면 다음과 같다.
$( 3 A + B ) - ( A + 2 B ) = 3 A + B - A - 2 B = 2 A - B$

여기에 $A = x^{2} + x y + y^{2}$, $B = - x^{2} + 2 x y$를 대입하면
$2 A - B = 2 ( x^{2} + x y + y^{2} ) - ( - x^{2} + 2 x y )$
$= 2 x^{2} + 2 x y + 2 y^{2} + x^{2} - 2 x y$
$= 3 x^{2} + 2 y^{2}$

정답: ②