## 문제
자연수 $n$ 에 대하여 
$a_{n} = \sqrt{4 n + 1 - 2 \sqrt{4 n^{2} + 2 n}}$, 
$b_{n} = \sqrt{2 n + 1 - 2 \sqrt{n^{2} + n}}$
이라 할 때, $\lim_{n \to \infty} \frac{a_{n}}{b_{n}}$ 의 값은?

## 보기
① $-\frac{\sqrt{2}}{2}$   ② $-\frac{\sqrt{2}}{4}$   ③ $1$   ④ $\frac{\sqrt{2}}{4}$   ⑤ $\frac{\sqrt{2}}{2}$

## 풀이
$a_{n} = \sqrt{(2 n + 1) + 2 n - 2 \sqrt{2 n (2 n + 1)}}$
$= \sqrt{(\sqrt{2 n + 1} - \sqrt{2 n})^{2}}$
$= \sqrt{2 n + 1} - \sqrt{2 n}$

$b_{n} = \sqrt{(n + 1) + n - 2 \sqrt{n (n + 1)}}$
$= \sqrt{(\sqrt{n + 1} - \sqrt{n})^{2}}$
$= \sqrt{n + 1} - \sqrt{n}$

$\lim_{n \to \infty} \frac{a_{n}}{b_{n}} = \lim_{n \to \infty} \frac{\sqrt{2 n + 1} - \sqrt{2 n}}{\sqrt{n + 1} - \sqrt{n}}$
$= \lim_{n \to \infty} \frac{(\sqrt{2 n + 1} - \sqrt{2 n})(\sqrt{2 n + 1} + \sqrt{2 n})(\sqrt{n + 1} + \sqrt{n})}{(\sqrt{n + 1} - \sqrt{n})(\sqrt{n + 1} + \sqrt{n})(\sqrt{2 n + 1} + \sqrt{2 n})}$
$= \lim_{n \to \infty} \frac{\sqrt{n + 1} + \sqrt{n}}{\sqrt{2 n + 1} + \sqrt{2 n}}$
$= \lim_{n \to \infty} \frac{\sqrt{1 + \frac{1}{n}} + 1}{\sqrt{2 + \frac{1}{n}} + \sqrt{2}}$
$= \frac{2}{2 \sqrt{2}} = \frac{\sqrt{2}}{2}$

정답 ⑤