## ë¬¸ì œ
ì‚¼ì°¨í•¨ìˆ˜ $y=f(x)$ ì˜ ê·¸ë˜í”„ê°€ ê·¸ë¦¼ê³¼ ê°™ë‹¤. ë‘ ì§‘í•© $A = \{ x \mid \frac{x}{f(x-2)} \leq 0 \}$, $B = \{ x \mid \frac{x-4}{x+4} < 0 \}$ ì— ëŒ€í•˜ì—¬ ì§‘í•© $A \cap B$ ì— ì†í•˜ëŠ” ì •ìˆ˜ì˜ ê°œìˆ˜ëŠ”?

> [!example] ğŸ“¸ (ê·¸ë¦¼/ê·¸ë˜í”„)

(ë‹¨, $f(-4)=f(-1)=f(3)=0$)

## ë³´ê¸°
â‘  $2$   â‘¡ $3$   â‘¢ $4$   â‘£ $5$   â‘¤ $6$

## í’€ì´
ë¶€ë“±ì‹ $\frac{x}{f(x-2)} \leq 0$ ì˜ í•´ë¥¼ êµ¬í•˜ë©´,
$x f(x-2) \leq 0$, $f(x-2) \neq 0$
(â…°) $x \leq 0$, $f(x-2) > 0$ ì¼ ë•Œ,
$\therefore -2 < x \leq 0$
(â…±) $x \geq 0$, $f(x-2) < 0$ ì¼ ë•Œ,
$\therefore 1 < x < 5$
(â…°), (â…±)ì— ì˜í•˜ì—¬
$A = \{ x \mid -2 < x \leq 0 \text{ ë˜ëŠ” } 1 < x < 5 \}$
ë¶€ë“±ì‹ $\frac{x-4}{x+4} < 0$ ì˜ í•´ë¥¼ êµ¬í•˜ë©´,
$(x-4)(x+4) < 0$
$\therefore -4 < x < 4$
$B = \{ x \mid -4 < x < 4 \}$
ë”°ë¼ì„œ $A \cap B = \{ x \mid -2 < x \leq 0 \text{ ë˜ëŠ” } 1 < x < 4 \}$ ì— ì†í•˜ëŠ” ì •ìˆ˜ì˜ ê°œìˆ˜ëŠ” $4$ ì´ë‹¤.

ì •ë‹µ: â‘¢