## 문제
행렬 $A = \left( \begin{array}{cc} a & a+1 \\ a-1 & a \end{array} \right)$ 에 대하여 행렬 $A^{2} + (A^{-1})^{2}$ 의 모든 성분의 합이 $124$ 일 때, $a^{2}$ 의 값을 구하시오.

## 풀이
행렬 $A = \left( \begin{array}{cc} a & a+1 \\ a-1 & a \end{array} \right)$ 에서 역행렬 $A^{-1}$ 을 구하면
$$ A^{-1} = \left( \begin{array}{cc} a & -a-1 \\ -a+1 & a \end{array} \right) $$
이므로
$$ A + A^{-1} = \left( \begin{array}{cc} a & a+1 \\ a-1 & a \end{array} \right) + \left( \begin{array}{cc} a & -a-1 \\ -a+1 & a \end{array} \right) = \left( \begin{array}{cc} 2a & 0 \\ 0 & 2a \end{array} \right) = 2aE $$
이다. 양변을 제곱하여 정리하면
$$ (A + A^{-1})^{2} = A^{2} + 2E + (A^{-1})^{2} = (2aE)^{2} = 4a^{2}E $$
$$ A^{2} + (A^{-1})^{2} = 4a^{2}E - 2E = (4a^{2} - 2)E $$
행렬 $A^{2} + (A^{-1})^{2}$ 의 모든 성분의 합이 $124$ 이므로
$$ 2(4a^{2} - 2) = 124 $$
$$ 4a^{2} - 2 = 62 $$
$$ 4a^{2} = 64 $$
$$ \therefore a^{2} = 16 $$
따라서 정답은 $16$ 이다.