## ë¬¸ì œ
ì§‘í•© $X = \{ 1, 2, 3, 4 \}$ ì— ëŒ€í•˜ì—¬ $X$ ì—ì„œ $X$ ë¡œì˜ ë‘ í•¨ìˆ˜ $f$ ì™€ $g$ ê°€ ê·¸ë¦¼ê³¼ ê°™ì„ ë•Œ, $(f \circ g^{-1} )(1) + (g \circ f)^{-1}(4)$ ì˜ ê°’ì€?

> [!example] ğŸ“¸ (ê·¸ë¦¼/ê·¸ë˜í”„)

## ë³´ê¸°
â‘  $4$   â‘¡ $5$   â‘¢ $6$   â‘£ $7$   â‘¤ $8$

## í’€ì´
$(f \circ g^{-1} )(1)$
$= f (g^{-1}(1) )$
$= f(2) = 3$

$(g \circ f)^{-1}(4) = (f^{-1} \circ g^{-1} )(4)$
$= f^{-1} (g^{-1}(4) )$
$= f^{-1}(3) = 2$

ë”°ë¼ì„œ
$(f \circ g^{-1} )(1) + (g \circ f)^{-1}(4) = 3 + 2 = 5$

[ì •ë‹µ] â‘¡