## ë¬¸ì œ
ë¬´ë¦¬í•¨ìˆ˜ $f(x) = \sqrt{x+1}$ê³¼ ìì—°ìˆ˜ $n$ì— ëŒ€í•˜ì—¬ ê·¸ë¦¼ê³¼ ê°™ì´ $y=f(x)$ì˜ ê·¸ë˜í”„ ìœ„ì˜ í•œ ì  $P_n(n, f(n))$ì—ì„œ $x$ì¶•ì— ë‚´ë¦° ìˆ˜ì„ ì˜ ë°œì„ $Q_n$, $y$ì¶•ì— ë‚´ë¦° ìˆ˜ì„ ì˜ ë°œì„ $R_n$ì´ë¼ í•˜ì. ì  $A(-1, 0)$ì— ëŒ€í•˜ì—¬ ì‚¬ê°í˜• $AQ_n P_n R_n$ì˜ ë„“ì´ë¥¼ $S_n$, ì‚¼ê°í˜• $AQ_n P_n$ì˜ ë„“ì´ë¥¼ $T_n$ì´ë¼ í•  ë•Œ, $\lim_{n \to \infty} \frac{S_n + T_n}{S_n - T_n}$ì˜ ê°’ì€?

> [!example] ğŸ“¸ (ê·¸ë¦¼/ê·¸ë˜í”„)

## ë³´ê¸°
â‘  $1$   â‘¡ $2$   â‘¢ $3$   â‘£ $4$   â‘¤ $5$

## í’€ì´
$\triangle AQ_n P_n$
$= \frac{1}{2} \overline{AQ_n} \times \overline{P_n Q_n}$
$= \frac{1}{2} (n+1) \sqrt{n+1}$

$\triangle AP_n R_n$
$= \frac{1}{2} \overline{P_n R_n} \times \overline{P_n Q_n}$
$= \frac{1}{2} n \sqrt{n+1}$ ì´ë¯€ë¡œ

$S_n$
$= \triangle AQ_n P_n + \triangle AP_n R_n$
$= \frac{1}{2} (2n+1) \sqrt{n+1}$

$T_n$
$= \frac{1}{2} (n+1) \sqrt{n+1}$

$\therefore \lim_{n \to \infty} \frac{S_n + T_n}{S_n - T_n}$
$= \lim_{n \to \infty} \frac{\frac{1}{2} (3n+2) \sqrt{n+1}}{\frac{1}{2} n \sqrt{n+1}}$
$= \lim_{n \to \infty} \left( 3 + \frac{2}{n} \right)$
$= 3$

ì •ë‹µ: â‘¢