## 문제
자연수 $n$ 에 대하여 
$a_{n}= \sqrt{4 n+1-2 \sqrt{4 n^{2}+2 n}}$, 
$b_{n}= \sqrt{2 n+1-2 \sqrt{n^{2}+n}}$
이라 할 때, $\lim_{n \rightarrow \infty} \frac{a_{n}}{b_{n}}$ 의 값은?

## 보기
① $-\frac{\sqrt{2}}{2}$   ② $-\frac{\sqrt{2}}{4}$   ③ $1$   ④ $\frac{\sqrt{2}}{4}$   ⑤ $\frac{\sqrt{2}}{2}$

## 풀이
[정답] ⑤

$a_{n}$
$= \sqrt{(2n+1)+2n-2 \sqrt{2n(2n+1)}}$
$= \sqrt{(\sqrt{2n+1}-\sqrt{2n})^{2}}$
$= \sqrt{2n+1}-\sqrt{2n}$

$b_{n}$
$= \sqrt{(n+1)+n-2 \sqrt{n(n+1)}}$
$= \sqrt{(\sqrt{n+1}-\sqrt{n})^{2}}$
$= \sqrt{n+1}-\sqrt{n}$

$\lim_{n \rightarrow \infty} \frac{a_{n}}{b_{n}}$
$= \lim_{n \rightarrow \infty} \frac{\sqrt{2n+1}-\sqrt{2n}}{\sqrt{n+1}-\sqrt{n}}$
$= \lim_{n \rightarrow \infty} \frac{(\sqrt{2n+1}-\sqrt{2n})(\sqrt{2n+1}+\sqrt{2n})(\sqrt{n+1}+\sqrt{n})}{(\sqrt{n+1}-\sqrt{n})(\sqrt{n+1}+\sqrt{n})(\sqrt{2n+1}+\sqrt{2n})}$
$= \lim_{n \rightarrow \infty} \frac{\sqrt{n+1}+\sqrt{n}}{\sqrt{2n+1}+\sqrt{2n}}$
$= \lim_{n \rightarrow \infty} \frac{\sqrt{1+\frac{1}{n}}+ 1}{\sqrt{2+\frac{1}{n}}+\sqrt{2}}$
$= \frac{2}{2 \sqrt{2}} = \frac{\sqrt{2}}{2}$