## ë¬¸ì œ
í•¨ìˆ˜ $f(x) = \sin \pi x$ ($x \ge 0$)ì˜ ê·¸ë˜í”„ì™€ ì§ì„  $y = \frac{2}{3}$ê°€ ë§Œë‚˜ëŠ” ì ì˜ $x$ ì¢Œí‘œë¥¼ ì‘ì€ ê²ƒë¶€í„° ì°¨ë¡€ëŒ€ë¡œ $\alpha$, $\beta$, $\gamma$ë¼ í•  ë•Œ, $f(\alpha + \beta + \gamma + 1) + f(\alpha + \beta + \frac{1}{2})$ì˜ ê°’ì€?

> [!example] ğŸ“¸ (ê·¸ë¦¼/ê·¸ë˜í”„)

## ë³´ê¸°
â‘  $-\frac{2}{3}$   â‘¡ $-\frac{1}{3}$   â‘¢ $0$   â‘£ $\frac{1}{3}$   â‘¤ $\frac{2}{3}$

## í’€ì´
í•¨ìˆ˜ $f(x) = \sin \pi x$ ($x \ge 0$)ì˜ ì£¼ê¸°ê°€ $\frac{2\pi}{\pi} = 2$ì´ë¯€ë¡œ ê·¸ë¦¼ì—ì„œ
$\beta = 1 - \alpha$, $\gamma = 2 + \alpha$ì´ë‹¤.

$f(\alpha + \beta + \gamma + 1) = f(\alpha + (1 - \alpha) + (2 + \alpha) + 1) = f(4 + \alpha)$
í•¨ìˆ˜ì˜ ì£¼ê¸°ê°€ $2$ì´ë¯€ë¡œ
$f(4 + \alpha) = f(\alpha) = \frac{2}{3}$

ë˜í•œ,
$f(\alpha + \beta + \frac{1}{2}) = f(\alpha + (1 - \alpha) + \frac{1}{2}) = f(\frac{3}{2})$
$f(\frac{3}{2}) = \sin (\frac{3}{2}\pi) = -1$

$\therefore f(\alpha + \beta + \gamma + 1) + f(\alpha + \beta + \frac{1}{2}) = \frac{2}{3} + (-1) = -\frac{1}{3}$

ì •ë‹µ: â‘¡