## 문제
두 행렬 $A$, $B$에 대하여
$$ A+B= \left( \begin{array}{cc} -3 & 4 \\ 2 & 3 \end{array} \right) $$, $$ A-2B= \left( \begin{array}{cc} -2 & 3 \\ 1 & 4 \end{array} \right) $$
일 때, 행렬 $A-B$의 모든 성분의 합은?

## 보기
① $5$   ② $6$   ③ $7$   ④ $8$   ⑤ $9$

## 풀이
$$ A+B= \left( \begin{array}{cc} -3 & 4 \\ 2 & 3 \end{array} \right) $$ $\cdots$ ㉠
$$ A-2B= \left( \begin{array}{cc} -2 & 3 \\ 1 & 4 \end{array} \right) $$ $\cdots$ ㉡

㉠ $-$ ㉡에서
$$ 3B= \left( \begin{array}{cc} -1 & 1 \\ 1 & -1 \end{array} \right) $$ 이므로
$$ B = \frac{1}{3} \left( \begin{array}{cc} -1 & 1 \\ 1 & -1 \end{array} \right) $$

㉠에서 $$ A = \left( \begin{array}{cc} -3 & 4 \\ 2 & 3 \end{array} \right) - B $$ 이므로
$$ A = \left( \begin{array}{cc} -3 & 4 \\ 2 & 3 \end{array} \right) - \frac{1}{3} \left( \begin{array}{cc} -1 & 1 \\ 1 & -1 \end{array} \right) $$
$$ A = \frac{1}{3} \left( \begin{array}{cc} -8 & 11 \\ 5 & 10 \end{array} \right) $$

따라서 $$ A-B = \frac{1}{3} \left( \begin{array}{cc} -7 & 10 \\ 4 & 11 \end{array} \right) $$ 에서 모든 성분의 합은
$$ \frac{1}{3} (-7 + 10 + 4 + 11) = \frac{18}{3} = 6 $$ 이다.

**[다른풀이]**
㉠ $+$ ㉡ $\times 2$ 에서
$$ (A+B) + 2(A-2B) = 3A-3B $$
$$ 3A-3B = \left( \begin{array}{cc} -3 & 4 \\ 2 & 3 \end{array} \right) + 2 \left( \begin{array}{cc} -2 & 3 \\ 1 & 4 \end{array} \right) = \left( \begin{array}{cc} -7 & 10 \\ 4 & 11 \end{array} \right) $$
이므로
$$ A-B = \frac{1}{3} \left( \begin{array}{cc} -7 & 10 \\ 4 & 11 \end{array} \right) $$
모든 성분의 합은 $6$ 이다.

정답: ②