## 문제
수열 $\{ a_{n} \}$ 이 $a_{1} = 1$, $a_{n+1} = 2a_{n} + 1$ ($n = 1, 2, 3, \dots$) 을 만족할 때, $\sum_{n=1}^{\infty} \frac{1}{\log_{2}(a_{n} + 1) \log_{2}(a_{n+1} + 1)}$ 의 값은?

## 보기
① $\frac{1}{5}$   ② $\frac{1}{4}$   ③ $\frac{1}{3}$   ④ $\frac{1}{2}$   ⑤ $1$

## 풀이
$a_{n+1} + 1 = 2(a_{n} + 1)$ 이고 $a_{1} + 1 = 2$ 이므로 수열 $\{ a_{n} + 1 \}$ 은 첫째항이 $2$, 공비가 $2$ 인 등비수열이다.
따라서 $a_{n} + 1 = 2 \cdot 2^{n-1} = 2^{n}$ 이므로 $a_{n} = 2^{n} - 1$ 이다.
준식에 대입하면
$$ \sum_{n=1}^{\infty} \frac{1}{\log_{2} 2^{n} \log_{2} 2^{n+1}} = \sum_{n=1}^{\infty} \frac{1}{n(n+1)} $$
$$ = \lim_{n \to \infty} \sum_{k=1}^{n} \left( \frac{1}{k} - \frac{1}{k+1} \right) $$
$$ = \lim_{n \to \infty} \left( 1 - \frac{1}{n+1} \right) = 1 $$
정답은 ⑤이다.