## 문제
함수 $f(x)$를
$$ f(x) = \begin{cases} -x(x-1) & (0 \le x < 1) \\ -\frac{1}{4^n}(x-n)(x-n-1) & (n \le x < n+1) \end{cases} $$
($n=1, 2, 3, \dots$)이라 정의하자. $S_n = \int_0^{n+1} f(x) dx$라 할 때, $\lim_{n \to \infty} S_n$의 값은?

## 보기
① $\frac{1}{9}$   ② $\frac{2}{9}$   ③ $\frac{1}{3}$   ④ $\frac{2}{3}$   ⑤ $\frac{5}{9}$

## 풀이
정답: ②

$-\frac{1}{4^n}(x-n)(x-n-1)$에 $n=0$을 대입하면 $-x(x-1)$이므로 음이 아닌 정수 $n$에 대하여
$f(x) = -\frac{1}{4^n}(x-n)(x-n-1)$ ($n \le x < n+1$)이다. 

이때, $a_n = \int_n^{n+1} f(x) dx$이라 하면
$$ \begin{aligned} S_n &= \int_0^{n+1} f(x) dx \\ &= \int_0^1 f(x) dx + \int_1^2 f(x) dx + \cdots + \int_n^{n+1} f(x) dx \\ &= a_0 + a_1 + \cdots + a_n \\ &= \sum_{i=0}^n a_i \end{aligned} $$
그런데
$$ \begin{aligned} a_n &= \int_n^{n+1} \left\{ -\frac{1}{4^n}(x-n)(x-n-1) \right\} dx \\ &= \frac{1}{6} \cdot \frac{1}{4^n} \end{aligned} $$
∴ $\left( \int_{\alpha}^{\beta} a(x-\alpha)(x-\beta) dx = -\frac{a}{6}(\beta-\alpha)^3 \right)$ 이므로
$$ \begin{aligned} \lim_{n \to \infty} S_n &= \sum_{n=0}^{\infty} a_n \\ &= \sum_{n=0}^{\infty} \frac{1}{6} \cdot \frac{1}{4^n} \\ &= \frac{\frac{1}{6}}{1 - \frac{1}{4}} \\ &= \frac{2}{9} \end{aligned} $$