## 문제
열린구간 ($0$, $2$)에서 미분가능한 함수 $f(x)$가
$$ f(x) = \begin{cases} 4x-3 & (0 \le x < 1) \\ ax^{2}+bx & (1 \le x \le 2) \end{cases} $$
(단, $a$, $b$는 상수)일 때, $\lim_{n \to \infty} \frac{1}{n} \sum_{k=1}^{n} f \left( \frac{2k}{n} \right)$의 값은?

## 보기
① $-\frac{3}{2}$   ② $1$   ③ $\frac{3}{2}$   ④ $\frac{7}{3}$   ⑤ $6$

## 풀이
$g_{1}(x)=4x-3$, $g_{2}(x)=ax^{2}+bx$라 하면 
$f(x)$가 열린구간 ($0$, $2$)에서 미분 가능하므로 $g_{1}(1)=g_{2}(1)$이고 $g_{1}'(1)=g_{2}'(1)$이다. 

따라서 $a+b=1$, $4=2a+b$에서 
$a=3$, $b=-2$ 

$\therefore g_{2}(x)=3x^{2}-2x$ 

$$ \begin{array}{l} \lim_{n \to \infty} \frac{1}{n} \sum_{k=1}^{n} f \left( \frac{2k}{n} \right) \\ = \frac{1}{2} \lim_{n \to \infty} \frac{2}{n} \sum_{k=1}^{n} f \left( \frac{2k}{n} \right) \\ = \frac{1}{2} \int_{0}^{2} f(x) dx \\ = \frac{1}{2} \left( \int_{0}^{1} f(x) dx + \int_{1}^{2} f(x) dx \right) \\ = \frac{1}{2} \left( \int_{0}^{1} (4x-3) dx + \int_{1}^{2} (3x^{2}-2x) dx \right) \\ = \frac{1}{2} \left( [2x^{2}-3x]_{0}^{1} + [x^{3}-x^{2}]_{1}^{2} \right) \\ = \frac{3}{2} \end{array} $$

정답: ③