## 문제
두 행렬 $A$, $B$에 대하여 
$A+B = \left( \begin{array}{cc} 2 & 2 \\ 3 & 1 \end{array} \right)$, $B = \left( \begin{array}{cc} 0 & 1 \\ 3 & 2 \end{array} \right)$ 
일 때, 행렬 $AB+B^{2}$은?

## 보기
① $\left( \begin{array}{cc} 3 & 5 \\ 6 & 6 \end{array} \right)$   ② $\left( \begin{array}{cc} 3 & 1 \\ 12 & 8 \end{array} \right)$   ③ $\left( \begin{array}{cc} 6 & 6 \\ 3 & 5 \end{array} \right)$   ④ $\left( \begin{array}{cc} 6 & 8 \\ 3 & 1 \end{array} \right)$   ⑤ $\left( \begin{array}{cc} 12 & 8 \\ 3 & 1 \end{array} \right)$

## 풀이
[정답] ③ 

[해설] 
$$ AB+B^{2} = (A+B)B = \left( \begin{array}{cc} 2 & 2 \\ 3 & 1 \end{array} \right) \left( \begin{array}{cc} 0 & 1 \\ 3 & 2 \end{array} \right) = \left( \begin{array}{cc} 6 & 6 \\ 3 & 5 \end{array} \right) $$ 
두 행렬 $A$, $B$에 대하여 
$A+B = \left( \begin{array}{cc} 2 & 2 \\ 3 & 1 \end{array} \right)$, $B = \left( \begin{array}{cc} 0 & 1 \\ 3 & 2 \end{array} \right)$ 일 때,
$$ AB+B^{2} = (A+B)B $$
$$ = \left( \begin{array}{cc} 2 \times 0 + 2 \times 3 & 2 \times 1 + 2 \times 2 \\ 3 \times 0 + 1 \times 3 & 3 \times 1 + 1 \times 2 \end{array} \right) $$
$$ = \left( \begin{array}{cc} 6 & 6 \\ 3 & 5 \end{array} \right) $$