## 문제
자연수 $n$에 대하여 집합 $A_{n}$, $B_{n}$을
$$ A_{n} = \{ (n, k) | k \leq n^{2} + n, k \text{는 자연수} \} $$
$$ B_{n} = \{ (n, k) | k \leq \frac{1}{2} n + 5, k \text{는 자연수} \} $$
라 하자. 집합 $A_{n} - B_{n}$의 원소의 개수를 $a_{n}$이라 할 때, $\sum_{n=1}^{20} a_{n}$의 값은?

## 보기
① $2883$   ② $2886$   ③ $2889$   ④ $2892$   ⑤ $2895$

## 풀이
[정답] ① 

$n^{2} + n \leq \frac{1}{2} n + 5$에서 
$2 n^{2} + n - 10 = (2 n + 5) (n - 2) \leq 0$ 
따라서 $n \leq 2$일 때, $n^{2} + n \leq \frac{1}{2} n + 5$가 성립한다. 
따라서 $A_{n} \subset B_{n} (n = 1, 2)$이고 $B_{n} \subset A_{n} (n = 3, 4, \cdots)$이다. 
따라서 $A_{n} - B_{n} = \emptyset (n = 1, 2)$이므로 $a_{n} = 0$이고 
$n \geq 3$일 때, $a_{n} = n (A_{n}) - n (B_{n}) = n^{2} + n - \left[ \frac{1}{2} n + 5 \right]$이다. 
그런데 $n$이 짝수일 때, $\left[ \frac{1}{2} n + 5 \right] = \frac{1}{2} n + 5$ 
$n$이 홀수일 때, $\left[ \frac{1}{2} n + 5 \right] = \frac{1}{2} n + 5 - \frac{1}{2}$이므로 

$\sum_{n=1}^{20} a_{n} = \sum_{n=3}^{20} (n^{2} + n - \left[ \frac{1}{2} n + 5 \right])$ 
$= \sum_{n=3}^{20} (n^{2} + n) - \sum_{n=3}^{20} ( \left[ \frac{1}{2} n + 5 \right] )$ 
이때, $\sum_{k=1}^{n} (k^{2} + k) = \frac{1}{3} n (n + 1) (n + 2)$이므로 

$\sum_{n=3}^{20} (n^{2} + n) = \sum_{n=1}^{20} (n^{2} + n) - \sum_{n=1}^{2} (n^{2} + n)$ 
$= \frac{1}{3} (20 \cdot 21 \cdot 22 - 2 \cdot 3 \cdot 4)$ 
$= \frac{1}{3} (9240 - 24) = 3072$ 
이고 

$\sum_{n=3}^{20} ( \left[ \frac{1}{2} n + 5 \right] ) = \sum_{n=3}^{20} ( \frac{1}{2} n + 5 ) - 9 \cdot \frac{1}{2}$ 
($\because 3 \sim 20$까지 자연수 중 홀수는 $9$개) 
$= ( \sum_{n=1}^{20} \frac{1}{2} n - \sum_{n=1}^{2} \frac{1}{2} n ) + 18 \times 5 - 9 \cdot \frac{1}{2}$ 
$= (105 - \frac{3}{2}) + 90 - \frac{9}{2} = 189$ 
이므로 
$\sum_{n=1}^{20} a_{n} = 3072 - 189 = 2883$