## 문제
다항식 $f(x)=x^{3}+9x^{2}+4x-45$에 대하여 등식 $f(x+a)=x^{3}+bx-3$이 $x$의 값에 관계없이 항상 성립한다. 이때, 두 상수 $a$, $b$의 합 $a+b$의 값은?

## 보기
① $-26$   ② $-24$   ③ $-22$   ④ $-20$   ⑤ $-18$

## 풀이
$$f(x+a)=(x+a)^{3}+9(x+a)^{2}+4(x+a)-45$$ 
$$= (x^{3}+3ax^{2}+3a^{2}x+a^{3})+9(x^{2}+2ax+a^{2})+4(x+a)-45$$ 
$$=x^{3}+3ax^{2}+3a^{2}x+a^{3}+9x^{2}+18ax+9a^{2}+4x+4a-45$$ 
$$=x^{3}+(3a+9)x^{2}+(3a^{2}+18a+4)x+a^{3}+9a^{2}+4a-45$$ 
주어진 조건에서 이차항의 계수가 $0$이므로 
$3a+9=0$에서 $a=-3$이다. 
$x^{3}+(3a+9)x^{2}+(3a^{2}+18a+4)x+a^{3}+9a^{2}+4a-45$에 $a=-3$을 대입하여 정리하면 
$x^{3}+(-9+9)x^{2}+(27-54+4)x-27+81-12-45 = x^{3}-23x-3$ 
따라서 $b=-23$이므로 $a+b=-26$

[다른풀이] 
$f(x+a)=x^{3}+bx-3$이고 $a=-3$이므로 
$f(x-3)=x^{3}+bx-3$ 
$x=3$을 대입하면 $f(0)=3^{3}+3b-3$ 
$f(x)=x^{3}+9x^{2}+4x-45$에 $x=0$을 대입하면 
$f(0)=-45$이다. 
그러므로 $24+3b=-45$에서 $b=-23$ 
따라서 $a+b=-26$이다.

정답: ①