## 문제
두 행렬 $A$, $B$에 대하여 
$$ A+B= \left( \begin{array}{cc} -3 & 4 \\ 2 & 3 \end{array} \right) $$, $$ A-2 B= \left( \begin{array}{cc} -2 & 3 \\ 1 & 4 \end{array} \right) $$
일 때, 행렬 $A-B$의 모든 성분의 합은?

## 보기
① $5$   ② $6$   ③ $7$   ④ $8$   ⑤ $9$

## 풀이
[정답] ② 

[해설] 
$$ A+B= \left( \begin{array}{cc} -3 & 4 \\ 2 & 3 \end{array} \right) \cdots \cdots $$ ㉠ 

$$ A-2 B= \left( \begin{array}{cc} -2 & 3 \\ 1 & 4 \end{array} \right) \cdots \cdots $$ ㉡ 

㉠ $-$ ㉡에서 
$$ 3 B= \left( \begin{array}{cc} -1 & 1 \\ 1 & -1 \end{array} \right) $$ 이므로 
$$ B=\frac{1}{3} \left( \begin{array}{cc} -1 & 1 \\ 1 & -1 \end{array} \right) $$ 

㉠에서 
$$ A= \left( \begin{array}{cc} -3 & 4 \\ 2 & 3 \end{array} \right) -B $$ 이므로 
$$ A = \left( \begin{array}{cc} -3 & 4 \\ 2 & 3 \end{array} \right) - \frac{1}{3} \left( \begin{array}{cc} -1 & 1 \\ 1 & -1 \end{array} \right) $$ 
$$ = \frac{1}{3} \left( \begin{array}{cc} -8 & 11 \\ 5 & 10 \end{array} \right) $$ 

따라서 
$$ A-B=\frac{1}{3} \left( \begin{array}{cc} -7 & 10 \\ 4 & 11 \end{array} \right) $$ 에서 모든 성분의 합은 $6$ 이다. 

[다른풀이] 
㉠ $+$ ㉡ $\times 2$ 에서 
$$ 3 A-3 B= \left( \begin{array}{cc} -7 & 10 \\ 4 & 11 \end{array} \right) $$ 
이므로 
$$ A-B=\frac{1}{3} \left( \begin{array}{cc} -7 & 10 \\ 4 & 11 \end{array} \right) $$ 에서 모든 성분의 합은 $6$ 이다.