## ë¬¸ì œ
$n$ì°¨ ì •ì‚¬ê°í–‰ë ¬ $A$ì˜ $(i, j)$ ì„±ë¶„ $a_{i, j}$ë¥¼ $a_{i, j}=(i-1) n+j$ (ë‹¨, $1 \leq i \leq n, 1 \leq j \leq n$)ì´ë¼ í•˜ì. $n$ ì´í•˜ì˜ ìì—°ìˆ˜ $k$ì— ëŒ€í•˜ì—¬ $f(k)$ë¥¼ í–‰ë ¬ $A$ì˜ $(k, n-k+1)$ ì„±ë¶„ì´ë¼ í•  ë•Œ, $12 \lim _{n \to \infty} \frac{\sum_{k=1}^{n} f(k)}{n^{3}}$ì˜ ê°’ì„ êµ¬í•˜ì‹œì˜¤. (ë‹¨, $n$ì€ ìì—°ìˆ˜ì´ë‹¤.)



> [!example] ğŸ“¸ (ê·¸ë¦¼/ê·¸ë˜í”„)

## ë³´ê¸°

## í’€ì´
$f(k) = (k-1) n+n-k+1 = (n-1) k+1$ì´ë¯€ë¡œ 
$$ \sum_{k=1}^{n} f(k) = \sum_{k=1}^{n} \{(n-1) k+1\} $$ 
$$ = (n-1) \frac{n(n+1)}{2}+n $$ 
$$ = \frac{1}{2} n (n^{2}+1) $$ 
$$ 12 \lim _{n \to \infty} \frac{\sum_{k=1}^{n} f(k)}{n^{3}} = \lim _{n \to \infty} \frac{6 n (n^{2}+1)}{n^{3}}=6 $$
ì •ë‹µ: $6$