## 문제
함수 $f(x) = \lim_{n \to \infty} \frac{(x^2 + \frac{1}{2})^n - 2}{(x^2 + \frac{1}{2})^n + 2}$ 에 대하여 $f(\frac{\sqrt{2}}{2}) + \lim_{x \to \frac{\sqrt{2}}{2}-} f(x)$ 의 값은?

## 보기
① $-\frac{4}{3}$   ② $-1$   ③ $0$   ④ $1$   ⑤ $\frac{4}{3}$

## 풀이
$f(x) = \lim_{n \to \infty} \frac{(x^2 + \frac{1}{2})^n - 2}{(x^2 + \frac{1}{2})^n + 2}$ 에서 공비 역할을 하는 $x^2 + \frac{1}{2}$ 의 범위에 따라 함수의 값을 나누면 다음과 같다.

$$ f(x) = \left\{ \begin{array}{ll} -1 & (|x| < \frac{\sqrt{2}}{2}) \\ -\frac{1}{3} & (|x| = \frac{\sqrt{2}}{2}) \\ 1 & (|x| > \frac{\sqrt{2}}{2}) \end{array} \right. $$

따라서 구하고자 하는 값은
$f(\frac{\sqrt{2}}{2}) = -\frac{1}{3}$
$\lim_{x \to \frac{\sqrt{2}}{2}-} f(x) = -1$ (단, $|x| < \frac{\sqrt{2}}{2}$ 인 범위에서 접근)

이므로
$f(\frac{\sqrt{2}}{2}) + \lim_{x \to \frac{\sqrt{2}}{2}-} f(x) = -\frac{1}{3} + (-1) = -\frac{4}{3}$

정답: ①