## 문제
세 행렬 $A = \left( \begin{array}{rr} 4 & 3 \\ -2 & 1 \end{array} \right)$, $B = \left( \begin{array}{rr} 1 & 2 \\ 6 & 0 \end{array} \right)$, $C = \left( \begin{array}{rr} 2 & 0 \\ -7 & 3 \end{array} \right)$에 대하여 행렬 $A(B+C)$는?

## 보기
① $\left( \begin{array}{rr} -9 & -17 \\ 7 & 1 \end{array} \right)$   ② $\left( \begin{array}{rr} -9 & 17 \\ -7 & 1 \end{array} \right)$   ③ $\left( \begin{array}{rr} -9 & 17 \\ 7 & -1 \end{array} \right)$   ④ $\left( \begin{array}{rr} 9 & 17 \\ 7 & 1 \end{array} \right)$   ⑤ $\left( \begin{array}{rr} 9 & 17 \\ -7 & -1 \end{array} \right)$

## 풀이
$$A(B+C)$$ 
$$= \left( \begin{array}{rr} 4 & 3 \\ -2 & 1 \end{array} \right) \left\{ \left( \begin{array}{rr} 1 & 2 \\ 6 & 0 \end{array} \right) + \left( \begin{array}{rr} 2 & 0 \\ -7 & 3 \end{array} \right) \right\}$$ 
$$= \left( \begin{array}{rr} 4 & 3 \\ -2 & 1 \end{array} \right) \left( \begin{array}{rr} 3 & 2 \\ -1 & 3 \end{array} \right) = \left( \begin{array}{rr} 9 & 17 \\ -7 & -1 \end{array} \right)$$ 

[다른 풀이] 
행렬의 연산에 대한 분배법칙을 적용하면 
$$A(B+C) = AB + AC$$ 
$$AB = \left( \begin{array}{rr} 4 & 3 \\ -2 & 1 \end{array} \right) \left( \begin{array}{rr} 1 & 2 \\ 6 & 0 \end{array} \right) = \left( \begin{array}{rr} 22 & 8 \\ 4 & -4 \end{array} \right)$$ 
$$AC = \left( \begin{array}{rr} 4 & 3 \\ -2 & 1 \end{array} \right) \left( \begin{array}{rr} 2 & 0 \\ -7 & 3 \end{array} \right) = \left( \begin{array}{rr} -13 & 9 \\ -11 & 3 \end{array} \right)$$ 
$$\therefore A B + A C = \left( \begin{array}{rr} 22 & 8 \\ 4 & -4 \end{array} \right) + \left( \begin{array}{rr} -13 & 9 \\ -11 & 3 \end{array} \right) = \left( \begin{array}{rr} 9 & 17 \\ -7 & -1 \end{array} \right)$$

정답: ⑤