## ๋ฌธ์
์ค์ $x$์ ๋ํ์ฌ ํจ์ $f(x)$๋ฅผ
$f(x) = ($๋ฑ์ $t^4 = x^2 - 4$๋ฅผ ๋ง์กฑ์ํค๋ $t$์ ๊ฐ์$)$
๋ก ์์ํ์. ํจ์ $y = f(x)$์ ๊ทธ๋ํ๋?

## ๋ณด๊ธฐ
โ > [!example] ๐ธ (๊ทธ๋ฆผ/๊ทธ๋ํ)   โก > [!example] ๐ธ (๊ทธ๋ฆผ/๊ทธ๋ํ)   โข > [!example] ๐ธ (๊ทธ๋ฆผ/๊ทธ๋ํ)   โฃ > [!example] ๐ธ (๊ทธ๋ฆผ/๊ทธ๋ํ)   โค > [!example] ๐ธ (๊ทธ๋ฆผ/๊ทธ๋ํ)

## ํ์ด
[์๋ต] โก 

$t^4 = x^2 - 4$์์ 

i) $x^2 - 4 > 0$์ผ ๋, 
$(x - 2)(x + 2) > 0$ 
$x < -2$ ๋๋ $x > 2$์ผ ๋, 
$t = \sqrt[4]{x^2 - 4}$ ๋๋ $t = -\sqrt[4]{x^2 - 4}$์ด๋ฏ๋ก ์ค์ $t$์ ๊ฐ์ $2$๊ฐ์ด๋ค. 
$\therefore f(x) = 2$ 

ii) $x^2 - 4 = 0$์ผ ๋, 
$(x - 2)(x + 2) = 0$ 
$x = -2$ ๋๋ $x = 2$์ผ ๋, 
$t = 0$์ด๋ฏ๋ก ์ค์ $t$์ ๊ฐ์ $1$๊ฐ์ด๋ค. 
$\therefore f(x) = 1$ 

iii) $x^2 - 4 < 0$์ผ ๋, 
$t^4 = x^2 - 4 < 0$์ ๋ง์กฑ์ํค๋ ์ค์ $t$์ ๊ฐ์ ์กด์ฌํ์ง ์๋๋ค. 
$\therefore f(x) = 0$ 

i), ii), iii)์ ์ํด ํจ์ $y = f(x)$์ ๊ทธ๋ํ๋ ๋ค์๊ณผ ๊ฐ๋ค. 

> [!example] ๐ธ (๊ทธ๋ฆผ/๊ทธ๋ํ)


[๋ค๋ฅธํ์ด] 

$t^4 = x^2 - 4$๋ฅผ ๋ง์กฑ์ํค๋ ์ค์ $t$๋ $x^2 - 4$์ ๋ค์๊ณฑ๊ทผ ์ค ์ค์์ธ ๊ฒ์ด๋ค. 

i) $x^2 - 4 > 0$์ผ ๋, 
$x^2 - 4$์ ๋ค์๊ณฑ๊ทผ ์ค ์ค์์ธ ๊ฒ์ 
$\sqrt[4]{x^2 - 4}$, $-\sqrt[4]{x^2 - 4}$์ด๋ฏ๋ก 
$f(x) = 2$ 

ii) $x^2 - 4 = 0$์ผ ๋, 
$x^2 - 4$์ ๋ค์๊ณฑ๊ทผ ์ค ์ค์์ธ ๊ฒ์ 
$\sqrt[4]{x^2 - 4} = \sqrt[4]{0} = 0$์ด๋ฏ๋ก 
$f(x) = 1$ 

iii) $x^2 - 4 < 0$์ผ ๋, 
$x^2 - 4$์ ๋ค์๊ณฑ๊ทผ ์ค ์ค์๋ ์กด์ฌํ์ง ์์ผ๋ฏ๋ก 
$f(x) = 0$