## ë¬¸ì œ
í•¨ìˆ˜ $f(x)=x^{3}+x-1$ì˜ ì—­í•¨ìˆ˜ë¥¼ $g(x)$ë¼ í•  ë•Œ, $\int_{1}^{9} g(x) dx$ì˜ ê°’ì€?

> [!example] ğŸ“¸ (ê·¸ë¦¼/ê·¸ë˜í”„)

## ë³´ê¸°
â‘  $\frac{47}{4}$   â‘¡ $\frac{49}{4}$   â‘¢ $\frac{51}{4}$   â‘£ $\frac{53}{4}$   â‘¤ $\frac{55}{4}$

## í’€ì´
ê·¸ë¦¼ì—ì„œ ì–´ë‘ìš´ ë‘ ë¶€ë¶„ì˜ ë„“ì´ê°€ ê°™ìœ¼ë¯€ë¡œ $f(1)=1$, $f(2)=9$ì„ì„ ì´ìš©í•˜ë©´

$$ \begin{array}{ll} \int_{1}^{9} g(x) dx & = 18 - 1 - \int_{1}^{2} f(x) dx \\ & = 18 - 1 - \int_{1}^{2} (x^{3} + x - 1) dx \\ & = 17 - \left[ \frac{1}{4} x^{4} + \frac{1}{2} x^{2} - x \right]_{1}^{2} \\ & = 17 - \left( (4 + 2 - 2) - (\frac{1}{4} + \frac{1}{2} - 1) \right) \\ & = 17 - \frac{17}{4} = \frac{51}{4} \end{array} $$

ì •ë‹µ: â‘¢