## ë¬¸ì œ

> [!example] ğŸ“¸ (ê·¸ë¦¼/ê·¸ë˜í”„)

ì‚¼ê°í˜• $ABC$ì—ì„œ $\overline{AB} = 1$ì´ê³  $\angle A = \theta$, $\angle B = 2\theta$ì´ë‹¤. ë³€ $AB$ ìœ„ì˜ ì  $D$ë¥¼ $\angle ACD = 2\angle BCD$ê°€ ë˜ë„ë¡ ì¡ëŠ”ë‹¤. $\lim_{\theta \to 0^+} \frac{\overline{CD}}{\theta} = a$ì¼ ë•Œ, $27a^2$ì˜ ê°’ì„ êµ¬í•˜ì‹œì˜¤. (ë‹¨, $0 < \theta < \frac{\pi}{4}$ì´ë‹¤.)

## ë³´ê¸°


## í’€ì´

[ì •ë‹µ] $16$

$\overline{AB} = 1$, $\angle A = \theta$, $\angle B = 2\theta$ì´ê³ , $\angle BCD = \alpha$ë¼ í•˜ë©´ $\angle ACD = 2\alpha$ì´ë¯€ë¡œ
$\angle CDB = \theta + 2\alpha$, $\angle CDA = 2\theta + \alpha$ì´ë‹¤.
$(\theta + 2\alpha) + (2\theta + \alpha) = \pi$ì´ë¯€ë¡œ
$\therefore \alpha = \frac{\pi}{3} - \theta$

ì‚¬ì¸ë²•ì¹™ì— ì˜í•´
(â…°) ì‚¼ê°í˜• $ADC$ì—ì„œ
$\frac{\overline{AD}}{\sin 2\alpha} = \frac{\overline{CD}}{\sin \theta}$
$\overline{AD} = \frac{\sin 2\alpha}{\sin \theta} \cdot \overline{CD} \cdots$ ã‰ 

(â…±) ì‚¼ê°í˜• $BDC$ì—ì„œ
$\frac{\overline{BD}}{\sin \alpha} = \frac{\overline{CD}}{\sin 2\theta}$
$\overline{BD} = \frac{\sin \alpha}{\sin 2\theta} \cdot \overline{CD} \cdots$ ã‰¡

ã‰ ê³¼ ã‰¡ì—ì„œ $\overline{AD} + \overline{BD} = 1$ì´ë¯€ë¡œ
$\overline{CD} \cdot \left( \frac{\sin 2\alpha}{\sin \theta} + \frac{\sin \alpha}{\sin 2\theta} \right) = 1$
$\overline{CD} = \frac{1}{\frac{\sin 2\alpha}{\sin \theta} + \frac{\sin \alpha}{\sin 2\theta}}$
$= \frac{1}{\frac{2 \sin \alpha \cos \alpha}{\sin \theta} + \frac{\sin \alpha}{2 \sin \theta \cos \theta}}$
$= \frac{\sin \theta}{\sin \alpha} \cdot \frac{1}{2 \cos \alpha + \frac{1}{2 \cos \theta}}$

ê·¸ëŸ°ë°,
$\lim_{\theta \to 0^+} \sin \alpha = \lim_{\theta \to 0^+} \sin \left( \frac{\pi}{3} - \theta \right) = \frac{\sqrt{3}}{2}$
$\lim_{\theta \to 0^+} \cos \alpha = \lim_{\theta \to 0^+} \cos \left( \frac{\pi}{3} - \theta \right) = \frac{1}{2}$
ì´ë¯€ë¡œ
$\therefore \lim_{\theta \to 0^+} \frac{\overline{CD}}{\theta}$
$= \lim_{\theta \to 0^+} \frac{\sin \theta}{\theta} \cdot \frac{1}{\sin \alpha} \cdot \frac{1}{2 \cos \alpha + \frac{1}{2 \cos \theta}}$
$= 1 \cdot \frac{1}{\frac{\sqrt{3}}{2}} \cdot \frac{1}{2 \cdot \frac{1}{2} + \frac{1}{2}}$
$= \frac{4}{3 \sqrt{3}}$

ë”°ë¼ì„œ $a = \frac{4}{3 \sqrt{3}}$ì´ë¯€ë¡œ
$\therefore 27a^2 = 27 \cdot \left( \frac{4}{3 \sqrt{3}} \right)^2 = 16$