## 문제
일차변환 $f$와 두 행렬 
$$ A = \left( \begin{array}{c} 6 \\ 0 \end{array} \right) , B = \left( \begin{array}{c} 0 \\ 3 \end{array} \right) $$
에 대하여 
$$ f(A) + f(B) = \left( \begin{array}{c} 0 \\ 9 \end{array} \right) $$
가 성립한다. 일차변환 $f$의 역변환 $f^{-1}$가 존재할 때, $f^{-1}(B)$는?

## 보기
① $\left( \begin{array}{c} 0 \\ 2 \end{array} \right)$ ② $\left( \begin{array}{c} 2 \\ 0 \end{array} \right)$ ③ $\left( \begin{array}{c} 2 \\ 1 \end{array} \right)$ ④ $\left( \begin{array}{c} 2 \\ 2 \end{array} \right)$ ⑤ $\left( \begin{array}{c} 4 \\ 2 \end{array} \right)$

## 풀이
[정답] ② 

$A + B = C$라 하면 
$$ C = \left( \begin{array}{c} 6 \\ 3 \end{array} \right) $$ 
$$ f(A) + f(B) = f(A + B) = f(C) = 3 B $$ 
따라서 $$ f^{-1}(B) = \frac{1}{3} C $$ 이므로 
$$ f^{-1}(B) = \left( \begin{array}{c} 2 \\ 1 \end{array} \right) $$