## 문제
$0$이 아닌 세 복소수 $\alpha$, $\beta$, $\gamma$가 다음 조건을 만족시킨다.

(가) $\alpha + \beta + \gamma = 0$
(나) $\frac{1}{\alpha} + \frac{1}{\beta} + \frac{1}{\gamma} = 0$

이때, $\frac{\gamma}{\alpha} + \overline{\left( \frac{\alpha}{\beta} \right)}$의 값은? (단, $\overline{\left( \frac{\alpha}{\beta} \right)}$는 $\frac{\alpha}{\beta}$의 켤레복소수이고, $i = \sqrt{-1}$이다.)

## 보기
① $-i$   ② $-1$   ③ $0$   ④ $i$   ⑤ $1$

## 풀이
(나)에서 
$\frac{1}{\alpha} + \frac{1}{\beta} = -\frac{1}{\gamma}$, 
$\frac{\alpha + \beta}{\alpha \beta} = -\frac{1}{\gamma}$ 
(가)에서 
$\alpha + \beta = -\gamma$ 이므로 
$\frac{-\gamma}{\alpha \beta} = -\frac{1}{\gamma}$ 
$\alpha \beta = \gamma^{2} \dots ㉠$ 

같은 방법으로 
$\beta \gamma = \alpha^{2} \dots ㉡$ 
$\gamma \alpha = \beta^{2} \dots ㉢$ 

(나)에서 
$\frac{\alpha \beta + \beta \gamma + \gamma \alpha}{\alpha \beta \gamma} = 0$ 이므로 
$\alpha \beta + \beta \gamma + \gamma \alpha = 0$ 

$㉠, ㉡, ㉢$에서 
$\alpha^{2} + \beta^{2} + \gamma^{2} = 0$ 
$\alpha^{2} + \alpha \gamma + \gamma^{2} = 0 \dots ㉣$ 

$㉣$에서 양변을 $\alpha^{2}$으로 나누면 
$\left( \frac{\gamma}{\alpha} \right)^{2} + \frac{\gamma}{\alpha} + 1 = 0$ 
$\therefore \frac{\gamma}{\alpha} = \frac{-1 + \sqrt{3}i}{2}$ 또는 $\frac{\gamma}{\alpha} = \frac{-1 - \sqrt{3}i}{2}$ 

$㉡$에서 $\frac{\alpha}{\beta} = \frac{\gamma}{\alpha}$ 이므로 
$\frac{\gamma}{\alpha} + \overline{\left( \frac{\alpha}{\beta} \right)} = \frac{\gamma}{\alpha} + \overline{\left( \frac{\gamma}{\alpha} \right)}$ 이다. 
따라서 
$\frac{\gamma}{\alpha} + \overline{\left( \frac{\alpha}{\beta} \right)} = -1$

정답: ②