## ë¬¸ì œ
ì „ì²´ì§‘í•© $U$ì˜ ë‘ ë¶€ë¶„ì§‘í•© $A$, $B$ì— ëŒ€í•˜ì—¬ $A = \{2, 3, 4, 5, 6\}$, $A - B = \{2, 6\}$ì¼ ë•Œ, ì§‘í•© $A \cap B$ì˜ ëª¨ë“  ì›ì†Œì˜ í•©ì„ êµ¬í•˜ì‹œì˜¤.



> [!example] ğŸ“¸ (ê·¸ë¦¼/ê·¸ë˜í”„)

## í’€ì´
ë²¤ ë‹¤ì´ì–´ê·¸ë¨ì—ì„œ 
$A \cap B = \{3, 4, 5\}$
ë”°ë¼ì„œ ëª¨ë“  ì›ì†Œì˜ í•©ì€ 
$12$

**[ë‹¤ë¥¸ í’€ì´]**
$A - (A - B)$
$= A \cap (A \cap B^{C})^{C}$
$= A \cap (A^{C} \cup B)$
$= (A \cap A^{C}) \cup (A \cap B)$
$= \emptyset \cup (A \cap B)$
$= A \cap B$
$\therefore A \cap B = \{2, 3, 4, 5, 6\} - \{2, 6\} = \{3, 4, 5\}$
ë”°ë¼ì„œ $A \cap B$ì˜ ëª¨ë“  ì›ì†Œì˜ í•©ì€ $3 + 4 + 5 = 12$

**ì •ë‹µ: $12$**