## 문제
$\sqrt[3]{10+2\sqrt{27}} + \sqrt[3]{10-2\sqrt{27}}$ 의 값은?

## 보기
① $1$   ② $\sqrt{2}$   ③ $\sqrt{3}$   ④ $2$   ⑤ $2\sqrt{3}$

## 풀이
$$(a \pm \sqrt{b})^{3} = (a^{3}+3ab) \pm \sqrt{b}(3a^{2}+b)$$
$a=1$, $b=3$ 일 때,
$a^{3}+3ab=10$, $3a^{2}+b=6$ 을 만족시킨다.
따라서
$$10+2\sqrt{27} = 10+6\sqrt{3} = (1+\sqrt{3})^{3}$$
$$10-2\sqrt{27} = 10-6\sqrt{3} = (1-\sqrt{3})^{3}$$
이다. 그러므로
$$\sqrt[3]{10+2\sqrt{27}} + \sqrt[3]{10-2\sqrt{27}}$$
$$= \sqrt[3]{(1+\sqrt{3})^{3}} + \sqrt[3]{(1-\sqrt{3})^{3}}$$
$$= (1+\sqrt{3}) + (1-\sqrt{3})$$
$$= 2$$
따라서 정답은 ④이다.