## 문제
$xy > 0$이고, $\frac{x^2 - 3xy - y^2}{x^2 - 3xy - 5y^2} = -3$일 때, $\frac{3x+4y}{x-3y}$의 값을 구하시오.

## 풀이
$\frac{x^2 - 3xy - y^2}{x^2 - 3xy - 5y^2} = -3$
$x^2 - 3xy - y^2 = -3(x^2 - 3xy - 5y^2)$
$x^2 - 3xy - y^2 = -3x^2 + 9xy + 15y^2$
$4x^2 - 12xy - 16y^2 = 0$
$4(x - 4y)(x + y) = 0$

(ⅰ) $x = -y$ 인 경우
$xy = (-y)y = -y^2 \le 0$
$xy > 0$에 모순이므로 $x \neq -y$

(ⅱ) $x = 4y$ 인 경우
$xy = (4y)y = 4y^2 > 0$ ($\because y \neq 0$)
(ⅰ), (ⅱ)에서 $x = 4y$

$\frac{3x + 4y}{x - 3y} = \frac{3(4y) + 4y}{4y - 3y}$
$= \frac{16y}{y}$
$= 16$ ($\because y \neq 0$)

**[다른 풀이]**
좌변의 분자 분모를 $y^2$ ($y \neq 0$)으로 나누면
$\frac{(\frac{x}{y})^2 - 3(\frac{x}{y}) - 1}{(\frac{x}{y})^2 - 3(\frac{x}{y}) - 5} = -3$
$\frac{x}{y} = t$ ($t > 0$)라 하면
$\frac{t^2 - 3t - 1}{t^2 - 3t - 5} = -3$
$4t^2 - 12t - 16 = 0$
$4(t^2 - 3t - 4) = 0$
$4(t - 4)(t + 1) = 0$
$t = 4$ 또는 $t = -1$
$\therefore t = 4$ ($\because t > 0$)
그러므로 $\frac{x}{y} = 4$에서 $x = 4y$
$\frac{3x + 4y}{x - 3y} = \frac{3(4y) + 4y}{4y - 3y} = \frac{16y}{y} = 16$ ($\because y \neq 0$)

정답: $16$