## 문제
연속함수 $f(x)$가 
$f(x) = e^{x^2} + \int_{0}^{1} tf(t) dt$
를 만족시킬 때, $\int_{0}^{1} xf(x) dx$의 값은?

## 보기
① $e-2$   ② $\frac{e-1}{2}$   ③ $\frac{e}{2}$   ④ $e-1$   ⑤ $\frac{e+1}{2}$

## 풀이
$f(x) = e^{x^2} + \int_{0}^{1} tf(t) dt$에서 
$\int_{0}^{1} tf(t) dt = a$ ($a$는 상수)
로 놓으면 $f(x) = e^{x^2} + a$이므로 
$a = \int_{0}^{1} tf(t) dt$ 
$= \int_{0}^{1} t (e^{t^2} + a) dt$ 
$= \int_{0}^{1} (te^{t^2} + at) dt$ 
$= \int_{0}^{1} te^{t^2} dt + \left[ \frac{a}{2} t^2 \right]_{0}^{1}$ 
$= \int_{0}^{1} te^{t^2} dt + \frac{a}{2}$ $\cdots \cdots$ ㉠ 

$\int_{0}^{1} te^{t^2} dt$에서 $t^2 = z$로 놓으면 $2t = \frac{dz}{dt}$이고, 
$t=0$일 때 $z=0$, $t=1$일 때 $z=1$이므로 
$\int_{0}^{1} t e^{t^2} dt = \int_{0}^{1} \frac{e^z}{2} dz = \left[ \frac{e^z}{2} \right]_{0}^{1} = \frac{e}{2} - \frac{1}{2}$ 

㉠에서 $a = \frac{e}{2} - \frac{1}{2} + \frac{a}{2}$이므로 
$\frac{a}{2} = \frac{e-1}{2}$
$a = e-1$ 

따라서 $\int_{0}^{1} xf(x) dx = \int_{0}^{1} tf(t) dt = a = e-1$

정답: ④