## 문제
함수 $f(x)=x|x|+|x-1|^{3}$ 에 대하여 $f'(0)+f'(1)$ 의 값은?

## 보기
① $-3$   ② $-1$   ③ $1$   ④ $3$   ⑤ $5$

## 풀이
[정답] ②

$g(x)=x|x|$, $h(x)=|x-1|^{3}$ 으로 놓으면 두 함수 $g(x)$, $h(x)$ 는 실수 전체에서 미분가능하므로 함수 $f(x)$ 도 실수 전체에서 미분가능하다.
$g'(0)=0$, $h'(1)=0$ 이고 $x>0$ 일 때 $g(x)=x^{2}$, $x<1$ 일 때 $h(x)=-(x-1)^{3}$ 이므로
$f'(0)=0+h'(0)=-3(0-1)^{2}=-3$
$f'(1)=g'(1)+0=2 \cdot 1=2$
$\therefore f'(0)+f'(1)=-3+2=-1$

[다른풀이1]
$f(x)=x|x|+|x-1|^{3}$ 에서 $f(0)=1$, $f(1)=1$
$\displaystyle \lim_{h \to 0^{+}} \frac{f(0+h)-f(0)}{h} = \lim_{h \to 0^{+}} \frac{h|h|+|h-1|^{3}-1}{h}$
$\displaystyle = \lim_{h \to 0^{+}} \frac{h^{2}-(h-1)^{3}-1}{h}$
$\displaystyle = \lim_{h \to 0^{+}} \frac{-h^{3}+4h^{2}-3h}{h}$
$\displaystyle = \lim_{h \to 0^{+}} (-h^{2}+4h-3) = -3$

$\displaystyle \lim_{h \to 0^{-}} \frac{f(0+h)-f(0)}{h} = \lim_{h \to 0^{-}} \frac{h|h|+|h-1|^{3}-1}{h}$
$\displaystyle = \lim_{h \to 0^{-}} \frac{-h^{2}-(h-1)^{3}-1}{h}$
$\displaystyle = \lim_{h \to 0^{-}} \frac{-h^{3}+2h^{2}-3h}{h}$
$\displaystyle = \lim_{h \to 0^{-}} (-h^{2}+2h-3) = -3$
$\therefore f'(0)=-3$

$\displaystyle \lim_{h \to 0^{+}} \frac{f(1+h)-f(1)}{h} = \lim_{h \to 0^{+}} \frac{(1+h)|1+h|+|1+h-1|^{3}-1}{h}$
$\displaystyle = \lim_{h \to 0^{+}} \frac{(1+h)^{2}+|h|^{3}-1}{h}$
$\displaystyle = \lim_{h \to 0^{+}} \frac{h^{3}+h^{2}+2h}{h}$
$\displaystyle = \lim_{h \to 0^{+}} (h^{2}+h+2) = 2$

$\displaystyle \lim_{h \to 0^{-}} \frac{f(1+h)-f(1)}{h} = \lim_{h \to 0^{-}} \frac{(1+h)|1+h|+|1+h-1|^{3}-1}{h}$
$\displaystyle = \lim_{h \to 0^{-}} \frac{(1+h)^{2}+|h|^{3}-1}{h}$
$\displaystyle = \lim_{h \to 0^{-}} \frac{-h^{3}+h^{2}+2h}{h}$
$\displaystyle = \lim_{h \to 0^{-}} (-h^{2}+h+2) = 2$
$\therefore f'(1)=2$
$\therefore f'(0)+f'(1)=-3+2=-1$

[다른풀이2]
$$ \begin{array}{l} f(x) = \begin{cases} x^{2}+(x-1)^{3} & (x \ge 1) \\ x^{2}-(x-1)^{3} & (0 \le x < 1) \\ -x^{2}-(x-1)^{3} & (x < 0) \end{cases} \end{array} $$
이므로
$$ \begin{array}{l} f'(x) = \begin{cases} 2x+3(x-1)^{2} & (x > 1) \\ 2x-3(x-1)^{2} & (0 < x < 1) \\ -2x-3(x-1)^{2} & (x < 0) \end{cases} \end{array} $$
$\displaystyle \lim_{x \to 0^{+}} f'(x) = 2 \cdot 0-3(0-1)^{2}=-3$
$\displaystyle \lim_{x \to 0^{-}} f'(x) = -2 \cdot 0-3(0-1)^{2}=-3$
$\therefore f'(0)=-3$
$\displaystyle \lim_{x \to 1^{+}} f'(x) = 2 \cdot 1+3(1-1)^{2}=2$
$\displaystyle \lim_{x \to 1^{-}} f'(x) = 2 \cdot 1-3(1-1)^{2}=2$
$\therefore f'(1)=2$

이상에서
$f'(0)+f'(1)=-3+2=-1$