## 문제
두 행렬 $A$, $B$에 대하여 
$$ A = \left( \begin{array}{cc} 1 & 3 \\ 2 & -1 \end{array} \right) , A - B = \left( \begin{array}{cc} 3 & -1 \\ 2 & 1 \end{array} \right) $$
일 때, $A^{2} - AB$의 모든 성분의 합은?

## 보기
① $12$   ② $10$   ③ $8$   ④ $6$   ⑤ $4$

## 풀이
$A^{2} - AB = A(A - B)$이므로 주어진 행렬을 대입하면 다음과 같다.
$$ \begin{array}{rl} A(A - B) & = \left( \begin{array}{cc} 1 & 3 \\ 2 & -1 \end{array} \right) \left( \begin{array}{cc} 3 & -1 \\ 2 & 1 \end{array} \right) \\ & = \left( \begin{array}{cc} 1 \times 3 + 3 \times 2 & 1 \times (-1) + 3 \times 1 \\ 2 \times 3 + (-1) \times 2 & 2 \times (-1) + (-1) \times 1 \end{array} \right) \\ & = \left( \begin{array}{cc} 9 & 2 \\ 4 & -3 \end{array} \right) \end{array} $$
따라서 모든 성분의 합은 
$9 + 2 + 4 + (-3) = 12$
정답: ①