## 문제
$x-y+z=0$, $2x-3y+z=0$ 일 때, $\frac{x^{2} -y^{2} +2z^{2}}{2xy+yz-3zx}$ 의 값은? (단, $xyz \neq 0$ 이다.)

## 보기
① $\frac{1}{3}$   ② $\frac{4}{9}$   ③ $\frac{5}{9}$   ④ $\frac{2}{3}$   ⑤ $\frac{7}{9}$

## 풀이
$$ \begin{cases} x-y+z=0 & \cdots ㉠ \\ 2x-3y+z=0 & \cdots ㉡ \end{cases} $$
$㉡-㉠$을 하면
$x-2y=0$
$\therefore x=2y \cdots ㉢$
$㉢$을 $㉠$에 대입하여 정리하면
$z=-y$
그러므로 주어진 식에 $x=2y$ 와 $z=-y$ 를 대입하면
$\frac{x^{2}-y^{2}+2z^{2}}{2xy+yz-3zx} = \frac{(2y)^{2}-y^{2}+2(-y)^{2}}{2(2y)y+y(-y)-3(-y)(2y)}$
$= \frac{4y^{2}-y^{2}+2y^{2}}{4y^{2}-y^{2}+6y^{2}}$
$= \frac{5y^{2}}{9y^{2}}$
$= \frac{5}{9}$

정답은 ③이다.