## 문제
$\lim_{x \to \infty} \left( \sqrt{x^{4}+2x^{3}+1}-x^{2} \right) \left( \sqrt{x^{2}+6}-x \right)$의 값은?

## 보기
① $1$   ② $2$   ③ $3$   ④ $4$   ⑤ $5$

## 풀이
정답: ③

$$\lim_{x \to \infty} \left( \sqrt{x^{4}+2x^{3}+1}-x^{2} \right) \left( \sqrt{x^{2}+6}-x \right)$$

$$= \lim_{x \to \infty} \left\{ \frac{2x^{3}+1}{\sqrt{x^{4}+2x^{3}+1}+x^{2}} \cdot \frac{6}{\sqrt{x^{2}+6}+x} \right\}$$

$$= \lim_{x \to \infty} \left\{ \frac{2+\frac{1}{x^{3}}}{\sqrt{1+\frac{2}{x^{2}}+\frac{1}{x^{4}}}+1} \cdot \frac{6}{\sqrt{1+\frac{6}{x^{2}}}+1} \right\}$$

$$= \frac{2+0}{\sqrt{1+0+0}+1} \cdot \frac{6}{\sqrt{1+0}+1} = 3$$