## 문제
첫째항이 $10$ 인 수열 $\{a_{n}\}$ 이 모든 자연수 $n$ 에 대하여 $a_{n} < a_{n+1}$ , $\sum_{k=1}^{n} (a_{k+1}-a_{k})^{2} = 2 (1 - \frac{1}{9^{n}})$ 을 만족시킬 때, $\lim_{n \to \infty} a_{n}$ 의 값을 구하시오.

## 보기

## 풀이
$\sum_{k=1}^{n} (a_{k+1}-a_{k})^{2} = 2 (1 - \frac{1}{9^{n}})$ 에서
$$ \begin{array}{l} (a_{n+1}-a_{n})^{2} = \sum_{k=1}^{n} (a_{k+1}-a_{k})^{2} - \sum_{k=1}^{n-1} (a_{k+1}-a_{k})^{2} \\ = 2 (1 - \frac{1}{9^{n}}) - 2 (1 - \frac{1}{9^{n-1}}) \\ = \frac{16}{9^{n}} (n \geq 2) \end{array} $$
이때, $n=1$ 이면
$(a_{2}-a_{1})^{2} = 2 (1 - \frac{1}{9}) = \frac{16}{9}$
한편, $a_{n+1} > a_{n}$ 이므로
$a_{n+1}-a_{n} = \frac{4}{3^{n}}$
$\therefore a_{n+1} = a_{n} + \frac{4}{3^{n}}$
이때, $a_{1} = 10$ 이므로
$$ \begin{array}{l} a_{n} = a_{1} + \sum_{k=1}^{n-1} \frac{4}{3^{k}} \\ = 10 + \frac{\frac{4}{3} \{ 1 - (\frac{1}{3})^{n-1} \} }{1 - \frac{1}{3}} \\ = 10 + 2 \{ 1 - (\frac{1}{3})^{n-1} \} (n \geq 2) \end{array} $$
따라서, $\lim_{n \to \infty} a_{n} = 12$