## 문제
두 행렬 $A$, $B$에 대하여 
$$ A = \left( \begin{array}{rr} 1 & 3 \\ 2 & -1 \end{array} \right), A-B = \left( \begin{array}{rr} 3 & -1 \\ 2 & 1 \end{array} \right) $$
일 때, $A^2 - AB$의 모든 성분의 합은?

## 보기
① $12$   ② $10$   ③ $8$   ④ $6$   ⑤ $4$

## 풀이
$A^2 - AB = A(A - B)$ 이므로 주어진 행렬을 대입하면 다음과 같다.
$$ A(A - B) = \left( \begin{array}{rr} 1 & 3 \\ 2 & -1 \end{array} \right) \left( \begin{array}{rr} 3 & -1 \\ 2 & 1 \end{array} \right) = \left( \begin{array}{rr} 9 & 2 \\ 4 & -3 \end{array} \right) $$
따라서 모든 성분의 합은 
$9 + 2 + 4 + (-3) = 12$
정답은 ①이다.