## 문제
$a_{n}+a_{n+1} = 6 \left( \frac{1}{n} - \frac{1}{n+2} \right) (n \geq 1)$ 수열 $\{ a_{n} \}$ 의 첫째항부터 제 $n$ 항까지의 합을 $S_{n}$ 이라 할 때, $S_{n} = \frac{6n}{n+1}$ 이다. $\sum _{n=1}^{\infty} ( a_{n} + a_{n+1} )$ 의 값을 구하시오.

## 풀이
정답: $9$

$S_{n}=\frac{6n}{n+1}$ 에서
$a_{n}=S_{n}-S_{n-1}$
$= \frac{6n}{n+1}-\frac{6(n-1)}{n}$
$= \frac{6n^{2}-6(n^{2}-1)}{n(n+1)}$
$= \frac{6}{n(n+1)} (n \geq 2)$

$a_{1}=S_{1}=3$ 이므로 $a_{n}=\frac{6}{n(n+1)} (n \geq 1)$

$\therefore a_{n}+a_{n+1} = \frac{6}{n(n+1)}+\frac{6}{(n+1)(n+2)}$
$= 6 \left( \frac{1}{n}-\frac{1}{n+1} \right) + 6 \left( \frac{1}{n+1}-\frac{1}{n+2} \right)$
$= 6 \left( \frac{1}{n}-\frac{1}{n+2} \right)$

$\therefore \sum_{n=1}^{\infty} (a_{n}+a_{n+1}) = 6 \sum_{n=1}^{\infty} \left( \frac{1}{n}-\frac{1}{n+2} \right)$
$= 6 \lim _{n \to \infty} \sum_{k=1}^{n} \left( \frac{1}{k}-\frac{1}{k+2} \right)$
$= 6 \lim _{n \to \infty} \left( 1+\frac{1}{2}-\frac{1}{n+1}-\frac{1}{n+2} \right)$
$= 6 \left( 1+\frac{1}{2} \right) = 9$

**[다른 풀이]**
$\lim _{n \to \infty} S_{n}= \lim _{n \to \infty} \frac{6n}{n+1}=6$
$\lim _{n \to \infty} S_{n+1}= \lim _{n \to \infty} \frac{6n+6}{n+2}=6$

$\sum_{n=1}^{\infty} (a_{n}+a_{n+1}) = \lim _{n \to \infty} \sum_{k=1}^{n} (a_{k}+a_{k+1})$
$= \lim _{n \to \infty} \left( \sum_{k=1}^{n} a_{k}+ \sum_{k=1}^{n} a_{k+1} \right)$
$= \lim _{n \to \infty} (S_{n}+S_{n+1}-a_{1})$
$= \lim _{n \to \infty} S_{n} + \lim _{n \to \infty} S_{n+1}-a_{1}$
$= 6+6-3=9$ ($\because a_{1}=S_{1}=3$)

**[다른 풀이]**
$a_{n}+a_{n+1} = (S_{n}-S_{n-1}) + (S_{n+1}-S_{n})$
$= S_{n+1}-S_{n-1}$
$= \frac{6(n+1)}{n+2} - \frac{6(n-1)}{n}$
$= \frac{6n(n+1)-6(n-1)(n+2)}{n(n+2)}$
$= \frac{12}{n(n+2)}$
$= 6 \left( \frac{1}{n}-\frac{1}{n+2} \right) (n \geq 2)$

$a_{1}+a_{2}= S_{2}=4$ 이므로