## ë¬¸ì œ
ë‘ ì§‘í•© 
$A = \{ x \mid x^{2} - ( a+b )x + ab < 0 \}$, 
$B = \{ x \mid 2^{2x+2} - 9 \cdot 2^{x} + 2 < 0 \}$ 
ì— ëŒ€í•˜ì—¬ $A \subset B$ ì¼ ë•Œ, $b-a$ ì˜ ìµœëŒ“ê°’ì„ êµ¬í•˜ì‹œì˜¤. (ë‹¨, $a < b$ ì´ë‹¤.)



> [!example] ğŸ“¸ (ê·¸ë¦¼/ê·¸ë˜í”„)

## í’€ì´
$x^{2} - (a+b)x + ab < 0$
$\Leftrightarrow (x-a)(x-b) < 0$
$a < b$ ì´ë¯€ë¡œ 
$a < x < b$
$\therefore A = \{ x \mid a < x < b \}$

í•œí¸, 
$2^{2x+2} - 9 \cdot 2^{x} + 2 < 0$
$\Leftrightarrow 4(2^{x})^{2} - 9 \cdot 2^{x} + 2 < 0$
$\Leftrightarrow (4 \cdot 2^{x} - 1)(2^{x} - 2) < 0$
$\Leftrightarrow \frac{1}{4} < 2^{x} < 2$
$\Leftrightarrow 2^{-2} < 2^{x} < 2^{1}$
$\therefore B = \{ x \mid -2 < x < 1 \}$

$A \subset B$ ì´ë¯€ë¡œ 
$-2 \le a < b \le 1$ 
ë”°ë¼ì„œ $b-a$ ì˜ ìµœëŒ“ê°’ì€ 
$1 - (-2) = 3$

ì •ë‹µ: $3$