## 문제
함수 $f(x) = x^{3} + 3x^{2} + 4x + 5$의 역함수 $g(x)$에 대하여 
$$\lim_{n \to \infty} n \left\{ g \left( 1 + \frac{1}{n} \right) - g \left( 1 - \frac{2}{n} \right) \right\}$$
의 값을 $p$라 할 때, $4p$의 값을 구하시오.

## 보기

## 풀이
$\frac{1}{n} = h$라 하면, $n \to \infty$일 때, $h \to 0$이다.
(준식)
$= \lim_{h \to 0} \frac{\{g(1+h) - g(1)\} - \{g(1-2h) - g(1)\}}{h}$
$= \lim_{h \to 0} \frac{g(1+h) - g(1)}{h} + 2 \lim_{h \to 0} \frac{g(1-2h) - g(1)}{-2h}$
$= g'(1) + 2g'(1) = 3g'(1)$

$g(1) = f^{-1}(1) = a$라 하면 $f(a) = 1$이므로
$f(a) = a^{3} + 3a^{2} + 4a + 5 = 1$에서 $a = -2$이다.

$f'(x) = 3x^{2} + 6x + 4$에서 $f'(-2) = 4$이고
$g(f(x)) = x$에서 $g'(f(x)) = \frac{1}{f'(x)}$이므로
$3g'(1) = 3 \times \frac{1}{f'(-2)} = \frac{3}{4}$이다.
따라서 $p = \frac{3}{4}$이므로 $4p = 3$이다.

[정답] $3$