## 문제
자연수 $n$ 에 대하여 $A_{n} = \left( \begin{array}{cc} n & 1 \\ 0 & n \end{array} \right)$ 이고
$$ \left( \begin{array}{c} a_{n} \\ b_{n} \end{array} \right) = A_{n} A_{n-1} \cdots A_{2} A_{1} \left( \begin{array}{c} 0 \\ 1 \end{array} \right) $$
일 때, 옳은 것만을 <보기>에서 있는 대로 고른 것은?

---
**<보 기>**
ㄱ. $\frac{a_{2}}{b_{2}} = \frac{3}{2}$
ㄴ. $\left( \begin{array}{c} a_{n+1} \\ b_{n+1} \end{array} \right) = A_{n+1} \left( \begin{array}{c} a_{n} \\ b_{n} \end{array} \right)$
ㄷ. $\frac{a_{n}}{b_{n}} = \sum_{k=1}^{n} \frac{1}{k}$
---

## 보기
① $ㄱ$   ② $ㄴ$   ③ $ㄱ, ㄴ$   ④ $ㄴ, ㄷ$   ⑤ $ㄱ, ㄴ, ㄷ$

## 풀이
[정답] ⑤ 

ㄱ. 
$$ \left( \begin{array}{c} a_{2} \\ b_{2} \end{array} \right) = \left( \begin{array}{cc} 2 & 1 \\ 0 & 2 \end{array} \right) \left( \begin{array}{cc} 1 & 1 \\ 0 & 1 \end{array} \right) \left( \begin{array}{c} 0 \\ 1 \end{array} \right) = \left( \begin{array}{cc} 2 & 1 \\ 0 & 2 \end{array} \right) \left( \begin{array}{c} 1 \\ 1 \end{array} \right) = \left( \begin{array}{c} 3 \\ 2 \end{array} \right) $$ 
이므로 
$\frac{a_{2}}{b_{2}} = \frac{3}{2}$ 이다. (참) 

ㄴ. 
$$ \left( \begin{array}{c} a_{n+1} \\ b_{n+1} \end{array} \right) = A_{n+1} A_{n} \cdots A_{2} A_{1} \left( \begin{array}{c} 0 \\ 1 \end{array} \right) $$ 
$$ = A_{n+1} \left( \begin{array}{c} a_{n} \\ b_{n} \end{array} \right) $$ 
(참) 

ㄷ. 
$$ \left( \begin{array}{c} a_{n+1} \\ b_{n+1} \end{array} \right) = \left( \begin{array}{cc} n+1 & 1 \\ 0 & n+1 \end{array} \right) \left( \begin{array}{c} a_{n} \\ b_{n} \end{array} \right) = \left( \begin{array}{c} (n+1) a_{n} + b_{n} \\ (n+1) b_{n} \end{array} \right) $$ 
$$ \frac{a_{n+1}}{b_{n+1}} = \frac{(n+1) a_{n} + b_{n}}{(n+1) b_{n}} = \frac{a_{n}}{b_{n}} + \frac{1}{n+1} $$ 
$$ \frac{a_{n}}{b_{n}} = 1 + \frac{1}{2} + \frac{1}{3} + \cdots + \frac{1}{n} = \sum_{k=1}^{n} \frac{1}{k} $$ 
$\therefore \frac{a_{n}}{b_{n}} = \sum_{k=1}^{n} \frac{1}{k}$ (참)