## 문제
수열 $\{ a_{n} \}$ 에 대하여 $\sum_{n=1}^{\infty} \left( na_{n} - \frac{n^{2}+1}{2n+1} \right) = 3$ 일 때, $\lim_{n \to \infty} ( a_{n}^{2} + 2a_{n} + 2 )$ 의 값은?

## 보기
① $\frac{13}{4}$   ② $3$   ③ $\frac{11}{4}$   ④ $\frac{5}{2}$   ⑤ $\frac{9}{4}$

## 풀이
무한급수 $\sum_{n=1}^{\infty} \left( na_{n} - \frac{n^{2}+1}{2n+1} \right)$ 이 수렴하므로 무한급수와 일반항 사이의 관계에 의하여 
$\lim_{n \to \infty} \left( na_{n} - \frac{n^{2}+1}{2n+1} \right) = 0$ 이다. 
따라서 $na_{n} - \frac{n^{2}+1}{2n+1} = b_{n}$ 이라 두면 $\lim_{n \to \infty} b_{n} = 0$ 이고, 
$na_{n} = b_{n} + \frac{n^{2}+1}{2n+1}$, 
$a_{n} = \frac{b_{n}}{n} + \frac{n^{2}+1}{2n^{2}+n}$ 이므로 
$\lim_{n \to \infty} a_{n} = \lim_{n \to \infty} \left( \frac{b_{n}}{n} + \frac{n^{2}+1}{2n^{2}+n} \right) = \frac{1}{2}$ 이다. 

$\therefore \lim_{n \to \infty} ( a_{n}^{2} + 2a_{n} + 2 ) = \left( \frac{1}{2} \right)^{2} + 2 \cdot \frac{1}{2} + 2$ 
$= \frac{1}{4} + 1 + 2$ 
$= \frac{13}{4}$

정답: ①