## 문제
행렬 $A = \left( \begin{array}{cc} 0 & 1 \\ -1 & 1 \end{array} \right)$ 에 대하여 $A^{2013} \left( \begin{array}{c} a \\ b \end{array} \right) = \left( \begin{array}{c} 1 \\ 2 \end{array} \right)$ 일 때, $a+b$ 의 값은?

## 보기
① $-3$   ② $-2$   ③ $0$   ④ $2$   ⑤ $3$

## 풀이
$$ A = \left( \begin{array}{cc} 0 & 1 \\ -1 & 1 \end{array} \right) $$ 

$$ A^{2} = \left( \begin{array}{cc} 0 & 1 \\ -1 & 1 \end{array} \right) \left( \begin{array}{cc} 0 & 1 \\ -1 & 1 \end{array} \right) = \left( \begin{array}{cc} -1 & 1 \\ -1 & 0 \end{array} \right) $$ 

$$ A^{3} = \left( \begin{array}{cc} -1 & 1 \\ -1 & 0 \end{array} \right) \left( \begin{array}{cc} 0 & 1 \\ -1 & 1 \end{array} \right) = \left( \begin{array}{cc} -1 & 0 \\ 0 & -1 \end{array} \right) = -E $$ 

$2013 = 3 \times 671$ 이므로 

$$ A^{2013} = (-E)^{671} = -E $$ 

$$ \therefore A^{2013} \left( \begin{array}{c} a \\ b \end{array} \right) = -E \left( \begin{array}{c} a \\ b \end{array} \right) = \left( \begin{array}{c} -a \\ -b \end{array} \right) $$ 

따라서 

$$ \left( \begin{array}{c} -a \\ -b \end{array} \right) = \left( \begin{array}{c} 1 \\ 2 \end{array} \right) $$ 

에서 

$a = -1$, $b = -2$ 

$\therefore a + b = -3$