## 문제
함수 $f(x) = \begin{cases} \frac{e^{x} - \sin 2x - a}{3x} & (x \neq 0) \\ b & (x = 0) \end{cases}$ 가 $x=0$ 에서 연속일 때, 두 상수 $a$, $b$ 에 대하여 $a+b$ 의 값은?

## 보기
① $\frac{1}{3}$   ② $\frac{2}{3}$   ③ $1$   ④ $\frac{4}{3}$   ⑤ $\frac{5}{3}$

## 풀이
함수 $f(x)$ 가 $x=0$ 에서 연속이므로 $\lim_{x \to 0} f(x) = f(0)$ 이어야 한다.
$\lim_{x \to 0} \frac{e^{x} - \sin 2x - a}{3x} = b$ 에서
$\lim_{x \to 0} 3x = 0$ 이므로 $\lim_{x \to 0} (e^{x} - \sin 2x - a) = 0$ 이다.
$e^{0} - \sin 0 - a = 0$
$1 - 0 - a = 0$
$\therefore a = 1$

위의 식을 극한식에 대입하여 $b$ 의 값을 구하면 다음과 같다.
$\lim_{x \to 0} \frac{e^{x} - \sin 2x - 1}{3x}$
$= \lim_{x \to 0} \frac{1}{3} \left( \frac{e^{x} - 1}{x} - \frac{\sin 2x}{x} \right)$
$= \lim_{x \to 0} \frac{1}{3} \left( \frac{e^{x} - 1}{x} - \frac{2 \sin 2x}{2x} \right)$
$= \frac{1}{3} (1 - 2) = -\frac{1}{3}$
$\therefore b = -\frac{1}{3}$

따라서
$a + b = 1 + \left( -\frac{1}{3} \right) = \frac{2}{3}$

정답: ②