## 문제
자연수 $n$에 대하여 함수 $y=f(x)$를 매개변수 $t$로 나타내면
$$ \begin{cases} x=e^{t} \\ y=(2t^{2}+nt+n)e^{t} \end{cases} $$
이고, $x \ge e^{-\frac{n}{2}}$일 때 함수 $y=f(x)$는 $x=a_{n}$에서 최솟값 $b_{n}$을 갖는다. $\frac{b_{3}}{a_{3}} + \frac{b_{4}}{a_{4}} + \frac{b_{5}}{a_{5}} + \frac{b_{6}}{a_{6}}$의 값은?

## 보기
① $\frac{23}{2}$   ② $12$   ③ $\frac{25}{2}$   ④ $13$   ⑤ $\frac{27}{2}$

## 풀이
$x=e^{t}$에서 $\frac{dx}{dt}=e^{t}$
$y=(2t^{2}+nt+n)e^{t}$에서
$\frac{dy}{dt}=(4t+n)e^{t}+(2t^{2}+nt+n)e^{t} = \{2t^{2}+(4+n)t+2n\}e^{t}$
$\frac{dy}{dx} = \frac{\frac{dy}{dt}}{\frac{dx}{dt}} = 2t^{2}+(4+n)t+2n = (2t+n)(t+2)=0$ $\cdots$ ㉠
$x \ge e^{-\frac{n}{2}}$이므로 $t \ge -\frac{n}{2}$이다.

(i) $n=3$일 때, ㉠에서 $t=-\frac{3}{2}$ 또는 $t=-2$
범위 $t \ge -\frac{3}{2}$에 의하여 $y=f(x)$는 $x=a_{3}=e^{-\frac{3}{2}}$에서 최솟값을 갖는다.
$b_{3} = \{2 \times \frac{9}{4} + 3 \times (-\frac{3}{2}) + 3\}e^{-\frac{3}{2}} = 3e^{-\frac{3}{2}}$

(ii) $n=4$일 때, ㉠에서 $t=-2$ (중근)
범위 $t \ge -2$에 의하여 $y=f(x)$는 $x=a_{4}=e^{-2}$에서 최솟값을 갖는다.
$b_{4} = \{2 \times 4 + 4 \times (-2) + 4\}e^{-2} = 4e^{-2}$

(iii) $n=5$일 때, ㉠에서 $t=-\frac{5}{2}$ 또는 $t=-2$
범위 $t \ge -\frac{5}{2}$에 의하여 $y=f(x)$는 $x=a_{5}=e^{-2}$에서 최솟값을 갖는다.
$b_{5} = \{2 \times 4 + 5 \times (-2) + 5\}e^{-2} = 3e^{-2}$

(iv) $n=6$일 때, ㉠에서 $t=-3$ 또는 $t=-2$
범위 $t \ge -3$에 의하여 $y=f(x)$는 $x=a_{6}=e^{-2}$에서 최솟값을 갖는다.
$b_{6} = \{2 \times 4 + 6 \times (-2) + 6\}e^{-2} = 2e^{-2}$

$\therefore \frac{b_{3}}{a_{3}}+\frac{b_{4}}{a_{4}}+\frac{b_{5}}{a_{5}}+\frac{b_{6}}{a_{6}}$
$= \frac{3e^{-\frac{3}{2}}}{e^{-\frac{3}{2}}} + \frac{4e^{-2}}{e^{-2}} + \frac{3e^{-2}}{e^{-2}} + \frac{2e^{-2}}{e^{-2}}$
$= 3+4+3+2 = 12$

정답 ②