## 문제
함수 $f(x) = \frac{x+3}{x}$에 대하여 두 수열 $\{a_{n}\}$, $\{b_{n}\}$은 다음 조건을 만족시킨다.

(가) $a_{1} = 1$
(나) $b_{n} = f(a_{n})$
(다) $a_{n+1} = a_{n} b_{n}$

이때, $\lim_{n \to \infty} \left( \frac{a_{n}}{n} + b_{n} \right)$의 값은?

## 보기
① $1$   ② $2$   ③ $3$   ④ $4$   ⑤ $5$

## 풀이
$a_{1} = 1$, $b_{1} = 4$

$b_{n} = f(a_{n}) = \frac{a_{n} + 3}{a_{n}}$

(다) 조건에 의해 $a_{n+1} = a_{n} b_{n}$이므로
$a_{n+1} = a_{n} \cdot \frac{a_{n} + 3}{a_{n}} = a_{n} + 3$

따라서 수열 $\{a_{n}\}$은 첫째항이 $1$이고 공차가 $3$인 등차수열이다.
$a_{n} = 1 + (n - 1) \cdot 3 = 3n - 2$
$b_{n} = \frac{a_{n} + 3}{a_{n}} = \frac{3n + 1}{3n - 2}$

그러므로
$\lim_{n \to \infty} \left( \frac{a_{n}}{n} + b_{n} \right)$
$= \lim_{n \to \infty} \left( \frac{3n - 2}{n} + \frac{3n + 1}{3n - 2} \right)$
$= \lim_{n \to \infty} \left( 3 - \frac{2}{n} \right) + \lim_{n \to \infty} \left( \frac{3 + \frac{1}{n}}{3 - \frac{2}{n}} \right)$
$= 3 + 1 = 4$

정답은 ④이다.