## 문제
행렬 $A = \left( \begin{array}{cc} 2 & -1 \\ -3 & 1 \end{array} \right)$ 에 대하여 행렬 $B$ 가 $A - 2B = \left( \begin{array}{cc} -3 & -1 \\ 1 & 0 \end{array} \right)$ 을 만족시킬 때, 행렬 $B$ 의 모든 성분의 합은?

## 보기
① $1$   ② $3$   ③ $5$   ④ $7$   ⑤ $9$

## 풀이
$A - 2B = \left( \begin{array}{cc} -3 & -1 \\ 1 & 0 \end{array} \right)$ 이므로
$$ 2B = A - \left( \begin{array}{cc} -3 & -1 \\ 1 & 0 \end{array} \right) $$
$$ 2B = \left( \begin{array}{cc} 2 & -1 \\ -3 & 1 \end{array} \right) - \left( \begin{array}{cc} -3 & -1 \\ 1 & 0 \end{array} \right) $$
$$ 2B = \left( \begin{array}{cc} 2 - (-3) & -1 - (-1) \\ -3 - 1 & 1 - 0 \end{array} \right) = \left( \begin{array}{cc} 5 & 0 \\ -4 & 1 \end{array} \right) $$
이므로
$$ B = \frac{1}{2} \left( \begin{array}{cc} 5 & 0 \\ -4 & 1 \end{array} \right) $$
따라서 행렬 $B$ 의 모든 성분의 합은
$$ \frac{1}{2} \times (5 + 0 - 4 + 1) = \frac{1}{2} \times 2 = 1 $$
정답은 ① 이다.