## 문제
다음 등식을 만족시키는 자연수 $n$ 의 값을 구하시오.
$$ \sum_{k=1}^{n+1} k^{2} - \sum_{k=1}^{n} (k^{2}+k) = 78 $$

## 보기

## 풀이
$$ \sum_{k=1}^{n+1} k^{2} - \sum_{k=1}^{n} (k^{2}+k) $$
$$ = \sum_{k=1}^{n} k^{2} + (n+1)^{2} - \sum_{k=1}^{n} (k^{2}+k) $$
$$ = (n+1)^{2} + \sum_{k=1}^{n} k^{2} - \sum_{k=1}^{n} (k^{2}+k) $$
$$ = (n+1)^{2} + \sum_{k=1}^{n} \{ k^{2} - (k^{2} + k) \} $$
$$ = (n+1)^{2} - \sum_{k=1}^{n} k $$
$$ = (n+1)^{2} - \frac{n(n+1)}{2} $$
$$ = \frac{(n+1)(n+2)}{2} $$
따라서 
$$ \frac{(n+1)(n+2)}{2} = 78 $$
$$ n^{2} + 3n - 154 = 0 $$
$$ (n-11)(n+14) = 0 $$
$\therefore$ $n$=$11$ ($\because$ $n$ 은 자연수)

정답: $11$