## 문제
다항함수 $f(x)$ 에 대하여 $\lim_{x \to 2} \frac{f(x) - 1}{x - 2} = 2$ 일 때, $\lim_{h \to 0} \frac{f(2 + h) - f(2 - h)}{h}$ 의 값은?

## 보기
① $-2$   ② $-1$   ③ $1$   ④ $2$   ⑤ $4$

## 풀이
[정답] ⑤

$\lim_{x \to 2} (x - 2) = 0$ 이므로 
$\lim_{x \to 2} \{ f(x) - 1 \} = 0$
$\therefore f(2) = 1$

$\lim_{x \to 2} \frac{f(x) - 1}{x - 2} = \lim_{x \to 2} \frac{f(x) - f(2)}{x - 2} = f'(2) = 2$

$\lim_{h \to 0} \frac{f(2 + h) - f(2 - h)}{h}$
$= \lim_{h \to 0} \frac{f(2 + h) - f(2)}{h} + \lim_{h \to 0} \frac{f(2 - h) - f(2)}{-h}$
$= f'(2) + f'(2) = 2f'(2)$
$= 2 \times 2 = 4$