## 문제
수열 $\{ a_{n} \}$ 을 다음과 같이 정의하자. 

$a_{n} = \int_{0}^{1} x^{n}(x-1) dx$ ($n=1, 2, 3, \dots$) 

$\sum_{n=1}^{10} a_{n}$ 의 값은?

## 보기
① $-\frac{5}{12}$  ② $-\frac{1}{3}$  ③ $-\frac{1}{4}$  ④ $-\frac{1}{6}$  ⑤ $-\frac{1}{12}$

## 풀이
$a_{n} = \int_{0}^{1} (x^{n+1}-x^{n}) dx$ 이므로 

$\sum_{n=1}^{10} a_{n}$ 
$= \int_{0}^{1} (x^{2}-x) dx + \int_{0}^{1} (x^{3}-x^{2}) dx + \dots + \int_{0}^{1} (x^{11}-x^{10}) dx$ 
$= \int_{0}^{1} \{ (x^{2}-x) + (x^{3}-x^{2}) + \dots + (x^{11}-x^{10}) \} dx$ 
$= \int_{0}^{1} (x^{11}-x) dx$ 
$= \left[ \frac{x^{12}}{12} - \frac{x^{2}}{2} \right]_{0}^{1} = -\frac{5}{12}$ 

**[다른 풀이]** 

$a_{n} = \int_{0}^{1} (x^{n+1}-x^{n}) dx$ 
$= \left[ \frac{x^{n+2}}{n+2} - \frac{x^{n+1}}{n+1} \right]_{0}^{1}$ 
$= \frac{1}{n+2} - \frac{1}{n+1}$ 

$\therefore \sum_{n=1}^{10} a_{n}$ 
$= \sum_{n=1}^{10} \left( \frac{1}{n+2} - \frac{1}{n+1} \right)$ 
$= \left( \frac{1}{3} - \frac{1}{2} \right) + \left( \frac{1}{4} - \frac{1}{3} \right) + \dots + \left( \frac{1}{12} - \frac{1}{11} \right)$ 
$= \frac{1}{12} - \frac{1}{2} = -\frac{5}{12}$ 

정답: ①