## ë¬¸ì œ

> [!example] ğŸ“¸ (ê·¸ë¦¼/ê·¸ë˜í”„)

í•¨ìˆ˜ 
$$ f(x) = \begin{cases} x+2 & (x \leq 0) \\ -\frac{1}{2}x & (x > 0) \end{cases} $$
ì˜ ê·¸ë˜í”„ê°€ ê·¸ë¦¼ê³¼ ê°™ë‹¤. í•¨ìˆ˜ $g(x)=f(x)\{ f(x)+k \}$ ê°€ $x=0$ ì—ì„œ ì—°ì†ì´ ë˜ë„ë¡ í•˜ëŠ” ìƒìˆ˜ $k$ ì˜ ê°’ì€?

## ë³´ê¸°

â‘  $-2$   â‘¡ $-1$   â‘¢ $0$   â‘£ $1$   â‘¤ $2$

## í’€ì´

[ì •ë‹µ] â‘  

(i) 
$$ g(0)=f(0) \{ f(0)+k \} $$ 
$$ =2(2+k)=2k+4 $$ 

(ii) 
$$ \lim_{x \to 0+} g(x) $$ 
$$ = \lim_{x \to 0+} f(x) \{ f(x)+k \} $$ 
$$ = \lim_{x \to 0+} f(x) \times \lim_{x \to 0+} \{ f(x)+k \} $$ 
$$ = 0 \times k = 0 $$ 

(iii) 
$$ \lim_{x \to 0-} g(x) $$ 
$$ = \lim_{x \to 0-} f(x) \{ f(x)+k \} $$ 
$$ = \lim_{x \to 0-} f(x) \times \lim_{x \to 0-} \{ f(x)+k \} $$ 
$$ = 2 \times (2+k) = 2k+4 $$ 

(i), (ii), (iii)ì— ì˜í•˜ì—¬ í•¨ìˆ˜ $g(x)$ ê°€ $x=0$ ì—ì„œ ì—°ì†ì´ ë˜ì–´ì•¼ í•˜ë¯€ë¡œ 
$$ 2k+4=0 $$ 
$$ \therefore k=-2 $$