## ë¬¸ì œ
ìì—°ìˆ˜ $n$ì— ëŒ€í•˜ì—¬ ê³¡ì„  $y = \frac{2n}{x}$ê³¼ ì§ì„  $y = -\frac{x}{n} + 3$ì˜ ë‘ êµì ì„ $A_n$, $B_n$ì´ë¼ í•˜ì. ê³¡ì„  $y = \frac{2n}{x}$ê³¼ ì§ì„  $y = -\frac{x}{n} + 3$ìœ¼ë¡œ ë‘˜ëŸ¬ì‹¸ì¸ ë¶€ë¶„ì˜ ë„“ì´ë¥¼ $S_n$ì´ë¼ í•  ë•Œ, $S_{n+1} - S_n$ì˜ ê°’ì€?



> [!example] ğŸ“¸ (ê·¸ë¦¼/ê·¸ë˜í”„)

## ë³´ê¸°
â‘  $\frac{3}{2} - 2\ln 2$   â‘¡ $1 - \ln 2$   â‘¢ $\frac{3}{2} - \ln 2$   â‘£ $1 + \ln 2$   â‘¤ $\frac{3}{2} + 2\ln 2$

## í’€ì´
ê³¡ì„  $y = \frac{2n}{x}$ê³¼ ì§ì„  $y = -\frac{x}{n} + 3$ì˜ êµì ì´ $A_n (n, 2)$, $B_n (2n, 1)$ì´ê³ , $n \le x \le 2n$ì—ì„œ $\frac{2n}{x} \le -\frac{x}{n} + 3$ì´ë¯€ë¡œ 
$S_n = \int_n^{2n} \left( -\frac{x}{n} + 3 - \frac{2n}{x} \right) dx$
$= \left[ -\frac{1}{2n} x^2 + 3x - 2n \ln |x| \right]_n^{2n}$
$= ( - 2n + 6n - 2n \ln 2n ) - ( - \frac{1}{2}n + 3n - 2n \ln n )$
$= n \left( \frac{3}{2} - 2 \ln 2 \right)$
ë”°ë¼ì„œ $S_{n+1} - S_n = (n+1) \left( \frac{3}{2} - 2 \ln 2 \right) - n \left( \frac{3}{2} - 2 \ln 2 \right) = \frac{3}{2} - 2\ln 2$

ì •ë‹µ: â‘ 