## 문제
모든 항이 양수인 등비수열 $\{ a_{n} \}$ 이 $a_{10} = 8 a_{4}$, $a_{3} + a_{7} = 10$ 을 만족시킬 때, $\sum_{n=1}^{10} \frac{a_{n+1} - a_{n}}{(a_{n} + 1)(a_{n+1} + 1)}$ 의 값은?

## 보기
① $\frac{31}{66}$   ② $\frac{17}{33}$   ③ $\frac{37}{66}$   ④ $\frac{20}{33}$   ⑤ $\frac{43}{66}$

## 풀이
[정답] ①

등비수열 $\{ a_{n} \}$ 의 첫째항을 $a$, 공비를 $r$ 라 하면 
$a_{10} = 8 a_{4}$ 에서 $a r^{9} = 8 a r^{3}$, $a r^{3} (r^{6} - 8) = 0$ 
$a r \neq 0$ 이므로 $r^{6} = 8$ 즉, $r = \sqrt{2}$ ($\because a_{n} > 0$) 

$a_{3} + a_{7} = 10$ 에서 $a r^{2} + a r^{6} = 10$ 이므로 
$a (\sqrt{2})^{2} + a (\sqrt{2})^{6} = 2 a + 8 a = 10$
$10 a = 10$
$a = 1$ 

$\therefore a_{n} = (\sqrt{2})^{n-1}$ 

$\sum_{n=1}^{10} \frac{a_{n+1} - a_{n}}{(a_{n} + 1)(a_{n+1} + 1)}$ 
$= \sum_{n=1}^{10} \frac{(a_{n+1} + 1) - (a_{n} + 1)}{(a_{n} + 1)(a_{n+1} + 1)}$
$= \sum_{n=1}^{10} \left( \frac{1}{a_{n} + 1} - \frac{1}{a_{n+1} + 1} \right)$ 
$= \frac{1}{a_{1} + 1} - \frac{1}{a_{11} + 1}$

$a_{1} = 1$ 이고 $a_{11} = (\sqrt{2})^{10} = 2^{5} = 32$ 이므로
$= \frac{1}{1 + 1} - \frac{1}{32 + 1} = \frac{1}{2} - \frac{1}{33} = \frac{31}{66}$ 

따라서 $\sum_{n=1}^{10} \frac{a_{n+1} - a_{n}}{(a_{n} + 1)(a_{n+1} + 1)} = \frac{31}{66}$ 이다.