## 문제
지수부등식 $(\frac{1}{3})^{x^{2}+1} > (\frac{1}{9})^{x+2}$ 의 해가 $\alpha < x < \beta$ 일 때, $\beta - \alpha$ 의 값은?

## 보기
① $4$  ② $5$  ③ $6$  ④ $7$  ⑤ $8$

## 풀이
$(\frac{1}{3})^{x^{2}+1} > (\frac{1}{9})^{x+2}$ 에서
$(\frac{1}{3})^{x^{2}+1} > ((\frac{1}{3})^{2})^{x+2}$
$(\frac{1}{3})^{x^{2}+1} > (\frac{1}{3})^{2(x+2)}$
밑이 $0 < \frac{1}{3} < 1$ 이므로 지수의 부동호 방향이 바뀐다.
$x^{2} + 1 < 2(x+2)$
$x^{2} - 2x - 3 < 0$
$(x+1)(x-3) < 0$
$\therefore -1 < x < 3$
따라서 $\alpha = -1$, $\beta = 3$ 이므로
$\beta - \alpha = 3 - (-1) = 4$

정답: ①