## 문제
서로 다른 두 실수 $a$, $b$에 대하여 
$$\frac{(a-5)^{2}}{a-b} + \frac{(b-5)^{2}}{b-a} = 0$$
일 때, $a+b$의 값을 구하시오.

## 보기

## 풀이
$$\frac{(a-5)^{2}}{a-b} + \frac{(b-5)^{2}}{b-a}$$ 
$$= \frac{(a-5)^{2}}{a-b} - \frac{(b-5)^{2}}{a-b}$$ 
$$= \frac{(a-5)^{2} - (b-5)^{2}}{a-b}$$ 
$$= \frac{(a^{2} - 10a + 25) - (b^{2} - 10b + 25)}{a-b}$$ 
$$= \frac{a^{2} - 10a + 25 - b^{2} + 10b - 25}{a-b}$$ 
$$= \frac{a^{2} - b^{2} - 10a + 10b}{a-b}$$ 
$$= \frac{(a+b)(a-b) - 10(a-b)}{a-b}$$ 
$$= \frac{(a+b-10)(a-b)}{a-b}$$ 
$$= a+b-10 = 0$$ 
따라서 
$$a+b=10$$

[정답] $10$