## 문제
두 수열 $\{a_{n}\}$, $\{b_{n}\}$의 일반항이 각각 $a_{n}= \left( \frac{1}{2} \right)^{n-1}$과 $b_{n}=2 \left( \frac{1}{3} \right)^{n-1}$일 때, $\sum_{n=1}^{\infty} \left( \sum_{k=1}^{n} a_{k} b_{n-k+1} \right)$의 값은?

## 보기
① $6$   ② $8$   ③ $9$   ④ $10$   ⑤ $12$

## 풀이
$a_{k} b_{n-k+1}$
$= \left( \frac{1}{2} \right)^{k-1} \cdot 2 \left( \frac{1}{3} \right)^{n-k}$
$= 2 \left( \frac{1}{2} \right)^{k-1} \left( \frac{1}{3} \right)^{n-1} \left( \frac{1}{3} \right)^{-k+1}$
$= 2 \left( \frac{1}{3} \right)^{n-1} \left( \frac{3}{2} \right)^{k-1}$

$\therefore \sum_{k=1}^{n} a_{k} b_{n-k+1}$
$= \sum_{k=1}^{n} 2 \left( \frac{1}{3} \right)^{n-1} \left( \frac{3}{2} \right)^{k-1}$
$= 2 \left( \frac{1}{3} \right)^{n-1} \cdot \sum_{k=1}^{n} \left( \frac{3}{2} \right)^{k-1}$
$= 2 \left( \frac{1}{3} \right)^{n-1} \cdot \frac{\left( \frac{3}{2} \right)^{n}-1}{\frac{3}{2}-1}$
$= 4 \left( \frac{1}{3} \right)^{n-1} \left\{ \left( \frac{3}{2} \right)^{n}-1 \right\}$
$= 6 \left( \frac{1}{2} \right)^{n-1}-4 \left( \frac{1}{3} \right)^{n-1}$

$\therefore \sum_{n=1}^{\infty} \left( \sum_{k=1}^{n} a_{k} b_{n-k+1} \right)$
$= \sum_{n=1}^{\infty} \left\{ 6 \left( \frac{1}{2} \right)^{n-1}-4 \left( \frac{1}{3} \right)^{n-1} \right\}$
$= \frac{6}{1-\frac{1}{2}}-\frac{4}{1-\frac{1}{3}}$
$= 12-6$
$= 6$

정답: ①