## 문제
수열 $\{ a_{n} \}$ 이 자연수 $n$ 에 대하여 
$$ \sum_{k=1}^{n}(-1)^{k} a_{k}=n^{3} $$
을 만족시킬 때, $\lim_{n \to \infty} \frac{a_{2 n-1}+a_{2 n}}{n}$ 의 값을 구하시오.

## 풀이
$-a_{1}=1$ 이므로 $a_{1}=-1$ 이다. 

$S_{n}=\sum_{k=1}^{n}(-1)^{k} a_{k}$ 라 하면 
$(-1)^{n} a_{n} = S_{n}-S_{n-1}$ 
$= \sum_{k=1}^{n}(-1)^{k} a_{k}- \sum_{k=1}^{n-1}(-1)^{k} a_{k}$ 
$= n^{3}-(n-1)^{3}$ 
$= 3 n^{2}-3 n+1$ ($n \geq 2$) 

따라서 
$a_{2 n}=12 n^{2}-6 n+1$ 
$a_{2 n-1}=-12 n^{2}+18 n-7$ 
이므로 
$a_{2 n-1}+a_{2 n}=12 n-6$ 

$\therefore \lim _{n \to \infty} \frac{a_{2 n-1}+a_{2 n}}{n} = \lim _{n \to \infty} \frac{12 n-6}{n}=12$

정답: $12$