## 문제
두 행렬 $A = \left( \begin{array}{cc} 1 & 1 \\ 2 & 3 \end{array} \right)$, $B = \left( \begin{array}{cc} -1 & a \\ b & -1 \end{array} \right)$ 에 대하여 $(AB)^{-1} = \left( \begin{array}{cc} -1 & 1 \\ 1 & 0 \end{array} \right)$ 일 때, $a+b$ 의 값은?

## 보기
① $2$   ② $3$   ③ $4$   ④ $5$   ⑤ $6$

## 풀이
$(AB)^{-1} = \left( \begin{array}{cc} -1 & 1 \\ 1 & 0 \end{array} \right)$ 에서 
$$ AB = \left( \begin{array}{cc} -1 & 1 \\ 1 & 0 \end{array} \right)^{-1} $$
$$ = \frac{1}{(-1) \times 0 - 1 \times 1} \left( \begin{array}{cc} 0 & -1 \\ -1 & -1 \end{array} \right) $$
$$ = \left( \begin{array}{cc} 0 & 1 \\ 1 & 1 \end{array} \right) \cdots ㉠ $$

$A = \left( \begin{array}{cc} 1 & 1 \\ 2 & 3 \end{array} \right)$, $B = \left( \begin{array}{cc} -1 & a \\ b & -1 \end{array} \right)$ 이므로 
$$ AB = \left( \begin{array}{cc} 1 & 1 \\ 2 & 3 \end{array} \right) \left( \begin{array}{cc} -1 & a \\ b & -1 \end{array} \right) = \left( \begin{array}{cc} -1+b & a-1 \\ -2+3b & 2a-3 \end{array} \right) \cdots ㉡ $$

$㉠, ㉡$ 에서 
$-1+b = 0$, $a-1 = 1$, $-2+3b = 1$, $2a-3 = 1$ 이므로 
$a = 2$, $b = 1$ 

따라서 $a+b = 3$ 

정답: ②