## 문제

수열 $\{ a_{n} \}$ 이 자연수 $n$ 에 대하여 
$\sum_{k=1}^{n} \frac{a_{k}}{k+1} = n^{2} + n$
을 만족시킬 때, $\sum_{n=1}^{10} \frac{1}{a_{n}}$ 의 값은? 

## 보기

① $\frac{5}{11}$   ② $\frac{1}{2}$   ③ $\frac{6}{11}$   ④ $\frac{13}{22}$   ⑤ $\frac{7}{11}$

## 풀이

$\sum_{k=1}^{n} \frac{a_{k}}{k+1} = n^{2} + n$ 을 전개하면 
$\frac{a_{1}}{2} + \frac{a_{2}}{3} + \frac{a_{3}}{4} + \dots + \frac{a_{n}}{n+1} = n^{2} + n \dots$ ㉠ 
㉠에 의해 $2$ 이상의 자연수 $n$ 에 대하여 
$\frac{a_{1}}{2} + \frac{a_{2}}{3} + \frac{a_{3}}{4} + \dots + \frac{a_{n-1}}{n} = (n-1)^{2} + (n-1) \dots$ ㉡ 
㉠ $-$ ㉡에서 
$\frac{a_{n}}{n+1} = n^{2} + n - \{ (n-1)^{2} + (n-1) \}$ 
$= 2n$ 
$\therefore a_{n} = 2n(n+1) \quad (n = 2, 3, 4, \dots)$ 
한편 ㉠에서 
$\frac{a_{1}}{2} = 1^{2} + 1$, $a_{1} = 4$ 
$\therefore a_{n} = 2n(n+1) \quad (n = 1, 2, 3, \dots)$ 
$\sum_{n=1}^{10} \frac{1}{a_{n}} = \sum_{n=1}^{10} \frac{1}{2n(n+1)}$ 
$= \frac{1}{2} \sum_{n=1}^{10} \left( \frac{1}{n} - \frac{1}{n+1} \right)$ 
$= \frac{1}{2} \{ (1 - \frac{1}{2}) + (\frac{1}{2} - \frac{1}{3}) + (\frac{1}{3} - \frac{1}{4}) + \dots + (\frac{1}{10} - \frac{1}{11}) \}$ 
$= \frac{1}{2} (1 - \frac{1}{11})$ 
$= \frac{5}{11}$

정답: ①