## 문제
다항함수 $f(x)$ 가
$\lim_{x \to 0} \frac{x}{f(x)} = 1$, $\lim_{x \to 1} \frac{x-1}{f(x)} = 2$
를 만족시킬 때, $\lim_{x \to 1} \frac{f(f(x))}{2x^2 - x - 1}$ 의 값은?

## 보기
① $\frac{1}{6}$   ② $\frac{1}{3}$   ③ $\frac{1}{2}$   ④ $\frac{2}{3}$   ⑤ $\frac{5}{6}$

## 풀이
$\lim_{x \to 0} \frac{x}{f(x)} = 1$ 에서 $x \to 0$ 일 때, (분자) $\to 0$ 이므로 (분모) $\to 0$ 이어야 한다.
$\therefore f(0) = 0$

$\lim_{x \to 0} \frac{x}{f(x)} = \lim_{x \to 0} \frac{x}{f(x) - f(0)} = \lim_{x \to 0} \frac{1}{\frac{f(x) - f(0)}{x}} = \frac{1}{f'(0)} = 1$
$\therefore f'(0) = 1$

$\lim_{x \to 1} \frac{x-1}{f(x)} = 2$ 에서 $x \to 1$ 일 때, (분자) $\to 0$ 이므로 (분모) $\to 0$ 이어야 한다.
$\therefore f(1) = 0$

$\lim_{x \to 1} \frac{x-1}{f(x)} = \lim_{x \to 1} \frac{x-1}{f(x) - f(1)} = \lim_{x \to 1} \frac{1}{\frac{f(x) - f(1)}{x-1}} = \frac{1}{f'(1)} = 2$
$\therefore f'(1) = \frac{1}{2}$

따라서
$\lim_{x \to 1} \frac{f(f(x))}{2x^2 - x - 1}$
$= \lim_{x \to 1} \left( \frac{f(f(x)) - f(f(1))}{f(x) - f(1)} \cdot \frac{f(x) - f(1)}{x - 1} \cdot \frac{1}{2x + 1} \right)$
$= f'(f(1)) \cdot f'(1) \cdot \frac{1}{3}$
$= f'(0) \cdot \frac{1}{2} \cdot \frac{1}{3}$
$= 1 \cdot \frac{1}{2} \cdot \frac{1}{3} = \frac{1}{6}$

**[다른 풀이]**
$\lim_{x \to 1} \frac{f(f(x))}{2x^2 - x - 1} = \lim_{x \to 1} \frac{f(f(x))}{(x - 1)(2x + 1)}$
$= \lim_{x \to 1} \left( \frac{f(f(x))}{f(x)} \times \frac{f(x)}{x - 1} \times \frac{1}{2x + 1} \right)$
$= \lim_{x \to 1} \frac{f(f(x))}{f(x)} \times \lim_{x \to 1} \frac{1}{\frac{x - 1}{f(x)}} \times \lim_{x \to 1} \frac{1}{2x + 1}$
$x \to 1$ 일 때 $f(x) \to 0$ 이므로, $f(x) = t$ 로 치환하면 $t \to 0$ 이다.
$= \lim_{t \to 0} \frac{f(t)}{t} \times \lim_{x \to 1} \frac{1}{\frac{x - 1}{f(x)}} \times \lim_{x \to 1} \frac{1}{2x + 1}$
$= 1 \times \frac{1}{2} \times \frac{1}{3} = \frac{1}{6}$

정답: ①