## 문제

수열 $\{ $ $a_{n}$ $ \}$은 $a_{1}$ $=$ $2$이고,
$n^{2}$ $a_{n+1}$ $=$ $(n^{2}$ $-$ $1)$ $a_{n}$ $+$ $n$ $(n$ $+$ $1)$ $2^{n}$ ($n$ $\geq$ $1$)
을 만족시킨다. 다음은 일반항 $a_{n}$을 구하는 과정이다.

주어진 식에 의하여
$a_{n+1}$ $=$ $\frac{(n+1)(n-1)}{n^{2}}$ $a_{n}$ $+$ $\frac{n+1}{n}$ $2^{n}$
이다. $b_{n}$ $=$ $\frac{n-1}{n}$ $a_{n}$이라 하면
$b_{n+1}$ $=$ $b_{n}$ $+$ $(가)$ ($n$ $\geq$ $1$)
이고, $b_{1}$ $=$ $0$이므로
$b_{n}$ $=$ $(나)$ ($n$ $\geq$ $1$)
이다. 그러므로
$a_{n}$ $=$ $\begin{cases} 2 & (n=1) \\ \frac{n}{n-1} \times (나) & (n \geq 2) \end{cases}$
이다. 위의 $(가)$, $(나)$에 알맞은 식을 각각 $f(n)$, $g(n)$이라 할 때, $f(5)$ $+$ $g(10)$의 값은?

## 보기
① $1014$   ② $1024$   ③ $1034$   ④ $1044$   ⑤ $1054$

## 풀이
[정답] ⑤

$b_{n}$ $=$ $\frac{n-1}{n}$ $a_{n}$이므로 
$b_{n+1}$ $=$ $\frac{n}{n+1}$ $a_{n+1}$
따라서, $a_{n+1}$ $=$ $\frac{(n+1)(n-1)}{n^{2}}$ $a_{n}$ $+$ $\frac{n+1}{n}$ $2^{n}$에서
$\frac{n}{n+1}$ $a_{n+1}$ $=$ $\frac{n-1}{n}$ $a_{n}$ $+$ $2^{n}$
이므로 
$b_{n+1}$ $=$ $b_{n}$ $+$ $2^{n}$
이때, $b_{n+1}$ $-$ $b_{n}$ $=$ $2^{n}$이므로 
$b_{n}$ $=$ $b_{1}$ $+$ $\sum_{k=1}^{n-1}$ $2^{k}$
$=$ $0$ $+$ $\frac{2(2^{n-1}-1)}{2-1}$ $=$ $2^{n}$ $-$ $2$ ($n$ $\geq$ $2$) $\cdots$ ㉠ 
그런데, ㉠에 $n$ $=$ $1$을 대입하면 $b_{1}$ $=$ $0$이므로 
$b_{n}$ $=$ $2^{n}$ $-$ $2$ ($n$ $\geq$ $1$)
그러므로 
$a_{n}$ $=$ $\begin{cases} 2 & (n=1) \\ \frac{n}{n-1} \times (2^{n}-2) & (n \geq 2) \end{cases}$
따라서 $f(n)$ $=$ $2^{n}$, $g(n)$ $=$ $2^{n}$ $-$ $2$이므로 
$f(5)$ $+$ $g(10)$
$=$ $2^{5}$ $+$ $(2^{10}-2)$
$=$ $32$ $+$ $1022$ $=$ $1054$