## 문제
선분 $A_{n}B_{n}$ 의 길이를 $l_{n}$ 이라 할 때, $\lim_{n \to \infty} (l_{n+1}-l_{n})$ 의 값은?

## 보기
① $\frac{1}{2}$   ② $\frac{\sqrt{2}}{2}$   ③ $1$   ④ $\sqrt{2}$   ⑤ $2$

## 풀이
[정답] ③

$y=\frac{2n}{x}$ 에 $y=-\frac{x}{n}+3$ 를 대입하면
$\frac{2n}{x}=-\frac{x}{n}+3$
$2n^{2}=-x^{2}+3nx$
$x^{2}-3nx+2n^{2}=0$
$(x-n)(x-2n)=0$
$\therefore x=n$ 또는 $x=2n$
$A_{n}(n, 2)$, $B_{n}(2n, 1)$
$\therefore l_{n}= \sqrt{(2n-n)^{2}+(1-2)^{2}}= \sqrt{n^{2}+1}$
$\lim_{n \to \infty} (l_{n+1}-l_{n})$
$= \lim_{n \to \infty} (\sqrt{(n+1)^{2}+1}-\sqrt{n^{2}+1})$
$= \lim_{n \to \infty} (\sqrt{n^{2}+2n+2}-\sqrt{n^{2}+1})$
$= \lim_{n \to \infty} \frac{n^{2}+2n+2-(n^{2}+1)}{\sqrt{n^{2}+2n+2}+\sqrt{n^{2}+1}}$
$= \lim_{n \to \infty} \frac{2n+1}{\sqrt{n^{2}+2n+2}+\sqrt{n^{2}+1}}$
$= \lim_{n \to \infty} \frac{2+\frac{1}{n}}{\sqrt{1+\frac{2}{n}+\frac{2}{n^{2}}}+\sqrt{1+\frac{1}{n^{2}}}}$
$= 1$