## 문제
선분 $A_{n} C_{n}$ 의 길이를 $f(n)$, 선분 $B_{n} C_{n}$ 의 길이를 $g(n)$ 이라 할 때, $\lim_{n \to \infty} n \{ f(n) - g(n) \}$ 의 값은?

## 보기
① $\frac{1}{5}$   ② $\frac{1}{4}$   ③ $\frac{1}{3}$   ④ $\frac{1}{2}$   ⑤ $1$

## 풀이
점 $A_{n}$ 이 곡선 $y = 2^{x}$ 위에 있으므로 $A_{n} ( \log_{2} n, n )$ 이다.
점 $B_{n}$ 의 좌표를 $( b_{n}, n )$ 이라 하면 점 $B_{n}$ 이 곡선 $y = 2^{x-1}$ 위의 점이므로 $2^{b_{n}-1} = n$ 이다.
$b_{n} - 1 = \log_{2} n$, $b_{n} = 1 + \log_{2} n = \log_{2} 2n$
$\therefore B_{n} ( \log_{2} 2n, n )$
또, 점 $C_{n}$ 이 곡선 $y = 2^{x}$ 위에 있으므로 $C_{n} ( \log_{2} 2n, 2n )$ 이다.
따라서 $\overline{A_{n} B_{n}} = 1$, $\overline{B_{n} C_{n}} = 2n - n = n$ 이므로
$\overline{A_{n} C_{n}} = \sqrt{n^{2} + 1}$ 이다.
$\therefore f(n) = \sqrt{n^{2} + 1}$, $g(n) = n$
$\therefore \lim_{n \to \infty} n \{ f(n) - g(n) \}$
$= \lim_{n \to \infty} n ( \sqrt{n^{2} + 1} - n )$
$= \lim_{n \to \infty} \frac{n ( \sqrt{n^{2} + 1} - n ) ( \sqrt{n^{2} + 1} + n )}{( \sqrt{n^{2} + 1} + n )}$
$= \lim_{n \to \infty} \frac{n}{\sqrt{n^{2} + 1} + n}$
$= \lim_{n \to \infty} \frac{1}{\sqrt{1 + \frac{1}{n^{2}}} + 1}$
$= \frac{1}{2}$

정답: ④