## 문제
수열 $\{ a_{n} \}$은 $a_{1} = 1$이고 $a_{n+1} = f (f (a_{n} ) ) \ (n \ge 1)$을 만족시킬 때, $\lim_{n \to \infty} a_{n}$의 값은?

## 보기
① $\frac{1}{3}$   ② $\frac{2}{3}$   ③ $1$   ④ $\frac{4}{3}$   ⑤ $\frac{5}{3}$

## 풀이
$a_{1} = 1$ 
$a_{2} = f (f (a_{1} ) ) = f (f (1) ) = f (-\frac{1}{2} ) = -\frac{1}{2} + 2$ 
$a_{3} = f (f (a_{2} ) ) = f ( (-\frac{1}{2} )^{2} + 2 (-\frac{1}{2} ) ) = (-\frac{1}{2} )^{2} + 2 (-\frac{1}{2} ) + 2$ 
$\cdots$ 
$a_{n} = (-\frac{1}{2} )^{n-1} + 2 (-\frac{1}{2} )^{n-2} + \cdots + 2 = (-\frac{1}{2} )^{n-1} + \sum_{k=1}^{n-1} 2 (-\frac{1}{2} )^{k-1}$ 
따라서, 
$\lim_{n \to \infty} a_{n} = \lim_{n \to \infty} \left\{ (-\frac{1}{2} )^{n-1} + \sum_{k=1}^{n-1} 2 (-\frac{1}{2} )^{k-1} \right\}$ 
$= \frac{2}{1 - (-\frac{1}{2} )} = \frac{4}{3}$

정답: ④