## ë¬¸ì œ

ê·¸ë¦¼ì€ ë‹¤ìŒ ì¡°ê±´ì„ ë§Œì¡±ì‹œí‚¤ëŠ” í•¨ìˆ˜ $y=f(x)$ì˜ ê·¸ë˜í”„ì˜ ì¼ë¶€ì´ë‹¤.

(ê°€) $f(x)=2|x-1|$ ($0 \leq x \leq 2$)
(ë‚˜) ëª¨ë“  ì‹¤ìˆ˜ $x$ì— ëŒ€í•˜ì—¬ $f(x+2)=f(x)$ì´ë‹¤.

> [!example] ğŸ“¸ (ê·¸ë¦¼/ê·¸ë˜í”„)

$g(k)=\int_{2k}^{4k} f(x) dx$ë¼ í•  ë•Œ, $\lim_{n \to \infty} \frac{1}{n^{2}} \sum_{k=1}^{n} g(k)$ì˜ ê°’ì€?

## ë³´ê¸°

â‘  $1$   â‘¡ $\frac{3}{2}$   â‘¢ $2$   â‘£ $\frac{5}{2}$   â‘¤ $3$

## í’€ì´

$\int_{0}^{2} f(x) dx = \int_{0}^{1} 2(1-x) dx + \int_{1}^{2} 2(x-1) dx = 2$

$\int_{0}^{2} f(x) dx = \int_{2}^{4} f(x) dx = \cdots = \int_{2(k-1)}^{2k} f(x) dx = 2$

$\int_{0}^{2k} f(x) dx = 2k$ ($k$ëŠ” ìì—°ìˆ˜)

$g(k) = \int_{2k}^{4k} f(x) dx = \int_{0}^{4k} f(x) dx - \int_{0}^{2k} f(x) dx = 4k-2k=2k$

$\therefore \lim_{n \to \infty} \frac{1}{n^{2}} \sum_{k=1}^{n} g(k) = \lim_{n \to \infty} \frac{1}{n^{2}} \sum_{k=1}^{n} 2k$

$= \lim_{n \to \infty} \frac{n(n+1)}{n^{2}} = 1$

ì •ë‹µ: â‘ 