## 문제
실수 전체의 집합에서 정의된 두 함수 $f(x)$, $g(x)$가
$$ f(x) = \left\{ \begin{array}{ll} 2 & (x > 2) \\ x & (|x| \le 2) \\ -2 & (x < -2) \end{array} \right. , g(x) = x^2 - 2 $$
일 때, <보기>에서 옳은 것만을 있는 대로 고른 것은?

---
**<보기>**
ㄱ. $(f \circ g)(2) = 2$
ㄴ. $(g \circ f)(-x) = (g \circ f)(x)$
ㄷ. $(f \circ g)(x) = (g \circ f)(x)$
---

## 보기
① ㄱ   ② ㄴ   ③ ㄱ, ㄴ   ④ ㄴ, ㄷ   ⑤ ㄱ, ㄴ, ㄷ

## 풀이
ㄱ. $f(g(2)) = f(2) = 2$ (참)

ㄴ. 함수 $(g \circ f)(x)$는
i ) $x > 2$ 일 때, $g(f(x)) = g(2) = 2$
ii) $|x| \le 2$ 일 때, $g(f(x)) = g(x) = x^2 - 2$
iii) $x < -2$ 일 때, $g(f(x)) = g(-2) = 2$

함수 $(g \circ f)(-x)$는
i ) $x > 2$ 일 때, $g(f(-x)) = g(-2) = 2$
ii) $|x| \le 2$ 일 때, $g(f(-x)) = g(-x) = x^2 - 2$
iii) $x < -2$ 일 때, $g(f(-x)) = g(2) = 2$

$\therefore (g \circ f)(-x) = (g \circ f)(x)$ (참)

ㄷ. 함수 $(f \circ g)(x)$는
i) $x > 2$ 일 때, $x^2 - 2 > 2$ 이므로 $f(g(x)) = f(x^2 - 2) = 2$
ii) $|x| \le 2$ 일 때, $-2 \le x^2 - 2 \le 2$ 이므로 $f(g(x)) = f(x^2 - 2) = x^2 - 2$
iii) $x < -2$ 일 때, $x^2 - 2 > 2$ 이므로 $f(g(x)) = f(x^2 - 2) = 2$

$\therefore (f \circ g)(x) = (g \circ f)(x)$ (참)

따라서 옳은 것은 ㄱ, ㄴ, ㄷ이다.

정답: ⑤