## 문제
두 상수 $a$, $b$에 대하여 $\lim_{x \to -2} \frac{x+2}{\sqrt{x+a} - b} = 6$일 때, $a+b$의 값을 구하시오.

## 풀이
$\lim_{x \to -2} (x+2) = 0$이고 $\lim_{x \to -2} \frac{x+2}{\sqrt{x+a} - b} = 6$이므로 
$\lim_{x \to -2} (\sqrt{x+a} - b) = 0$
$\therefore b = \sqrt{a-2}$

$\lim_{x \to -2} \frac{x+2}{\sqrt{x+a} - b}$
$= \lim_{x \to -2} \frac{x+2}{\sqrt{x+a} - \sqrt{a-2}}$
$= \lim_{x \to -2} \frac{(x+2)(\sqrt{x+a} + \sqrt{a-2})}{(x+a) - (a-2)}$
$= \lim_{x \to -2} \frac{(x+2)(\sqrt{x+a} + \sqrt{a-2})}{x+2}$
$= \lim_{x \to -2} (\sqrt{x+a} + \sqrt{a-2})$
$= 2\sqrt{a-2} = 6$

$\therefore a = 11$, $b = 3$
따라서 $a+b = 14$