## ë¬¸ì œ

ì´ì°¨í•¨ìˆ˜ $y=f(x)$ ì˜ ê·¸ë˜í”„ëŠ” ê·¸ë¦¼ê³¼ ê°™ê³ , $f(0)=f(3)=0$ ì´ë‹¤. 
$\lim_{n \to \infty} \frac{1}{n} \sum_{k=1}^{n} f \left( \frac{k}{n} \right) = \frac{7}{6}$ ì¼ ë•Œ, $f'(0)$ ì˜ ê°’ì€?

> [!example] ğŸ“¸ (ê·¸ë¦¼/ê·¸ë˜í”„)

## ë³´ê¸°
â‘  $\frac{5}{2}$   â‘¡ $3$   â‘¢ $\frac{7}{2}$   â‘£ $4$   â‘¤ $\frac{9}{2}$

## í’€ì´
$f(x)=ax(x-3)$ ìœ¼ë¡œ ì¡ìœ¼ë©´ ë¬¸ì œì—ì„œ 
$\frac{k}{n} \to x$, 
$\frac{1}{n} \to dx$, 
$\lim_{n \to \infty} \sum_{k=1}^{n} \to \int_{0}^{1}$ ë¡œ ë³€í˜•ëœë‹¤. 

$\lim_{n \to \infty} \frac{1}{n} \sum_{k=1}^{n} f \left( \frac{k}{n} \right) = \frac{7}{6}$ ì—ì„œ 
$\int_{0}^{1} f(x) dx = a \int_{0}^{1} (x^2 -3x) dx$ 
$= a \left[ \frac{x^3}{3} - \frac{3}{2}x^2 \right]_{0}^{1} = -\frac{7}{6} a = \frac{7}{6}$ 
$\therefore a = -1$ 

$f(x) = -x^2 + 3x$ ë¥¼ $x$ ì— ê´€í•˜ì—¬ ë¯¸ë¶„í•˜ë©´ 
$f'(x) = -2x+3$ 
$\therefore f'(0) = 3$ 

ì´ì°¨í•¨ìˆ˜ $y=f(x)$ ì˜ ê·¸ë˜í”„ëŠ” ê·¸ë¦¼ê³¼ ê°™ê³ , $f(0)=f(3)=0$ ì´ë‹¤. 

ì •ë‹µ: â‘¡