## ë¬¸ì œ
ì‹¤ìˆ˜ $m$ì— ëŒ€í•˜ì—¬ í•¨ìˆ˜ $f(x) = mx + 1$ì˜ ê·¸ëž˜í”„ì™€ í•¨ìˆ˜ 
$$ g(x) = \lim_{n \to \infty} \frac{x^{2n+1} - 3x + 4}{x^{2n} + 1} $$
ì˜ ê·¸ëž˜í”„ê°€ ë§Œë‚˜ëŠ” ì ì˜ ê°œìˆ˜ë¥¼ $h(m)$ì´ë¼ í•˜ìž. $h(-2) + \lim_{m \to 1} h(m)$ì˜ ê°’ì€?



> [!example] ðŸ“¸ (ê·¸ë¦¼/ê·¸ëž˜í”„)

## ë³´ê¸°
â‘  $1$   â‘¡ $2$   â‘¢ $3$   â‘£ $4$   â‘¤ $5$

## í’€ì´
$$ g(x) = \left\{ \begin{array}{ll} x & (|x| > 1) \\ 3 & (x = -1) \\ -3x + 4 & (|x| < 1) \\ 1 & (x = 1) \end{array} \right. $$
ì´ë¯€ë¡œ 

(â…°) $f(x) = -2x + 1$ì€ $y = g(x)$ì™€ $(-1, 3)$ì—ì„œ ë§Œë‚˜ë¯€ë¡œ $h(-2) = 1$ì´ë‹¤. 

(â…±) í•¨ìˆ˜ $h(m)$ì—ì„œ 
$0 < m < 1$ì¼ ë•Œ, $h(m) = 2$ 
$\lim_{m \to 1^-} h(m) = 2$ 
$1 < m < 2$ì¼ ë•Œ, $h(m) = 2$ 
$\lim_{m \to 1^+} h(m) = 2$ 

ë”°ë¼ì„œ $\lim_{m \to 1} h(m) = 2$ì´ë‹¤.

ê·¸ëŸ¬ë¯€ë¡œ $h(-2) + \lim_{m \to 1} h(m) = 1 + 2 = 3$ì´ë‹¤.

ì •ë‹µ: â‘¢