## 문제
방정식 $x^{3} + 1 = 0$의 한 허근을 $\alpha$라 할 때, $\sum_{k=1}^{\infty} \frac{1}{(k-\alpha)(k-\alpha^{2})}$의 값은?

## 보기
① $\alpha$   ② $\alpha-1$   ③ $1-\alpha$   ④ $1$   ⑤ $-1$

## 풀이
$x^{3} + 1 = (x+1)(x^{2} - x + 1) = 0$이므로 $\alpha$는 방정식 $x^{2} - x + 1 = 0$의 근이다.
$\therefore \alpha^{2} - \alpha + 1 = 0$

$\therefore \frac{1}{(k-\alpha)(k-\alpha^{2})} = \frac{1}{(k-\alpha)(k+1-\alpha)} = \frac{1}{k-\alpha} - \frac{1}{k+1-\alpha}$

$\sum_{k=1}^{n} \frac{1}{(k-\alpha)(k-\alpha^{2})} = \sum_{k=1}^{n} \left( \frac{1}{k-\alpha} - \frac{1}{k+1-\alpha} \right) = \frac{1}{1-\alpha} - \frac{1}{n+1-\alpha}$

$\therefore \sum_{k=1}^{\infty} \frac{1}{(k-\alpha)(k-\alpha^{2})} = \lim_{n \to \infty} \left( \frac{1}{1-\alpha} - \frac{1}{n+1-\alpha} \right)$
$= \frac{1}{1-\alpha} + \lim_{t \to +0} \frac{t}{1+(1-\alpha)t}$
$= \frac{1}{1-\alpha} + \frac{0}{1+0}$
$= -\frac{1}{\alpha^{2}}$ ($\because \alpha^{2} - \alpha + 1 = 0$)
$= \alpha$ ($\because \alpha^{3} = -1$)

정답: ①