## 문제
두 행렬 $A = \left( \begin{array}{rr} 3 & 0 \\ -1 & 2 \end{array} \right)$, $B = \left( \begin{array}{rr} 0 & 2 \\ 1 & 0 \end{array} \right)$에 대하여 행렬 $2A - AB$는?

## 보기
① $\left( \begin{array}{rr} 6 & 6 \\ 4 & 6 \end{array} \right)$ ② $\left( \begin{array}{rr} 6 & -6 \\ -4 & 6 \end{array} \right)$ ③ $\left( \begin{array}{rr} 6 & 4 \\ -4 & 6 \end{array} \right)$ ④ $\left( \begin{array}{rr} 6 & -4 \\ 4 & 6 \end{array} \right)$ ⑤ $\left( \begin{array}{rr} 6 & -6 \\ -4 & -6 \end{array} \right)$

## 풀이
$2A = 2 \left( \begin{array}{rr} 3 & 0 \\ -1 & 2 \end{array} \right) = \left( \begin{array}{rr} 6 & 0 \\ -2 & 4 \end{array} \right)$

$AB = \left( \begin{array}{rr} 3 & 0 \\ -1 & 2 \end{array} \right) \left( \begin{array}{rr} 0 & 2 \\ 1 & 0 \end{array} \right) = \left( \begin{array}{rr} 3 \times 0 + 0 \times 1 & 3 \times 2 + 0 \times 0 \\ -1 \times 0 + 2 \times 1 & -1 \times 2 + 2 \times 0 \end{array} \right) = \left( \begin{array}{rr} 0 & 6 \\ 2 & -2 \end{array} \right)$

따라서,
$$ \begin{array}{l} 2A - AB \\ = \left( \begin{array}{rr} 6 & 0 \\ -2 & 4 \end{array} \right) - \left( \begin{array}{rr} 0 & 6 \\ 2 & -2 \end{array} \right) \\ = \left( \begin{array}{rr} 6 - 0 & 0 - 6 \\ -2 - 2 & 4 - (-2) \end{array} \right) \\ = \left( \begin{array}{rr} 6 & -6 \\ -4 & 6 \end{array} \right) \end{array} $$

정답은 ②입니다.