## ë¬¸ì œ
ë‘ í•¨ìˆ˜ $y=2^{x}$ ì™€ $y=\left(\frac{1}{2}\right)^{x-3}$ ì— ëŒ€í•˜ì—¬ $x=\frac{5}{2}$ ì¼ ë•Œì˜ ë‘ ì ì„ ê°ê° $A$, $B$ë¼ í•  ë•Œ, ì„ ë¶„ $AB$ì˜ ê¸¸ì´ëŠ”?



> [!example] ğŸ“¸ (ê·¸ë¦¼/ê·¸ë˜í”„)

## ë³´ê¸°
â‘  $\frac{3\sqrt{2}}{2}$   â‘¡ $2\sqrt{2}$   â‘¢ $\frac{5\sqrt{2}}{2}$   â‘£ $3\sqrt{2}$   â‘¤ $\frac{7\sqrt{2}}{2}$

## í’€ì´
í•¨ìˆ˜ $y=2^{x}$ ì— $x=\frac{5}{2}$ ë¥¼ ëŒ€ì…í•˜ë©´ 
$$y=2^{\frac{5}{2}}=2^{2} \cdot 2^{\frac{1}{2}}=4\sqrt{2}$$ 
ì´ê³  í•¨ìˆ˜ $y=\left(\frac{1}{2}\right)^{x-3}$ ì— $x=\frac{5}{2}$ ë¥¼ ëŒ€ì…í•˜ë©´ 
$$y=\left(\frac{1}{2}\right)^{\frac{5}{2}-3}=\left(\frac{1}{2}\right)^{-\frac{1}{2}}=2^{\frac{1}{2}}=\sqrt{2}$$ 
ì´ë‹¤. ë”°ë¼ì„œ ë‘ ì  $A$, $B$ì˜ ì¢Œí‘œëŠ” 
$A\left(\frac{5}{2}, 4\sqrt{2}\right)$, $B\left(\frac{5}{2}, \sqrt{2}\right)$ ì´ë¯€ë¡œ ì„ ë¶„ $AB$ì˜ ê¸¸ì´ëŠ” 
$$4\sqrt{2}-\sqrt{2}=3\sqrt{2}$$ 
ì´ë‹¤.

ì •ë‹µ: â‘£