## 문제
자연수 $n$에 대하여 다항식 $(x-1)^{2n} + (x+1)^{n}$을 $x-3$으로 나눈 나머지를 $a_{n}$, $x-1$로 나눈 나머지를 $b_{n}$이라 할 때, $\lim_{n \to \infty} \frac{\log_{2} a_{n} + \log_{2} b_{n}}{n}$의 값은?

## 보기
① $1$   ② $2$   ③ $3$   ④ $4$   ⑤ $5$

## 풀이
$f(x) = (x-1)^{2n} + (x+1)^{n}$이라 하면 나머지 정리에 의해
$a_{n} = f(3) = (3-1)^{2n} + (3+1)^{n} = 2^{2n} + 4^{n} = 2^{2n} + 2^{2n} = 2 \cdot 2^{2n} = 2^{2n+1}$
$b_{n} = f(1) = (1-1)^{2n} + (1+1)^{n} = 2^{n}$
$\therefore \lim_{n \to \infty} \frac{\log_{2} a_{n} + \log_{2} b_{n}}{n} = \lim_{n \to \infty} \frac{\log_{2} 2^{2n+1} + \log_{2} 2^{n}}{n}$
$= \lim_{n \to \infty} \frac{(2n+1) + n}{n}$
$= \lim_{n \to \infty} \frac{3n+1}{n}$
$= \lim_{n \to \infty} (3 + \frac{1}{n})$
$= 3$

정답은 ③이다.