## 문제
두 행렬 $A = \left( \begin{array}{cc} 2 & 1 \\ 1 & 1 \end{array} \right)$, $B = \left( \begin{array}{cc} 1 & 2 \\ -1 & 0 \end{array} \right)$ 에 대하여 행렬 $A B - A$ 의 모든 성분의 합은?

## 보기
① $-2$   ② $-1$   ③ $0$   ④ $1$   ⑤ $2$

## 풀이
$A B - A = A ( B - E )$
$= \left( \begin{array}{cc} 2 & 1 \\ 1 & 1 \end{array} \right) \left( \begin{array}{cc} 0 & 2 \\ -1 & -1 \end{array} \right)$
$= \left( \begin{array}{cc} -1 & 3 \\ -1 & 1 \end{array} \right)$
그러므로 행렬 $A B - A$ 의 모든 성분의 합은 $(-1) + 3 + (-1) + 1 = 2$ 이다.

정답: ⑤