## 문제
네 실수 $a$, $b$, $x$, $y$가 다음 조건을 만족시킨다.

(가) $a^{3} b^{2} = 9$
(나) $a^{2x} = \frac{1}{(2b)^{3y}} = 6$

이때, $\frac{3}{2x} - \frac{2}{3y}$의 값은? (단, $a > 0$, $b > 0$)

## 보기
① $1$   ② $2$   ③ $3$   ④ $4$   ⑤ $5$

## 풀이
(나)의 $a^{2x} = 6$에서 $a = 6^{\frac{1}{2x}}$이므로
$a^{3} = 6^{\frac{3}{2x}}$

$\frac{1}{(2b)^{3y}} = 6$에서 $2b = 6^{-\frac{1}{3y}}$이므로
$(2b)^{2} = 6^{-\frac{2}{3y}}$

$6^{\frac{3}{2x} - \frac{2}{3y}} = 6^{\frac{3}{2x}} \times 6^{-\frac{2}{3y}}$
$= a^{3} \times (2b)^{2}$
$= a^{3} \times 4b^{2}$
$= 4 \times a^{3}b^{2}$

(가)에서 $a^{3}b^{2} = 9$이므로
$= 4 \times 9$
$= 36 = 6^{2}$

따라서
$\frac{3}{2x} - \frac{2}{3y} = 2$

정답: ②