## 문제
최고차항의 계수가 $1$인 두 삼차함수 $f(x)$, $g(x)$가 다음 조건을 만족시킨다.

(가) $g(1)=0$
(나) $\lim_{x \to n} \frac{f(x)}{g(x)}=(n-1)(n-2)$ ($n=1, 2, 3, 4$)

$g(5)$의 값은?

## 보기
① $4$   ② $6$   ③ $8$   ④ $10$   ⑤ $12$

## 풀이
조건 (나)에서 $\lim_{x \to 1} \frac{f(x)}{g(x)}=0$이고, 조건 (가) $\lim_{x \to 1} g(x)=g(1)=0$이므로 $\lim_{x \to 1} f(x)=f(1)=0$이다. 

또한, $\lim_{x \to 1} \frac{f(x)}{g(x)}=0$이므로 
$f(x)=(x-1)^{2}(x+a)$, 
$g(x)=(x-1)(x+b)(x+c)$ 
($a$, $b$, $c$는 상수)로 놓을 수 있다. 

조건 (나)에서 $\lim_{x \to 2} \frac{f(x)}{g(x)}=0$이고, $f(x)$는 $(x-2)^{2}$을 인수로 가질 수 없으므로 
$\lim_{x \to 2} g(x)=g(2) \neq 0$, 
$\lim_{x \to 2} f(x)=f(2)=0$이다. 

따라서 $f(x)=(x-1)^{2}(x-2)$이다. 

조건 (나)에서 $\lim_{x \to 3} \frac{f(x)}{g(x)}=2$, $\lim_{x \to 4} \frac{f(x)}{g(x)}=6$이고, 

$\lim_{x \to 3} \frac{f(x)}{g(x)} = \lim_{x \to 3} \frac{(x-1)^{2}(x-2)}{(x-1)(x+b)(x+c)}$ 
$= \lim_{x \to 3} \frac{(x-1)(x-2)}{(x+b)(x+c)}$ 
$= \frac{2}{(3+b)(3+c)} = 2$ 

$\lim_{x \to 4} \frac{f(x)}{g(x)} = \lim_{x \to 4} \frac{(x-1)^{2}(x-2)}{(x-1)(x+b)(x+c)}$ 
$= \frac{6}{(4+b)(4+c)} = 6$ 

이므로 
$(3+b)(3+c)=1$, 
$(4+b)(4+c)=1$ 

즉, 
$bc+3(b+c)=-8 \cdots$ ㉠ 
$bc+4(b+c)=-15 \cdots$ ㉡ 

㉠, ㉡에서 
$b+c=-7$, 
$bc=13$ 

따라서 
$g(5) = 4(5+b)(5+c)$ 
$= 4 \{ bc+5(b+c)+25 \}$ 
$= 4(13-35+25)$ 
$= 12$