## ë¬¸ì œ
ë‹¤í•­ì‹ $f(x) = x^3 - (a+4)x^2 + (4a-5)x + 5a$ ì— ëŒ€í•˜ì—¬ $f(a) = f(a+3) = 0$ ì„ ë§Œì¡±ì‹œí‚¤ëŠ” ì‹¤ìˆ˜ $a$ ì˜ ê°’ì˜ í•©ì€?



> [!example] ğŸ“¸ (ê·¸ë¦¼/ê·¸ë˜í”„)

## ë³´ê¸°
â‘  $-4$   â‘¡ $-2$   â‘¢ $0$   â‘£ $2$   â‘¤ $4$

## í’€ì´
$f(x) = x^3 - (a+4)x^2 + (4a-5)x + 5a$ ì— ëŒ€í•˜ì—¬ 
$f(a) = a^3 - a^3 - 4a^2 + 4a^2 - 5a + 5a = 0$ ì´ë¯€ë¡œ ì¡°ë¦½ì œë²•ì„ ì´ìš©í•˜ì—¬ $f(x)$ ë¥¼ ì¸ìˆ˜ë¶„í•´í•˜ë©´ 

$$ \begin{array}{c|rrrr} a & 1 & -a-4 & 4a-5 & 5a \\ & & a & -4a & -5a \\ \hline & 1 & -4 & -5 & 0 \end{array} $$

$\therefore f(x) = (x-a)(x^2-4x-5) = (x-a)(x+1)(x-5)$ 

ë”°ë¼ì„œ ì‚¼ì°¨ë°©ì •ì‹ $f(x) = 0$ ì˜ ê·¼ì€ 
$x=a$ ë˜ëŠ” $x = -1$ ë˜ëŠ” $x = 5$ 

$f(a+3)=0$ ì´ë¯€ë¡œ 
$a+3 = -1$ ë˜ëŠ” $a+3 = 5$ 

$\therefore a = -4$ ë˜ëŠ” $a = 2$ 

ë”°ë¼ì„œ ì‹¤ìˆ˜ $a$ ì˜ ê°’ì˜ í•©ì€ $(-4) + 2 = -2$ ì´ë‹¤. 

**[ë‹¤ë¥¸ í’€ì´]** 

$f(a+3) = 0$ ì—ì„œ 
$(a+3)^3 - (a+4)(a+3)^2 + (4a-5)(a+3) + 5a = 0$ 
$3a^2 + 6a - 24 = 0$, $a^2 + 2a - 8 = 0$ 
$(a+4)(a-2) = 0$ 
$\therefore a = -4$ ë˜ëŠ” $a = 2$ 

$a = -4$ ì¼ ë•Œ $f(-4) = 0$, $a = 2$ ì¼ ë•Œ $f(2) = 0$ ì´ë¯€ë¡œ 
$a = -4$, $a = 2$ ì¼ ë•Œ, ì£¼ì–´ì§„ ì¡°ê±´ì„ ë§Œì¡±ì‹œí‚¨ë‹¤. 
ë”°ë¼ì„œ ì‹¤ìˆ˜ $a$ ì˜ ê°’ì˜ í•©ì€ $(-4) + 2 = -2$ ì´ë‹¤.