## 문제
자연수 $k$에 대하여 
$a_{k} = \lim_{n \to \infty} \frac{\left( \frac{6}{k} \right)^{n+1}}{\left( \frac{6}{k} \right)^{n} + 1}$
이라 할 때, $\sum_{k=1}^{10} ka_{k}$의 값을 구하시오.

## 보기

## 풀이
$a_{k} = \lim_{n \to \infty} \frac{\left( \frac{6}{k} \right)^{n+1}}{\left( \frac{6}{k} \right)^{n} + 1}$에서 공비가 $\frac{6}{k}$이므로 각 경우로 나누면 다음과 같다.

(ⅰ) $\frac{6}{k} < 1$ 즉, $k > 6$일 때, 
$\lim_{n \to \infty} \left( \frac{6}{k} \right)^{n} = 0$이므로 
$a_{k} = \lim_{n \to \infty} \frac{\left( \frac{6}{k} \right)^{n+1}}{\left( \frac{6}{k} \right)^{n} + 1} = \frac{0}{0+1} = 0$

(ⅱ) $\frac{6}{k} = 1$ 즉, $k = 6$일 때, 
$\lim_{n \to \infty} \left( \frac{6}{k} \right)^{n} = 1$이므로 
$a_{k} = \lim_{n \to \infty} \frac{1^{n+1}}{1^{n} + 1} = \frac{1}{2}$

(ⅲ) $\frac{6}{k} > 1$ 즉, $k < 6$일 때, 
$\lim_{n \to \infty} \left( \frac{6}{k} \right)^{n} = \infty$이므로 
$a_{k} = \lim_{n \to \infty} \frac{\left( \frac{6}{k} \right)^{n+1}}{\left( \frac{6}{k} \right)^{n} + 1} = \lim_{n \to \infty} \frac{\left( \frac{6}{k} \right)}{1 + \frac{1}{\left( \frac{6}{k} \right)^{n}}} = \frac{\frac{6}{k}}{1+0} = \frac{6}{k}$

따라서 
$\sum_{k=1}^{10} ka_{k} = 1 \times a_{1} + 2 \times a_{2} + \cdots + 10 \times a_{10}$
$= 1 \times \frac{6}{1} + 2 \times \frac{6}{2} + 3 \times \frac{6}{3} + 4 \times \frac{6}{4} + 5 \times \frac{6}{5} + 6 \times \frac{1}{2} + 7 \times 0 + 8 \times 0 + 9 \times 0 + 10 \times 0$
$= 6 + 6 + 6 + 6 + 6 + 3 = 33$