## 문제
이차방정식 $(x-a)(x-b) + (x-b)(x-c) + (x-c)(x-a)=0$ 의 두 근의 합과 곱이 각각 $4$, $-3$ 일 때, 이차방정식 $(x-a)^{2} + (x-b)^{2} + (x-c)^{2} = 0$ 의 두 근의 곱은? (단, $a$, $b$, $c$ 는 상수이다.)

## 보기
① $15$   ② $16$   ③ $17$   ④ $18$   ⑤ $19$

## 풀이
방정식 $(x-a)(x-b) + (x-b)(x-c) + (x-c)(x-a)=0$ 에서
$x^{2} - (a+b)x+ab+x^{2} - (b+c)x+bc+x^{2} - (c+a)x+ca=0$
$\therefore 3x^{2} - 2(a+b+c)x+ab+bc+ca = 0$

근과 계수의 관계에 의하여
$\frac{2(a+b+c)}{3} = 4$, $\frac{ab+bc+ca}{3} = -3$
$\therefore a+b+c=6$, $ab+bc+ca=-9$

따라서 방정식 $(x-a)^{2} + (x-b)^{2} + (x-c)^{2} = 0$ 에서
$3x^{2} - 2(a+b+c)x+a^{2} + b^{2} + c^{2} = 0$

근과 계수의 관계에 의하여 두 근의 곱은
$\frac{a^{2} + b^{2} + c^{2}}{3}$
$= \frac{1}{3} \{ (a+b+c)^{2} - 2(ab+bc+ca) \}$
$= \frac{1}{3} \{ 6^{2} - 2(-9) \}$
$= \frac{1}{3} (36+18)$
$= 18$

정답: ④