## 문제
두 실수 $x$, $y$에 대하여 두 행렬 $A$, $B$를 
$$ A = \left( \begin{array}{rr} -1 & x \\ 3 & 0 \end{array} \right), \quad B = \left( \begin{array}{rr} -2 & 2 \\ y & -1 \end{array} \right) $$
이라 하자. $(A+B)(A-B)=A^{2}-B^{2}$일 때 $x^{2}+y^{2}$의 값을 구하시오.

## 풀이
$(A+B)(A-B)=A^{2}-AB+BA-B^{2}$이므로
$(A+B)(A-B)=A^{2}-B^{2}$가 성립하려면 
$AB=BA$이어야 한다.

$$ AB = \left( \begin{array}{cc} -1 & x \\ 3 & 0 \end{array} \right) \left( \begin{array}{cc} -2 & 2 \\ y & -1 \end{array} \right) = \left( \begin{array}{cc} 2+xy & -2-x \\ -6 & 6 \end{array} \right) $$

$$ BA = \left( \begin{array}{cc} -2 & 2 \\ y & -1 \end{array} \right) \left( \begin{array}{cc} -1 & x \\ 3 & 0 \end{array} \right) = \left( \begin{array}{cc} 8 & -2x \\ -y-3 & xy \end{array} \right) $$

두 행렬이 서로 같아야 하므로 각 성분을 비교하면
$-2-x = -2x$ 에서 $x=2$
$-6 = -y-3$ 에서 $y=3$
(이때 $2+xy = 2+(2)(3) = 8$ 이고 $xy = (2)(3) = 6$ 이므로 모든 성분이 일치한다.)

그러므로 
$x^{2}+y^{2} = 2^{2}+3^{2} = 4+9 = 13$

정답: $13$