## ë¬¸ì œ
í•¨ìˆ˜ $f(x)$ëŠ” ëª¨ë“  ì‹¤ìˆ˜ $x$ì— ëŒ€í•˜ì—¬ $f(x+3) = f(x)$ë¥¼ ë§Œì¡±ì‹œí‚¤ê³ ,
$$ f(x) = \left\{ \begin{array}{ll} x & (0 \le x < 1) \\ 1 & (1 \le x < 2) \\ -x+3 & (2 \le x < 3) \end{array} \right. $$
ì´ë‹¤. $\int_{-a}^a f(x) dx = 13$ì¼ ë•Œ, ìƒìˆ˜ $a$ì˜ ê°’ì€? (ë‹¨, ê³¡ì„  $y = f(x)$ëŠ” $y$ì¶•ì— ëŒ€í•˜ì—¬ ëŒ€ì¹­ì´ë‹¤.)



> [!example] ğŸ“¸ (ê·¸ë¦¼/ê·¸ë˜í”„)

## ë³´ê¸°
â‘  $10$   â‘¡ $12$   â‘¢ $14$   â‘£ $16$   â‘¤ $18$

## í’€ì´
ê³¡ì„  $y = f(x)$ëŠ” $y$ì¶•ì— ëŒ€í•˜ì—¬ ëŒ€ì¹­ì´ë¯€ë¡œ 
$\int_{-a}^a f(x) dx = 13$ì—ì„œ 
$2 \int_0^a f(x) dx = 13$ 
$\therefore \int_0^a f(x) dx = \frac{13}{2}$ 

í•œí¸, 
$\int_0^3 f(x) dx = \frac{1}{2} \times (3 + 1) \times 1 = 2$ 
ì´ê³ , $f(x + 3) = f(x)$ì´ë¯€ë¡œ 
$\int_0^3 f(x) dx = \int_3^6 f(x) dx = \int_6^9 f(x) dx = 2$ 
$\therefore \int_0^9 f(x) dx = 6$ 

ë”°ë¼ì„œ $\int_0^9 f(x) dx + \int_9^a f(x) dx = \frac{13}{2}$ì—ì„œ 
$\int_9^a f(x) dx = \frac{1}{2}$ 

í•œí¸ 
$\int_9^{10} f(x) dx = \int_0^1 f(x) dx = \int_0^1 x dx = \left[ \frac{1}{2}x^2 \right]_0^1 = \frac{1}{2}$ 
ì´ë¯€ë¡œ 
$a = 10$ 

ì •ë‹µ: â‘ 