## 문제
두 다항함수 $f(x)$, $g(x)$가 다음 조건을 만족시킨다.

(가) $\lim_{x \to \infty} \frac{f(x)-2g(x)}{x^2} = 1$
(나) $\lim_{x \to \infty} \frac{f(x)+3g(x)}{x^3} = 1$

$\lim_{x \to \infty} \frac{f(x)+g(x)}{x^3}$의 값은?

## 보기
① $\frac{1}{5}$   ② $\frac{2}{5}$   ③ $\frac{3}{5}$   ④ $\frac{4}{5}$   ⑤ $1$

## 풀이
$\lim_{x \to \infty} \frac{f(x)-2g(x)}{x^2} = 1$이므로 $f(x)-2g(x)$는 최고차항의 계수가 $1$인 이차함수이다. 

$\lim_{x \to \infty} \frac{f(x)+3g(x)}{x^3} = 1$이므로 $f(x)+3g(x)$는 최고차항의 계수가 $1$인 삼차함수이다. 

$\{f(x)+3g(x)\} - \{f(x)-2g(x)\} = 5g(x)$이므로 $g(x)$는 최고차항의 계수가 $\frac{1}{5}$인 삼차함수이다. 

$\lim_{x \to \infty} \frac{g(x)}{x^3} = \frac{1}{5}$ 

$\therefore \lim_{x \to \infty} \frac{f(x)+g(x)}{x^3}$ 
$= \lim_{x \to \infty} \left\{ \frac{f(x)+3g(x)}{x^3} - \frac{2g(x)}{x^3} \right\}$ 
$= \lim_{x \to \infty} \frac{f(x)+3g(x)}{x^3} - 2 \times \lim_{x \to \infty} \frac{g(x)}{x^3}$ 
$= 1 - \frac{2}{5}$ 
$= \frac{3}{5}$

정답: ③