## 문제
수열 $\{ a_{n} \}$ 은 $a_{1}=2$ 이고 
$\frac{a_{n}}{n}-\frac{a_{n+1}}{n+1}=\frac{a_{n} a_{n+1}}{n+1} (n \geq 1)$
을 만족시킨다. 다음은 일반항 $a_{n}$ 을 구하는 과정이다.

수열 $\{ a_{n} \}$ 의 모든 항이 $0$ 이 아니므로 
$\frac{a_{n}}{n}-\frac{a_{n+1}}{n+1}=\frac{a_{n} a_{n+1}}{n+1}$
을 변형하면 
$\frac{n+1}{a_{n+1}}-\frac{n}{a_{n}}=(가)$
이다. $b_{n}=\frac{n}{a_{n}}$ 이라 하면 $b_{1}=\frac{1}{2}$ 이고 
$b_{n+1}-b_{n}=(가) (n \geq 1)$
이므로 
$a_{n}=(나)$
이다.

위의 $(가)$, $(나)$에 알맞은 식을 각각 $f(n)$, $g(n)$이라 할 때, $f(13) g(4)$의 값은?

## 보기
① $8$   ② $9$   ③ $10$   ④ $11$   ⑤ $12$

## 풀이
수열 $\{ a_{n} \}$ 의 모든 항이 $0$ 이 아니므로 
$\frac{a_{n}}{n}-\frac{a_{n+1}}{n+1}=\frac{a_{n} a_{n+1}}{n+1}$
의 양변에 $\frac{n(n+1)}{a_{n} a_{n+1}}$ 을 곱하면 
$\frac{n+1}{a_{n+1}}-\frac{n}{a_{n}}= n$
이다. $b_{n}=\frac{n}{a_{n}}$ 이라 하면 $b_{1}=\frac{1}{2}$ 이고 
$b_{n+1}-b_{n}= n (n \geq 1)$
이므로 
$b_{n}=\frac{1}{2}+ \sum_{k=1}^{n-1} k=\frac{1}{2}+\frac{n(n-1)}{2}=\frac{n^{2}-n+1}{2}$
$a_{n}=\frac{n}{b_{n}}= \frac{2 n}{n^{2}-n+1}$
따라서 $f(n)=n$, $g(n)=\frac{2 n}{n^{2}-n+1}$ 이다. 
$\therefore f(13) g(4)=13 \times \frac{8}{13}=8$

정답 ①