## 문제
이차정사각행렬 $A$, $B$가 
$$(A+B)^{2} = \left( \begin{array}{rr} 2 & 2 \\ -1 & -1 \end{array} \right)$$, $$A^{2}+B^{2} = \left( \begin{array}{rr} 0 & -2 \\ 1 & 3 \end{array} \right)$$
을 만족시킬 때, 행렬 $AB+BA$는?

## 보기
① $\left( \begin{array}{rr} -1 & -3 \\ 5 & -2 \end{array} \right)$   ② $\left( \begin{array}{rr} 1 & 5 \\ -1 & 8 \end{array} \right)$   ③ $\left( \begin{array}{rr} 1 & 7 \\ 8 & 4 \end{array} \right)$   ④ $\left( \begin{array}{rr} 2 & 4 \\ -2 & -4 \end{array} \right)$   ⑤ $\left( \begin{array}{rr} 2 & -7 \\ 6 & -2 \end{array} \right)$

## 풀이
$$(A+B)^{2} = A^{2} + AB + BA + B^{2} = \left( \begin{array}{rr} 2 & 2 \\ -1 & -1 \end{array} \right)$$ 이고
$$A^{2} + B^{2} = \left( \begin{array}{rr} 0 & -2 \\ 1 & 3 \end{array} \right)$$ 이므로
$$AB+BA = (A+B)^{2} - (A^{2} + B^{2})$$
$$AB+BA = \left( \begin{array}{rr} 2 & 2 \\ -1 & -1 \end{array} \right) - \left( \begin{array}{rr} 0 & -2 \\ 1 & 3 \end{array} \right)$$
$$AB+BA = \left( \begin{array}{rr} 2 & 4 \\ -2 & -4 \end{array} \right)$$
이다.
따라서 행렬 $AB+BA$는 $\left( \begin{array}{rr} 2 & 4 \\ -2 & -4 \end{array} \right)$ 이다.

정답: ④