## 문제
수열 $\{ a_{n} \}$ 은 $a_{1} = 3$ 이고, 
$2a_{n+1} = 3a_{n} - \frac{6n+2}{(n+1)!} (n \geq 1)$ 
을 만족시킨다. 다음은 일반항 $a_{n}$ 을 구하는 과정이다. 

$$
\begin{array}{|l|}
\hline
\text{주어진 식에 의하여} \\
2a_{n+1} = 3a_{n} - \frac{6(n+1)-4}{(n+1)!} \\
\text{이다.} \\
2a_{n+1} - \frac{4}{(n+1)!} = 3a_{n} - 3 \times (가) \\
\text{이므로 } b_{n} = a_{n} - (가) \text{ 라 하면} \\
2b_{n+1} = 3b_{n} \\
\text{이다. } b_{n+1} = \frac{3}{2} b_{n} \text{ 이고 } b_{1} = 1 \text{ 이므로} \\
b_{n} = (나) \\
\text{이다. 그러므로 } a_{n} = (가) + (나) \text{ 이다.} \\
\hline
\end{array}
$$

위의 $(가)$, $(나)$에 알맞은 식을 각각 $f(n), g(n)$ 이라 할 때, $f(3) \times g(3)$ 의 값은? 

## 보기
① $\frac{1}{2}$   ② $\frac{7}{12}$   ③ $\frac{2}{3}$   ④ $\frac{3}{4}$   ⑤ $\frac{5}{6}$

## 풀이
$f(n) = \frac{2}{n!}$, $g(n) = \left( \frac{3}{2} \right)^{n-1}$ 이므로 

$f(3) = \frac{2}{3!} = \frac{1}{3}$
$g(3) = \left( \frac{3}{2} \right)^{2} = \frac{9}{4}$ 

$\therefore f(3) \times g(3) = \frac{3}{4}$

정답은 ④ 이다.