## 문제
다항식 $( x^{2} + 2x ) ( x^{2} + 2x - 3 ) + 2$ 를 인수분해하면 $( x^{2} + ax + b ) ( x^{2} + 2x - 2 )$ 일 때, $a + b$ 의 값은? (단, $a$, $b$ 는 상수이다.)

## 보기
① $-3$   ② $-1$   ③ $1$   ④ $3$   ⑤ $5$

## 풀이
$x^{2} + 2x = X$ 라 하면
$( x^{2} + 2x ) ( x^{2} + 2x - 3 ) + 2$
$= X ( X - 3 ) + 2$
$= X^{2} - 3X + 2$
$= ( X - 1 ) ( X - 2 )$
이므로
$( x^{2} + 2x ) ( x^{2} + 2x - 3 ) + 2 = ( x^{2} + 2x - 1 ) ( x^{2} + 2x - 2 )$
따라서 $a = 2$, $b = -1$ 이므로
$a + b = 1$

**[다른 풀이]**
등식 $( x^{2} + 2x ) ( x^{2} + 2x - 3 ) + 2 = ( x^{2} + ax + b ) ( x^{2} + 2x - 2 )$ 는 $x$ 에 대한 항등식이므로 이 식의 양변에 $x = 0$ 을 대입하면
$2 = -2b$
$\therefore b = -1$
위 식의 양변에 $x = 1$ 을 대입하면
$2 = 1 + a + b$
$\therefore a = 2$ ($\because b = -1$)
따라서 $a + b = 1$

[정답] ③