## ë¬¸ì œ
$a>3$ ì¸ ìƒìˆ˜ $a$ ì— ëŒ€í•˜ì—¬ ë‘ ê³¡ì„  $y=a^{x-1}$ ê³¼ $y=3^x$ ì´ ì  $P$ ì—ì„œ ë§Œë‚œë‹¤. ì  $P$ ì˜ $x$ ì¢Œí‘œë¥¼ $k$ ë¼ í•  ë•Œ, $\lim_{n \to \infty} \frac{\left( \frac{a}{3} \right)^{n+k}}{\left( \frac{a}{3} \right)^{n+1} + 1}$ ì˜ ê°’ì€?



> [!example] ğŸ“¸ (ê·¸ë¦¼/ê·¸ë˜í”„)

## ë³´ê¸°
â‘  $1$   â‘¡ $2$   â‘¢ $3$   â‘£ $4$   â‘¤ $5$

## í’€ì´
$a > 3$ ì´ë¯€ë¡œ $\frac{a}{3} > 1$ ì´ë‹¤.
ë”°ë¼ì„œ,
$\lim_{n \to \infty} \frac{\left( \frac{a}{3} \right)^{n+k}}{\left( \frac{a}{3} \right)^{n+1} + 1}$
$= \lim_{n \to \infty} \frac{\left( \frac{a}{3} \right)^k}{\frac{a}{3} + \frac{1}{\left( \frac{a}{3} \right)^n}}$
$= \frac{\left( \frac{a}{3} \right)^k}{\frac{a}{3} + 0} = \left( \frac{a}{3} \right)^{k-1}$

ë‘ ê³¡ì„  $y = a^{x-1}$ ê³¼ $y = 3^x$ ì˜ êµì ì˜ $x$ ì¢Œí‘œê°€ $k$ ì´ë¯€ë¡œ
$a^{k-1} = 3^k$
$a^{k-1} = 3 \cdot 3^{k-1}$
$\frac{a^{k-1}}{3^{k-1}} = \left( \frac{a}{3} \right)^{k-1} = 3$

ê·¸ëŸ¬ë¯€ë¡œ,
$\lim_{n \to \infty} \frac{\left( \frac{a}{3} \right)^{n+k}}{\left( \frac{a}{3} \right)^{n+1} + 1} = \left( \frac{a}{3} \right)^{k-1} = 3$

ì •ë‹µì€ â‘¢ ì´ë‹¤.