## ë¬¸ì œ
ìì—°ìˆ˜ $n$ì— ëŒ€í•˜ì—¬ ì§ì„  $y = \left( \frac{1}{2} \right)^{n-1} (x - 1)$ê³¼ ì´ì°¨í•¨ìˆ˜ $y = 3x(x - 1)$ì˜ ê·¸ë˜í”„ê°€ ë§Œë‚˜ëŠ” ë‘ ì ì„ $A(1, 0)$ê³¼ $P_n$ì´ë¼ í•˜ì. ì  $P_n$ì—ì„œ $x$ì¶•ì— ë‚´ë¦° ìˆ˜ì„ ì˜ ë°œì„ $H_n$ì´ë¼ í•  ë•Œ, $\sum_{n=1}^{\infty} \overline{P_n H_n}$ì˜ ê°’ì€?



> [!example] ğŸ“¸ (ê·¸ë¦¼/ê·¸ë˜í”„)

## ë³´ê¸°
â‘  $\frac{3}{2}$   â‘¡ $\frac{14}{9}$   â‘¢ $\frac{29}{18}$   â‘£ $\frac{5}{3}$   â‘¤ $\frac{31}{18}$

## í’€ì´
[ì •ë‹µ] â‘¡ 

$x \neq 1$ ì¼ ë•Œ, 
$\left( \frac{1}{2} \right)^{n-1} (x - 1) = 3x(x - 1)$ ì—ì„œ 
$\left( \frac{1}{2} \right)^{n-1} = 3x$ 
$\therefore x = \frac{1}{3} \left( \frac{1}{2} \right)^{n-1}$ 

ì¦‰, $P_n \left( \frac{1}{3} \left( \frac{1}{2} \right)^{n-1}, \left( \frac{1}{2} \right)^{n-1} \left\{ \frac{1}{3} \left( \frac{1}{2} \right)^{n-1} - 1 \right\} \right)$ 
$P_n \left( \frac{1}{3} \left( \frac{1}{2} \right)^{n-1}, \frac{1}{3} \left( \frac{1}{4} \right)^{n-1} - \left( \frac{1}{2} \right)^{n-1} \right)$ 

ì´ë¯€ë¡œ 
$\overline{P_n H_n} = \left( \frac{1}{2} \right)^{n-1} - \frac{1}{3} \left( \frac{1}{4} \right)^{n-1}$ 

$\therefore \sum_{n=1}^{\infty} \overline{P_n H_n}$ 
$= \sum_{n=1}^{\infty} \left\{ \left( \frac{1}{2} \right)^{n-1} - \frac{1}{3} \left( \frac{1}{4} \right)^{n-1} \right\}$ 
$= \sum_{n=1}^{\infty} \left( \frac{1}{2} \right)^{n-1} - \frac{1}{3} \sum_{n=1}^{\infty} \left( \frac{1}{4} \right)^{n-1}$ 
$= \frac{1}{1 - \frac{1}{2}} - \frac{1}{3} \times \frac{1}{1 - \frac{1}{4}}$ 
$= 2 - \frac{4}{9} = \frac{14}{9}$