## 문제
함수 $f$는 임의의 실수 $x$, $y$에 대하여 다음을 만족시킨다.

$f(1)>0$, $f(xy)=f(x)f(y)-x-y$

이때, $\lim_{n \to \infty} \sum_{k=1}^{n} \left\{ \frac{6}{\sqrt{n}} f \left( 2+ \frac{4k}{n} \right) \right\}^{2}$의 값은?

## 보기
① $510$   ② $624$   ③ $756$   ④ $832$   ⑤ $948$

## 풀이
$f(xy)=f(x)f(y)-x-y$ 에 $x=y=1$ 대입하여 정리하면
$f(1) = \{f(1)\}^{2}-2$
$f(1)^{2}-f(1)-2=0$
$(f(1)-2)(f(1)+1)=0$
$f(1)>0$ 이므로 $f(1)=2$ 이며,
$y=1$ 을 대입하면 $f(x)=f(x)f(1)-x-1$ 이므로
$f(x)=2f(x)-x-1$, 즉 $f(x)=x+1$ 이다.

$\lim_{n \to \infty} \sum_{k=1}^{n} \left\{ \frac{6}{\sqrt{n}} f \left( 2+ \frac{4k}{n} \right) \right\}^{2}$ 의 계산을 위해
$x=2+ \frac{4k}{n}$ 이라 하면 $dx = \frac{4}{n}$ 이며
따라서
$\lim_{n \to \infty} \sum_{k=1}^{n} \left\{ \frac{6}{\sqrt{n}} f \left( 2+ \frac{4k}{n} \right) \right\}^{2}$
$= \lim_{n \to \infty} \sum_{k=1}^{n} \frac{36}{n} \left\{ f \left( 2+ \frac{4k}{n} \right) \right\}^{2}$
$= 9 \lim_{n \to \infty} \sum_{k=1}^{n} \left\{ f \left( 2+ \frac{4k}{n} \right) \right\}^{2} \frac{4}{n}$
$= 9 \int_{2}^{6} \{f(x)\}^{2} dx$
$= 9 \int_{2}^{6} (x+1)^{2} dx$
$= 9 \int_{2}^{6} (x^{2} +2x+1) dx$
$= 9 \left[ \frac{1}{3}x^{3} + x^{2} + x \right]_{2}^{6}$
$= 9 \left\{ (72+36+6) - \left( \frac{8}{3}+4+2 \right) \right\}$
$= 9 \left( 114 - \frac{26}{3} \right)$
$= 1026 - 78$
$= 948$

정답: ⑤