## 문제
수열 $\{ a_n \}$이 모든 자연수 $n$에 대하여 부등식 
$$\frac{2n^2 - n}{3n - 1} < a_n < \frac{2n^2 + n}{3n - 1}$$ 
을 만족시킬 때, $\lim_{n \to \infty} \frac{a_n}{2n + 3}$의 값은? 

## 보기
① $\frac{1}{12}$   ② $\frac{1}{6}$   ③ $\frac{1}{4}$   ④ $\frac{1}{3}$   ⑤ $\frac{5}{12}$

## 풀이
[정답] ④ 

부등식 $\frac{2n^2 - n}{3n - 1} < a_n < \frac{2n^2 + n}{3n - 1}$에서 각 변을 $( 2n + 3 )$으로 나누면 
$$\frac{2n^2 - n}{( 3n - 1 )( 2n + 3 )} < \frac{a_n}{2n + 3} < \frac{2n^2 + n}{( 3n - 1 )( 2n + 3 )}$$ 
이다. 
$$\lim_{n \to \infty} \frac{2n^2 - n}{( 3n - 1 )( 2n + 3 )} \le \lim_{n \to \infty} \frac{a_n}{2n + 3} \le \lim_{n \to \infty} \frac{2n^2 + n}{( 3n - 1 )( 2n + 3 )}$$ 
이고 
$$\lim_{n \to \infty} \frac{2n^2 - n}{( 3n - 1 )( 2n + 3 )} = \frac{1}{3}, \lim_{n \to \infty} \frac{2n^2 + n}{( 3n - 1 )( 2n + 3 )} = \frac{1}{3}$$ 
이다. 따라서 
$$\lim_{n \to \infty} \frac{a_n}{2n + 3} = \frac{1}{3}$$ 
이다.