## 문제
첫째항이 $1$인 두 등비수열 $\{ a_{n} \}$, $\{ b_{n} \}$이 다음 조건을 만족시킬 때, $\sum_{n=1}^{\infty} ( a_{n}^{2} + b_{n}^{2} )$의 값은?

(가) $\sum_{n=1}^{\infty} a_{n}$, $\sum_{n=1}^{\infty} b_{n}$이 각각 수렴한다.
(나) $\sum_{n=1}^{\infty} ( a_{n} + b_{n} ) = \frac{9}{4}$이고 $\sum_{n=1}^{\infty} ( a_{n} - b_{n} ) = \frac{3}{4}$이다.

## 보기
① $\frac{9}{4}$   ② $\frac{11}{4}$   ③ $\frac{13}{4}$   ④ $\frac{15}{4}$   ⑤ $\frac{17}{4}$

## 풀이
$\sum_{n=1}^{\infty} a_{n} = x$, $\sum_{n=1}^{\infty} b_{n} = y$라 하면
$\sum_{n=1}^{\infty} ( a_{n} + b_{n} ) = \frac{9}{4}$이므로 $x + y = \frac{9}{4}$이다.
$\sum_{n=1}^{\infty} ( a_{n} - b_{n} ) = \frac{3}{4}$이므로 $x - y = \frac{3}{4}$이다.
따라서 $x = \frac{3}{2}$, $y = \frac{3}{4}$이다.
첫째항이 $1$인 두 등비수열 $\{ a_{n} \}$, $\{ b_{n} \}$의 공비를 각각 $p$, $q$라 하면
$\frac{1}{1 - p} = \frac{3}{2}$, $\frac{1}{1 - q} = \frac{3}{4}$이다.
따라서 $p = \frac{1}{3}$, $q = -\frac{1}{3}$이다.
그러므로 $a_{n} = ( \frac{1}{3} )^{n-1}$, $b_{n} = ( -\frac{1}{3} )^{n-1}$이다.
$\therefore \sum_{n=1}^{\infty} ( a_{n}^{2} + b_{n}^{2} ) = 2 \sum_{n=1}^{\infty} ( \frac{1}{9} )^{n-1} = \frac{2}{1 - \frac{1}{9}} = \frac{9}{4}$

[다른 풀이]
첫째항이 $1$인 두 등비수열 $\{ a_{n} \}$, $\{ b_{n} \}$의 공비를 각각 $p$, $q$라 하면
$\sum_{n=1}^{\infty} ( a_{n} + b_{n} ) = \sum_{n=1}^{\infty} a_{n} + \sum_{n=1}^{\infty} b_{n} = \frac{1}{1 - p} + \frac{1}{1 - q} = \frac{9}{4} \cdots ㉠$
$\sum_{n=1}^{\infty} ( a_{n} - b_{n} ) = \sum_{n=1}^{\infty} a_{n} - \sum_{n=1}^{\infty} b_{n} = \frac{1}{1 - p} - \frac{1}{1 - q} = \frac{3}{4} \cdots ㉡$
$㉠$과 $㉡$을 연립하여 풀면 $p = \frac{1}{3}$, $q = -\frac{1}{3}$이다.
첫째항이 $1$인 두 등비수열 $\{ a_{n} \}$, $\{ b_{n} \}$의 공비가 각각 $p$, $q$이므로 두 등비수열 $\{ a_{n}^{2} \}$, $\{ b_{n}^{2} \}$의 공비는 각각 $p^{2}$, $q^{2}$이다.
$\therefore \sum_{n=1}^{\infty} ( a_{n}^{2} + b_{n}^{2} ) = \sum_{n=1}^{\infty} a_{n}^{2} + \sum_{n=1}^{\infty} b_{n}^{2} = \frac{1}{1 - p^{2}} + \frac{1}{1 - q^{2}} = \frac{1}{1 - \frac{1}{9}} + \frac{1}{1 - \frac{1}{9}} = \frac{9}{9 - 1} + \frac{9}{9 - 1} = \frac{9}{4}$