## 문제
두 행렬 $A = \left( \begin{array}{cc} 1 & 2 \\ 0 & 1 \end{array} \right)$, $B = \left( \begin{array}{cc} -1 & 0 \\ 1 & -4 \end{array} \right)$ 에 대하여 행렬 $A(A+B)$ 의 모든 성분의 합은?

## 보기
① $-4$   ② $-2$   ③ $0$   ④ $2$   ⑤ $4$

## 풀이
$A+B = \left( \begin{array}{cc} 1 & 2 \\ 0 & 1 \end{array} \right) + \left( \begin{array}{cc} -1 & 0 \\ 1 & -4 \end{array} \right) = \left( \begin{array}{cc} 0 & 2 \\ 1 & -3 \end{array} \right)$ 이므로
$$ A(A+B) = \left( \begin{array}{cc} 1 & 2 \\ 0 & 1 \end{array} \right) \left( \begin{array}{cc} 0 & 2 \\ 1 & -3 \end{array} \right) = \left( \begin{array}{cc} 2 & -4 \\ 1 & -3 \end{array} \right) $$
따라서 행렬 $A(A+B)$ 의 모든 성분의 합은
$2 + (-4) + 1 + (-3) = -4$
정답: ①