## 문제
수열 $\{a_{n}\}$ 에 대하여 급수 $\sum_{n=1}^{\infty} \left( a_{n} - \frac{5n}{n+1} \right)$ 이 수렴할 때, $\lim_{n \to \infty} \frac{a_{n} + 3}{a_{n} - 1}$ 의 값은?

## 보기
① $-2$   ② $-1$   ③ $0$   ④ $1$   ⑤ $2$

## 풀이
무한급수 $\sum_{n=1}^{\infty} \left( a_{n} - \frac{5n}{n+1} \right)$ 이 수렴하므로 
$\lim_{n \to \infty} \left( a_{n} - \frac{5n}{n+1} \right) = 0$

$\lim_{n \to \infty} \frac{5n}{n+1} = 5$ 이므로 
$\lim_{n \to \infty} \frac{a_{n} + 3}{a_{n} - 1}$
$= \lim_{n \to \infty} \frac{a_{n} - \frac{5n}{n+1} + \frac{5n}{n+1} + 3}{a_{n} - \frac{5n}{n+1} + \frac{5n}{n+1} - 1}$
$= \frac{\lim_{n \to \infty} \left( a_{n} - \frac{5n}{n+1} \right) + \lim_{n \to \infty} \frac{5n}{n+1} + \lim_{n \to \infty} 3}{\lim_{n \to \infty} \left( a_{n} - \frac{5n}{n+1} \right) + \lim_{n \to \infty} \frac{5n}{n+1} - \lim_{n \to \infty} 1}$
$= \frac{0 + 5 + 3}{0 + 5 - 1}$
$= 2$

**[다른 풀이]**
$b_{n} = a_{n} - \frac{5n}{n+1}$ 이라 하자. 
무한급수 $\sum_{n=1}^{\infty} \left( a_{n} - \frac{5n}{n+1} \right)$ 이 수렴하므로 
$\lim_{n \to \infty} \left( a_{n} - \frac{5n}{n+1} \right) = \lim_{n \to \infty} b_{n} = 0$

$a_{n} = b_{n} + \frac{5n}{n+1}$ 이고, $\lim_{n \to \infty} \frac{5n}{n+1} = 5$
$\lim_{n \to \infty} a_{n} = \lim_{n \to \infty} \left( b_{n} + \frac{5n}{n+1} \right)$
$= \lim_{n \to \infty} b_{n} + \lim_{n \to \infty} \frac{5n}{n+1}$
$= 0 + 5 = 5$

$\lim_{n \to \infty} \frac{a_{n} + 3}{a_{n} - 1} = \frac{\lim_{n \to \infty} ( a_{n} + 3 )}{\lim_{n \to \infty} ( a_{n} - 1 )}$
$= \frac{5 + 3}{5 - 1} = 2$

정답: ⑤