## ë¬¸ì œ
í•¨ìˆ˜ $f(x)$ ê°€ $f(x) = (x-3)^2$ ì´ë‹¤. ìì—°ìˆ˜ $n$ ì— ëŒ€í•˜ì—¬ ë°©ì •ì‹ $f(x) = n$ ì˜ ë‘ ê·¼ì´ $\alpha$, $\beta$ ì¼ ë•Œ $h(n) = |\alpha - \beta|$ ë¼ í•˜ì. $\lim_{n \to \infty} \sqrt{n} \{ h(n+1) - h(n) \}$ ì˜ ê°’ì€?

> [!example] ğŸ“¸ (ê·¸ë¦¼/ê·¸ë˜í”„)

## ë³´ê¸°
â‘  $\frac{1}{2}$   â‘¡ $1$   â‘¢ $\frac{3}{2}$   â‘£ $2$   â‘¤ $\frac{5}{2}$

## í’€ì´
ë°©ì •ì‹ $f(x) = n$ ì¦‰, $(x-3)^2 = n$ ì—ì„œ
$x-3 = \sqrt{n}$ ë˜ëŠ” $x-3 = -\sqrt{n}$
$\therefore x = 3 + \sqrt{n}$ ë˜ëŠ” $x = 3 - \sqrt{n}$

ë”°ë¼ì„œ
$h(n) = |\alpha - \beta|$
$= |(3 + \sqrt{n}) - (3 - \sqrt{n})|$
$= 2\sqrt{n}$
ì´ë¯€ë¡œ

$\lim_{n \to \infty} \sqrt{n} \{ h(n+1) - h(n) \}$
$= \lim_{n \to \infty} \sqrt{n} (2\sqrt{n+1} - 2\sqrt{n})$
$= \lim_{n \to \infty} \frac{2\sqrt{n} (\sqrt{n+1} - \sqrt{n})(\sqrt{n+1} + \sqrt{n})}{\sqrt{n+1} + \sqrt{n}}$
$= \lim_{n \to \infty} \frac{2\sqrt{n}}{\sqrt{n+1} + \sqrt{n}}$
$= \lim_{n \to \infty} \frac{2}{\sqrt{1 + \frac{1}{n}} + 1}$
$= \frac{2}{1 + 1}$
$= 1$

ì •ë‹µ: â‘¡