## 문제
수열 $\{ a_{n} \}$ 에 대하여 $\sum _{n=1} ^{\infty} \left( a_{n} - \frac{5n^{2} + 1}{2n + 3} \right) = 4$ 일 때, $\lim _{n \to \infty} \frac{2a_{n}}{n + 1}$ 의 값은? 

## 보기
① $3$   ② $\frac{7}{2}$   ③ $4$   ④ $\frac{9}{2}$   ⑤ $5$

## 풀이
[정답] ⑤ 

[해설] 
$b_{n} = a_{n} - \frac{5n^{2} + 1}{2n + 3}$ 이라 하면 
$\sum _{n=1} ^{\infty} b_{n} = 4$ 이므로 
$\lim _{n \to \infty} b_{n} = 0$ 

$a_{n} = b_{n} + \frac{5n^{2} + 1}{2n + 3}$ 이므로 
$\lim _{n \to \infty} \frac{2 a_{n}}{n + 1}$ 
$= \lim _{n \to \infty} \left( \frac{2 b_{n}}{n + 1} + \frac{2(5n^{2} + 1)}{(2n + 3)(n + 1)} \right)$ 
$= \lim _{n \to \infty} \frac{2 b_{n}}{n + 1} + \lim _{n \to \infty} \frac{2(5n^{2} + 1)}{(2n + 3)(n + 1)}$ 
$= 0 + 5$ 
$= 5$ 

[참고] 
문제의 조건을 만족시키는 수열 $\{ a_{n} \}$ 의 여러 예 중 하나는 
$a_{n} = \frac{5n^{2} + 1}{2n + 3} + \frac{4}{2^{n}}$ 이다.