## 문제
두 수열 $\{ a_{n} \}$, $\{ b_{n} \}$ 이 모든 자연수 $n$ 에 대하여 다음 조건을 만족시킨다. $a_{10}$ 의 값을 구하시오.

$$ \begin{array}{l} (가) \sum_{k=1}^{n} b_{k}=n^{2}+n \\ (나) \sum_{k=1}^{n} a_{k} b_{k}-5 \sum_{k=1}^{n} b_{k}=\frac{n^{2}(n+1)^{2}}{2} \end{array} $$

## 보기

## 풀이
$\sum_{k=1}^{n} k = \frac{n(n+1)}{2} = \frac{n^{2}+n}{2}$ 이므로
$\sum_{k=1}^{n} b_{k} = 2 \sum_{k=1}^{n} k = \sum_{k=1}^{n} 2k$ 이다. 그러므로 $b_{k} = 2k$ 이다.

$\sum_{k=1}^{n} k^{3} = \left\{ \frac{n(n+1)}{2} \right\}^{2} = \frac{n^{2}(n+1)^{2}}{4}$ 이므로
$\sum_{k=1}^{n} ( a_{k} - 5 ) b_{k} = 2 \sum_{k=1}^{n} k^{3} = \sum_{k=1}^{n} 2k^{3}$ 이다. 
그러므로 $( a_{k} - 5 ) b_{k} = 2k^{3}$ 이다. 
따라서 $b_{k} = 2k$ 이므로 $a_{k} - 5 = k^{2}$ 이다. 

$a_{k} = k^{2} + 5$ 이므로 $a_{10} = 105$ 이다. 

[다른 풀이] 
수열의 합과 일반항 사이의 관계에 의해서 
$b_{n} = ( n^{2} + n ) - \{ ( n - 1 )^{2} + ( n - 1 ) \} = 2n$ ($n \ge 2$) 
$b_{1} = 1^{2} + 1 = 2$ 이므로 모든 자연수 $n$ 에 대하여 $b_{n} = 2n$ 이다. 

$\sum_{k=1}^{n} a_{k} b_{k} - 5 \sum_{k=1}^{n} b_{k} = \sum_{k=1}^{n} (a_{k} - 5)b_{k}$ 이므로 
$( a_{n} - 5 ) b_{n} = \frac{n^{2} ( n + 1 )^{2}}{2} - \frac{( n - 1 )^{2} n^{2}}{2} = 2n^{3}$ ($n \ge 2$) 
$( a_{1} - 5 ) b_{1} = \frac{1^{2} \times 2^{2}}{2} = 2$ 이므로 모든 자연수 $n$ 에 대하여 $( a_{n} - 5 ) b_{n} = 2n^{3}$ 이다. 

$b_{n} = 2n$ 이므로 $a_{n} = n^{2} + 5$ 이다. 
따라서 $a_{10} = 105$ 이다.