## 문제
수열 $\{ a_{n} \}$ 에 대하여 급수 $\sum_{n=1}^{\infty} \left( a_{n} - \frac{2 \times 3^{n+1} + 2^{n}}{3^{n} + 2^{n}} \right)$ 이 수렴할 때, $\lim_{n \to \infty} a_{n}$ 의 값은?

## 보기
① $2$   ② $3$   ③ $4$   ④ $5$   ⑤ $6$

## 풀이
급수 $\sum_{n=1}^{\infty} \left( a_{n} - \frac{2 \times 3^{n+1} + 2^{n}}{3^{n} + 2^{n}} \right)$ 이 수렴하므로 
$\lim_{n \to \infty} \left( a_{n} - \frac{2 \times 3^{n+1} + 2^{n}}{3^{n} + 2^{n}} \right) = 0$ 이다.

$b_{n} = a_{n} - \frac{2 \times 3^{n+1} + 2^{n}}{3^{n} + 2^{n}}$ 이라 하자. 따라서 
$a_{n} = b_{n} + \frac{2 \times 3^{n+1} + 2^{n}}{3^{n} + 2^{n}}$, $\lim_{n \to \infty} b_{n} = 0$ 이고

$\lim_{n \to \infty} \frac{2 \times 3^{n+1} + 2^{n}}{3^{n} + 2^{n}} = \lim_{n \to \infty} \frac{2 \times \frac{3^{n+1}}{3^{n}} + \frac{2^{n}}{3^{n}}}{1 + \frac{2^{n}}{3^{n}}}$
$= \lim_{n \to \infty} \frac{6 + \left( \frac{2}{3} \right)^{n}}{1 + \left( \frac{2}{3} \right)^{n}} = 6$ 이다.

따라서 
$\lim_{n \to \infty} a_{n} = \lim_{n \to \infty} \left( b_{n} + \frac{2 \times 3^{n+1} + 2^{n}}{3^{n} + 2^{n}} \right)$
$= 0 + 6 = 6$ 이다.

정답: ⑤