## 문제
두 수열 $\{ a_n \}$, $\{ b_n \}$이 다음 조건을 만족시킨다.

(가) $\sum_{k=1}^{n} (a_k + b_k) = \frac{1}{n+1} \quad (n \geq 1)$
(나) $\lim_{n \to \infty} n^2 b_n = 2$

$\lim_{n \to \infty} n^2 a_n$의 값은?

## 보기
① $-3$   ② $-2$   ③ $-1$   ④ $0$   ⑤ $1$

## 풀이
$\sum_{k=1}^{n} (a_k + b_k) = S_n$이라 하면
$a_n + b_n = S_n - S_{n-1}$ ($n \geq 2$)
$= \frac{1}{n+1} - \frac{1}{n}$
$= -\frac{1}{n(n+1)}$

$\lim_{n \to \infty} n^2 (a_n + b_n) = \lim_{n \to \infty} (n^2 a_n + n^2 b_n)$
$= \lim_{n \to \infty} -\frac{n^2}{n(n+1)}$
$= -1$

또, 조건 (나)에 의해
$\lim_{n \to \infty} n^2 b_n = 2$

따라서
$\lim_{n \to \infty} n^2 a_n = \lim_{n \to \infty} (n^2 a_n + n^2 b_n - n^2 b_n)$
$= \lim_{n \to \infty} (n^2 a_n + n^2 b_n) - \lim_{n \to \infty} n^2 b_n$
$= -1 - 2$
$= -3$

정답: ①