## 문제
수열 $\{$ $a_{n}$ $\}$ 에 대하여 
$$\sum_{n=1}^{\infty} \left( na_{n} - \frac{6n^{2}+1}{n+2} \right)$$
이 수렴할 때, $\lim_{n \to \infty} (2a_{n})^{2}$ 의 값을 구하시오.

## 보기

## 풀이
$\sum_{n=1}^{\infty} \left( na_{n} - \frac{6n^{2}+1}{n+2} \right)$ 이 수렴하므로 
$$\lim_{n \to \infty} \left( na_{n} - \frac{6n^{2}+1}{n+2} \right) = 0$$ 
$na_{n} - \frac{6n^{2}+1}{n+2} = b_{n}$ 이라 하면 
$$\lim_{n \to \infty} b_{n} = 0$$ 
$a_{n} = \frac{b_{n}}{n} + \frac{6n^{2}+1}{n(n+2)}$ 이므로 
$$\lim_{n \to \infty} a_{n} = \lim_{n \to \infty} \left( \frac{b_{n}}{n} + \frac{6n^{2}+1}{n(n+2)} \right) = 6$$ 
따라서 
$$\lim_{n \to \infty} (2a_{n})^{2} = 144$$

[정답] $144$