## 문제
$f(\log_{3} 6) = \frac{\log_{3} 6 + 1}{2 \log_{3} 6 - 1}$ 이고, $\log 2 = a$, $\log 3 = b$ 라 할 때, $f(\log_{3} 6)$ 의 값을 $a$, $b$ 로 나타낸 것은?

## 보기
① $\frac{a + 2b}{a + b}$   ② $\frac{2a + b}{a + b}$   ③ $\frac{2a + b}{a + 2b}$   ④ $\frac{a + b}{2a + b}$   ⑤ $\frac{a + 2b}{2a + b}$

## 풀이
$f(\log_{3} 6) = \frac{\log_{3} 6 + 1}{2 \log_{3} 6 - 1}$ 에서 
$\log_{3} 6 + 1 = \log_{3} 6 + \log_{3} 3 = \log_{3} 18$
$2 \log_{3} 6 - 1 = \log_{3} 6^{2} - \log_{3} 3 = \log_{3} 12$
로그의 밑의 변환 공식에 의하여
$f(\log_{3} 6) = \frac{\log_{3} 18}{\log_{3} 12}$
$= \frac{\frac{\log 18}{\log 3}}{\frac{\log 12}{\log 3}} = \frac{\log 18}{\log 12}$
$= \frac{\log(2 \times 3^{2})}{\log(2^{2} \times 3)} = \frac{\log 2 + 2 \log 3}{2 \log 2 + \log 3} = \frac{a + 2b}{2a + b}$

[다른 풀이]
$\log_{3} 6 = \frac{\log 6}{\log 3} = \frac{\log(2 \times 3)}{\log 3} = \frac{\log 2 + \log 3}{\log 3} = \frac{a + b}{b}$
$f(\log_{3} 6) = f\left( \frac{a + b}{b} \right) = \frac{\frac{a + b}{b} + 1}{2 \times \frac{a + b}{b} - 1}$
$= \frac{\frac{a + 2b}{b}}{\frac{2a + b}{b}} = \frac{\frac{a + 2b}{b} \times b}{\frac{2a + b}{b} \times b} = \frac{a + 2b}{2a + b}$

따라서 정답은 ⑤이다.