## ë¬¸ì œ
ìžì—°ìˆ˜ $n$ ì— ëŒ€í•˜ì—¬ í•¨ìˆ˜ $y = e^{-x} - \frac{n-1}{e}$ ì˜ ê·¸ëž˜í”„ì™€ í•¨ìˆ˜ $y = |\ln x|$ ì˜ ê·¸ëž˜í”„ê°€ ë§Œë‚˜ëŠ” ì ì˜ ê°œìˆ˜ë¥¼ $f(n)$ ì´ë¼ í•  ë•Œ, $f(1) + f(2)$ ì˜ ê°’ì€?

## ë³´ê¸°
â‘  $1$   â‘¡ $2$   â‘¢ $3$   â‘£ $4$   â‘¤ $5$

## í’€ì´
ì •ë‹µ â‘¢

$y = e^{-x} - \frac{n-1}{e}$, 
$y = |\ln x|$ ì˜ êµì ì˜ ê°œìˆ˜ëŠ” 

â…°) $n = 1$ ì¼ ë•Œ, 
$y = e^{-x}$ ê³¼ $y = |\ln x|$ ì˜ êµì ì˜ ê°œìˆ˜ê°€ $2$ ì´ë¯€ë¡œ 
$f(1) = 2$ 

â…±) $n = 2$ ì¼ ë•Œ, 
$y = e^{-x} - \frac{1}{e}$ ê³¼ $y = |\ln x|$ ì˜ êµì ì´ $(1, 0)$ ë¿ì´ë¯€ë¡œ 
$f(2) = 1$ 

ë”°ë¼ì„œ 
$f(1) + f(2) = 2 + 1 = 3$

> [!example] ðŸ“¸ (ê·¸ë¦¼/ê·¸ëž˜í”„)