## ë¬¸ì œ

í•¨ìˆ˜ $f(x) = \begin{cases} e^{x} & (x \le 0, x \ge 2) \\ \ln (x+1) & (0 < x < 2) \end{cases}$ ì´ê³ , í•¨ìˆ˜ $y=g(x)$ì˜ ê·¸ë˜í”„ê°€ ê·¸ë¦¼ê³¼ ê°™ë‹¤.

> [!example] ğŸ“¸ (ê·¸ë¦¼/ê·¸ë˜í”„)

$\lim_{x \to 2+} f(g(x)) + \lim_{x \to 0+} g(f(x))$ì˜ ê°’ì€?

## ë³´ê¸°

â‘  $e$   â‘¡ $e+1$   â‘¢ $e+2$   â‘£ $e^{2}+1$   â‘¤ $e^{2}+2$

## í’€ì´

[ì •ë‹µ] â‘¤

í•¨ìˆ˜ $f(x) = \begin{cases} e^{x} & (x \le 0, x \ge 2) \\ \ln (x+1) & (0 < x < 2) \end{cases}$ ì™€ í•¨ìˆ˜ $g(x)$ì— ëŒ€í•˜ì—¬

$i$) $g(x)=t$ë¡œ ë†“ìœ¼ë©´ 
$x \to 2+$ì¼ ë•Œ $g(x) \to 2+$ì´ë¯€ë¡œ 
$\lim_{x \to 2+} f(g(x)) = \lim_{t \to 2+} f(t) = e^{2}$

$ii$) $f(x)=s$ë¡œ ë†“ìœ¼ë©´ 
$x \to 0+$ì¼ ë•Œ $f(x) \to 0+$ì´ë¯€ë¡œ 
$\lim_{x \to 0+} g(f(x)) = \lim_{s \to 0+} g(s) = 2$

ë”°ë¼ì„œ 
$\lim_{x \to 2+} f(g(x)) + \lim_{x \to 0+} g(f(x)) = e^{2}+2$