## 문제
함수 `$f(x) = 3x^{2} + ax + b$` 가 `$\lim_{h \to 0} \frac{f(2+h)-4}{h} = 3$` 을 만족시킬 때, 두 상수 `$a$`, `$b$` 에 대하여 `$a^{2} + b^{2}$` 의 값을 구하시오.

## 풀이
`$\lim_{h \to 0} \frac{f(2+h)-4}{h} = 3$` 에서
`$\lim_{h \to 0} h = 0$` 이므로
`$\lim_{h \to 0} \{f(2+h) - 4\} = 0$` 이다.
`$\therefore f(2) = 4$`
`$f(2) = 12 + 2a + b = 4$` 에서
`$2a + b = -8$` `$\cdots \cdots$` ㉠
`$\lim_{h \to 0} \frac{f(2+h)-4}{h} = \lim_{h \to 0} \frac{f(2+h) - f(2)}{h} = f'(2) = 3$`
`$f'(x) = 6x + a$` 이므로
`$f'(2) = 12 + a = 3$`, `$a = -9$` `$\cdots \cdots$` ㉡
㉠, ㉡에서
`$a = -9$`, `$b = 10$`
`$\therefore a^{2} + b^{2} = 81 + 100 = 181$`