## ๋ฌธ์
๋ถ๋ฑ์ $(x^{2}-y ) (x^{2}+y-1 ) \geq 0$ ์ ์์ญ์ ์ขํํ๋ฉด ์์ ์ด๋์ด ๋ถ๋ถ์ผ๋ก ๋ฐ๋ฅด๊ฒ ๋ํ๋ธ ๊ฒ์? (๋จ, ๊ฒฝ๊ณ์์ ํฌํจํ๋ค.)

## ๋ณด๊ธฐ
โ > [!example] ๐ธ (๊ทธ๋ฆผ/๊ทธ๋ํ)

โก > [!example] ๐ธ (๊ทธ๋ฆผ/๊ทธ๋ํ)

โข > [!example] ๐ธ (๊ทธ๋ฆผ/๊ทธ๋ํ)

โฃ > [!example] ๐ธ (๊ทธ๋ฆผ/๊ทธ๋ํ)

โค > [!example] ๐ธ (๊ทธ๋ฆผ/๊ทธ๋ํ)

## ํ์ด
[์๋ต] โข 

$(x^{2}-y ) (x^{2}+y-1 ) \geq 0$ ์์ 
$$ \left\{ \begin{array}{l} x^{2}-y \geq 0 \\ x^{2}+y-1 \geq 0 \end{array} \right. $$ ๋๋ $$ \left\{ \begin{array}{l} x^{2}-y \leq 0 \\ x^{2}+y-1 \leq 0 \end{array} \right. $$ 

($i$) $$ \left\{ \begin{array}{l} x^{2}-y \geq 0 \\ x^{2}+y-1 \geq 0 \end{array} \right. $$ ์ ์์ญ์ 
$y=x^{2}$ ์ ๊ทธ๋ํ์ ์๋ซ๋ถ๋ถ(๊ฒฝ๊ณ์ ํฌํจ)๊ณผ ์ด์ฐจํจ์ $y=-x^{2}+1$ ์ ๊ทธ๋ํ์ ์๋ถ๋ถ(๊ฒฝ๊ณ์ ํฌํจ)์ ๊ณตํต๋ถ๋ถ์ผ๋ก [๊ทธ๋ฆผ $1$]์ ์ด๋์ด ๋ถ๋ถ์ด๋ค.

> [!example] ๐ธ (๊ทธ๋ฆผ/๊ทธ๋ํ)
[๊ทธ๋ฆผ $1$]

($ii$) $$ \left\{ \begin{array}{l} x^{2}-y \leq 0 \\ x^{2}+y-1 \leq 0 \end{array} \right. $$ ์ ์์ญ์ 
$y=x^{2}$ ์ ๊ทธ๋ํ์ ์๋ถ๋ถ(๊ฒฝ๊ณ์ ํฌํจ)๊ณผ ์ด์ฐจํจ์ $y=-x^{2}+1$ ์ ๊ทธ๋ํ์ ์๋ซ๋ถ๋ถ(๊ฒฝ๊ณ์ ํฌํจ)์ ๊ณตํต๋ถ๋ถ์ผ๋ก [๊ทธ๋ฆผ $2$]์ ์ด๋์ด ๋ถ๋ถ์ด๋ค. 

> [!example] ๐ธ (๊ทธ๋ฆผ/๊ทธ๋ํ)
[๊ทธ๋ฆผ $2$]

($i$), ($ii$)์ ์ํ์ฌ ๊ตฌํ๋ ์์ญ์ [๊ทธ๋ฆผ $3$]์ ์ด๋์ด ๋ถ๋ถ์ด๋ค. 

> [!example] ๐ธ (๊ทธ๋ฆผ/๊ทธ๋ํ)
[๊ทธ๋ฆผ $3$]

(๋จ, ๊ฒฝ๊ณ์์ ํฌํจํ๋ค.)