## 문제
수열 $\{ a_{n} \}$은 $a_{1}+a_{2}=8$이고, 
$$\sum_{k=2}^{n} a_{k}- \sum_{k=1}^{n-1} a_{k}=2 n^{2}+2 \ (n \geq 2)$$ 
를 만족시킨다. 
$\sum_{k=1}^{10} a_{k}$의 값은? 

## 보기
① $756$   ② $766$   ③ $776$   ④ $786$   ⑤ $796$

## 풀이
$$\sum_{k=2}^{n} a_{k}- \sum_{k=1}^{n-1} a_{k}=2 n^{2}+2 \ (n \geq 2) \cdots \cdots$$ ㉠ 
㉠에 $n=2$를 대입하면 
$$a_{2}-a_{1}=10$$ 
두 식 $a_{1}+a_{2}=8$, $a_{2}-a_{1}=10$을 연립하여 풀면 
$$a_{1}=-1, a_{2}=9$$ 

$2$ 이상인 자연수 $n$에 대하여 
$$\sum_{k=2}^{n} a_{k}- \sum_{k=1}^{n-1} a_{k}$$ 
$$= (a_{2}+a_{3}+ \cdots+a_{n-1}+a_{n} )- (a_{1}+a_{2}+ \cdots+a_{n-1} )$$ 
$$=a_{n}-a_{1}$$ 
$$=a_{n}+1$$ 
㉠에서 
$$a_{n}+1=2 n^{2}+2$$ 
$$a_{n}=2 n^{2}+1 \ (n \geq 2)$$ 
따라서 수열 $\{ a_{n} \}$은 
$$a_{1}=-1, a_{n}=2 n^{2}+1 \ (n \geq 2)$$ 

$$\sum_{k=1}^{10} a_{k}=a_{1}+ \sum_{k=2}^{10} a_{k}$$ 
$$=-1+ \sum_{k=2}^{10} (2 k^{2}+1 )$$ 
$$=-1+ \sum_{k=1}^{10} (2 k^{2}+1 )-(2 \cdot 1^2 + 1)$$
$$=-1+ \sum_{k=1}^{10} (2 k^{2}+1 )-3$$ 
$$=-4+2 \sum_{k=1}^{10} k^{2}+1 \times 10$$ 
$$=-4+2 \times \frac{10 \times 11 \times 21}{6}+10$$ 
$$=776$$ 
정답은 ③입니다.