## 문제
실수 $x$, $y$, $z$가 
$x+y+z=5$, $x^{2}+y^{2}+z^{2}=15$, $xyz=-3$
을 만족시킬 때, $x^{5}+y^{5}+z^{5}$의 값을 구하시오.

## 보기

## 풀이
$x+y+z=5$, $x^{2}+y^{2}+z^{2}=15$, $xyz=-3$이므로 
$xy+yz+zx = \frac{1}{2} \{ (x+y+z)^{2}-(x^{2}+y^{2}+z^{2}) \} = \frac{1}{2} (5^{2}-15) = 5$

$x^{3}+y^{3}+z^{3} = (x+y+z)(x^{2}+y^{2}+z^{2}-xy-yz-zx)+3xyz$
$= 5 \times (15-5) + 3 \times (-3) = 50-9 = 41$

$x^{5}+y^{5}+z^{5} = (x^{2}+y^{2}+z^{2})(x^{3}+y^{3}+z^{3}) - \{ x^{2}y^{2}(x+y)+y^{2}z^{2}(y+z)+z^{2}x^{2}(z+x) \}$
$= (x^{2}+y^{2}+z^{2})(x^{3}+y^{3}+z^{3}) - \{ x^{2}y^{2}(5-z)+y^{2}z^{2}(5-x)+z^{2}x^{2}(5-y) \}$
$= (x^{2}+y^{2}+z^{2})(x^{3}+y^{3}+z^{3}) - 5(x^{2}y^{2}+y^{2}z^{2}+z^{2}x^{2})+xyz(xy+yz+zx)$
$= (x^{2}+y^{2}+z^{2})(x^{3}+y^{3}+z^{3}) - 5 \{ (xy+yz+zx)^{2}-2xyz(x+y+z) \} + xyz(xy+yz+zx)$
$= 15 \times 41 - 5(5^{2}+30) - 3 \times 5$
$= 615 - 275 - 15$
$= 325$

정답: $325$