## ë¬¸ì œ
ìì—°ìˆ˜ $n$ì— ëŒ€í•˜ì—¬ ì§ì„  $x=4^{n}$ì´ ê³¡ì„  $y=\sqrt{x}$ì™€ ë§Œë‚˜ëŠ” ì ì„ $P_{n}$ì´ë¼ í•˜ì. ì„ ë¶„ $P_{n}P_{n+1}$ì˜ ê¸¸ì´ë¥¼ $L_{n}$ì´ë¼ í•  ë•Œ, $\lim_{n \to \infty} \left( \frac{L_{n+1}}{L_{n}} \right)^{2}$ì˜ ê°’ì„ êµ¬í•˜ì‹œì˜¤.



> [!example] ğŸ“¸ (ê·¸ë¦¼/ê·¸ë˜í”„)

## í’€ì´
$P_{n}(4^{n}, 2^{n})$, $P_{n+1}(4^{n+1}, 2^{n+1})$ì´ë¯€ë¡œ 
$$L_{n} = \sqrt{(4^{n+1} - 4^{n})^{2} + (2^{n+1} - 2^{n})^{2}}$$
$$= \sqrt{(3 \times 4^{n})^{2} + (2^{n})^{2}}$$
$$= \sqrt{9 \times 16^{n} + 4^{n}}$$
ë”°ë¼ì„œ
$$\lim_{n \to \infty} \left( \frac{L_{n+1}}{L_{n}} \right)^{2}$$
$$= \lim_{n \to \infty} \frac{9 \times 16^{n+1} + 4^{n+1}}{9 \times 16^{n} + 4^{n}}$$
$$= \lim_{n \to \infty} \frac{9 \times 16 + 4 \times \left( \frac{1}{4} \right)^{n}}{9 + \left( \frac{1}{4} \right)^{n}}$$
$$= \frac{9 \times 16 + 4 \times 0}{9 + 0} = 16$$

ì •ë‹µ: $16$