## 문제
두 다항함수 $f(x)$, $g(x)$가 
$$\lim_{x \to 0} \frac{f(x)-2}{x} = 3, \lim_{x \to 3} \frac{g(x-3)-1}{x-3} = 6$$ 
을 만족시킨다. 함수 $h(x)=f(x)g(x)$일 때, $h'(0)$의 값을 구하시오.

## 보기


## 풀이
$\lim_{x \to 0} \frac{f(x)-2}{x} = 3$ 이므로 
$f(0)=2$ 이고 $f'(0)=3$ 

$\lim_{x \to 3} \frac{g(x-3)-1}{x-3} = 6$ 이므로 
$x-3=t$ 라 두면 $x \to 3$ 일 때 $t \to 0$ 

$\lim_{t \to 0} \frac{g(t)-1}{t} = 6$ 
$g(0)=1$ 이고 $g'(0)=6$ 

$h(x)=f(x)g(x)$ 이므로 
$h'(x)=f'(x)g(x) + f(x)g'(x)$ 

$h'(0)=f'(0)g(0)+f(0)g'(0) = 3 \times 1 + 2 \times 6 = 15$ 

정답: $15$