## 문제
다항식 $x ^{4} -2x ^{3} +2x ^{2} -x-6$이 $( x+1 ) ( x+a ) ( x ^{2} +bx+c )$로 인수분해될 때, 세 정수 $a$, $b$, $c$의 합 $a+b+c$의 값은?

## 보기
① $-2$   ② $-1$   ③ $0$   ④ $1$   ⑤ $2$

## 풀이
$P ( x ) = x ^{4} -2x ^{3} +2x ^{2} -x-6$로 놓으면 
$P ( -1 ) = ( -1 )^{4} - 2 ( -1 )^{3} +2 ( -1 )^{2} - ( -1 )-6=0$ 
$P ( 2 ) = ( 2 ) ^{4} -2 ( 2 ) ^{3} +2 (2 )^{2} - ( 2 ) -6=0$ 
이므로 조립제법을 이용하여 $P ( x )$를 인수분해하면 

$$ \begin{array}{r|rrrrr} -1 & 1 & -2 & 2 & -1 & -6 \\ \multicolumn{1}{r|}{} & & -1 & 3 & -5 & 6 \\ \hline 2 & 1 & -3 & 5 & -6 & 0 \\ \multicolumn{1}{r|}{} & & 2 & -2 & 6 & \\ \hline & 1 & -1 & 3 & 0 & \end{array} $$

$x ^{4} -2x ^{3} +2x ^{2} -x-6$ 
$= ( x+1 ) ( x^{3}-3x^{2}+5x-6 )$ 
$= ( x+1 ) ( x-2 ) ( x^{2}-x+3 )$ 

따라서 
$a=-2$, $b=-1$, $c=3$ 
이므로 
$a+b+c=0$ 

정답은 ③입니다.