## 문제
실수 전체의 집합에서 미분가능한 함수 $f(x)$가 다음 조건을 만족시킨다.

$$
\begin{array}{|l|}
\hline
(\text{가}) \ f(0)=0, \ f'(0)=1 \\
(\text{나}) \ \text{모든 실수 } x, y \text{에 대하여 } f(x+y)= \frac{f(x)+f(y)}{1+f(x)f(y)} \text{이다.} \\
\hline
\end{array}
$$

$f(-1)=k$ ($-1 < k < 0$)일 때, $\int_{0}^{1} f(x)^2 dx$의 값을 $k$로 나타낸 것은?

## 보기
① $1-k^2$   ② $1-2k$   ③ $1-k$   ④ $1+k$   ⑤ $1+k^2$

## 풀이
$f(x+y)= \frac{f(x)+f(y)}{1+f(x)f(y)}$에서 $x=1, y=-1$을 대입하면
$f(0)= \frac{f(1)+f(-1)}{1+f(1)f(-1)}$
$f(0)=0$이므로 $f(1)+f(-1)=0$
따라서 $f(1)=-f(-1)=-k$이다.

$f'(x) = \lim_{h \to 0} \frac{f(x+h)-f(x)}{h}$
$= \lim_{h \to 0} \frac{\frac{f(x)+f(h)}{1+f(x)f(h)} -f(x)}{h}$
$= \lim_{h \to 0} \frac{f(h)(1-f(x)^2)}{h(1+f(x)f(h))}$
$= \lim_{h \to 0} \frac{f(h)}{h} \times \lim_{h \to 0} \frac{1-f(x)^2}{1+f(x)f(h)}$
$f(0)=0$이므로 $\lim_{h \to 0} \frac{f(h)}{h} = f'(0) = 1$이고, $\lim_{h \to 0} f(h) = f(0) = 0$이다.
$= f'(0) \times (1-f(x)^2)$
$= 1-f(x)^2$

따라서 $f(x)^2 = 1-f'(x)$이므로
$\int_{0}^{1} f(x)^2 dx = \int_{0}^{1} (1-f'(x)) dx$
$= [x-f(x)]_{0}^{1}$
$= (1-f(1)) - (0-f(0))$
$= 1-(-k) - 0 = 1+k$

정답은 ④이다.