## ë¬¸ì œ
ë‘ ì  $O(0, 0)$, $A(3, 0)$ì— ëŒ€í•˜ì—¬ ì  $P$ê°€ ê³¡ì„  $y = 2x^2$ ìœ„ë¥¼ ì›€ì§ì¼ ë•Œ, $\overline{OP}^2 + \overline{AP}^2$ì˜ ìµœì†Ÿê°’ì€?



> [!example] ğŸ“¸ (ê·¸ë¦¼/ê·¸ë˜í”„)

## ë³´ê¸°
â‘  $7$   â‘¡ $\frac{15}{2}$   â‘¢ $8$   â‘£ $\frac{17}{2}$   â‘¤ $9$

## í’€ì´
$OA$ì˜ ì¤‘ì ì„ $M$ì´ë¼ê³  í•˜ë©´ $M\left(\frac{3}{2}, 0\right)$ì´ë‹¤.
íŒŒí‘¸ìŠ¤ì˜ ì¤‘ì„ ì •ë¦¬ì— ì˜í•´
$\overline{OP}^2 + \overline{AP}^2 = 2(\overline{OM}^2 + \overline{PM}^2)$ì´ê³ , $\overline{OM}^2 = \frac{9}{4}$ì´ë‹¤.
$\overline{PM}^2 = \left(x - \frac{3}{2}\right)^2 + y^2 = x^2 - 3x + \frac{9}{4} + 4x^4 = f(x)$ë¼ í•˜ë©´
$f'(x) = 16x^3 + 2x - 3 = (2x - 1)(8x^2 + 4x + 3)$
ë”°ë¼ì„œ $x = \frac{1}{2}$ì¼ ë•Œ $f(x)$ëŠ” ìµœì†Ÿê°’(ê·¹ì†Ÿê°’)ì„ ê°€ì§„ë‹¤.
$x = \frac{1}{2}$ì¼ ë•Œ $y = 2x^2 = \frac{1}{2}$ì´ë¯€ë¡œ
$\overline{PM}^2$ì˜ ìµœì†Ÿê°’ì€ $\left(\frac{1}{2} - \frac{3}{2}\right)^2 + \left(\frac{1}{2}\right)^2 = 1 + \frac{1}{4} = \frac{5}{4}$ì´ë‹¤.
ê·¸ëŸ¬ë¯€ë¡œ êµ¬í•˜ë ¤ëŠ” ìµœì†Ÿê°’ì€
$2\left(\frac{9}{4} + \frac{5}{4}\right) = 2 \times \frac{14}{4} = 7$ì´ë‹¤.

ì •ë‹µ: â‘ 