## 문제
세 다항식 $f(x) = x^{2} + x$, $g(x) = x^{2} - 2x - 1$, $h(x)$에 대하여 
$\{f(x)\}^{3} + \{g(x)\}^{3} = (2x^{2} - x - 1)h(x)$
가 $x$에 대한 항등식일 때, $h(x)$를 $x - 1$로 나누었을 때의 나머지는?

## 보기
① $8$   ② $9$   ③ $10$   ④ $11$   ⑤ $12$

## 풀이
$\{f(x)\}^{3} + \{g(x)\}^{3} = (2x^{2} - x - 1)h(x)$이므로 
$\{f(x) + g(x)\}[\{f(x)\}^{2} - f(x)g(x) + \{g(x)\}^{2}] = (2x^{2} - x - 1)h(x)$
이때, 
$f(x) + g(x) = (x^{2} + x) + (x^{2} - 2x - 1) = 2x^{2} - x - 1$이므로 
$h(x) = \{f(x)\}^{2} - f(x)g(x) + \{g(x)\}^{2}$
$f(1) = 2$, $g(1) = -2$이므로 위 식의 양변에 $x = 1$을 대입하면 
$h(1) = 2^{2} - 2 \times (-2) + (-2)^{2} = 12$
따라서 $h(x)$를 $x - 1$로 나누었을 때의 나머지는 $h(1) = 12$이다.

정답: ⑤