## ë¬¸ì œ
ê³¡ì„  $y = 1 - x^{2}$ ($0 < x < 1$) ìœ„ì˜ ì  $P$ì—ì„œ $y$ì¶•ì— ë‚´ë¦° ìˆ˜ì„ ì˜ ë°œì„ $H$ë¼ í•˜ê³ , ì›ì  $O$ì™€ ì  $A(0, 1)$ì— ëŒ€í•˜ì—¬ $\angle APH = \theta_{1}$, $\angle HPO = \theta_{2}$ë¼ í•˜ì. $\tan \theta_{1} = \frac{1}{2}$ ì¼ ë•Œ, $\tan (\theta_{1} + \theta_{2})$ì˜ ê°’ì€?



> [!example] ğŸ“¸ (ê·¸ë¦¼/ê·¸ë˜í”„)

## ë³´ê¸°
â‘  $2$   â‘¡ $4$   â‘¢ $6$   â‘£ $8$   â‘¤ $10$

## í’€ì´
ì  $P$ì˜ ì¢Œí‘œë¥¼ $(t, 1 - t^{2})$ì´ë¼ í•˜ì.
ì§ê°ì‚¼ê°í˜• $AHP$ì—ì„œ $\tan \theta_{1} = \frac{1}{2}$ì´ë¯€ë¡œ
$\tan \theta_{1} = \frac{\overline{AH}}{\overline{HP}} = \frac{\overline{AO} - \overline{HO}}{\overline{HP}} = \frac{1 - (1 - t^{2})}{t} = \frac{t^{2}}{t} = t = \frac{1}{2}$
ì´ë•Œ, $P \left( \frac{1}{2}, \frac{3}{4} \right)$ì´ê³  ì§ê°ì‚¼ê°í˜• $PHO$ì—ì„œ
$\tan \theta_{2} = \frac{\overline{HO}}{\overline{PH}} = \frac{\frac{3}{4}}{\frac{1}{2}} = \frac{3}{2}$
ë”°ë¼ì„œ
$\tan (\theta_{1} + \theta_{2}) = \frac{\tan \theta_{1} + \tan \theta_{2}}{1 - \tan \theta_{1} \tan \theta_{2}} = \frac{\frac{1}{2} + \frac{3}{2}}{1 - \frac{1}{2} \times \frac{3}{2}} = \frac{2}{1 - \frac{3}{4}} = \frac{2}{\frac{1}{4}} = 8$

ì •ë‹µ: â‘£