## 문제
수열 $\{ a_{n} \}$ 에 대하여 $\sum_{n=1}^{\infty} \frac{2^{n} a_{n} - 2^{n+1}}{2^{n} + 1} = 1$ 일 때, $\lim_{n \to \infty} a_{n}$ 의 값은?

## 보기
① $1$   ② $2$   ③ $3$   ④ $4$   ⑤ $5$

## 풀이
$\sum_{n=1}^{\infty} \frac{2^{n} a_{n} - 2^{n+1}}{2^{n} + 1} = 1$ 이므로 
$\lim_{n \to \infty} \frac{2^{n} a_{n} - 2^{n+1}}{2^{n} + 1} = 0$ 

$\frac{2^{n} a_{n} - 2^{n+1}}{2^{n} + 1} = b_{n}$ 이라 하면 
$\lim_{n \to \infty} b_{n} = 0$ 

$a_{n} = \frac{( 2^{n} + 1 ) b_{n} + 2^{n+1}}{2^{n}}$ 이므로 

$\lim_{n \to \infty} a_{n}$ 
$= \lim_{n \to \infty} \frac{( 2^{n} + 1 ) b_{n} + 2^{n+1}}{2^{n}}$ 
$= \lim_{n \to \infty} \left\{ \left( 1 + \frac{1}{2^{n}} \right) b_{n} + 2 \right\} = 2$

따라서 정답은 ② 이다.