## 문제
수열 $\{ a_{n} \}$ 에 대하여 $\sum_{k=1}^{n} a_{k} = n^{2} - 2 n$ 일 때, $\sum_{k=6}^{10} a_{k}$ 의 값을 구하시오.

## 보기


## 풀이
$\sum_{k=6}^{10} a_{k}$
$= \sum_{k=1}^{10} a_{k} - \sum_{k=1}^{5} a_{k}$
$= ( 10^{2} - 2 \times 10 ) - ( 5^{2} - 2 \times 5 )$
$= 80 - 15$
$= 65$

**[다른 풀이]**
수열 $\{ a_{n} \}$ 의 첫째항부터 제 $n$ 항까지의 합을 $S_{n}$ 이라 하면
$a_{n} = S_{n} - S_{n-1}$
$= ( n^{2} - 2 n ) - \{ ( n - 1 )^{2} - 2 ( n - 1 ) \}$
$= 2 n - 3$ ($n \ge 2$)
$a_{1} = S_{1} = -1$ 이므로
$a_{n} = 2 n - 3$ ($n \ge 1$)
따라서 수열 $\{ a_{n} \}$ 은 첫째항이 $-1$ 이고 공차가 $2$ 인 등차수열이다.
$a_{6} = 9$, $a_{10} = 17$ 이므로
$\sum_{k=6}^{10} a_{k} = \frac{5 ( 9 + 17 )}{2} = 65$