## 문제
$\frac{218^{3} + 1}{217^{3} - 1}$ 의 값은?

## 보기
① $\frac{73}{72}$   ② $\frac{37}{36}$   ③ $\frac{25}{24}$   ④ $\frac{19}{18}$   ⑤ $\frac{13}{12}$

## 풀이
[정답] ①

$218 = n$ 으로 놓으면 
$218^{3} + 1 = n^{3} + 1 = (n + 1)(n^{2} - n + 1)$
$217^{3} - 1 = (n - 1)^{3} - 1$
$= \{(n - 1) - 1\}\{(n - 1)^{2} + (n - 1) + 1\}$
$= (n - 2)(n^{2} - n + 1)$
이므로
$\frac{218^{3} + 1}{217^{3} - 1} = \frac{(n + 1)(n^{2} - n + 1)}{(n - 2)(n^{2} - n + 1)}$
$= \frac{n + 1}{n - 2}$
$= \frac{218 + 1}{218 - 2}$
$= \frac{219}{216}$
$= \frac{73}{72}$

[다른 풀이]
$217 = n$ 으로 놓으면
$218^{3} + 1 = (n + 1)^{3} + 1$
$= \{(n + 1) + 1\}\{(n + 1)^{2} - (n + 1) + 1\}$
$= (n + 2)(n^{2} + n + 1)$
$217^{3} - 1 = n^{3} - 1 = (n - 1)(n^{2} + n + 1)$
이므로
$\frac{218^{3} + 1}{217^{3} - 1} = \frac{(n + 2)(n^{2} + n + 1)}{(n - 1)(n^{2} + n + 1)}$
$= \frac{n + 2}{n - 1}$
$= \frac{217 + 2}{217 - 1}$
$= \frac{219}{216}$
$= \frac{73}{72}$