## 문제
함수 $f(x) = \begin{cases} \sqrt{2x} & (x \ge 0) \\ 4x & (x < 0) \end{cases}$ 의 역함수 $g(x)$ 에 대하여 부등식 $g(x) \le -\frac{1}{4}x^2 + 3$ 의 해가 $a \le x \le b$ 일 때, $a+b$ 의 값은?

## 보기
① $-2$   ② $-1$   ③ $0$   ④ $1$   ⑤ $2$

## 풀이
$f(x) = \begin{cases} \sqrt{2x} & (x \ge 0) \\ 4x & (x < 0) \end{cases}$ 이므로 함수 $f(x)$ 의 역함수 $g(x)$ 를 구하면 다음과 같다.
$g(x) = \begin{cases} \frac{1}{2}x^2 & (x \ge 0) \\ \frac{1}{4}x & (x < 0) \end{cases}$

(ⅰ) $x \ge 0$ 인 경우
$g(x) \le -\frac{1}{4}x^2 + 3$
$\frac{1}{2}x^2 \le -\frac{1}{4}x^2 + 3$
$\frac{3}{4}x^2 \le 3$
$x^2 \le 4$
$-2 \le x \le 2$
$x \ge 0$ 이므로 $0 \le x \le 2$

(ⅱ) $x < 0$ 인 경우
$g(x) \le -\frac{1}{4}x^2 + 3$
$\frac{1}{4}x \le -\frac{1}{4}x^2 + 3$
$\frac{1}{4}x^2 + \frac{1}{4}x - 3 \le 0$
$x^2 + x - 12 \le 0$
$(x+4)(x-3) \le 0$
$-4 \le x \le 3$
$x < 0$ 이므로 $-4 \le x < 0$

(ⅰ), (ⅱ)에서 부등식의 해는 $-4 \le x \le 2$ 이다.
따라서 $a = -4$, $b = 2$ 이므로
$a+b = -2$

정답: ①