## 문제
첫째항이 $1$인 등차수열 $\{ a_{n} \}$에 대하여 수열 $\{ b_{n} \}$을 
$b_{n} = a_{1} + 2 a_{2} + 3 a_{3} + \cdots + n a_{n} \quad ( n \ge 1 )$
이라 하자. $b_{10} = 715$일 때, $\sum_{n=1}^{10} \frac{b_{n}}{n ( n+1 )}$의 값은?

## 보기
① $30$   ② $35$   ③ $40$   ④ $45$   ⑤ $50$

## 풀이
[정답] ②

등차수열 $\{ a_{n} \}$의 공차를 $d$라 하면 
$a_{n} = 1 + ( n-1 ) d$이므로 

$b_{n} = \sum_{k=1}^{n} k \{ 1 + ( k-1 ) d \}$
$= \sum_{k=1}^{n} \{ d k^{2} + ( 1-d ) k \}$
$= d \sum_{k=1}^{n} k^{2} + ( 1-d ) \sum_{k=1}^{n} k$
$= \frac{d n ( n+1 ) ( 2n+1 )}{6} + \frac{( 1-d ) n ( n+1 )}{2}$
$= \frac{n ( n+1 )}{6} \times \{ d ( 2n+1 ) + 3 ( 1-d ) \}$
$= \frac{n ( n+1 )}{6} \times ( 2dn-2d+3 )$

$b_{10} = 715$이므로 
$\frac{10 \times 11}{6} \times ( 20d-2d+3 ) = 715$
$18d+3 = 39$
$18d = 36$
$d = 2$

$b_{n} = \frac{n ( n+1 )}{6} \times ( 2 \times 2 \times n - 2 \times 2 + 3 )$
$= \frac{n ( n+1 )}{6} \times ( 4n-1 )$

$\frac{b_{n}}{n ( n+1 )} = \frac{1}{6} ( 4n-1 )$

따라서 
$\sum_{n=1}^{10} \frac{b_{n}}{n ( n+1 )} = \sum_{n=1}^{10} \frac{1}{6} ( 4n-1 )$
$= \frac{1}{6} ( 220-10 )$
$= 35$

[다른 풀이] 
등차수열 $\{ a_{n} \}$의 공차를 $d$라 하면 
$a_{n} = 1 + ( n-1 ) d$이므로 

$b_{n} = \sum_{k=1}^{n} k \{ 1 + ( k-1 ) d \}$
$= \sum_{k=1}^{n} \{ d k^{2} + ( 1-d ) k \}$
$= d \sum_{k=1}^{n} k^{2} + ( 1-d ) \sum_{k=1}^{n} k$
$= \frac{d n ( n+1 ) ( 2n+1 )}{6} + \frac{( 1-d ) n ( n+1 )}{2}$
$= \frac{n ( n+1 )}{6} \times \{ d ( 2n+1 ) + 3 ( 1-d ) \}$
$= \frac{n ( n+1 )}{6} \times ( 2dn-2d+3 )$

$\frac{b_{n}}{n ( n+1 )} = \frac{3-2d+2dn}{6}$
$= \frac{1}{2} + ( n-1 ) \frac{d}{3}$

이므로 수열 $\{ \frac{b_{n}}{n ( n+1 )} \}$은 첫째항이 $\frac{1}{2}$이고 공차가 $\frac{d}{3}$인 등차수열이다. 

$b_{10} = 715$이므로 수열 $\{ \frac{b_{n}}{n ( n+1 )} \}$의 제 $10$항은 
$\frac{b_{10}}{10 \times 11} = \frac{715}{10 \times 11} = \frac{13}{2}$

따라서 
$\sum_{n=1}^{10} \frac{b_{n}}{n ( n+1 )} = \frac{10 \times ( \frac{1}{2} + \frac{13}{2} )}{2}$
$= \frac{10 \times 7}{2}$
$= 35$