## 문제
수열 $\{ a_{n} \}$ 에 대하여 급수 $\sum_{n=1}^{\infty} \left( \frac{2n}{12n+3} a_{n} - 1 \right)$ 이 수렴할 때, $\lim_{n \to \infty} a_{n}$ 의 값을 구하시오.

## 보기
(해당 문제에는 객관식 보기가 없습니다.)

## 풀이
급수 $\sum_{n=1}^{\infty} \left( \frac{2n}{12n+3} a_{n} - 1 \right)$ 이 수렴하므로 
$\lim_{n \to \infty} \left( \frac{2n}{12n+3} a_{n} - 1 \right) = 0$ 이고, $\lim_{n \to \infty} \frac{2n}{12n+3} a_{n} = 1$ 이다.
수열 $\{ b_{n} \}$ 을 $b_{n} = \frac{2n}{12n+3} a_{n}$ 이라 하면 $\lim_{n \to \infty} b_{n} = 1$ 이다.
이때 $a_{n} = \frac{12n+3}{2n} b_{n}$ 이므로
$$\lim_{n \to \infty} a_{n} = \lim_{n \to \infty} \left( \frac{12n+3}{2n} b_{n} \right)$$
$$= \lim_{n \to \infty} \frac{12n+3}{2n} \times \lim_{n \to \infty} b_{n}$$
$$= 6 \times 1 = 6$$

정답: $6$