## 문제
다항식 $x^{10}+x^{5}+3$을 $x^{2}+x+1$, $x^{2}-x+1$, $(x^{2}+x+1)(x^{2}-x+1)$로 나눈 나머지를 각각 $r_{1}(x)$, $r_{2}(x)$, $r_{3}(x)$라 할 때, $r_{1}(x)r_{2}(x)r_{3}(x)$를 $x-1$로 나눈 나머지는?

## 보기
① $-4$   ② $-2$   ③ $2$   ④ $4$   ⑤ $6$

## 풀이
ㄱ. $x^{10}+x^{5}+3 = (x^{2}+x+1)Q_{1}(x)+r_{1}(x)$에서
$x^{10}+x^{5}+3 = x(x^{9}-1)+x^{2}(x^{3}-1)+(x^{2}+x+1)+2$이므로
$r_{1}(x) = 2$

ㄴ. $x^{10}+x^{5}+3 = (x^{2}-x+1)Q_{2}(x)+r_{2}(x)$에서
$x^{10}+x^{5}+3 = x(x^{9}+1)+x^{2}(x^{3}+1)-(x^{2}-x+1)-2x+4$ 이므로
$r_{2}(x) = -2x+4$

ㄷ. $x^{10}+x^{5}+3 = (x^{4}+x^{2}+1)Q_{3}(x)+r_{3}(x)$에서
$x^{10}+x^{5}+3 = x^{4}(x^{3}+1)(x^{3}-1)+(x+1)(x^{4}+x^{2}+1)+(-x^{3}-x^{2}-x+2)$이므로
$r_{3}(x) = -x^{3}-x^{2}-x+2$

따라서 $r_{1}(1) = 2$, $r_{2}(1) = 2$, $r_{3}(1) = -1$이다.
나머지 정리에 의해 구하는 나머지는 
$\therefore r_{1}(1)r_{2}(1)r_{3}(1) = 2 \times 2 \times (-1) = -4$

정답: ①