## 문제
함수 $f(x)=(x-1)^{4}(x+1)$ 에 대하여 이차함수 $g(x)$, $h(x)$ 가 
$$ f(x)=g(x)+ \int_{0}^{x}(x-t)^{2} h(t) d t $$
를 만족시킬 때, $g(2)+h(2)$ 의 값을 구하시오.

## 풀이
$f(x)=(x-1)^{4}(x+1)$ 에서 
$$ f'(x)=4(x-1)^{3}(x+1)+(x-1)^{4}=(x-1)^{3}(5x+3) $$ 
$$ f''(x)=3(x-1)^{2}(5x+3)+5(x-1)^{3}=(x-1)^{2}(20x+4) $$ 
이차함수 $g(x)=ax^{2}+bx+c$ 라 하고 
$$ \begin{aligned} f(x) &= g(x)+\int_{0}^{x}(x-t)^{2} h(t) dt \\ &= g(x)+x^{2} \int_{0}^{x} h(t) dt-2x \int_{0}^{x} t h(t) dt+\int_{0}^{x} t^{2} h(t) dt \end{aligned} $$ 
$x=0$ 을 대입하면 $f(0)=g(0)$ 이므로 $\therefore c=1$ 

이제 양변을 미분하면 
$$ \begin{aligned} f'(x) &= (x-1)^{3}(5x+3) \\ &= 2ax+b+2x \int_{0}^{x} h(t) dt+x^{2} h(x)-2 \int_{0}^{x} t h(t) dt-2xh(x)+xh(x) \\ &= 2ax+b+2x \int_{0}^{x} h(t) dt-2 \int_{0}^{x} t h(t) dt \end{aligned} $$ 
$x=0$ 을 대입하면 $-3=b$ 

또 양변을 미분하면 
$$ \begin{aligned} f''(x) &= (x-1)^{2}(20x+4) \\ &= 2a+2 \int_{0}^{x} h(t) dt+2xh(x)-2xh(x) \\ &= 2a+2 \int_{0}^{x} h(t) dt \end{aligned} $$ 
$x=0$ 을 대입하면 $4=2a$ 이므로 $\therefore a=2$ 

또 양변을 미분하면 
$$ f'''(x) = 12(x-1)(5x-1)=2h(x) $$ 
그러므로 
$$ g(x)=2x^{2}-3x+1, h(x)=6(x-1)(5x-1) $$ 
$\therefore g(2)+h(2)=3+54=57$