## 문제
두 양수 $a$, $b$에 대하여 
$2^{a} = 3^{b}$, $(a-2)(b-2)=4$
일 때, $4^{a} \times 3^{-b}$의 값은?

## 보기
① $12$   ② $18$   ③ $36$   ④ $54$   ⑤ $72$

## 풀이
[정답] ③ 

[해설] 
$2^{a} = 3^{b} = k$ ($k>1$)이라 놓으면 
$2=k^{\frac{1}{a}}$, $3=k^{\frac{1}{b}}$ 

$(a-2)(b-2)=4$에서 
$ab-2a-2b+4=4$
$ab-2(a+b)=0$
$\frac{a+b}{ab}=\frac{1}{2}$ 

$k^{\frac{1}{a}} \times k^{\frac{1}{b}} = k^{\frac{a+b}{ab}} = k^{\frac{1}{2}} = 2 \times 3 = 6$ 
따라서 
$4^{a} \times 3^{-b} = \frac{(2^{a})^{2}}{3^{b}} = \frac{k^{2}}{k} = k = 36$ 

[다른 풀이] 
$2^{a} = 3^{b} = k$ ($k>1$)이라 놓으면 
$a=\log_{2} k$, $b=\log_{3} k$ 

$(a-2)(b-2)=(\log_{2} k-2)(\log_{3} k-2)$ 
$= \log_{2} k \times \log_{3} k - 2\log_{2} k - 2\log_{3} k + 4 = 4$ 
$\log_{2} k \times \log_{3} k - 2(\log_{2} k + \log_{3} k) = 0$ 

$\frac{\log_{2} k + \log_{3} k}{\log_{2} k \times \log_{3} k} = \frac{1}{2}$ 
$\frac{1}{\log_{2} k} + \frac{1}{\log_{3} k} = \frac{1}{2}$ 

$\log_{k} 2 + \log_{k} 3 = \log_{k} 6 = \frac{1}{2}$ 
즉, $k^{\frac{1}{2}} = 6$ 
따라서 
$4^{a} \times 3^{-b} = \frac{(2^{a})^{2}}{3^{b}} = \frac{k^{2}}{k} = k = 36$