## 문제
함수 $f(x) = \frac{1}{1+e^{-x}}$의 역함수를 $g(x)$라 할 때, $g'(f(-1))$의 값은?

## 보기
① $\frac{1}{(1+e)^{2}}$   ② $\frac{1}{1+e}$   ③ $\left(\frac{1+e}{e}\right)^{2}$   ④ $\frac{e^{2}}{1+e}$   ⑤ $\frac{(1+e)^{2}}{e}$

## 풀이
함수 $f(x) = \frac{1}{1+e^{-x}}$를 미분하면
$f'(x) = \frac{e^{-x}}{(1+e^{-x})^{2}}$ $\cdots$ $㉠$

$g(x)$는 $f(x)$의 역함수이므로 $g(f(x)) = x$가 성립한다. 
양변을 $x$에 대하여 미분하면 $g'(f(x))f'(x) = 1$
즉, $g'(f(x)) = \frac{1}{f'(x)}$이므로 $x = -1$을 대입하면
$\therefore g'(f(-1)) = \frac{1}{f'(-1)}$

$㉠$에 $x = -1$을 대입하면
$f'(-1) = \frac{e^{-(-1)}}{(1+e^{-(-1)})^{2}} = \frac{e}{(1+e)^{2}}$

따라서
$g'(f(-1)) = \frac{1}{\frac{e}{(1+e)^{2}}} = \frac{(1+e)^{2}}{e}$

정답: ⑤