## ë¬¸ì œ
ê³¡ì„  $y=e^{\frac{x}{3}}$ê³¼ ì´ ê³¡ì„  ìœ„ì˜ ì  $(3, e)$ì—ì„œì˜ ì ‘ì„  ë° $y$ì¶•ìœ¼ë¡œ ë‘˜ëŸ¬ì‹¸ì¸ ë„í˜•ì˜ ë„“ì´ëŠ”?



> [!example] ğŸ“¸ (ê·¸ë¦¼/ê·¸ë˜í”„)

## ë³´ê¸°
â‘  $\frac{e}{2}-1$   â‘¡ $e-2$   â‘¢ $\frac{3}{2}e-3$   â‘£ $2e-4$   â‘¤ $\frac{5}{2}e-5$

## í’€ì´
$y' = \frac{1}{3} e^{\frac{x}{3}}$ ì´ë¯€ë¡œ ì  $(3, e)$ì—ì„œì˜ ì ‘ì„ ì˜ ë°©ì •ì‹ì€ 
$y = \frac{e}{3}x$ ì´ë‹¤.

êµ¬í•˜ëŠ” ë„í˜•ì˜ ë„“ì´ $S$ëŠ”
$$ \begin{array}{l} S = \int_{0}^{3} \left( e^{\frac{x}{3}} - \frac{e}{3}x \right) dx \\ S = \left[ 3e^{\frac{x}{3}} - \frac{e}{6}x^2 \right]_{0}^{3} \\ S = \left( 3e - \frac{9e}{6} \right) - \left( 3e^0 - 0 \right) \\ S = \frac{3}{2}e - 3 \end{array} $$

ì •ë‹µ: â‘¢