## 문제
두 다항함수 $f(x)$, $g(x)$에 대하여 $f(1)=2$, $f'(1)=3$, $g(1)=5$, $g'(1)=2$일 때,
$$\lim_{n \to \infty} n \left\{ f \left( 1+\frac{1}{n} \right) g \left( 1+\frac{3}{n} \right) - f(1)g(1) \right\}$$
의 값을 구하시오.

## 풀이
$\frac{1}{n} = h$라 하면, $n \to \infty$일 때, $h \to 0+$이다.
$$\lim_{h \to 0+} \frac{f(1+h)g(1+3h) - f(1)g(1)}{h}$$
$$= \lim_{h \to 0+} \frac{f(1+h)g(1+3h) - f(1+h)g(1)}{h} + \lim_{h \to 0+} \frac{f(1+h)g(1) - f(1)g(1)}{h}$$
$$= 3 \times \lim_{h \to 0+} \frac{f(1+h) \{ g(1+3h) - g(1) \}}{3h} + \lim_{h \to 0+} \frac{ \{ f(1+h) - f(1) \} g(1)}{h}$$
$$= 3f(1)g'(1) + f'(1)g(1)$$
주어진 조건 $f(1)=2$, $f'(1)=3$, $g(1)=5$, $g'(1)=2$를 대입하면
$$3 \times 2 \times 2 + 3 \times 5 = 12 + 15 = 27$$
따라서 정답은 $27$이다.