## ë¬¸ì œ
í•¨ìˆ˜ $y=f(x)$ì˜ ê·¸ë˜í”„ê°€ ê·¸ë¦¼ê³¼ ê°™ë‹¤. ìµœê³ ì°¨í•­ì˜ ê³„ìˆ˜ê°€ $1$ì¸ ì´ì°¨í•¨ìˆ˜ $g(x)$ì— ëŒ€í•˜ì—¬ 
$$\lim_{x \to 0+} \frac{g(x)}{f(x)}=1$$, $$\lim_{x \to 1-} f(x-1) g(x)=3$$
ì¼ ë•Œ, $g(2)$ì˜ ê°’ì€? 

> [!example] ğŸ“¸ (ê·¸ë¦¼/ê·¸ë˜í”„)

## ë³´ê¸°
â‘  $3$   â‘¡ $5$   â‘¢ $7$   â‘£ $9$   â‘¤ $11$

## í’€ì´
ê·¸ë˜í”„ì—ì„œ $\lim_{x \to 0+} f(x)=-1$ì´ë¯€ë¡œ,
$$\lim_{x \to 0+} \frac{g(x)}{f(x)}=\frac{g(0)}{-1}=1$$
$g(0)=-1$

ë˜í•œ, $\lim_{x \to 1-} f(x-1)= \lim_{x \to 0-} f(x)=1$ì´ë¯€ë¡œ,
$$\lim_{x \to 1-} f(x-1) g(x)=1 \times g(1)=3$$
$g(1)=3$

$g(x)=x^{2}+a x+b$ë¼ ë†“ìœ¼ë©´
$g(0)=b=-1$,
$g(1)=1+a+b=3$ì´ë¯€ë¡œ
$1+a-1=3$ì—ì„œ $a=3$ì´ë‹¤.

ë”°ë¼ì„œ $g(x)=x^{2}+3 x-1$ì´ë©°,
$\therefore g(2)=2^{2}+3 \times 2-1=4+6-1=9$

ì •ë‹µ: â‘£