## 문제
자연수 $n$ 에 대하여 $x$ 에 대한 이차방정식 $x^{2} - 2nx + n^{2} - 1 = 0$ 의 두 근의 곱을 $a_{n}$ 이라 할 때, $\sum_{n=2}^{\infty} \frac{2}{a_{n}}$ 의 값은?

## 보기
① $\frac{1}{2}$   ② $1$   ③ $\frac{3}{2}$   ④ $2$   ⑤ $\frac{5}{2}$

## 풀이
이차방정식의 근과 계수의 관계에서 $a_{n} = n^{2} - 1$ 이다. 따라서 
$$\sum_{n=2}^{\infty} \frac{2}{a_{n}} = \lim_{n \to \infty} \sum_{k=2}^{n} \frac{2}{a_{k}}$$
$$= \lim_{n \to \infty} \sum_{k=2}^{n} \frac{2}{(k-1)(k+1)}$$
$$= \lim_{n \to \infty} \sum_{k=2}^{n} \left( \frac{1}{k-1} - \frac{1}{k+1} \right)$$
$$= \lim_{n \to \infty} \left\{ \left( \frac{1}{1} - \frac{1}{3} \right) + \left( \frac{1}{2} - \frac{1}{4} \right) + \left( \frac{1}{3} - \frac{1}{5} \right) + \dots + \left( \frac{1}{n-2} - \frac{1}{n} \right) + \left( \frac{1}{n-1} - \frac{1}{n+1} \right) \right\}$$
$$= \lim_{n \to \infty} \left( \frac{1}{1} + \frac{1}{2} - \frac{1}{n} - \frac{1}{n+1} \right)$$
$$= \frac{3}{2}$$
이다.
그러므로 정답은 ③이다.