## 문제
$x$ 에 대한 방정식 
$$(1+x)(1+x^{2})(1+x^{4})=x^{7}+x^{6}+x^{5}+x^{4}$$
의 세 근을 각각 $\alpha$, $\beta$, $\gamma$ 라 할 때, $\alpha^{4}+\beta^{4}+\gamma^{4}$ 의 값은?

## 보기
① $3$   ② $7$   ③ $11$   ④ $15$   ⑤ $19$

## 풀이
방정식 $(1+x)(1+x^{2})(1+x^{4})=x^{7}+x^{6}+x^{5}+x^{4}$ 에서 
$$1+x+x^{2}+x^{3}+x^{4}+x^{5}+x^{6}+x^{7}=x^{7}+x^{6}+x^{5}+x^{4}$$ 
$$x^{3}+x^{2}+x+1=0$$ 
$$(x+1)+x^{2}(x+1)=0$$ 
$$(x+1)(x^{2}+1)=0$$ 
$\therefore$ $x=-1$ 또는 $x^{2}=-1$ 

따라서 주어진 방정식의 세 근은 $-1$, $i$, $-i$ 이므로 
$$\alpha^{4}+\beta^{4}+\gamma^{4}$$ 
$$=(-1)^{4}+i^{4}+(-i)^{4}$$ 
$$=1+1+1$$ 
$$=3$$ 

**[다른 풀이]** 
방정식 $(1+x)(1+x^{2})(1+x^{4})=x^{7}+x^{6}+x^{5}+x^{4}$ 에서 우변을 인수분해하면 
$$x^{4}(x^{3}+x^{2}+x+1)$$ 
$$=x^{4}\{x^{2}(x+1)+x+1\}$$ 
$$=x^{4}(x^{2}+1)(x+1)$$ 
이므로 
$$(x+1)(x^{2}+1)(x^{4}+1)=x^{4}(x^{2}+1)(x+1)$$ 
$$(x+1)(x^{2}+1)(x^{4}+1)-x^{4}(x^{2}+1)(x+1)=0$$ 
$$(x+1)(x^{2}+1)(x^{4}+1-x^{4})=0$$ 
$$(x+1)(x^{2}+1)=0$$ 
$\therefore$ $x=-1$ 또는 $x^{2}=-1$ 

따라서 주어진 방정식의 세 근은 $-1$, $i$, $-i$ 이므로 
$$\alpha^{4}+\beta^{4}+\gamma^{4}$$ 
$$=(-1)^{4}+i^{4}+(-i)^{4}$$ 
$$=1+1+1$$ 
$$=3$$