## 문제
$x=0$ 에서 $x=\ln 2$ 까지의 곡선 $y = \frac{1}{8} e^{2x} + \frac{1}{2} e^{-2x}$ 의 길이는?

## 보기
① $\frac{1}{2}$   ② $\frac{9}{16}$   ③ $\frac{5}{8}$   ④ $\frac{11}{16}$   ⑤ $\frac{3}{4}$

## 풀이
$y = \frac{1}{8} e^{2x} + \frac{1}{2} e^{-2x}$ 에서
$\frac{dy}{dx} = \frac{1}{8} e^{2x} \times 2 + \frac{1}{2} e^{-2x} \times (-2) = \frac{1}{4} e^{2x} - e^{-2x}$
이므로 구하는 곡선의 길이는
$\int_{0}^{\ln 2} \sqrt{1 + \left( \frac{dy}{dx} \right)^{2}} dx$
$= \int_{0}^{\ln 2} \sqrt{1 + \left( \frac{1}{4} e^{2x} - e^{-2x} \right)^{2}} dx$
$= \int_{0}^{\ln 2} \sqrt{1 + \left( \frac{1}{16} e^{4x} - \frac{1}{2} + e^{-4x} \right)} dx$
$= \int_{0}^{\ln 2} \sqrt{\frac{1}{16} e^{4x} + \frac{1}{2} + e^{-4x}} dx$
$= \int_{0}^{\ln 2} \sqrt{\left( \frac{1}{4} e^{2x} + e^{-2x} \right)^{2}} dx$
$= \int_{0}^{\ln 2} \left( \frac{1}{4} e^{2x} + e^{-2x} \right) dx$
$= \left[ \frac{1}{8} e^{2x} - \frac{1}{2} e^{-2x} \right]_{0}^{\ln 2}$
$= \left( \frac{1}{8} e^{2 \ln 2} - \frac{1}{2} e^{-2 \ln 2} \right) - \left( \frac{1}{8} e^{0} - \frac{1}{2} e^{0} \right)$
$= \left( \frac{1}{8} e^{\ln 4} - \frac{1}{2} e^{\ln \frac{1}{4}} \right) - \left( \frac{1}{8} - \frac{1}{2} \right)$
$= \left( \frac{1}{8} \times 4 - \frac{1}{2} \times \frac{1}{4} \right) - \left( -\frac{3}{8} \right)$
$= \left( \frac{1}{2} - \frac{1}{8} \right) + \frac{3}{8}$
$= \frac{3}{8} + \frac{3}{8} = \frac{3}{4}$

정답: ⑤