## 문제
수열 $\{ a_{n} \}$ 은 $a_{1}=1$ 이고,
$\sum _{k=1} ^{n} \left( \frac{1}{a_{k}} - \frac{1}{a_{k+1}} \right) = \frac{2n}{2n+1}$ ($n=1, 2, 3, \dots$)
을 만족시킨다. $a_{10}$ 의 값은?

## 보기
① $10$   ② $13$   ③ $16$   ④ $19$   ⑤ $22$

## 풀이
$\sum _{k=1} ^{n} \left( \frac{1}{a_{k}} - \frac{1}{a_{k+1}} \right)$
$= \left( \frac{1}{a_{1}} - \frac{1}{a_{2}} \right) + \left( \frac{1}{a_{2}} - \frac{1}{a_{3}} \right) + \dots + \left( \frac{1}{a_{n}} - \frac{1}{a_{n+1}} \right)$
$= \frac{1}{a_{1}} - \frac{1}{a_{n+1}}$
$= 1 - \frac{1}{a_{n+1}}$
이므로
$\sum _{k=1} ^{n} \left( \frac{1}{a_{k}} - \frac{1}{a_{k+1}} \right) = \frac{2n}{2n+1}$ ($n \ge 1$)에서
$1 - \frac{1}{a_{n+1}} = \frac{2n}{2n+1}$
$1 - \frac{1}{a_{n+1}} = 1 - \frac{1}{2n+1}$
이므로
$\frac{1}{a_{n+1}} = \frac{1}{2n+1}$
$a_{n+1} = 2n+1$ ($n \ge 1$)
$a_{n} = 2n-1$ ($n \ge 2$)
$a_{1} = 1$ 이므로
$a_{n} = 2n-1$ ($n \ge 1$)
따라서
$a_{10} = 2 \times 10 - 1 = 19$

[정답] ④