## ë¬¸ì œ
í•¨ìˆ˜ $f(x)=(x-1)^{3}+(x-1)$ ì˜ ì—­í•¨ìˆ˜ë¥¼ $g(x)$ ë¼ í•  ë•Œ, $\int_{2}^{10} g(x) dx$ ì˜ ê°’ì€?



> [!example] ğŸ“¸ (ê·¸ë¦¼/ê·¸ë˜í”„)

## ë³´ê¸°
â‘  $\frac{51}{4}$   â‘¡ $\frac{59}{4}$   â‘¢ $\frac{67}{4}$   â‘£ $\frac{75}{4}$   â‘¤ $\frac{83}{4}$

## í’€ì´
$f(2) = (2-1)^3 + (2-1) = 2$
$f(3) = (3-1)^3 + (3-1) = 10$ ì´ë¯€ë¡œ 
ì—­í•¨ìˆ˜ì˜ ì ë¶„ ì„±ì§ˆì— ì˜í•´
$$\int_{2}^{10} g(x) dx = (3 \times 10 - 2 \times 2) - \int_{2}^{3} f(x) dx$$
$$\int_{2}^{10} g(x) dx = 26 - \int_{2}^{3} f(x) dx$$

ì´ë•Œ, 
$$\int_{2}^{3} f(x) dx = \int_{2}^{3} \{ (x-1)^{3}+(x-1) \} dx$$
$$= \left[ \frac{1}{4}(x-1)^{4} + \frac{1}{2}(x-1)^{2} \right]_{2}^{3}$$
$$= \left( \frac{16}{4} + \frac{4}{2} \right) - \left( \frac{1}{4} + \frac{1}{2} \right)$$
$$= 6 - \frac{3}{4} = \frac{21}{4}$$

ë”°ë¼ì„œ
$$\int_{2}^{10} g(x) dx = 26 - \frac{21}{4} = \frac{83}{4}$$

ì •ë‹µ: â‘¤