## 문제
함수 $f(x) = \frac{x-1}{2x-6}$과 $3$ 이상의 자연수 $k$에 대하여 
$$\lim_{n \to \infty} \frac{|f(3-a)|^{n+1}}{2^{n} + |1-f(3+a)|^{n}} = k$$ 
를 만족시키는 모든 실수 $a$의 값의 합을 $g(k)$라 하자. 
$\sum_{k=3}^{17} g(k)$의 값은?

## 보기
① $-\frac{2}{7}$   ② $-\frac{12}{35}$   ③ $-\frac{2}{5}$   ④ $-\frac{16}{35}$   ⑤ $-\frac{18}{35}$

## 풀이
[정답] ② 

함수 $f(x) = \frac{x-1}{2x-6}$에 대하여 

$|f(3-a)| = \left| \frac{(3-a)-1}{2(3-a)-6} \right| = \left| \frac{2-a}{-2a} \right| = \left| \frac{a-2}{2a} \right|$ 

$|1-f(3+a)| = \left| 1- \frac{(3+a)-1}{2(3+a)-6} \right| = \left| \frac{a-2}{2a} \right|$ 

이다. 
$h(a) = \frac{a-2}{2a}$ ($a \neq 0$)라 하면 

$$\lim_{n \to \infty} \frac{|f(3-a)|^{n+1}}{2^{n} + |1-f(3+a)|^{n}} = \lim_{n \to \infty} \frac{|h(a)|^{n+1}}{2^{n} + |h(a)|^{n}}$$ 

이다. 

(ⅰ) $|h(a)| < 2$일 때, 
$\left| \frac{h(a)}{2} \right| < 1$이고 $\lim_{n \to \infty} \left| \frac{h(a)}{2} \right|^{n} = 0$이므로 

$$\lim_{n \to \infty} \frac{|h(a)|^{n+1}}{2^{n} + |h(a)|^{n}} = \lim_{n \to \infty} \frac{2 \left| \frac{h(a)}{2} \right|^{n+1}}{1+ \left| \frac{h(a)}{2} \right|^{n}} = 0$$ 

이 되어 $k=0$이다. 

(ⅱ) $|h(a)| = 2$일 때, 

$$\lim_{n \to \infty} \frac{|h(a)|^{n+1}}{2^{n} + |h(a)|^{n}} = \lim_{n \to \infty} \frac{2^{n+1}}{2^{n} + 2^{n}} = 1$$ 

이 되어 $k=1$이다. 

(ⅲ) $|h(a)| > 2$일 때, 
$\left| \frac{2}{h(a)} \right| < 1$이고 $\lim_{n \to \infty} \left| \frac{2}{h(a)} \right|^{n} = 0$이므로 

$$\lim_{n \to \infty} \frac{|h(a)|^{n+1}}{2^{n} + |h(a)|^{n}} = \lim_{n \to \infty} \frac{|h(a)|}{\left| \frac{2}{h(a)} \right|^{n} + 1} = |h(a)|$$ 

이다. 

$|h(a)| = \left| \frac{a-2}{2a} \right| = \left| \frac{1}{a} - \frac{1}{2} \right| = k$ ($k \ge 3$인 자연수)를 만족시키는 $a$를 구하면 

$\frac{1}{a} - \frac{1}{2} = k$일 때, $a = \frac{2}{2k+1}$ 

$\frac{1}{a} - \frac{1}{2} = -k$일 때, $a = -\frac{2}{2k-1}$ 

이다. 따라서 $g(k) = -2 \left( \frac{1}{2k-1} - \frac{1}{2k+1} \right)$이다. 

$$\sum_{k=3}^{17} g(k) = -2 \sum_{k=3}^{17} \left( \frac{1}{2k-1} - \frac{1}{2k+1} \right)$$ 

$$= -2 \left( \frac{1}{5} - \frac{1}{7} + \frac{1}{7} - \frac{1}{9} + \cdots + \frac{1}{33} - \frac{1}{35} \right)$$ 

$$= -2 \left( \frac{1}{5} - \frac{1}{35} \right) = -\frac{12}{35}$$