## ë¬¸ì œ
ê·¸ë¦¼ê³¼ ê°™ì´ ìì—°ìˆ˜ $n$ ì— ëŒ€í•˜ì—¬ ì§ì„  $x=n$ ì´ ë‘ ê³¡ì„  $y= \sqrt{5x+4}$ , $y= \sqrt{2x-1}$ ê³¼ ë§Œë‚˜ëŠ” ì ì„ ê°ê° $A_{n}$ , $B_{n}$ ì´ë¼ í•˜ì. ì„ ë¶„ $OA_{n}$ ì˜ ê¸¸ì´ë¥¼ $a_{n}$ , ì„ ë¶„ $OB_{n}$ ì˜ ê¸¸ì´ë¥¼ $b_{n}$ ì´ë¼ í•  ë•Œ, $\lim_{n \to \infty} \frac{12}{a_{n} - b_{n}}$ ì˜ ê°’ì€? (ë‹¨, $O$ ëŠ” ì›ì ì´ë‹¤.)

> [!example] ğŸ“¸ (ê·¸ë¦¼/ê·¸ë˜í”„)

## ë³´ê¸°
â‘  $4$   â‘¡ $6$   â‘¢ $8$   â‘£ $10$   â‘¤ $12$

## í’€ì´
$A_{n} (n, \sqrt{5n+4})$ , $B_{n} (n, \sqrt{2n-1})$ ì´ë¯€ë¡œ 

$a_{n} = \sqrt{n^{2} +5n+4}$ , $b_{n} = \sqrt{n^{2} +2n-1}$ 

$\lim_{n \to \infty} \frac{12}{a_{n} - b_{n}}$ 

$= \lim_{n \to \infty} \frac{12}{\sqrt{n^{2} +5n+4} - \sqrt{n^{2} +2n-1}}$ 

$= \lim_{n \to \infty} \frac{12 (\sqrt{n^{2} +5n+4} + \sqrt{n^{2} +2n-1})}{3n+5}$ 

$= \lim_{n \to \infty} \frac{12 (\sqrt{1+ \frac{5}{n} + \frac{4}{n^{2}}} + \sqrt{1+ \frac{2}{n} - \frac{1}{n^{2}}})}{3+ \frac{5}{n}}$ 

$= \frac{12 \times (1+1)}{3} = 8$ 

ì •ë‹µ â‘¢