## 문제
수열 $\{ a_{n} \}$ 이 모든 자연수 $n$ 에 대하여 
$$\sum_{k=1}^{n} a_{2k-1} = 3n^{2} - n, \quad \sum_{k=1}^{2n} a_{k} = 6n^{2} + n$$ 
을 만족시킬 때, $\sum_{k=1}^{24} ( -1 )^{k} a_{k}$ 의 값은?

## 보기
① $18$   ② $24$   ③ $30$   ④ $36$   ⑤ $42$

## 풀이
$\sum_{k=1}^{24} ( -1 )^{k} a_{k}$ 
$= -a_{1} + a_{2} - a_{3} + a_{4} - \cdots - a_{23} + a_{24}$ 
$= ( a_{1} + a_{2} + a_{3} + \cdots + a_{24} ) - 2 ( a_{1} + a_{3} + a_{5} + \cdots + a_{23} )$ 
$= \sum_{k=1}^{24} a_{k} - 2 \sum_{k=1}^{12} a_{2k-1}$ 

주어진 식 $\sum_{k=1}^{2n} a_{k} = 6n^{2} + n$ 에 $n=12$ 를 대입하면
$\sum_{k=1}^{24} a_{k} = 6 \times 12^{2} + 12$ 

주어진 식 $\sum_{k=1}^{n} a_{2k-1} = 3n^{2} - n$ 에 $n=12$ 를 대입하면
$\sum_{k=1}^{12} a_{2k-1} = 3 \times 12^{2} - 12$ 

따라서 구하는 값은
$( 6 \times 12^{2} + 12 ) - 2 \times ( 3 \times 12^{2} - 12 )$ 
$= ( 864 + 12 ) - 2 \times ( 432 - 12 )$ 
$= 876 - 2 \times 420$ 
$= 876 - 840 = 36$ 

정답은 ④ 이다.