## ë¬¸ì œ
ë‘ í•¨ìˆ˜ $f(x) = \frac{1}{3}x(4-x)$, $g(x) = |x-1|-1$ì˜ ê·¸ëž˜í”„ë¡œ ë‘˜ëŸ¬ì‹¸ì¸ ë¶€ë¶„ì˜ ë„“ì´ë¥¼ $S$ë¼ í•  ë•Œ, $4S$ì˜ ê°’ì„ êµ¬í•˜ì‹œì˜¤.

## í’€ì´
ë‘ í•¨ìˆ˜ $f(x) = \frac{1}{3}x(4-x)$, $g(x) = |x-1|-1$ì˜ ê·¸ëž˜í”„ëŠ” ë‹¤ìŒê³¼ ê°™ë‹¤.

> [!example] ðŸ“¸ (ê·¸ë¦¼/ê·¸ëž˜í”„)

$x < 1$ì¼ ë•Œ, $g(x) = -x$ì´ë¯€ë¡œ $\frac{1}{3}x(4-x) = -x$ì—ì„œ
$x = 0$

$x \ge 1$ì¼ ë•Œ, $g(x) = x-2$ì´ë¯€ë¡œ $\frac{1}{3}x(4-x) = x-2$ì—ì„œ
$4x - x^2 = 3x - 6$,
$x^2 - x - 6 = 0$,
$(x-3)(x+2) = 0$ì´ë¯€ë¡œ
$x = 3$

$S = \int_{0}^{1} \{ f(x) - g(x) \} dx + \int_{1}^{3} \{ f(x) - g(x) \} dx$
$= \int_{0}^{1} ( - \frac{1}{3}x^2 + \frac{7}{3}x ) dx + \int_{1}^{3} ( - \frac{1}{3}x^2 + \frac{1}{3}x + 2 ) dx$
$= [ - \frac{1}{9}x^3 + \frac{7}{6}x^2 ]_{0}^{1} + [ - \frac{1}{9}x^3 + \frac{1}{6}x^2 + 2x ]_{1}^{3}$
$= ( - \frac{1}{9} + \frac{7}{6} ) + \{ ( -3 + \frac{3}{2} + 6 ) - ( - \frac{1}{9} + \frac{1}{6} + 2 ) \} = \frac{7}{2}$

ì´ë¯€ë¡œ
$4S = 14$

**ì •ë‹µ: $14$**