## 문제
함수 $f(x) = e^{x^{3} + 2x - 2}$ 의 역함수를 $g(x)$ 라 할 때, $g'(e)$ 의 값은?

## 보기
① $\frac{1}{e}$   ② $\frac{1}{3e}$   ③ $\frac{1}{5e}$   ④ $\frac{1}{7e}$   ⑤ $\frac{1}{9e}$

## 풀이
$g(e) = t$ 라 하면 
$f(t) = e$ 이다.

$e^{t^{3} + 2t - 2} = e$ 에서 
$t^{3} + 2t - 2 = 1$
$t^{3} + 2t - 3 = 0$
$(t-1)(t^{2} + t + 3) = 0$
$t$ 는 실수이므로 $t = 1$ 이고, 
$g(e) = 1$ 이다.

$f'(x) = (3x^{2} + 2)e^{x^{3} + 2x - 2}$ 이므로 
역함수의 미분법에 의해
$g'(e) = \frac{1}{f'(g(e))} = \frac{1}{f'(1)}$ 이다.

$f'(1) = (3 \cdot 1^{2} + 2)e^{1^{3} + 2 \cdot 1 - 2} = 5e$ 이므로
$g'(e) = \frac{1}{5e}$ 이다.

정답: ③