## 문제
실수 전체의 집합에서 미분가능한 두 함수 $f(x)$, $g(x)$에 대하여 함수 $h(x)$를 $h(x)= ( f \circ g ) (x)$라 하자. 
$\lim _{x \to 1} \frac{g(x)+1}{x-1} = 2$, $\lim _{x \to 1} \frac{h(x)-2}{x-1} = 12$일 때, $f(-1)+f'(-1)$의 값은? 

## 보기
① $4$   ② $5$   ③ $6$   ④ $7$   ⑤ $8$

## 풀이
$\lim _{x \to 1} \frac{g(x)+1}{x-1} = 2$에서 $x \to 1$일 때 (분모) $\to 0$이면 (분자) $\to 0$이므로 
$\lim _{x \to 1} \{ g(x)+1 \} = g(1)+1 = 0$, $g(1)=-1$ 
$\lim _{x \to 1} \frac{g(x)+1}{x-1} = \lim _{x \to 1} \frac{g(x)-g(1)}{x-1} = g'(1) = 2$ 

$\lim _{x \to 1} \frac{h(x)-2}{x-1} = 12$에서 $x \to 1$일 때 (분모) $\to 0$이면 (분자) $\to 0$이므로 
$\lim _{x \to 1} \{ h(x)-2 \} = h(1)-2=0$, $h(1)=2$ 
$\lim _{x \to 1} \frac{h(x)-2}{x-1} = \lim _{x \to 1} \frac{h(x)-h(1)}{x-1} = h'(1) = 12$ 

$h(x)= (f \circ g)(x)$에서 $x=1$일 때 
$h(1) = f(g(1)) = f(-1) = 2$ 

$h'(x) = f'(g(x))g'(x)$에서 $x=1$일 때 
$h'(1) = f'(g(1))g'(1) = f'(-1) \times 2 = 12$ 
즉, $f'(-1)=6$ 

따라서 
$f(-1)+f'(-1) = 2+6=8$ 
정답은 ⑤입니다.