## 문제
수열 $\{ a_{n} \}$ 이 $\sum_{n=1}^{\infty} (2a_{n}-3)=2$ 를 만족시킨다. $\lim_{n \to \infty} a_{n}=r$ 일 때, $\lim_{n \to \infty} \frac{r^{n+2}-1}{r^{n}+1}$ 의 값은?

## 보기
① $\frac{7}{4}$   ② $2$   ③ $\frac{9}{4}$   ④ $\frac{5}{2}$   ⑤ $\frac{11}{4}$

## 풀이
$\sum_{n=1}^{\infty} (2a_{n}-3)=2$ 에서 
$\lim_{n \to \infty} (2a_{n}-3)=0$ 이다.
$\lim_{n \to \infty} a_{n}$
$= \lim_{n \to \infty} \{ \frac{1}{2} (2a_{n}-3) + \frac{3}{2} \}$
$= \frac{1}{2} \lim_{n \to \infty} (2a_{n}-3) + \lim_{n \to \infty} \frac{3}{2}$
$= \frac{1}{2} \times 0 + \frac{3}{2} = \frac{3}{2}$
즉, 
$r = \frac{3}{2}$
$r > 1$ 이면 
$\lim_{n \to \infty} r^{n} = \infty$ 에서 
$\lim_{n \to \infty} \frac{1}{r^{n}} = 0$ 이므로 
$\lim_{n \to \infty} \frac{r^{n+2}-1}{r^{n}+1}$
$= \lim_{n \to \infty} \frac{r^{2} - \frac{1}{r^{n}}}{1 + \frac{1}{r^{n}}}$
$= \frac{r^{2}-0}{1+0} = r^{2}$
$= ( \frac{3}{2} )^{2} = \frac{9}{4}$

정답: ③