## 문제
두 수열 $\{ a_{n} \}$, $\{ b_{n} \}$ 에 대하여 
$\lim_{n \to \infty} (a_{n} + 2b_{n}) = 9$, $\lim_{n \to \infty} (2a_{n} + b_{n}) = 90$ 
일 때, $\lim_{n \to \infty} (a_{n} + b_{n})$ 의 값을 구하시오.

## 풀이
$a_{n} + 2b_{n} = c_{n}$ $\cdots$ ㉠ 
$2a_{n} + b_{n} = d_{n}$ $\cdots$ ㉡ 
이라 하면 
$\lim_{n \to \infty} c_{n} = \lim_{n \to \infty} (a_{n} + 2b_{n}) = 9$, 
$\lim_{n \to \infty} d_{n} = \lim_{n \to \infty} (2a_{n} + b_{n}) = 90$ 
$2 \times$ ㉡ $-$ ㉠ 에서 
$3a_{n} = 2d_{n} - c_{n}$ 이므로 
$a_{n} = \frac{1}{3} (2d_{n} - c_{n})$ 

$2 \times$ ㉠ $-$ ㉡ 에서 
$3b_{n} = 2c_{n} - d_{n}$ 이므로 
$b_{n} = \frac{1}{3} (2c_{n} - d_{n})$ 
따라서 
$a_{n} + b_{n} = \frac{1}{3} (c_{n} + d_{n})$ 이므로 
$\lim_{n \to \infty} (a_{n} + b_{n}) = \lim_{n \to \infty} \left\{ \frac{1}{3} (c_{n} + d_{n}) \right\}$ 
$= \frac{1}{3} \lim_{n \to \infty} (c_{n} + d_{n})$ 
$= \frac{1}{3} ( \lim_{n \to \infty} c_{n} + \lim_{n \to \infty} d_{n} )$ 
$= \frac{1}{3} \times ( 9 + 90 ) = 33$ 

**[다른 풀이]** 
$\lim_{n \to \infty} (a_{n} + 2b_{n}) = 9$, $\lim_{n \to \infty} (2a_{n} + b_{n}) = 90$ 이므로 
$\lim_{n \to \infty} (a_{n} + 2b_{n}) + \lim_{n \to \infty} (2a_{n} + b_{n})$ 
$= \lim_{n \to \infty} \{ (a_{n} + 2b_{n}) + (2a_{n} + b_{n}) \}$ 
$= \lim_{n \to \infty} 3(a_{n} + b_{n})$ 
그러므로 
$\lim_{n \to \infty} 3(a_{n} + b_{n}) = 9 + 90 = 99$ 
따라서 
$\lim_{n \to \infty} (a_{n} + b_{n}) = \frac{1}{3} \lim_{n \to \infty} 3(a_{n} + b_{n})$ 
$= \frac{1}{3} \times 99 = 33$ 

정답: $33$