## 문제
$x \ge -1$에서 정의된 함수 $f(x) = \sqrt{x+1} + 1$과 $x \ge 1$에서 정의된 함수 $g(x) = (x-1)^{2} - 1$에 대하여 $(g \circ f \circ f)(15)$의 값은?

## 보기
① $1$   ② $3$   ③ $5$   ④ $7$   ⑤ $9$

## 풀이
[정답] ③ 

[해설] 
함수 $f$ 와 함수 $g$ 는 서로 역함수이므로 $g \circ f = I$ (단, $I$ 는 항등함수)이다. 
그러므로 
$(g \circ f \circ f) = (g \circ f) \circ f = I \circ f = f$ 
따라서 
$(g \circ f \circ f)(15) = ((g \circ f) \circ f)(15)$ 
$= (I \circ f)(15)$ 
$= f(15)$ 
$= \sqrt{15+1} + 1$ 
$= 5$ 

[다른 풀이] 
$f(15) = \sqrt{15+1} + 1 = 5$, 
$f(5) = \sqrt{5+1} + 1 = \sqrt{6} + 1$, 
$g(\sqrt{6} + 1) = (\sqrt{6} + 1 - 1)^{2} - 1 = 5$ 
이므로 
$(g \circ f \circ f)(15) = g(f(f(15)))$ 
$= g(f(5))$ 
$= g(\sqrt{6} + 1)$ 
$= 5$