## 문제
$\sqrt{(-2)^{6}} + (\sqrt[3]{3} - \sqrt[3]{2})(\sqrt[3]{9} + \sqrt[3]{6} + \sqrt[3]{4})$ 의 값은?

## 보기
① $7$   ② $9$   ③ $11$   ④ $13$   ⑤ $15$

## 풀이
$\sqrt{(-2)^{6}} = \sqrt{2^{6}} = 8$이고,
$(\sqrt[3]{3} - \sqrt[3]{2})(\sqrt[3]{9} + \sqrt[3]{6} + \sqrt[3]{4}) = (\sqrt[3]{3} - \sqrt[3]{2}) \{ (\sqrt[3]{3})^{2} + \sqrt[3]{3} \cdot \sqrt[3]{2} + (\sqrt[3]{2})^{2} \}$
이 식은 $(a - b)(a^{2} + ab + b^{2}) = a^{3} - b^{3}$의 꼴이므로
$(\sqrt[3]{3})^{3} - (\sqrt[3]{2})^{3} = 3 - 2 = 1$ 이다.
따라서 $\sqrt{(-2)^{6}} + (\sqrt[3]{3} - \sqrt[3]{2})(\sqrt[3]{9} + \sqrt[3]{6} + \sqrt[3]{4}) = 8 + 1 = 9$ 이다.

[정답] ②