## 문제
두 수열 $\{ a_{n} \}$, $\{ b_{n} \}$ 에 대하여 
$\sum_{n=1}^{10} ( 2a_{n} - b_{n} ) = 7$, $\sum_{n=1}^{10} ( a_{n} + b_{n} ) = 5$ 일 때, $\sum_{n=1}^{10} ( a_{n} - 2b_{n} )$ 의 값은?

## 보기
① $1$   ② $2$   ③ $3$   ④ $4$   ⑤ $5$

## 풀이
$\sum_{n=1}^{10} ( 2a_{n} - b_{n} ) = 7$, $\sum_{n=1}^{10} ( a_{n} + b_{n} ) = 5$ 이므로 
$\sum_{n=1}^{10} \{ ( 2a_{n} - b_{n} ) + ( a_{n} + b_{n} ) \} = 7 + 5$ 
$\sum_{n=1}^{10} 3a_{n} = 12$ 
$\sum_{n=1}^{10} a_{n} = 4$ 이고, $\sum_{n=1}^{10} ( a_{n} + b_{n} ) = 5$ 에서 $\sum_{n=1}^{10} b_{n} = 1$ 이다.
따라서 
$\sum_{n=1}^{10} ( a_{n} - 2b_{n} ) = \sum_{n=1}^{10} a_{n} - 2 \sum_{n=1}^{10} b_{n} = 4 - 2 \times 1 = 2$

정답: ②