## 문제
두 양수 $a$, $b$ ($a > b$)에 대하여 $9^a = 2^{\frac{1}{b}}$, $(a+b)^2 = \log_3 64$일 때, $\frac{a-b}{a+b}$의 값은?

## 보기
① $\frac{\sqrt{6}}{6}$   ② $\frac{\sqrt{3}}{3}$   ③ $\frac{\sqrt{2}}{2}$   ④ $\frac{\sqrt{6}}{3}$   ⑤ $\frac{\sqrt{30}}{6}$

## 풀이
$9^a = 2^{\frac{1}{b}}$에서 $3^{2a} = 2^{\frac{1}{b}}$이므로 $3^{2ab} = 2$이다.
$(a+b)^2 = \log_3 64$에서 $3^{(a+b)^2} = 64 = 2^6$이므로 $3^{\frac{(a+b)^2}{6}} = 2$이다.
따라서 $2ab = \frac{(a+b)^2}{6}$이 성립한다.
식 정리하면,
$12ab = a^2 + 2ab + b^2$
$a^2 - 10ab + b^2 = 0$

$t = \frac{a}{b}$라 하면 $a > b > 0$에서 $t > 1$이고, 위 식의 양변을 $b^2$으로 나누면
$(\frac{a}{b})^2 - 10(\frac{a}{b}) + 1 = 0$
$t^2 - 10t + 1 = 0$
$t = 5 + 2\sqrt{6}$ ($t > 1$)

구하는 값은 다음과 같다.
$\frac{a-b}{a+b} = \frac{\frac{a}{b}-1}{\frac{a}{b}+1}$
$= \frac{t-1}{t+1}$
$= \frac{5 + 2\sqrt{6} - 1}{5 + 2\sqrt{6} + 1}$
$= \frac{4 + 2\sqrt{6}}{6 + 2\sqrt{6}}$
$= \frac{2 + \sqrt{6}}{3 + \sqrt{6}}$
$= \frac{(2 + \sqrt{6})(3 - \sqrt{6})}{(3 + \sqrt{6})(3 - \sqrt{6})}$
$= \frac{6 - 2\sqrt{6} + 3\sqrt{6} - 6}{9 - 6}$
$= \frac{\sqrt{6}}{3}$

정답은 ④이다.