## 문제
다항식 $P(x)$에 대하여 등식 $x^{3} + 3x^{2} - x - 3 = (x^{2} - 1)P(x)$가 $x$에 대한 항등식일 때, $P(1)$의 값은?

## 보기
① $1$   ② $2$   ③ $3$   ④ $4$   ⑤ $5$

## 풀이
정답: ④

조립제법을 활용하여 $x^{3} + 3x^{2} - x - 3$을 인수분해하면 
$$ \begin{array}{c|rrrr} 1 & 1 & 3 & -1 & -3 \\ \multicolumn{1}{r}{} & & 1 & 4 & 3 \\ \hline \multicolumn{1}{r}{} & 1 & 4 & 3 & 0 \end{array} $$
따라서 좌변을 인수분해하면 다음과 같다.
$(x - 1)(x^{2} + 4x + 3) = (x - 1)(x + 1)P(x)$
$(x - 1)(x + 1)(x + 3) = (x - 1)(x + 1)P(x)$

이때 $P(x) = x + 3$이다.
따라서 $P(1) = 1 + 3 = 4$이다.