## 문제
다항함수 $f(x)$의 한 부정적분 $g(x)$가 다음 조건을 만족시킨다.

(가) $f(x) = 2x + 2 \int_{0}^{1} g(t) dt$
(나) $g(0) - \int_{0}^{1} g(t) dt = \frac{2}{3}$

$g(1)$의 값은?

## 보기
① $-2$   ② $-\frac{5}{3}$   ③ $-\frac{4}{3}$   ④ $-1$   ⑤ $-\frac{2}{3}$

## 풀이
$\int_{0}^{1} g(t) dt = a$라 하면 (가)에서
$f(x) = 2x + 2a$

$g(x)$는 $f(x)$의 한 부정적분이므로
$g(x) = \int f(x) dx = x^{2} + 2ax + C$ ($C$는 적분상수)

(나)에서
$g(0) - \int_{0}^{1} g(t) dt = \frac{2}{3}$
$C - \int_{0}^{1} (t^{2} + 2at + C) dt = \frac{2}{3}$
$C - \left[ \frac{1}{3} t^{3} + at^{2} + Ct \right]_{0}^{1} = \frac{2}{3}$
$C - (\frac{1}{3} + a + C) = \frac{2}{3}$에서
$-\frac{1}{3} - a = \frac{2}{3}$
$a = -1$

$\int_{0}^{1} g(t) dt = a$에서
$\int_{0}^{1} (t^{2} - 2t + C) dt = -1$
$\left[ \frac{1}{3} t^{3} - t^{2} + Ct \right]_{0}^{1} = -1$
$\frac{1}{3} - 1 + C = -1$
즉, $C = -\frac{1}{3}$이므로
$g(x) = x^{2} - 2x - \frac{1}{3}$

따라서
$g(1) = 1^{2} - 2 \times 1 - \frac{1}{3}$
$= 1 - 2 - \frac{1}{3}$
$= -\frac{4}{3}$

정답: ③