## 문제
$a_1 = 1$ 인 수열 $\{ a_n \}$ 이 모든 자연수 $n$ 에 대하여 
$(4 - a_{n+1})(2 + a_n) = 8$ 
을 만족시킬 때, $\sum_{k=1}^{9} \frac{8}{a_k}$ 의 정수 부분은? 

## 보기
① $43$   ② $44$   ③ $45$   ④ $46$   ⑤ $47$

## 풀이
$a_1 = 1$ 인 수열 $\{ a_n \}$ 이 모든 자연수 $n$ 에 대하여 
$(4 - a_{n+1})(2 + a_n) = 8$
$8 + 4a_n - 2a_{n+1} - a_n a_{n+1} = 8$
$\therefore a_n a_{n+1} + 2a_{n+1} - 4a_n = 0$

$a_n a_{n+1}$ 로 나누면 
$1 + \frac{2}{a_n} - \frac{4}{a_{n+1}} = 0$

$\frac{4}{a_n} = b_n$ 이라 하면 
$1 + \frac{b_n}{2} - b_{n+1} = 0$
$b_{n+1} = \frac{1}{2} b_n + 1$

즉, 
$b_1 = \frac{4}{a_1} = 4$, 
$(b_{n+1} - 2) = \frac{1}{2} (b_n - 2)$ 이므로 
$b_n - 2 = (4 - 2) \cdot \left( \frac{1}{2} \right)^{n-1}$, 
$b_n = 2 + 2 \cdot \left( \frac{1}{2} \right)^{n-1}$

$\sum_{k=1}^{9} \frac{8}{a_k}$
$= 2 \sum_{k=1}^{9} b_k$
$= 2 \left( 18 + \frac{2 \{ 1 - ( \frac{1}{2} )^9 \}}{1 - (\frac{1}{2})} \right)$
$= 36 + 8 \{ 1 - ( \frac{1}{2} )^9 \}$
$= 44 - (\frac{1}{2})^6$

따라서 구하는 정수 부분은 $43$ 이다.