## 문제
연립방정식 
$$ \begin{cases} x^{2} - 3xy + 2y^{2} = 0 \\ x^{2} - y^{2} = 9 \end{cases} $$
의 해를 
$$ \begin{cases} x = \alpha_{1} \\ y = \beta_{1} \end{cases} $$ 또는 $$ \begin{cases} x = \alpha_{2} \\ y = \beta_{2} \end{cases} $$
라 하자. $ \alpha_{1} < \alpha_{2} $ 일 때, $ \beta_{1} - \beta_{2} $ 의 값은?

## 보기
① $-2\sqrt{3}$   ② $-2\sqrt{2}$   ③ $2\sqrt{2}$   ④ $2\sqrt{3}$   ⑤ $4$

## 풀이
$x^{2} - 3xy + 2y^{2} = 0$ 에서 
$(x - y)(x - 2y) = 0$ 
$x = y$ 또는 $x = 2y$ 

$1$) $x = y$ 일 때, 
$x^{2} - y^{2} = y^{2} - y^{2} = 0$ 이므로 
$x^{2} - y^{2} = 9$ 라는 조건을 만족시키지 않는다. 

$2$) $x = 2y$ 일 때, 
$x^{2} - y^{2} = (2y)^{2} - y^{2} = 3y^{2} = 9$ 에서 
$y^{2} = 3$ 
$y = \sqrt{3}$ 또는 $y = -\sqrt{3}$ 

$y = \sqrt{3}$ 이면 $x = 2\sqrt{3}$ 
$y = -\sqrt{3}$ 이면 $x = -2\sqrt{3}$ 

$\alpha_{1} < \alpha_{2}$ 이므로 
$\alpha_{1} = -2\sqrt{3}$, $\beta_{1} = -\sqrt{3}$ 
$\alpha_{2} = 2\sqrt{3}$, $\beta_{2} = \sqrt{3}$ 

따라서 
$\beta_{1} - \beta_{2} = -\sqrt{3} - \sqrt{3} = -2\sqrt{3}$ 

정답: ①