## 문제
$\lim_{n \to \infty} (\sqrt{4n^{2} + 2n + 1} - \sqrt{4n^{2} - 2n - 1})$ 의 값은? [$2$점]

## 보기
① $1$   ② $2$   ③ $3$   ④ $4$   ⑤ $5$

## 풀이
$$\begin{aligned} &\lim _{n \to \infty} (\sqrt{4n^{2} + 2n + 1} - \sqrt{4n^{2} - 2n - 1}) \\ &= \lim _{n \to \infty} \frac{(\sqrt{4n^{2} + 2n + 1} - \sqrt{4n^{2} - 2n - 1})(\sqrt{4n^{2} + 2n + 1} + \sqrt{4n^{2} - 2n - 1})}{\sqrt{4n^{2} + 2n + 1} + \sqrt{4n^{2} - 2n - 1}} \\ &= \lim _{n \to \infty} \frac{(4n^{2} + 2n + 1) - (4n^{2} - 2n - 1)}{\sqrt{4n^{2} + 2n + 1} + \sqrt{4n^{2} - 2n - 1}} \\ &= \lim _{n \to \infty} \frac{4n + 2}{\sqrt{4n^{2} + 2n + 1} + \sqrt{4n^{2} - 2n - 1}} \\ &= \lim _{n \to \infty} \frac{4 + \frac{2}{n}}{\sqrt{4 + \frac{2}{n} + \frac{1}{n^{2}}} + \sqrt{4 - \frac{2}{n} - \frac{1}{n^{2}}}} \\ &= \frac{4}{\sqrt{4} + \sqrt{4}} \\ &= \frac{4}{2 + 2} \\ &= 1 \end{aligned}$$
따라서 정답은 ① 이다.