## ë¬¸ì œ

í•¨ìˆ˜ $y=f(x)$ì˜ ê·¸ë˜í”„ê°€ ê·¸ë¦¼ê³¼ ê°™ë‹¤.

> [!example] ğŸ“¸ (ê·¸ë¦¼/ê·¸ë˜í”„)

$\lim_{x \to 0+} f(x-1) + \lim_{x \to 1+} f(f(x))$ì˜ ê°’ì€?

## ë³´ê¸°

â‘  $-2$   â‘¡ $-1$   â‘¢ $0$   â‘£ $1$   â‘¤ $2$

## í’€ì´

$x-1=t$ë¼ í•˜ë©´ $x \to 0+$ì¼ ë•Œ, $t \to -1+$ì´ë¯€ë¡œ 
$\lim_{x \to 0+} f(x-1) = \lim_{t \to -1+} f(t) = -1$

$f(x)=s$ë¼ í•˜ë©´ $x \to 1+$ì¼ ë•Œ, $s \to -1-$ì´ë¯€ë¡œ 
$\lim_{x \to 1+} f(f(x)) = \lim_{s \to -1-} f(s) = 2$

ë”°ë¼ì„œ 
$\lim_{x \to 0+} f(x-1) + \lim_{x \to 1+} f(f(x)) = (-1) + 2 = 1$

[ì •ë‹µ] â‘£