## 문제
실수 전체의 집합에서 미분가능한 함수 $f(x)$ 에 대하여 함수 $g(x)$ 를 $g(x) = \frac{f(x)}{(e^x + 1)^2}$ 라 하자. $f'(0) - f(0) = 2$ 일 때, $g'(0)$ 의 값은?

## 보기
① $\frac{1}{4}$   ② $\frac{3}{8}$   ③ $\frac{1}{2}$   ④ $\frac{5}{8}$   ⑤ $\frac{3}{4}$

## 풀이
$g(x) = \frac{f(x)}{(e^x + 1)^2}$ 의 양변을 미분하면
$g'(x) = \frac{f'(x)(e^x + 1)^2 - 2f(x)(e^x + 1)e^x}{(e^x + 1)^4}$
$x = 0$ 을 대입하면
$g'(0) = \frac{4f'(0) - 4f(0)}{16} = \frac{f'(0) - f(0)}{4}$
$\because f'(0) - f(0) = 2$
$g'(0) = \frac{2}{4} = \frac{1}{2}$
$\therefore g'(0) = \frac{1}{2}$
정답 ③