## 문제
$x = \frac{1+\sqrt{2}+\sqrt{3}}{1-\sqrt{2}+\sqrt{3}}$ 일 때, $x(x-\sqrt{2})(x-\sqrt{3})$ 의 값은?

## 보기
① $2\sqrt{2} + 3\sqrt{3}$   ② $3\sqrt{2} + 2\sqrt{3}$   ③ $2(\sqrt{2} + \sqrt{3})$   ④ $3\sqrt{2} + \sqrt{6}$   ⑤ $\sqrt{6} + 2\sqrt{3}$

## 풀이
[정답] ②

$x = \frac{1+\sqrt{2}+\sqrt{3}}{1-\sqrt{2}+\sqrt{3}}$

$= \frac{(1+\sqrt{2}+\sqrt{3})^2}{(1-\sqrt{2}+\sqrt{3})(1+\sqrt{2}+\sqrt{3})}$

$= \frac{6+2\sqrt{2}+2\sqrt{3}+2\sqrt{6}}{2+2\sqrt{3}}$

$= \frac{3+\sqrt{2}+\sqrt{3}+\sqrt{6}}{1+\sqrt{3}}$

$= \frac{\sqrt{3}(1+\sqrt{3}) + \sqrt{2}(1+\sqrt{3})}{1+\sqrt{3}}$

$= \sqrt{3} + \sqrt{2}$

$\therefore x(x-\sqrt{2})(x-\sqrt{3})$
$= (\sqrt{3} + \sqrt{2})(\sqrt{3})(\sqrt{2})$
$= 3\sqrt{2} + 2\sqrt{3}$