## 문제
함수 $f(x) = \lim_{n \to \infty} \frac{2 \times \left( \frac{x}{4} \right)^{2n+1} - 1}{\left( \frac{x}{4} \right)^{2n} + 3}$ 에 대하여 $f(k) = -\frac{1}{3}$ 을 만족시키는 정수 $k$ 의 개수는? [$3$점]

## 보기
① $5$   ② $7$   ③ $9$   ④ $11$   ⑤ $13$

## 풀이
[정답] ② 

(ⅰ) $\left| \frac{x}{4} \right| > 1$ 즉, $|x| > 4$ 일 때, 
$\lim_{n \to \infty} \left( \frac{x}{4} \right)^{2n} = \infty$ 이므로 
$f(x) = \lim_{n \to \infty} \frac{2 \times \left( \frac{x}{4} \right)^{2n+1} - 1}{\left( \frac{x}{4} \right)^{2n} + 3} = \frac{2 \times \frac{x}{4} - 0}{1 + 0} = \frac{x}{2}$ 

(ⅱ) $\left| \frac{x}{4} \right| < 1$ 즉, $|x| < 4$ 일 때, 
$\lim_{n \to \infty} \left( \frac{x}{4} \right)^{2n} = 0$ 이므로 
$f(x) = \lim_{n \to \infty} \frac{2 \times \left( \frac{x}{4} \right)^{2n+1} - 1}{\left( \frac{x}{4} \right)^{2n} + 3} = \frac{0 - 1}{0 + 3} = -\frac{1}{3}$ 

(ⅲ) $x = 4$ 일 때, 
$f(4) = \lim_{n \to \infty} \frac{2 \times \left( \frac{4}{4} \right)^{2n+1} - 1}{\left( \frac{4}{4} \right)^{2n} + 3} = \frac{2 \times 1 - 1}{1 + 3} = \frac{1}{4}$ 

(ⅳ) $x = -4$ 일 때, 
$f(-4) = \lim_{n \to \infty} \frac{2 \times \left( -\frac{4}{4} \right)^{2n+1} - 1}{\left( -\frac{4}{4} \right)^{2n} + 3} = \frac{2 \times (-1) - 1}{1 + 3} = -\frac{3}{4}$ 

따라서 (ⅰ), (ⅱ), (ⅲ), (ⅳ)에 의하여 $f(k) = -\frac{1}{3}$ 을 만족시키는 정수 $k$ 는 $\left| \frac{k}{4} \right| < 1$ 인 경우이므로 만족하는 정수 $k$ 의 값은 
$-3, -2, -1, 0, 1, 2, 3$
즉, $7$개다.