## 문제
수열 $\{ a_{n} \}$은 $a_{1} = 1$이고, 모든 자연수 $n$에 대하여
$$\sum_{k=1}^{n} (a_{k} - a_{k+1}) = -n^{2} + n$$
을 만족시킨다. $a_{11}$의 값은?

## 보기
① $88$   ② $91$   ③ $94$   ④ $97$   ⑤ $100$

## 풀이
$$\sum_{k=1}^{n} (a_{k} - a_{k+1})$$
$$= ( a_{1} - a_{2} ) + ( a_{2} - a_{3} ) + \cdots + ( a_{n} - a_{n+1} )$$
$$= a_{1} - a_{n+1}$$
그런데 조건에서 $\sum_{k=1}^{n} (a_{k} - a_{k+1}) = -n^{2} + n$, $a_{1} = 1$이므로
$$1 - a_{n+1} = -n^{2} + n$$
$$a_{n+1} = n^{2} - n + 1$$
$\therefore a_{11}$의 값은 $n = 10$을 대입하면
$$a_{11} = 10^{2} - 10 + 1 = 91$$
정답: ②