## 문제
함수 $f(x) = (1 + x^{4} + x^{8} + x^{12})(1 + x + x^{2} + x^{3})$ 일 때, $\frac{f(2)}{(f(1) - 1)(f(1) + 1)}$ 의 값을 구하시오.

## 보기

## 풀이
(ⅰ) $x \neq 1$ 일 때
$f(x) = (1 + x^{4} + x^{8} + x^{12})(1 + x + x^{2} + x^{3})$
$= \frac{(x^{4})^{4} - 1}{x^{4} - 1} \times \frac{x^{4} - 1}{x - 1}$
$= \frac{x^{16} - 1}{x - 1}$

(ⅱ) $x = 1$ 일 때
$f(1) = 4 \times 4 = 16$

따라서 구하는 식에 대입하면
$\frac{f(2)}{(f(1) - 1)(f(1) + 1)}$
$= \frac{\frac{2^{16} - 1}{2 - 1}}{(16 - 1)(16 + 1)}$
$= \frac{2^{16} - 1}{(2^{4} - 1)(2^{4} + 1)}$
$= \frac{(2^{8} - 1)(2^{8} + 1)}{2^{8} - 1}$
$= 2^{8} + 1$
$= 257$

정답: $257$