## 문제
두 수열 $\{ a_{n} \}$, $\{ b_{n} \}$에 대하여
$\sum_{n=1}^{10} a_{n}^{2} = 10$, $\sum_{n=1}^{10} a_{n} ( 2b_{n} - 3a_{n} ) = 16$
일 때, $\sum_{n=1}^{10} a_{n} ( 6a_{n} + 7b_{n} )$의 값을 구하시오.

## 보기

## 풀이
$\sum_{n=1}^{10} a_{n} ( 2b_{n} - 3a_{n} ) = 2 \sum_{n=1}^{10} a_{n} b_{n} - 3 \sum_{n=1}^{10} a_{n}^{2}$
$2 \sum_{n=1}^{10} a_{n} b_{n} - 3 \times 10 = 16$
$2 \sum_{n=1}^{10} a_{n} b_{n} = 46$
$\sum_{n=1}^{10} a_{n} b_{n} = 23$

$\sum_{n=1}^{10} a_{n} ( 6a_{n} + 7b_{n} ) = 6 \sum_{n=1}^{10} a_{n}^{2} + 7 \sum_{n=1}^{10} a_{n} b_{n}$
$= 6 \times 10 + 7 \times 23$
$= 60 + 161 = 221$

따라서 구하는 값은 $221$이다.