## 문제
최고차항의 계수가 $1$ 인 이차함수 $f(x)$ 에 대하여 함수 $g(x)$ 는 
$$g(x) = \int_{-1}^{x} f(t) dt$$
이다. $\lim_{x \to 1} \frac{g(x)}{x-1} = 2$ 일 때, $f(4)$ 의 값을 구하시오.

## 보기

## 풀이
$\lim_{x \to 1} \frac{g(x)}{x-1} = 2$ 에서 $x \to 1$ 일 때 (분모) $\to 0$ 이므로 (분자) $\to 0$ 이다.
즉, $\lim_{x \to 1} g(x) = 0$ 이므로 $g(1) = 0$ 이다.
$$\lim_{x \to 1} \frac{g(x) - g(1)}{x-1} = g'(1) = 2$$
$g(x) = \int_{-1}^{x} f(t) dt$ 에서 $x = -1$ 을 대입하면
$$g(-1) = 0$$
양변을 미분하면
$$g'(x) = \frac{d}{dx} \int_{-1}^{x} f(t) dt = f(x)$$
그런데 $g(x)$ 는 최고차항의 계수가 $\frac{1}{3}$ 이고 $g(1) = 0$, $g(-1) = 0$, $g'(1) = 2$ 이므로
$$g(x) = \frac{1}{3} (x-1)(x+1)(x-\alpha) = \frac{1}{3} (x^2-1)(x-\alpha)$$
양변을 미분하면
$$g'(x) = \frac{1}{3} \{ 2x(x-\alpha) + (x^2-1) \} \cdots ㉠$$
이므로
$$g'(1) = \frac{1}{3} \{ 2 \times 1 \times (1-\alpha) + (1-1) \} = \frac{1}{3} (2-2\alpha) = 2$$
즉, $2\alpha = -4$ 이므로 $\alpha = -2$ 이다.
㉠에 대입하면
$$g'(x) = \frac{1}{3} \{ 2x(x+2) + (x^2-1) \} = x^2 + \frac{4}{3}x - \frac{1}{3}$$
따라서
$$f(x) = x^2 + \frac{4}{3}x - \frac{1}{3}$$
$\therefore f(4) = 4^2 + \frac{4}{3} \times 4 - \frac{1}{3} = 21$