## 문제
다항함수 $f(x)$ 가 다음 조건을 만족시킬 때, 상수 $a$ 의 값은?

(가) 모든 실수 $x$ 에 대하여
$$\frac{d}{dx} \int_{1}^{x} (f(t) + t^{2} + 2at - 3) dt = \int_{1}^{x} \frac{d}{dt} (2f(t) - 3t + 7) dt$$
(나) $$\lim_{h \to 0} \frac{f(3+h) - f(3-h)}{h} = 6$$

## 보기
① $-1$   ② $-2$   ③ $-3$   ④ $-4$   ⑤ $-5$

## 풀이
조건 (가)로부터
$$f(x) + x^{2} + 2ax - 3 = [2f(t) - 3t + 7]_{1}^{x}$$
$$= 2f(x) - 3x + 7 - \{2f(1) - 3(1) + 7\}$$
$$= 2f(x) - 3x - 2f(1) + 3$$
$\therefore f(x) = x^{2} + (2a + 3)x + 2f(1) - 6$

위 식에서 $x=1$ 을 대입하면
$$f(1) = 1 + 2a + 3 + 2f(1) - 6$$
$\therefore f(1) = -2a + 2$

$\therefore f(x) = x^{2} + (2a + 3)x - 4a - 2$

조건 (나)로부터
$$\lim_{h \to 0} \frac{f(3+h) - f(3-h)}{h}$$
$$= \lim_{h \to 0} \frac{f(3+h) - f(3) + f(3) - f(3-h)}{h}$$
$$= \lim_{h \to 0} \left[ \frac{f(3+h) - f(3)}{h} - \frac{f(3-h) - f(3)}{h} \right]$$
$$= \lim_{h \to 0} \left[ \frac{f(3+h) - f(3)}{h} + \frac{f(3-h) - f(3)}{-h} \right]$$
$$= f'(3) + f'(3) = 2f'(3)$$

$2f'(3) = 6$ 이므로 $f'(3) = 3$

$\therefore f'(x) = 2x + 2a + 3$
즉, $f'(3) = 6 + 2a + 3 = 2a + 9 = 3$ 이므로
$a = -3$

정답: ③