## 문제
복소수 $z$에 대하여 $z + \bar{z} = -1$, $z\bar{z} = 1$일 때, 
$$\frac{\bar{z}}{z^{5}} + \frac{(\bar{z})^{2}}{z^{4}} + \frac{(\bar{z})^{3}}{z^{3}} + \frac{(\bar{z})^{4}}{z^{2}} + \frac{(\bar{z})^{5}}{z}$$
의 값은? (단, $\bar{z}$는 $z$의 켤레복소수이다.)

## 보기
① $2$   ② $3$   ③ $4$   ④ $5$   ⑤ $6$

## 풀이
$z + \bar{z} = -1$, $z\bar{z} = 1$이므로 $z$, $\bar{z}$는 이차방정식 $x^{2} + x + 1 = 0$의 두 근이다. 
양변에 $x - 1$을 곱하면 $x^{3} - 1 = 0$이므로 $x^{3} = 1$이다. 
그러므로 $z^{3} = 1$, $(\bar{z})^{3} = 1$이다. 
따라서 

$$\frac{\bar{z}}{z^{5}} + \frac{(\bar{z})^{2}}{z^{4}} + \frac{(\bar{z})^{3}}{z^{3}} + \frac{(\bar{z})^{4}}{z^{2}} + \frac{(\bar{z})^{5}}{z}$$ 
$$= \frac{\bar{z}}{z^{2}} + \frac{(\bar{z})^{2}}{z} + \frac{1}{1} + \frac{\bar{z}}{z^{2}} + \frac{(\bar{z})^{2}}{z}$$ 
$$= \frac{2\bar{z}}{z^{2}} + \frac{2(\bar{z})^{2}}{z} + 1$$ 
$$= \frac{2z\bar{z}}{z^{3}} + \frac{2z^{2}(\bar{z})^{2}}{z^{3}} + 1$$ 
$$= 2 + 2 + 1$$ 
$$= 5$$ 

**[다른 풀이]** 

$z^{3} = 1$, $(\bar{z})^{3} = 1$, $z\bar{z} = 1$에서 $\bar{z} = \frac{1}{z}$이다. 

$$\frac{\bar{z}}{z^{5}} + \frac{(\bar{z})^{2}}{z^{4}} + \frac{(\bar{z})^{3}}{z^{3}} + \frac{(\bar{z})^{4}}{z^{2}} + \frac{(\bar{z})^{5}}{z}$$ 
$$= (\bar{z})^{6} + (\bar{z})^{6} + (\bar{z})^{6} + (\bar{z})^{6} + (\bar{z})^{6}$$ 
$$= 5(\bar{z})^{6} = 5$$ 

정답: ④