## 문제
두 다항함수 $f(x)$, $g(x)$ 가
$$\lim _{x \rightarrow 1} \frac{f(x)-a+2}{x-1}=4, \lim _{x \rightarrow 1} \frac{g(x)+a-2}{x-1}=a$$
를 만족시킨다. 함수 $f(x)g(x)$ 의 $x=1$ 에서의 미분계수가 $-1$ 일 때, 상수 $a$ 의 값은?

## 보기
① $1$   ② $2$   ③ $3$   ④ $4$   ⑤ $5$

## 풀이
[정답] ③

$$\lim _{x \rightarrow 1} \frac{f(x)-a+2}{x-1}=4$$ 이고 $$\lim _{x \rightarrow 1} (x-1) =0$$ 이므로
$$\lim _{x \rightarrow 1} \{ f(x)-a+2 \} =0$$
함수 $f(x)$ 는 다항함수이므로
$$\lim _{x \rightarrow 1} f(x)=f(1)=a-2$$
$$\lim _{x \rightarrow 1} \frac{f(x)-a+2}{x-1} = \lim _{x \rightarrow 1} \frac{f(x)-f(1)}{x-1} =f'(1)=4$$
$$\lim _{x \rightarrow 1} \frac{g(x)+a-2}{x-1} =a$$ 이고 $$\lim _{x \rightarrow 1} (x-1) =0$$ 이므로
$$\lim _{x \rightarrow 1} \{ g(x)+a-2 \} =0$$
함수 $g(x)$ 는 다항함수이므로
$$\lim _{x \rightarrow 1} g(x) =g(1)= -a+2$$
$$\lim _{x \rightarrow 1} \frac{g(x)+a-2}{x-1} =\lim _{x \rightarrow 1} \frac{g(x)-g(1)}{x-1} = g'(1) =a$$
함수 $f(x)g(x)$ 의 $x=1$ 에서의 미분계수는
$$f'(1)g(1)+f(1)g'(1)$$
$$= 4 \times (-a+2)+(a-2) \times a$$
$$= a^2 -6a+8 = -1$$
$$a^2 -6a+9 =0$$ 에서
$$(a-3)^2 =0$$
따라서 $a=3$