## 문제
두 수열 $\{ a_{n} \}$, $\{ b_{n} \}$에 대하여 $\sum_{k=1}^{10} (a_{k} + 2b_{k}) = 45$, $\sum_{k=1}^{10} (a_{k} - b_{k}) = 3$일 때, $\sum_{k=1}^{10} \left( b_{k} - \frac{1}{2} \right)$의 값을 구하시오.

## 풀이
$\sum_{k=1}^{10} (a_{k} + 2b_{k}) = 45$에서 
$\sum_{k=1}^{10} a_{k} + 2 \sum_{k=1}^{10} b_{k} = 45 \cdots \cdots$ ㉠ 

$\sum_{k=1}^{10} (a_{k} - b_{k}) = 3$에서 
$\sum_{k=1}^{10} a_{k} - \sum_{k=1}^{10} b_{k} = 3 \cdots \cdots$ ㉡ 

㉠, ㉡에서 
$3 \sum_{k=1}^{10} b_{k} = 42$ 
즉, $\sum_{k=1}^{10} b_{k} = 14$ 

따라서 
$\sum_{k=1}^{10} \left( b_{k} - \frac{1}{2} \right) = \sum_{k=1}^{10} b_{k} - 10 \times \frac{1}{2}$ 
$= 14 - 5 = 9$

정답: $9$