## 문제
삼차함수 $f(x)$가 다음 조건을 만족시킨다.

(가) $\lim_{x \to 1} \frac{f(x)}{x-1} = 3$
(나) $1$이 아닌 상수 $\alpha$에 대하여 $\lim_{x \to 2} \frac{f(x)}{(x-2) f'(x)} = \alpha$이다.

$\alpha \times f(4)$의 값을 구하시오.

## 풀이
조건 (가)에서 $\lim_{x \to 1} \frac{f(x)}{x-1} = 3$이고 $\lim_{x \to 1} (x-1) = 0$이므로 $\lim_{x \to 1} f(x) = 0$이다.
함수 $f(x)$는 $x=1$에서 연속이므로 $f(1) = 0$ $\cdots \cdots$ ㉠ 
조건 (나)에서 $\lim_{x \to 2} \frac{f(x)}{(x-2) f'(x)} = \alpha$ ($\alpha \neq 1$)이고 $\lim_{x \to 2} (x-2) f'(x) = 0$이므로 $\lim_{x \to 2} f(x) = 0$이다.
함수 $f(x)$는 $x=2$에서 연속이므로 $f(2) = 0$ $\cdots \cdots$ ㉡ 
㉠, ㉡에 의해 $f(x) = k(x-1)(x-2)(x+a)$ ($k$, $a$는 상수, $k \neq 0$)라 하면
$f'(x) = k \{ (x-2)(x+a) + (x-1)(x+a) + (x-1)(x-2) \}$
$a \neq -2$라 하면
$\lim_{x \to 2} \frac{f(x)}{(x-2) f'(x)} = \lim_{x \to 2} \frac{k(x-1)(x+a)}{f'(x)} = \frac{2+a}{2+a} = 1 \neq \alpha$
그러므로 $a = -2$이며 $f(x) = k(x-1)(x-2)^2$이다.
$\alpha = \lim_{x \to 2} \frac{f(x)}{(x-2) f'(x)}$
$= \lim_{x \to 2} \frac{k(x-1)(x-2)^2}{(x-2) \{ k(x-2)^2 + 2k(x-1)(x-2) \}}$
$= \lim_{x \to 2} \frac{(x-1)}{(x-2) + 2(x-1)}$
$= \frac{1}{0 + 2 \times 1} = \frac{1}{2}$
조건 (가)에서 $\lim_{x \to 1} \frac{f(x)}{x-1} = \lim_{x \to 1} \frac{f(x) - f(1)}{x-1} = f'(1) = 3$이므로 $k = 3$이다.
따라서 $\alpha \times f(4) = \frac{1}{2} \times (3 \times 3 \times 2^2) = 18$