## 문제
두 함수 $f(x)$, $g(x)$ 가 $\lim_{x \to \infty} \{ 2f(x) - 3g(x) \} = 1$, $\lim_{x \to \infty} g(x) = \infty$ 를 만족시킬 때, $\lim_{x \to \infty} \frac{4f(x) + g(x)}{3f(x) - g(x)}$ 의 값은?

## 보기
① $1$   ② $2$   ③ $3$   ④ $4$   ⑤ $5$

## 풀이
$h(x) = 2f(x) - 3g(x)$ 라 하면 
$f(x) = \frac{3g(x) + h(x)}{2}$ 

$\lim_{x \to \infty} g(x) = \infty$, $\lim_{x \to \infty} h(x) = 1$ 이므로 
$\lim_{x \to \infty} \frac{h(x)}{g(x)} = 0$ 

$\lim_{x \to \infty} \frac{4f(x) + g(x)}{3f(x) - g(x)}$ 
$= \lim_{x \to \infty} \frac{4 \left( \frac{3g(x) + h(x)}{2} \right) + g(x)}{3 \left( \frac{3g(x) + h(x)}{2} \right) - g(x)}$ 
$= \lim_{x \to \infty} \frac{14g(x) + 4h(x)}{7g(x) + 3h(x)}$ 
$= \lim_{x \to \infty} \frac{14 + 4 \times \frac{h(x)}{g(x)}}{7 + 3 \times \frac{h(x)}{g(x)}}$ 
$= 2$

정답: ②