## ë¬¸ì œ
ê³¡ì„  $y=x^{3}+2x$ ì™€ $y$ ì¶• ë° ì§ì„  $y=3x+6$ ìœ¼ë¡œ ë‘˜ëŸ¬ì‹¸ì¸ ë¶€ë¶„ì˜ ë„“ì´ë¥¼ êµ¬í•˜ì‹œì˜¤.

## ë³´ê¸°


## í’€ì´
$x^{3}+2x=3x+6$ ì—ì„œ
$x^{3}-x-6=0$
$(x-2)(x^{2}+2x+3)=0$
$\therefore x=2$

ê³¡ì„  $y=x^{3}+2x$ ì™€ ì§ì„  $y=3x+6$ ì˜ ê·¸ë˜í”„ëŠ” ë‹¤ìŒ ê·¸ë¦¼ê³¼ ê°™ë‹¤.

> [!example] ğŸ“¸ (ê·¸ë¦¼/ê·¸ë˜í”„)

ë”°ë¼ì„œ êµ¬í•˜ëŠ” ë„“ì´ë¥¼ $S$ ë¼ í•˜ë©´
$S = \int_{0}^{2} \{3x+6-(x^{3}+2x)\} dx$
$= \int_{0}^{2} (-x^{3}+x+6) dx$
$= \left[ -\frac{1}{4}x^{4}+\frac{1}{2}x^{2}+6x \right]_{0}^{2}$
$= -4+2+12$
$= 10$

ì •ë‹µ: $10$