## 문제
수열 $\{ a_n \}$ 의 일반항이 $a_n = \frac{\sqrt{9n^2 - 3n - 2} + 6n - 1}{\sqrt{3n + 1} + \sqrt{3n - 2}}$ 일 때, $\sum_{n=1}^{16} a_n$ 의 값은?

## 보기
① $110$   ② $114$   ③ $118$   ④ $122$   ⑤ $126$

## 풀이
정답 ②

$\sqrt{3n + 1} = x$, $\sqrt{3n - 2} = y$ 라 하면
$\sqrt{9n^2 - 3n - 2} = \sqrt{(3n + 1)(3n - 2)} = xy$
$6n - 1 = (3n + 1) + (3n - 2) = x^2 + y^2$
$x^2 - y^2 = 3$ 이므로
$a_n = \frac{\sqrt{9n^2 - 3n - 2} + 6n - 1}{\sqrt{3n + 1} + \sqrt{3n - 2}}$
$= \frac{xy + x^2 + y^2}{x + y}$
$= \frac{(x - y)(x^2 + xy + y^2)}{(x - y)(x + y)}$
$= \frac{x^3 - y^3}{x^2 - y^2}$
$= \frac{x^3 - y^3}{3}$
$= \frac{(\sqrt{3n + 1})^3 - (\sqrt{3n - 2})^3}{3}$

따라서
$\sum_{n=1}^{16} a_n = \sum_{n=1}^{16} \frac{(\sqrt{3n + 1})^3 - (\sqrt{3n - 2})^3}{3}$
$= \frac{1}{3} \{ ((\sqrt{4})^3 - (\sqrt{1})^3) + ((\sqrt{7})^3 - (\sqrt{4})^3) + \cdots + ((\sqrt{49})^3 - (\sqrt{46})^3) \}$
$= \frac{1}{3} (7^3 - 1^3)$
$= \frac{1}{3} (343 - 1)$
$= 114$