## 문제
$\int_{-3}^{2} (2 x^{3} + 6 |x|) d x - \int_{-3}^{-2} (2 x^{3} - 6 x) d x$ 의 값을 구하시오.

## 보기

## 풀이
$\int_{-3}^{2} (2 x^{3} + 6 |x|) d x - \int_{-3}^{-2} (2 x^{3} - 6 x) d x$
$= \int_{-3}^{-2} (2 x^{3} + 6 |x|) d x + \int_{-2}^{2} (2 x^{3} + 6 |x|) d x - \int_{-3}^{-2} (2 x^{3} - 6 x) d x$
$-3 \le x \le -2$ 일 때, $|x| = -x$ 이므로
$\int_{-3}^{-2} (2 x^{3} + 6 |x|) d x = \int_{-3}^{-2} (2 x^{3} - 6 x) d x$
따라서 식을 정리하면 다음과 같다.
$= \int_{-2}^{2} (2 x^{3} + 6 |x|) d x$
이때 $2 x^{3}$은 기함수이므로 $\int_{-2}^{2} 2 x^{3} d x = 0$ 이고, $6 |x|$는 우함수이므로
$= 2 \int_{0}^{2} 6 x d x$
$= 2 [ 3 x^{2} ]_{0}^{2}$
$= 2 \times (3 \times 2^{2} - 0)$
$= 24$

정답: $24$