## 문제
두 다항함수 $f(x)$, $g(x)$에 대하여 $f(1) = 2$, $g(1) = 0$, $f'(1) = 0$, $g'(1) = 2$일 때, $\lim_{x \to \infty} \sum_{k=1}^{4} x f \left( 1+ \frac{3^k}{x} \right) g \left( 1+ \frac{3^k}{x} \right)$의 값은?

## 보기
① $400$   ② $440$   ③ $480$   ④ $520$   ⑤ $560$

## 풀이
[정답] ③

$\lim_{x \to \infty} \sum_{k=1}^{4} x f \left( 1+ \frac{3^k}{x} \right) g \left( 1+ \frac{3^k}{x} \right)$에서 $\frac{1}{x} = h$, $p(x) = f(x)g(x)$라 하면

$\lim_{x \to \infty} \sum_{k=1}^{4} x f \left( 1+ \frac{3^k}{x} \right) g \left( 1+ \frac{3^k}{x} \right)$
$= \lim_{h \to 0} \frac{\sum_{k=1}^{4} p(1 + 3^k h)}{h}$
$= \lim_{h \to 0} \sum_{k=1}^{4} \frac{p(1 + 3^k h) - p(1)}{3^k h} \cdot 3^k$ ($\because p(1) = f(1)g(1) = 2 \cdot 0 = 0$)
$= \sum_{k=1}^{4} p'(1) \cdot 3^k$
$= \{f'(1)g(1) + f(1)g'(1)\} \sum_{k=1}^{4} 3^k$
$= (0 \cdot 0 + 2 \cdot 2) \sum_{k=1}^{4} 3^k$
$= 4 \sum_{k=1}^{4} 3^k$
$= 4 \times \frac{3(3^4 - 1)}{3 - 1}$
$= 480$