## ë¬¸ì œ
> [!example] ğŸ“¸ (ê·¸ë¦¼/ê·¸ë˜í”„)

ë‘ í•¨ìˆ˜ $f(x) = x^{2} - 4x$, $g(x) = \begin{cases} -x^{2} + 2x & (x < 2) \\ -x^{2} + 6x - 8 & (x \geq 2) \end{cases}$ ì˜ ê·¸ë˜í”„ë¡œ ë‘˜ëŸ¬ì‹¸ì¸ ë¶€ë¶„ì˜ ë„“ì´ëŠ”?

## ë³´ê¸°
â‘  $\frac{40}{3}$   â‘¡ $14$   â‘¢ $\frac{44}{3}$   â‘£ $\frac{46}{3}$   â‘¤ $16$

## í’€ì´
[ì •ë‹µ] â‘ 

ë‘ í•¨ìˆ˜ $y = f(x)$, $y = g(x)$ ì˜ ê·¸ë˜í”„ë¡œ ë‘˜ëŸ¬ì‹¸ì¸ ë¶€ë¶„ì—ì„œ $0 \leq x \leq 2$ ì¸ ë¶€ë¶„ê³¼ $2 \leq x \leq 4$ ì¸ ë¶€ë¶„ì˜ ë„“ì´ê°€ ê°™ìœ¼ë¯€ë¡œ êµ¬í•˜ëŠ” ë„“ì´ë¥¼ $S$ ë¼ í•˜ë©´ 

$$ S = \int_{0}^{4} \{ g(x) - f(x) \} dx $$ 
$$ = 2 \int_{0}^{2} (-2x^{2} + 6x) dx $$ 
$$ = 2 \left[ -\frac{2}{3}x^{3} + 3x^{2} \right]_{0}^{2} = \frac{40}{3} $$