## 문제
다항함수 $f(x)$에 대하여 함수 $g(x)$를
$$g(x) = (x^{2} - 2x + 2)f(x)$$
라 하자.
$$\lim_{x \to 2} \frac{g(x) - 1}{2f(x) - 1} = -2$$
일 때, $g'(2)$의 값은?

## 보기
① $\frac{1}{3}$   ② $\frac{2}{3}$   ③ $1$   ④ $\frac{4}{3}$   ⑤ $\frac{5}{3}$

## 풀이
$g(x) = (x^{2} - 2x + 2)f(x)$에서
$g(2) = 2f(2)$

$g'(x) = (2x - 2)f(x) + (x^{2} - 2x + 2)f'(x)$에서
$g'(2) = 2f(2) + 2f'(2)$

$\lim_{x \to 2} \frac{g(x) - 1}{2f(x) - 1} = -2$에서
$f(2) \neq \frac{1}{2}$이라 하면
$\lim_{x \to 2} \frac{g(x) - 1}{2f(x) - 1} = \frac{g(2) - 1}{2f(2) - 1} = \frac{2f(2) - 1}{2f(2) - 1} = 1 \neq -2$
이므로
$f(2) = \frac{1}{2}$
그러므로
$g(2) = 2f(2) = 1$이고
$g'(2) = 2f'(2) + 1$

$\lim_{x \to 2} \frac{g(x) - 1}{2f(x) - 1}$
$= \lim_{x \to 2} \frac{g(x) - g(2)}{2\{f(x) - f(2)\}}$
$= \lim_{x \to 2} \frac{\frac{g(x) - g(2)}{x - 2}}{2 \times \frac{f(x) - f(2)}{x - 2}}$

이때 $f'(2) = 0$이라 하면
$g'(2) = 1$이므로
$\lim_{x \to 2} \frac{g(x) - 1}{2f(x) - 1}$의 값이 존재하지 않는다.
그러므로
$f'(2) \neq 0$

$\lim_{x \to 2} \frac{g(x) - 1}{2f(x) - 1}$
$= \frac{g'(2)}{2f'(2)}$
$= \frac{g'(2)}{g'(2) - 1} = -2$

따라서
$g'(2) = \frac{2}{3}$

[정답] ②