## 문제
수열 $\{ a_{n} \}$ 의 첫째항부터 제 $n$ 항까지의 합을 $S_{n}$ 이라 하자. $S_{n} = \frac{1}{n(n+1)}$ 일 때, $\sum_{k=1}^{10} (S_{k} - a_{k} )$ 의 값은?

## 보기
① $\frac{1}{2}$   ② $\frac{3}{5}$   ③ $\frac{7}{10}$   ④ $\frac{4}{5}$   ⑤ $\frac{9}{10}$

## 풀이
[정답] ⑤

$$ \sum_{k=1}^{10} (S_{k} - a_{k} ) $$
$$ = \sum_{k=1}^{10} S_{k} - \sum_{k=1}^{10} a_{k} $$
$$ = \sum_{k=1}^{10} S_{k} - S_{10} $$
$$ = \sum_{k=1}^{9} S_{k} + S_{10} - S_{10} $$
$$ = \sum_{k=1}^{9} S_{k} $$
$$ = \sum_{k=1}^{9} \frac{1}{k(k+1)} $$
$$ = \sum_{k=1}^{9} \left( \frac{1}{k} - \frac{1}{k+1} \right) $$
$$ = \left( 1 - \frac{1}{2} \right) + \left( \frac{1}{2} - \frac{1}{3} \right) + \cdots + \left( \frac{1}{9} - \frac{1}{10} \right) $$
$$ = 1 - \frac{1}{10} = \frac{9}{10} $$

[다른 풀이]
$S_{n} - a_{n} = S_{n-1}$ ($n \geq 2$) 이므로
$$ \sum_{k=1}^{10} (S_{k} - a_{k} ) $$
$$ = S_{1} - a_{1} + \sum_{k=2}^{10} (S_{k} - a_{k} ) $$
($S_{1} - a_{1} = 0$ 이므로)
$$ = \sum_{k=2}^{10} S_{k-1} $$
$$ = \sum_{k=2}^{10} \frac{1}{(k-1)k} $$
$$ = \sum_{k=2}^{10} \left( \frac{1}{k-1} - \frac{1}{k} \right) $$
$$ = \left( 1 - \frac{1}{2} \right) + \left( \frac{1}{2} - \frac{1}{3} \right) + \cdots + \left( \frac{1}{9} - \frac{1}{10} \right) $$
$$ = 1 - \frac{1}{10} = \frac{9}{10} $$