## ë¬¸ì œ
> [!example] ğŸ“¸ (ê·¸ë¦¼/ê·¸ë˜í”„)

ì‹¤ìˆ˜ $t$ ($t > 0$)ì— ëŒ€í•˜ì—¬ ì§ì„  $y = tx + t + 1$ê³¼ ê³¡ì„  $y = x^{2} - tx - 1$ì´ ë§Œë‚˜ëŠ” ë‘ ì ì„ $A$, $B$ë¼ í•  ë•Œ, $\lim_{t \to \infty} \frac{\overline{AB}}{t^{2}}$ì˜ ê°’ì€?

## ë³´ê¸°
â‘  $\frac{\sqrt{2}}{2}$   â‘¡ $1$   â‘¢ $\sqrt{2}$   â‘£ $2$   â‘¤ $2\sqrt{2}$

## í’€ì´
ë‘ ì  $A$, $B$ì˜ $x$ì¢Œí‘œë¥¼ ê°ê° $\alpha$, $\beta$ ($\alpha < \beta$)ë¼ í•˜ë©´ $\alpha$, $\beta$ëŠ” ì´ì°¨ë°©ì •ì‹ $x^{2} - tx - 1 = tx + t + 1$, ì¦‰ $x^{2} - 2tx - t - 2 = 0$ì˜ ë‘ ì‹¤ê·¼ì´ë¯€ë¡œ 

$$\alpha = t - \sqrt{t^{2} + t + 2}, \beta = t + \sqrt{t^{2} + t + 2}$$ 

$\beta - \alpha = 2\sqrt{t^{2} + t + 2}$ì´ê³  ì§ì„  $AB$ì˜ ê¸°ìš¸ê¸°ê°€ $t$ì´ë¯€ë¡œ 

$$\overline{AB} = 2\sqrt{t^{2} + t + 2} \sqrt{t^{2} + 1}$$ 

$$\lim_{t \to \infty} \frac{\overline{AB}}{t^{2}} = \lim_{t \to \infty} \frac{2\sqrt{(t^{2} + t + 2)(t^{2} + 1)}}{t^{2}}$$ 

$$= 2\lim_{t \to \infty} \sqrt{\left(1 + \frac{1}{t} + \frac{2}{t^{2}}\right)\left(1 + \frac{1}{t^{2}}\right)} = 2$$ 

ì •ë‹µ: â‘£