## ë¬¸ì œ
ìì—°ìˆ˜ $n$ ì— ëŒ€í•˜ì—¬ ì› $x^{2}+y^{2}=n$ ì´ ì§ì„  $y= \sqrt{3} x$ ì™€ ì œ $1$ ì‚¬ë¶„ë©´ì—ì„œ ë§Œë‚˜ëŠ” ì ì˜ $x$ ì¢Œí‘œë¥¼ $x_{n}$ ì´ë¼ í•˜ì. $\sum _{k=1} ^{80} \frac{1}{x _{k} +x _{k+1}}$ ì˜ ê°’ì€?



> [!example] ğŸ“¸ (ê·¸ë¦¼/ê·¸ë˜í”„)

## ë³´ê¸°
â‘  $8$   â‘¡ $10$   â‘¢ $12$   â‘£ $14$   â‘¤ $16$

## í’€ì´
ì› $x^{2}+y^{2}=n$ ì´ ì§ì„  $y= \sqrt{3} x$ ì™€ ì œ $1$ ì‚¬ë¶„ë©´ì—ì„œ ë§Œë‚˜ëŠ” ì ì˜ ì¢Œí‘œë¥¼ $(x_{n}, y_{n} )$ ì´ë¼ í•˜ë©´ 
$x _{n}^{2} +y _{n}^{2} =n$, $y _{n} = \sqrt{3} x _{n}$ 

$x _{n}^{2} + ( \sqrt{3} x _{n} ) ^{2} =n$, $x _{n}^{2} = \frac{n}{4}$ 

$x _{n} >0$ ì´ë¯€ë¡œ $x _{n} = \frac{\sqrt{n}}{2}$ 

$\sum _{k=1} ^{80} \frac{1}{x _{k} +x _{k+1}}$ 
$= \sum _{k=1} ^{80} \frac{1}{\frac{\sqrt{k}}{2} + \frac{\sqrt{k+1}}{2}}$ 
$= \sum _{k=1} ^{80} \frac{2}{\sqrt{k} + \sqrt{k+1}}$ 
$= \sum _{k=1} ^{80} \frac{2 ( \sqrt{k+1} - \sqrt{k} )}{(k+1 )-k}$ 
$=2 \sum _{k=1} ^{80} ( \sqrt{k+1} - \sqrt{k} )$ 
$=2 ( \sqrt{81} -1 )=2 \times 8=16$

ì •ë‹µ: â‘¤