## 문제
수열 $\{ a_{n} \}$ 이 모든 자연수 $n$ 에 대하여 
$$\sum_{k=1}^{n} \frac{1}{(2k-1)a_{k}} = n^{2} + 2n$$
을 만족시킬 때, $\sum_{n=1}^{10} a_{n}$ 의 값은?

## 보기
① $\frac{10}{21}$   ② $\frac{4}{7}$   ③ $\frac{2}{3}$   ④ $\frac{16}{21}$   ⑤ $\frac{6}{7}$

## 풀이
$\sum_{k=1}^{n} \frac{1}{(2k-1) a_{k}} = n^{2} + 2n$ 에 대하여 
(ⅰ) $n = 1$ 일 때, 
$\frac{1}{a_{1}} = 1^{2} + 2 \times 1 = 3$ 

(ⅱ) $n \ge 2$ 일 때, 
$\frac{1}{(2n-1) a_{n}} = \sum_{k=1}^{n} \frac{1}{(2k-1) a_{k}} - \sum_{k=1}^{n-1} \frac{1}{(2k-1) a_{k}}$ 
$= n^{2} + 2n - \{ (n-1)^{2} + 2 (n-1) \}$ 
$= 2n + 1$ $\cdots \cdots$ ㉠ 

이때 $\frac{1}{a_{1}} = 3$ 은 ㉠에 $n = 1$ 을 대입한 것과 같으므로 
$\frac{1}{(2n-1)a_{n}} = 2n + 1$ 
$\therefore a_{n} = \frac{1}{(2n-1)(2n+1)}$ 

$\therefore \sum_{n=1}^{10} a_{n} = \sum_{n=1}^{10} \frac{1}{(2n-1)(2n+1)}$ 
$= \frac{1}{2} \sum_{n=1}^{10} \left( \frac{1}{2n-1} - \frac{1}{2n+1} \right)$ 
$= \frac{1}{2} \left( 1 - \frac{1}{3} + \frac{1}{3} - \frac{1}{5} + \cdots + \frac{1}{19} - \frac{1}{21} \right)$ 
$= \frac{1}{2} \left( 1 - \frac{1}{21} \right)$ 
$= \frac{10}{21}$

정답 ①