## 문제
두 수열 $\{ a_{n} \}$, $\{ b_{n} \}$ 에 대하여 
$\sum_{k=1}^{10} ( 2a_{k} + 3 ) = 40$, $\sum_{k=1}^{10} ( a_{k} - b_{k} ) = -10$
일 때, $\sum_{k=1}^{10} ( b_{k} + 5 )$ 의 값을 구하시오.

## 보기

## 풀이
$\sum_{k=1}^{10} ( 2a_{k} + 3 ) = 2 \sum_{k=1}^{10} a_{k} + \sum_{k=1}^{10} 3 = 40$ 이므로
$2 \sum_{k=1}^{10} a_{k} + 30 = 40$
$\sum_{k=1}^{10} a_{k} = 5$

$\sum_{k=1}^{10} ( a_{k} - b_{k} ) = \sum_{k=1}^{10} a_{k} - \sum_{k=1}^{10} b_{k} = -10$ 이므로
$5 - \sum_{k=1}^{10} b_{k} = -10$
$\sum_{k=1}^{10} b_{k} = 15$

따라서 
$\sum_{k=1}^{10} ( b_{k} + 5 ) = \sum_{k=1}^{10} b_{k} + \sum_{k=1}^{10} 5 = 15 + 50 = 65$

정답: $65$