## 문제
두 수열 $\{ a_{n} \}$, $\{ b_{n} \}$ 에 대하여 
$\sum_{k=1}^{10} a_{k} = \sum_{k=1}^{10} ( 2b_{k} - 1 )$, $\sum_{k=1}^{10} ( 3a_{k} + b_{k} ) = 33$
일 때, $\sum_{k=1}^{10} b_{k}$ 의 값을 구하시오.

## 보기

## 풀이
$\sum_{k=1}^{10} a_{k} = A$, $\sum_{k=1}^{10} b_{k} = B$ 라 하자. 

$\sum_{k=1}^{10} a_{k} = \sum_{k=1}^{10} ( 2b_{k} - 1 ) = 2 \sum_{k=1}^{10} b_{k} - \sum_{k=1}^{10} 1$ 에서 
$A = 2B - 10$ $\cdots \cdots$ ㉠ 

$\sum_{k=1}^{10} ( 3a_{k} + b_{k} ) = 3 \sum_{k=1}^{10} a_{k} + \sum_{k=1}^{10} b_{k} = 33$ 에서 
$3A + B = 33$ $\cdots \cdots$ ㉡ 

㉠과 ㉡을 연립하면 
$B = 9$ 

$\therefore \sum_{k=1}^{10} b_{k} = 9$