## 문제
모든 항이 음수인 수열 $\{ a_{n} \}$ 이
$$ \frac{1}{2} \left( a_{n} - \frac{2}{a_{n}} \right) = \sqrt{n-1} \quad ( n \ge 1 ) $$
을 만족시킬 때, $\sum_{n=1}^{99} a_{n}$ 의 값은?

## 보기
① $-20$   ② $-10-3 \sqrt{11}$   ③ $-10-7 \sqrt{2}$   ④ $-9-3 \sqrt{11}$   ⑤ $-9-7 \sqrt{2}$

## 풀이
$$ \frac{1}{2} \left( a_{n} - \frac{2}{a_{n}} \right) = \sqrt{n-1} \quad ( n \ge 1 ) $$ 에서 
$a_{n} < 0$ 이고, 주어진 등식을 정리하면 
$$ a_{n}^{2} - 2 \sqrt{n-1} a_{n} - 2 = 0 $$
근의 공식에 의하여 
$$ a_{n} = \sqrt{n-1} \pm \sqrt{ ( \sqrt{n-1} )^{2} + 2 } = \sqrt{n-1} \pm \sqrt{n+1} $$ 
에서 $a_{n} < 0$ 이므로 
$$ a_{n} = \sqrt{n-1} - \sqrt{n+1} $$
$\therefore \sum_{n=1}^{99} a_{n}$
$= \sum_{n=1}^{99} ( \sqrt{n-1} - \sqrt{n+1} )$
$= ( \sqrt{0} - \sqrt{2} ) + ( \sqrt{1} - \sqrt{3} ) + ( \sqrt{2} - \sqrt{4} ) + \cdots + ( \sqrt{97} - \sqrt{99} ) + ( \sqrt{98} - \sqrt{100} )$
$= \sqrt{0} + \sqrt{1} - \sqrt{99} - \sqrt{100}$
$= 0 + 1 - 3 \sqrt{11} - 10$
$= -9 - 3 \sqrt{11}$

정답: ④