## ë¬¸ì œ
ë‘ ê³¡ì„  $y=3x^{3}-7x^{2}$ê³¼ $y=-x^{2}$ìœ¼ë¡œ ë‘˜ëŸ¬ì‹¸ì¸ ë¶€ë¶„ì˜ ë„“ì´ë¥¼ êµ¬í•˜ì‹œì˜¤.

## ë³´ê¸°


## í’€ì´
ë‘ ê³¡ì„  $y=3x^{3}-7x^{2}$ê³¼ $y=-x^{2}$ì„ ì—°ë¦½í•˜ë©´
$x=0$ (ì¤‘ê·¼) ë˜ëŠ” $x=2$ë¥¼ ì–»ëŠ”ë‹¤. 
ë”°ë¼ì„œ ì•„ëž˜ ê·¸ë¦¼ìœ¼ë¡œë¶€í„° ë‘ ê³¡ì„ ìœ¼ë¡œ ë‘˜ëŸ¬ì‹¸ì¸ ë¶€ë¶„ì˜ ë„“ì´ëŠ”
$\int_{0}^{2} (-x^{2}-3x^{3}+7x^{2}) dx$
$= \int_{0}^{2} (-3x^{3}+6x^{2}) dx$
$= \left[ -\frac{3}{4}x^{4}+2x^{3} \right]_{0}^{2}$
$= (-12)+16=4$

> [!example] ðŸ“¸ (ê·¸ë¦¼/ê·¸ëž˜í”„)

[ì •ë‹µ] $4$