## ë¬¸ì œ
í•¨ìˆ˜ $y=f(x)$ ì˜ ê·¸ë˜í”„ê°€ ê·¸ë¦¼ê³¼ ê°™ë‹¤.

> [!example] ğŸ“¸ (ê·¸ë¦¼/ê·¸ë˜í”„)

$\lim_{x \to 1-} (f \circ f)(x) + \lim_{x \to -\infty} f \left( -2- \frac{1}{x+1} \right)$ ì˜ ê°’ì€?

## ë³´ê¸°
â‘  $-4$   â‘¡ $-2$   â‘¢ $0$   â‘£ $2$   â‘¤ $4$

## í’€ì´
ì£¼ì–´ì§„ ê·¸ë¦¼ì—ì„œ $t= f(x)$ ë¼ í•˜ë©´ $x \to 1-$ ì¼ ë•Œ $t= 1$ ì´ë¯€ë¡œ 
$$\lim _{x \to 1-} (f \circ f)(x) = f(1) = 2$$ 
$s= -2 - \frac{1}{x+1}$ ì´ë¼ í•˜ë©´ $x \to -\infty$ ì¼ ë•Œ $s \to -2+$ ì´ë¯€ë¡œ 
$$\lim _{x \to -\infty} f \left( -2- \frac{1}{x+1} \right) = \lim _{s \to -2+} f(s) = 2$$ 
$\therefore \lim _{x \to 1-} (f \circ f)(x) + \lim _{x \to -\infty} f \left( -2- \frac{1}{x+1} \right) = 4$

ì •ë‹µ: â‘¤