## 문제
첫째항이 $1$ 이고 모든 항이 양수인 수열 $\{ a_{n} \}$ 이 $n \geq 2$ 인 모든 자연수 $n$ 에 대하여 
$$\sum_{k=1}^{n-1} ( \sqrt{a_{k}} - \sqrt{a_{k+1}} ) = \frac{n-1}{n}$$
을 만족시킬 때, $\sum_{k=1}^{10} \frac{1}{a_{k}}$ 의 값을 구하시오.

## 보기


## 풀이
$n \geq 2$ 인 모든 자연수 $n$ 에 대하여 
$$\sum_{k=1}^{n-1} ( \sqrt{a_{k}} - \sqrt{a_{k+1}} )$$ 
$= ( \sqrt{a_{1}} - \sqrt{a_{2}} ) + ( \sqrt{a_{2}} - \sqrt{a_{3}} ) + \cdots + ( \sqrt{a_{n-1}} - \sqrt{a_{n}} )$ 
$= \sqrt{a_{1}} - \sqrt{a_{n}} = \frac{n-1}{n}$ 

$a_{1} = 1$ 이므로 $n \geq 2$ 일 때 
$\sqrt{a_{n}} = 1 - \frac{n-1}{n} = \frac{1}{n}$ 
그러므로 모든 자연수 $n$ 에 대하여 
$a_{n} = \frac{1}{n^{2}}$ 
따라서 
$$\sum_{k=1}^{10} \frac{1}{a_{k}} = \sum_{k=1}^{10} k^{2} = \frac{10 \times 11 \times 21}{6} = 385$$

정답: $385$