## 문제
함수 $f(x) = \frac{2^{x}}{2^{x} + \sqrt{2}}$ 에 대하여 수열 $\{ a_{n} \}$ 의 일반항이 $a_{n} = f \left( \frac{1}{n} \right) + f \left( \frac{2}{n} \right) + f \left( \frac{3}{n} \right) + \cdots + f \left( \frac{n-1}{n} \right) + f \left( \frac{n}{n} \right)$ 일 때, $\sum_{n=1}^{20} a_{n} = p + q \sqrt{2}$ 이다. 정수 $p$, $q$ 에 대하여 $p+q$ 의 값을 구하시오.

## 풀이
함수 $f(x) = \frac{2^{x}}{2^{x} + \sqrt{2}}$ 에서 
$f(1-x) = \frac{2^{1-x}}{2^{1-x} + \sqrt{2}} = \frac{\sqrt{2}}{2^{x} + \sqrt{2}}$ 
이므로 
$f(x) + f(1-x) = 1 \dots \dots$ ㉠ 

$f(0) = \frac{1}{1 + \sqrt{2}} = \sqrt{2} - 1$, 
$f \left( \frac{1}{2} \right) = \frac{1}{2} \dots \dots$ ㉡ 

$a_{n} = f \left( \frac{1}{n} \right) + f \left( \frac{2}{n} \right) + f \left( \frac{3}{n} \right) + \cdots + f \left( \frac{n-1}{n} \right) + f \left( \frac{n}{n} \right)$ 에서 자연수 $k$ 에 대하여 
$a_{2k} = f \left( \frac{1}{2k} \right) + f \left( \frac{2}{2k} \right) + \cdots + f \left( \frac{k}{2k} \right) + \cdots + f \left( \frac{2k}{2k} \right)$ 
$= f \left( \frac{0}{2k} \right) + f \left( \frac{1}{2k} \right) + \cdots + f \left( \frac{2k}{2k} \right) - f(0)$ 
$= k + \frac{1}{2} - \sqrt{2} + 1$ ($\because$ ㉠, ㉡) 

$a_{2k-1} = f \left( \frac{1}{2k-1} \right) + f \left( \frac{2}{2k-1} \right) + \cdots + f \left( \frac{2k-1}{2k-1} \right)$ 
$= f \left( \frac{0}{2k-1} \right) + f \left( \frac{1}{2k-1} \right) + \cdots + f \left( \frac{2k-1}{2k-1} \right) - f(0)$ 
$= k - \sqrt{2} + 1$ ($\because$ ㉠, ㉡) 

$\therefore \sum_{n=1}^{20} a_{n} = \sum_{k=1}^{10} ( a_{2k-1} + a_{2k} )$ 
$= \sum_{k=1}^{10} \left( 2k + \frac{5}{2} - 2 \sqrt{2} \right)$ 
$= 2 \times \frac{10 \times 11}{2} + 10 \times \frac{5}{2} - 20 \sqrt{2}$ 
$= 135 - 20 \sqrt{2}$ 

이므로 $p = 135$, $q = -20$ 
$\therefore p+q = 115$