## 문제
두 수열 $\{ a_{n} \}$, $\{ b_{n} \}$에 대하여 
$\sum_{k=1}^{10} ( 2a_{k} + b_{k} + k ) = 60$, $\sum_{k=1}^{10} ( a_{k} - 2b_{k} + 1 ) = 10$일 때, $\sum_{k=1}^{10} ( a_{k} + b_{k} )$의 값은?

## 보기
① $1$   ② $3$   ③ $5$   ④ $7$   ⑤ $9$

## 풀이
두 수열 $\{ a_{n} \}$, $\{ b_{n} \}$에 대하여 

$\sum_{k=1}^{10} ( 2a_{k} + b_{k} + k ) = 2 \sum_{k=1}^{10} a_{k} + \sum_{k=1}^{10} b_{k} + \frac{10 \times 11}{2} = 60$

$\therefore 2 \sum_{k=1}^{10} a_{k} + \sum_{k=1}^{10} b_{k} = 5$ $\cdots$ ㉠ 

$\sum_{k=1}^{10} ( a_{k} - 2b_{k} + 1 ) = \sum_{k=1}^{10} a_{k} - 2 \sum_{k=1}^{10} b_{k} + 10 = 10$

$\therefore \sum_{k=1}^{10} a_{k} = 2 \sum_{k=1}^{10} b_{k}$ $\cdots$ ㉡ 

㉠, ㉡을 연립하면 
$\sum_{k=1}^{10} a_{k} = 2$, $\sum_{k=1}^{10} b_{k} = 1$

$\therefore \sum_{k=1}^{10} ( a_{k} + b_{k} ) = 2 + 1 = 3$

정답: ②