## 문제
삼차방정식 $x^{3} + x^{2} + x - 3 = 0$의 서로 다른 두 허근을 $\alpha$, $\beta$라 할 때, $(\alpha^{2} + 2\alpha + 6)(\beta^{2} + 2\beta + 8)$의 값은?

## 보기
① $11$   ② $12$   ③ $13$   ④ $14$   ⑤ $15$

## 풀이
[정답] ⑤

$x^{3} + x^{2} + x - 3 = 0$ 에서 
$$(x - 1)(x^{2} + 2x + 3) = 0$$
이므로 삼차방정식 $x^{3} + x^{2} + x - 3 = 0$의 두 허근 $\alpha$, $\beta$는 이차방정식 $x^{2} + 2x + 3 = 0$의 두 근이다. 
그러므로 
$$\alpha^{2} + 2\alpha + 3 = 0, \beta^{2} + 2\beta + 3 = 0$$
이다. 
따라서 
$$(\alpha^{2} + 2\alpha + 6)(\beta^{2} + 2\beta + 8)$$
$$= (\alpha^{2} + 2\alpha + 3 + 3)(\beta^{2} + 2\beta + 3 + 5)$$
$$= (0 + 3)(0 + 5) = 15$$
이다.