## 문제
$a_{1}=2$ 인 수열 $\{a_{n}\}$ 과 $b_{1}=2$ 인 등차수열 $\{b_{n}\}$ 이 모든 자연수 $n$ 에 대하여 
$\sum_{k=1}^{n} \frac{a_{k}}{b_{k+1}}=\frac{1}{2} n^{2}$
을 만족시킬 때, $\sum_{k=1}^{5} a_{k}$ 의 값은? 

## 보기
① $120$   ② $125$   ③ $130$   ④ $135$   ⑤ $140$

## 풀이
$a_{1} = 2$ 인 수열 $\{ a_{n} \}$ 과 $b_{1} = 2$ 인 등차수열 $\{ b_{n} \}$ 에 대하여 
$\sum_{k=1}^{n} \frac{a_{k}}{b_{k+1}} = \frac{1}{2} n^{2} \cdots \cdots$ ㉠ 
이 성립하므로 등식의 양변에 $n= 1$ 을 대입하면 
$\frac{a_{1}}{b_{2}} = \frac{1}{2}$, $\frac{2}{b_{2}} = \frac{1}{2}$, $b_{2} = 4$ 
이때 등차수열 $\{ b_{n} \}$ 에서 $b_{2} - b_{1} = 2$ 이므로 
$b_{n} = 2+ 2 ( n-1 ) = 2n$ 
즉 $b_{k+1} = 2 ( k+1 )$ 이므로 ㉠에서 
$\sum_{k=1}^{n} \frac{a_{k}}{2 ( k+1 )} = \frac{1}{2} n^{2}$, $\sum_{k=1}^{n} \frac{a_{k}}{k+1} = n^{2}$ 
$n \ge 2$ 인 자연수 $n$ 에 대하여 
$\sum_{k=1}^{n} \frac{a_{k}}{k+1} - \sum_{k=1}^{n-1} \frac{a_{k}}{k+1} = n^{2} - ( n-1 )^{2} = 2n-1$ 
즉 $a_{n} = ( n+1 ) ( 2n-1 )$ ($n \ge 2$) 이고 $a_{1} = 2$ 이므로 
$a_{n} = ( n+1 ) ( 2n-1 ) = 2n^{2} +n -1$ 
$\therefore \sum_{k=1}^{5} a_{k} = \sum_{k=1}^{5} ( 2k^{2} +k -1 )$ 
$= 2 \times \frac{5 \times 6 \times 11}{6} + \frac{5 \times 6}{2} - 5 = 120$