## 문제
수열 $\{ a_{n} \}$ 의 첫째항부터 제 $n$ 항까지의 합을 $S_{n}$ 이라 할 때, 모든 자연수 $n$ 에 대하여 
$$S_{n}=2 a_{n}-p n$$
이다. $\sum _{k=1} ^{6} \frac{p+a _{k}}{a _{k} a _{k+1}} = 3$ 일 때, 상수 $p$ 의 값은?

## 보기
① $\frac{36}{127}$   ② $\frac{38}{127}$   ③ $\frac{40}{127}$   ④ $\frac{42}{127}$   ⑤ $\frac{44}{127}$

## 풀이
$S_n = 2a_n - pn$ 에서
$S_1 = a_1 = 2a_1 - p$
$\therefore a_1 = p$

$S_n - S_{n-1} = 2(a_n - a_{n-1}) - pn + p(n-1) \quad (n \ge 2)$
$\therefore a_n = 2a_{n-1} + p \quad (n \ge 2)$

$a_n = 2a_{n-1} + p$ 에서
$a_n + p = 2(a_{n-1} + p)$ 이므로
$a_n + p = (a_1 + p) \times 2^{n-1} = 2p \times 2^{n-1}$
$\therefore a_n = p(2^n - 1) \quad (n \ge 2)$

$S_1 = a_1$ 이므로
$a_n = p(2^n - 1) \quad (n \ge 1)$

$\sum _{k=1} ^{6} \frac{p+a_k}{a_k a_{k+1}}$
$= \sum _{k=1} ^{6} \frac{p+a_k}{a_k (2a_k + p)}$
$= \sum _{k=1} ^{6} (\frac{1}{a_k} - \frac{1}{2a_k + p})$
$= \sum _{k=1} ^{6} (\frac{1}{a_k} - \frac{1}{a_{k+1}})$
$= (\frac{1}{a_1} - \frac{1}{a_2}) + (\frac{1}{a_2} - \frac{1}{a_3}) + \cdots + (\frac{1}{a_6} - \frac{1}{a_7})$
$= \frac{1}{a_1} - \frac{1}{a_7}$
$= \frac{1}{p} - \frac{1}{127p}$
$= \frac{126}{127p}$

따라서 $\frac{126}{127p} = 3$ 이므로
$p = \frac{42}{127}$

정답: ④