## 문제
자연수 $n$에 대하여 $x$에 대한 이차방정식 $x^{2}+88x- (n+1 ) (n+3 )=0$의 두 근을 각각 $\alpha_{n}$, $\beta_{n}$이라 할 때, $\sum_{n=1}^{9} \left( \frac{1}{\alpha_{n}}+\frac{1}{\beta_{n}} \right)$의 값은?

## 보기
① $27$   ② $28$   ③ $29$   ④ $30$   ⑤ $31$

## 풀이
이차방정식 $x^{2}+88x- (n+1 ) (n+3 )=0$에서 근과 계수의 관계에 의하여 
$\alpha_{n} + \beta_{n} = -88$, $\alpha_{n} \beta_{n} = - ( n+1 ) ( n+3 )$

$\therefore \sum_{n=1}^{9} \left( \frac{1}{\alpha_{n}}+\frac{1}{\beta_{n}} \right)$
$= \sum_{n=1}^{9} \frac{\alpha_{n} + \beta_{n}}{\alpha_{n} \beta_{n}}$
$= \sum_{n=1}^{9} \frac{-88}{-(n+1)(n+3)}$
$= \sum_{n=1}^{9} \frac{88}{(n+1)(n+3)}$
$= 44 \sum_{n=1}^{9} \left( \frac{1}{n+1} - \frac{1}{n+3} \right)$
$= 44 \left\{ \left( \frac{1}{2} - \frac{1}{4} \right) + \left( \frac{1}{3} - \frac{1}{5} \right) + \left( \frac{1}{4} - \frac{1}{6} \right) + \left( \frac{1}{5} - \frac{1}{7} \right) + \cdots + \left( \frac{1}{9} - \frac{1}{11} \right) + \left( \frac{1}{10} - \frac{1}{12} \right) \right\}$
$= 44 \left( \frac{1}{2} + \frac{1}{3} - \frac{1}{11} - \frac{1}{12} \right)$
$= 22 + \frac{44}{3} - 4 - \frac{11}{3}$
$= 18 + \frac{33}{3}$
$= 29$

정답: ③