## 문제
이차함수 $f(x)$ 가 $\int_{-1}^{1} f'(x) dx = 0$ 을 만족시킬 때, 
$f(0) - f(-1) + \int_{0}^{1} \{x^{2} + 2x + f'(x)\} dx$ 의 값은?

## 보기
① $\frac{1}{3}$   ② $\frac{2}{3}$   ③ $1$   ④ $\frac{4}{3}$   ⑤ $\frac{5}{3}$

## 풀이
$f(0) - f(-1) = \int_{-1}^{0} f'(x) dx$ 이므로 

$$f(0) - f(-1) + \int_{0}^{1} \{x^{2} + 2x + f'(x)\} dx$$ 

$$= \int_{-1}^{0} f'(x) dx + \int_{0}^{1} (x^{2} + 2x) dx + \int_{0}^{1} f'(x) dx$$ 

$$= \int_{-1}^{1} f'(x) dx + \int_{0}^{1} (x^{2} + 2x) dx$$ 

이차함수 $f(x)$ 가 $\int_{-1}^{1} f'(x) dx = 0$ 을 만족시키므로 

$$= 0 + \left[ \frac{1}{3}x^{3} + x^{2} \right]_{0}^{1}$$ 

$$= \left( \frac{1}{3} + 1 \right) - 0 = \frac{4}{3}$$ 

따라서 정답은 ④이다.