## 문제
두 상수 $a$, $k$에 대하여 함수 $f(x)=a|x-2|$가
$$ \lim_{x \to k+} \frac{f(x)-f(k)}{x-k} - \lim_{x \to k-} \frac{f(x)-f(k)}{x-k} = 6 $$
을 만족시킬 때, $f(a+k)$의 값을 구하시오.

## 보기

## 풀이
함수 
$$ f(x) = \begin{cases} -ax+2a & (x < 2) \\ ax-2a & (x \ge 2) \end{cases} $$
에 대하여 

(ⅰ) $k < 2$ 일 때 
$$ \lim_{x \to k} \frac{f(x)-f(k)}{x-k} = \lim_{x \to k} \frac{-ax+2a-(-ak+2a)}{x-k} $$
$$ = \lim_{x \to k} \frac{-a(x-k)}{x-k} = -a $$
이므로 
$$ \lim_{x \to k+} \frac{f(x)-f(k)}{x-k} - \lim_{x \to k-} \frac{f(x)-f(k)}{x-k} = -a - (-a) = 0 \ne 6 $$

(ⅱ) $k = 2$ 일 때 
$$ \lim_{x \to 2+} \frac{f(x)-f(2)}{x-2} - \lim_{x \to 2-} \frac{f(x)-f(2)}{x-2} $$
$$ = \lim_{x \to 2+} \frac{ax-2a}{x-2} - \lim_{x \to 2-} \frac{-ax+2a}{x-2} $$
$$ = a - (-a) = 2a $$
$2a = 6$ 에서 $a = 3$ 

(ⅲ) $k > 2$ 일 때 
$$ \lim_{x \to k} \frac{f(x)-f(k)}{x-k} = \lim_{x \to k} \frac{ax-2a-(ak-2a)}{x-k} $$
$$ = \lim_{x \to k} \frac{a(x-k)}{x-k} = a $$
이므로 
$$ \lim_{x \to k+} \frac{f(x)-f(k)}{x-k} - \lim_{x \to k-} \frac{f(x)-f(k)}{x-k} = a - a = 0 \ne 6 $$

(ⅰ), (ⅱ), (ⅲ)에 의하여 $a = 3$, $k = 2$ 이므로 
$$ f(a+k) = f(3+2) = f(5) = 9 $$
정답: $9$