## ë¬¸ì œ
$| \cos (x + \frac{\pi}{3}) + \frac{1}{6} | = \frac{5}{6}$ë¥¼ ë§Œì¡±ì‹œí‚¤ëŠ” ëª¨ë“  ì‹¤ìˆ˜ $x$ ($0 \le x < 2 \pi$)ì˜ ê°’ì˜ í•©ì€?

## ë³´ê¸°
â‘  $3 \pi$   â‘¡ $\frac{10}{3} \pi$   â‘¢ $\frac{11}{3} \pi$   â‘£ $4 \pi$   â‘¤ $\frac{13}{3} \pi$

## í’€ì´
$| \cos (x + \frac{\pi}{3}) + \frac{1}{6} | = \frac{5}{6}$ ì—ì„œ
$\cos (x + \frac{\pi}{3}) + \frac{1}{6} = \frac{5}{6}$ ë˜ëŠ” $\cos (x + \frac{\pi}{3}) + \frac{1}{6} = -\frac{5}{6}$
$\therefore \cos (x + \frac{\pi}{3}) = \frac{2}{3}$ ë˜ëŠ” $\cos (x + \frac{\pi}{3}) = -1$

$x + \frac{\pi}{3} = t$ ë¡œ ë†“ìœ¼ë©´
$\cos t = \frac{2}{3}$ ë˜ëŠ” $\cos t = -1$

> [!example] ðŸ“¸ (ê·¸ë¦¼/ê·¸ëž˜í”„)

$0 \le x < 2 \pi$ ì¼ ë•Œ $\frac{\pi}{3} \le t < \frac{7}{3} \pi$ ì´ë¯€ë¡œ
(â…°) $\cos t = -1$ ì¼ ë•Œ
$t = \pi$ ì´ë¯€ë¡œ $x + \frac{\pi}{3} = \pi$
$\therefore x = \frac{2}{3} \pi$

(â…±) $\cos t = \frac{2}{3}$ ì¼ ë•Œ
ë°©ì •ì‹ $\cos t = \frac{2}{3}$ ì˜ ë‘ ê·¼ì„ $t_{1}$, $t_{2}$ ë¼ í•˜ë©´ ë‘ ê·¼ì€ ì§ì„  $t = 2 \pi$ ì— ëŒ€í•˜ì—¬ ëŒ€ì¹­ì´ë¯€ë¡œ
$t_{1} + t_{2} = 4 \pi$
$t_{1} = x_{1} + \frac{\pi}{3}$, $t_{2} = x_{2} + \frac{\pi}{3}$ ì´ë¯€ë¡œ
$(x_{1} + \frac{\pi}{3}) + (x_{2} + \frac{\pi}{3}) = 4 \pi$
$\therefore x_{1} + x_{2} = \frac{10}{3} \pi$

(â…°), (â…±)ì—ì„œ ëª¨ë“  ì‹¤ìˆ˜ $x$ ì˜ ê°’ì˜ í•©ì€
$\frac{2}{3} \pi + \frac{10}{3} \pi = 4 \pi$

ì •ë‹µ: â‘£