## ë¬¸ì œ
ë‘ ê³¡ì„  $y=x^{2}+3$, $y=-\frac{1}{5}x^{2}+3$ê³¼ ì§ì„  $x=2$ë¡œ ë‘˜ëŸ¬ì‹¸ì¸ ë¶€ë¶„ì˜ ë„“ì´ëŠ”?

> [!example] ğŸ“¸ (ê·¸ë¦¼/ê·¸ë˜í”„)

## ë³´ê¸°
â‘  $\frac{18}{5}$  â‘¡ $\frac{7}{2}$  â‘¢ $\frac{17}{5}$  â‘£ $\frac{33}{10}$  â‘¤ $\frac{16}{5}$

## í’€ì´
[ì •ë‹µ] â‘¤

êµ¬í•˜ëŠ” ë„“ì´ëŠ” ë‹¤ìŒê³¼ ê°™ë‹¤.
$$ \int_{0}^{2} \left\{ (x^{2}+3) - \left( -\frac{1}{5}x^{2}+3 \right) \right\} dx $$
$$ = \int_{0}^{2} \left( \frac{6}{5}x^{2} \right) dx $$
$$ = \left[ \frac{2}{5}x^{3} \right]_{0}^{2} $$
$$ = \frac{2}{5} \times 2^{3} $$
$$ = \frac{16}{5} $$