## ë¬¸ì œ
> [!example] ğŸ“¸ (ê·¸ë¦¼/ê·¸ë˜í”„)

ì‹¤ìˆ˜ $t$ ($t > 0$)ì— ëŒ€í•˜ì—¬ ê³¡ì„  $y=x^{2}-3x$ì™€ ì§ì„  $y=tx$ê°€ ë§Œë‚˜ëŠ” ì  ì¤‘ ì›ì  $O$ê°€ ì•„ë‹Œ ì ì„ $P$ë¼ í•˜ê³ , ì  $P$ì—ì„œ $x$ì¶•ì— ë‚´ë¦° ìˆ˜ì„ ì˜ ë°œì„ $H$ë¼ í•˜ì. $\lim_{t \to 0+} \frac{\overline{OP}-\overline{OH}}{t^{2}}$ì˜ ê°’ì€?

## ë³´ê¸°
â‘  $\frac{1}{2}$   â‘¡ $1$   â‘¢ $\frac{3}{2}$   â‘£ $2$   â‘¤ $\frac{5}{2}$

## í’€ì´
[ì •ë‹µ] â‘¢ 

$x^{2}-3x=tx$ì—ì„œ 
$x(x-t-3)=0$ 
$x=0$ ë˜ëŠ” $x=t+3$ 
ì  $P$ëŠ” ì›ì  $O$ê°€ ì•„ë‹ˆë¯€ë¡œ ì  $P$ì˜ ì¢Œí‘œëŠ” $(t+3, t^{2}+3t)$ 
$\overline{OP} = \sqrt{(t+3)^{2}+t^{2}(t+3)^{2}} = (t+3)\sqrt{t^{2}+1}$ 
$\overline{OH} = t+3$ 

ë”°ë¼ì„œ 
$\lim_{t \to 0+} \frac{\overline{OP}-\overline{OH}}{t^{2}}$ 
$= \lim_{t \to 0+} \frac{(t+3)\sqrt{t^{2}+1}-(t+3)}{t^{2}}$ 
$= \lim_{t \to 0+} \frac{(t+3)(\sqrt{t^{2}+1}-1)(\sqrt{t^{2}+1}+1)}{t^{2}(\sqrt{t^{2}+1}+1)}$ 
$= \lim_{t \to 0+} \frac{(t+3)\{(t^{2}+1)-1\}}{t^{2}(\sqrt{t^{2}+1}+1)}$ 
$= \lim_{t \to 0+} \frac{t+3}{\sqrt{t^{2}+1}+1} = \frac{3}{2}$